Prefix(:=<http://purl.obolibrary.org/obo/bfo.owl#>)
Prefix(dc:=<http://purl.org/dc/elements/1.1/>)
Prefix(obo:=<http://purl.obolibrary.org/obo/>)
Prefix(owl:=<http://www.w3.org/2002/07/owl#>)
Prefix(rdf:=<http://www.w3.org/1999/02/22-rdf-syntax-ns#>)
Prefix(xml:=<http://www.w3.org/XML/1998/namespace>)
Prefix(xsd:=<http://www.w3.org/2001/XMLSchema#>)
Prefix(rdfs:=<http://www.w3.org/2000/01/rdf-schema#>)
Prefix(skos:=<http://www.w3.org/2004/02/skos/core#>)


Ontology(<http://purl.obolibrary.org/obo/eso.owl>
<http://purl.obolibrary.org/obo/eso.owl>
Annotation(dc:contributor "Flavio Affinito")
Annotation(dc:license <https://creativecommons.org/licenses/by/4.0/>)
Annotation(rdfs:label "ESO 2024")

Declaration(Class(obo:BFO_0000001))
Declaration(Class(obo:BFO_0000002))
Declaration(Class(obo:BFO_0000003))
Declaration(Class(obo:BFO_0000004))
Declaration(Class(obo:BFO_0000006))
Declaration(Class(obo:BFO_0000008))
Declaration(Class(obo:BFO_0000009))
Declaration(Class(obo:BFO_0000011))
Declaration(Class(obo:BFO_0000015))
Declaration(Class(obo:BFO_0000017))
Declaration(Class(obo:BFO_0000018))
Declaration(Class(obo:BFO_0000019))
Declaration(Class(obo:BFO_0000020))
Declaration(Class(obo:BFO_0000023))
Declaration(Class(obo:BFO_0000024))
Declaration(Class(obo:BFO_0000026))
Declaration(Class(obo:BFO_0000027))
Declaration(Class(obo:BFO_0000028))
Declaration(Class(obo:BFO_0000029))
Declaration(Class(obo:BFO_0000030))
Declaration(Class(obo:BFO_0000035))
Declaration(Class(obo:BFO_0000038))
Declaration(Class(obo:BFO_0000040))
Declaration(Class(obo:BFO_0000141))
Declaration(Class(obo:BFO_0000148))
Declaration(Class(obo:BFO_0000202))
Declaration(Class(obo:BFO_0000203))
Declaration(Class(:Abiotic_component))
Declaration(Class(:Actor))
Declaration(Class(:Anthropogenic_asset))
Declaration(Class(:Anthropogenic_asset_aggregate))
Declaration(Class(:Biotic_component))
Declaration(Class(:Commercial_fisher))
Declaration(Class(:Commercial_fishing))
Declaration(Class(:Commodity_aggregate))
Declaration(Class(:Cultural_ecosystem_service))
Declaration(Class(:Direct_driver))
Declaration(Class(:Driver_of_change))
Declaration(Class(:Economic_activity))
Declaration(Class(:Economic_actor))
Declaration(Class(:Ecosystem))
Declaration(Class(:Ecosystem_component))
Declaration(Class(:Ecosystem_condition))
Declaration(Class(:Ecosystem_extent))
Declaration(Class(:Ecosystem_function))
Declaration(Class(:Ecosystem_good))
Declaration(Class(:Ecosystem_process))
Declaration(Class(:Ecosystem_service))
Declaration(Class(:Enjoyment_value))
Declaration(Class(:Epipelagic_ocean))
Declaration(Class(:Exploitation))
Declaration(Class(:Fauna))
Declaration(Class(:Fishing_fleet))
Declaration(Class(:Flora))
Declaration(Class(:Food_value))
Declaration(Class(:Household))
Declaration(Class(:Human_activity))
Declaration(Class(:Indirect_driver))
Declaration(Class(:Instrumental_value))
Declaration(Class(:Intrinsic_value))
Declaration(Class(:Monetary_instrumental_value))
Declaration(Class(:Non_economic_activity))
Declaration(Class(:Non_economic_actor))
Declaration(Class(:Non_monetary_instrumental_value))
Declaration(Class(:Permanent_lowland_rivers))
Declaration(Class(:Pollution))
Declaration(Class(:Provisioning_ecosystem_service))
Declaration(Class(:Regulating_ecosystem_service))
Declaration(Class(:Relational_value))
Declaration(Class(:Value))
Declaration(Class(:Vessel_fleet))
Declaration(Class(:Warming))
Declaration(Class(:Water_quality_regulation_service))
Declaration(Class(:Whale_watcher))
Declaration(Class(:Whale_watching))
Declaration(Class(:Whalewatching_fleet))
Declaration(Class(:Wild_fish_provisioning_service))
Declaration(Class(:Wildcaught_fish))
Declaration(Class(:Wildlife_viewing_service))
Declaration(Class(<http://purl.obolibrary.org/obo/eso.owl#Actor_aggregate>))
Declaration(Class(<http://purl.obolibrary.org/obo/eso.owl#Biological_control>))
Declaration(Class(<http://purl.obolibrary.org/obo/eso.owl#Biomass_production>))
Declaration(Class(<http://purl.obolibrary.org/obo/eso.owl#Carbon_fixation>))
Declaration(Class(<http://purl.obolibrary.org/obo/eso.owl#Clean_freshwater>))
Declaration(Class(<http://purl.obolibrary.org/obo/eso.owl#Commodity>))
Declaration(Class(<http://purl.obolibrary.org/obo/eso.owl#Concept>))
Declaration(Class(<http://purl.obolibrary.org/obo/eso.owl#Decomposition>))
Declaration(Class(<http://purl.obolibrary.org/obo/eso.owl#EESV_anthropogenic_contribution>))
Declaration(Class(<http://purl.obolibrary.org/obo/eso.owl#EESV_demand>))
Declaration(Class(<http://purl.obolibrary.org/obo/eso.owl#EESV_ecological_supply>))
Declaration(Class(<http://purl.obolibrary.org/obo/eso.owl#EESV_instrumental_value>))
Declaration(Class(<http://purl.obolibrary.org/obo/eso.owl#EESV_relational_value>))
Declaration(Class(<http://purl.obolibrary.org/obo/eso.owl#EESV_use>))
Declaration(Class(<http://purl.obolibrary.org/obo/eso.owl#Ecosystem_good_aggregate>))
Declaration(Class(<http://purl.obolibrary.org/obo/eso.owl#Essential_ecosystem_service_variable_class>))
Declaration(Class(<http://purl.obolibrary.org/obo/eso.owl#Fish_biomass_production>))
Declaration(Class(<http://purl.obolibrary.org/obo/eso.owl#Fish_population>))
Declaration(Class(<http://purl.obolibrary.org/obo/eso.owl#Habitat_provisioning>))
Declaration(Class(<http://purl.obolibrary.org/obo/eso.owl#Infrastructure>))
Declaration(Class(<http://purl.obolibrary.org/obo/eso.owl#Net_primary_production>))
Declaration(Class(<http://purl.obolibrary.org/obo/eso.owl#Nutrient_cycling>))
Declaration(Class(<http://purl.obolibrary.org/obo/eso.owl#Photosynthesis>))
Declaration(Class(<http://purl.obolibrary.org/obo/eso.owl#Predation>))
Declaration(Class(<http://purl.obolibrary.org/obo/eso.owl#Reproduction>))
Declaration(Class(<http://purl.obolibrary.org/obo/eso.owl#River_access_infrastructure>))
Declaration(Class(<http://purl.obolibrary.org/obo/eso.owl#Swimmer>))
Declaration(Class(<http://purl.obolibrary.org/obo/eso.owl#Swimming>))
Declaration(Class(<http://purl.obolibrary.org/obo/eso.owl#Tour_operator>))
Declaration(Class(<http://purl.obolibrary.org/obo/eso.owl#Water_purification>))
Declaration(Class(<http://purl.obolibrary.org/obo/eso.owl#Whale_habitat_provisioning>))
Declaration(Class(<http://purl.obolibrary.org/obo/eso.owl#Whale_population>))
Declaration(ObjectProperty(obo:BFO_0000054))
Declaration(ObjectProperty(obo:BFO_0000055))
Declaration(ObjectProperty(obo:BFO_0000056))
Declaration(ObjectProperty(obo:BFO_0000057))
Declaration(ObjectProperty(obo:BFO_0000062))
Declaration(ObjectProperty(obo:BFO_0000063))
Declaration(ObjectProperty(obo:BFO_0000066))
Declaration(ObjectProperty(obo:BFO_0000082))
Declaration(ObjectProperty(obo:BFO_0000108))
Declaration(ObjectProperty(obo:BFO_0000110))
Declaration(ObjectProperty(obo:BFO_0000111))
Declaration(ObjectProperty(obo:BFO_0000113))
Declaration(ObjectProperty(obo:BFO_0000115))
Declaration(ObjectProperty(obo:BFO_0000117))
Declaration(ObjectProperty(obo:BFO_0000118))
Declaration(ObjectProperty(obo:BFO_0000121))
Declaration(ObjectProperty(obo:BFO_0000124))
Declaration(ObjectProperty(obo:BFO_0000129))
Declaration(ObjectProperty(obo:BFO_0000132))
Declaration(ObjectProperty(obo:BFO_0000136))
Declaration(ObjectProperty(obo:BFO_0000137))
Declaration(ObjectProperty(obo:BFO_0000138))
Declaration(ObjectProperty(obo:BFO_0000139))
Declaration(ObjectProperty(obo:BFO_0000153))
Declaration(ObjectProperty(obo:BFO_0000166))
Declaration(ObjectProperty(obo:BFO_0000167))
Declaration(ObjectProperty(obo:BFO_0000170))
Declaration(ObjectProperty(obo:BFO_0000171))
Declaration(ObjectProperty(obo:BFO_0000172))
Declaration(ObjectProperty(obo:BFO_0000173))
Declaration(ObjectProperty(obo:BFO_0000174))
Declaration(ObjectProperty(obo:BFO_0000175))
Declaration(ObjectProperty(obo:BFO_0000176))
Declaration(ObjectProperty(obo:BFO_0000177))
Declaration(ObjectProperty(obo:BFO_0000178))
Declaration(ObjectProperty(obo:BFO_0000181))
Declaration(ObjectProperty(obo:BFO_0000183))
Declaration(ObjectProperty(obo:BFO_0000194))
Declaration(ObjectProperty(obo:BFO_0000195))
Declaration(ObjectProperty(obo:BFO_0000196))
Declaration(ObjectProperty(obo:BFO_0000197))
Declaration(ObjectProperty(obo:BFO_0000199))
Declaration(ObjectProperty(obo:BFO_0000200))
Declaration(ObjectProperty(obo:BFO_0000210))
Declaration(ObjectProperty(obo:BFO_0000211))
Declaration(ObjectProperty(obo:BFO_0000216))
Declaration(ObjectProperty(obo:BFO_0000217))
Declaration(ObjectProperty(obo:BFO_0000218))
Declaration(ObjectProperty(:benefits_from))
Declaration(ObjectProperty(:causal_relation_between_entities))
Declaration(ObjectProperty(:causal_relation_between_processes))
Declaration(ObjectProperty(:causally_influences))
Declaration(ObjectProperty(:causally_related_to))
Declaration(ObjectProperty(:causally_upstream_of))
Declaration(ObjectProperty(:causally_upstream_of_with_negative_effect))
Declaration(ObjectProperty(:causally_upstream_or_within))
Declaration(ObjectProperty(:has_output))
Declaration(ObjectProperty(:has_quality))
Declaration(ObjectProperty(:output_of))
Declaration(ObjectProperty(<http://purl.obolibrary.org/obo/eso.owl#measure_of>))
Declaration(DataProperty(:Abundance))
Declaration(DataProperty(:Area))
Declaration(DataProperty(:Catch))
Declaration(DataProperty(:Coordinates))
Declaration(DataProperty(:Count))
Declaration(DataProperty(:Income))
Declaration(DataProperty(:Latitude))
Declaration(DataProperty(:Longitude))
Declaration(DataProperty(:Retail_value))
Declaration(DataProperty(:Year))
Declaration(AnnotationProperty(dc:contributor))
Declaration(AnnotationProperty(dc:identifier))
Declaration(AnnotationProperty(dc:license))
Declaration(AnnotationProperty(skos:altLabel))
Declaration(AnnotationProperty(skos:definition))
Declaration(AnnotationProperty(skos:example))
Declaration(AnnotationProperty(skos:prefLabel))
Declaration(AnnotationProperty(skos:scopeNote))

############################
#   Object Properties
############################

# Object Property: obo:BFO_0000054 (has realization)

AnnotationAssertion(dc:identifier obo:BFO_0000054 "206-BFO")
AnnotationAssertion(rdfs:label obo:BFO_0000054 "has realization"@en)
AnnotationAssertion(skos:definition obo:BFO_0000054 "b has realization c =Def c realizes b"@en)
AnnotationAssertion(skos:example obo:BFO_0000054 "As for realizes"@en)
AnnotationAssertion(skos:prefLabel obo:BFO_0000054 "has realization"@en)
InverseObjectProperties(obo:BFO_0000054 obo:BFO_0000055)
ObjectPropertyDomain(obo:BFO_0000054 obo:BFO_0000017)
ObjectPropertyRange(obo:BFO_0000054 obo:BFO_0000015)

# Object Property: obo:BFO_0000055 (realizes)

AnnotationAssertion(dc:identifier obo:BFO_0000055 "059-BFO")
AnnotationAssertion(rdfs:label obo:BFO_0000055 "realizes"@en)
AnnotationAssertion(skos:definition obo:BFO_0000055 "(Elucidation) b realizes c means: b is a process & c is a realizable entity that inheres in d & for all t, if b has participant d at t then c exists at t & the type instantiated by b is correlated with the type instantiated by c"@en)
AnnotationAssertion(skos:example obo:BFO_0000055 "A disposition to go bald is realized in a balding process; a role of student is realized in studying processes; the pumping function of a heart is realized in processes of pumping."@en)
AnnotationAssertion(skos:prefLabel obo:BFO_0000055 "realizes"@en)
ObjectPropertyDomain(obo:BFO_0000055 obo:BFO_0000015)
ObjectPropertyRange(obo:BFO_0000055 obo:BFO_0000017)

# Object Property: obo:BFO_0000056 (participates in at some time)

AnnotationAssertion(dc:identifier obo:BFO_0000056 "250-BFO")
AnnotationAssertion(rdfs:label obo:BFO_0000056 "participates in at some time"@en)
AnnotationAssertion(skos:definition obo:BFO_0000056 "b participates in p at some time =Def for some time t (p has participant b at t)"@en)
AnnotationAssertion(skos:prefLabel obo:BFO_0000056 "participates in at some time"@en)
InverseObjectProperties(obo:BFO_0000056 obo:BFO_0000057)
ObjectPropertyRange(obo:BFO_0000056 obo:BFO_0000015)

# Object Property: obo:BFO_0000057 (has participant at some time)

AnnotationAssertion(dc:identifier obo:BFO_0000057 "248-BFO")
AnnotationAssertion(rdfs:label obo:BFO_0000057 "has participant at some time"@en)
AnnotationAssertion(skos:definition obo:BFO_0000057 "p has participant c at some time =Def for some time t (p is a process, c is a continuant, and c participates in p some way at t)"@en)
AnnotationAssertion(skos:prefLabel obo:BFO_0000057 "has participant at some time"@en)
ObjectPropertyDomain(obo:BFO_0000057 obo:BFO_0000015)

# Object Property: obo:BFO_0000062 (preceded by)

AnnotationAssertion(dc:identifier obo:BFO_0000062 "213-BFO")
AnnotationAssertion(rdfs:label obo:BFO_0000062 "preceded by"@en)
AnnotationAssertion(skos:definition obo:BFO_0000062 "b preceded by c =Def b precedes c"@en)
AnnotationAssertion(skos:example obo:BFO_0000062 "The temporal region occupied by the second half of the match is preceded by the temporal region occupied by the first half of the match."@en)
AnnotationAssertion(skos:prefLabel obo:BFO_0000062 "preceded by"@en)
InverseObjectProperties(obo:BFO_0000062 obo:BFO_0000063)
TransitiveObjectProperty(obo:BFO_0000062)
ObjectPropertyDomain(obo:BFO_0000062 obo:BFO_0000003)
ObjectPropertyRange(obo:BFO_0000062 obo:BFO_0000003)

# Object Property: obo:BFO_0000063 (precedes)

AnnotationAssertion(dc:identifier obo:BFO_0000063 "270-BFO")
AnnotationAssertion(rdfs:label obo:BFO_0000063 "precedes"@en)
AnnotationAssertion(skos:definition obo:BFO_0000063 "(Elucidation) If o, o' are occurrents and t is the temporal extent of o and t' is the temporal extent of o' then o precedes o' means: either last instant of o is before first instant of o'  or last instant of o = first instant of o' and neither o nor o' are temporal instants"@en)
AnnotationAssertion(skos:example obo:BFO_0000063 "The temporal region occupied by Mary's birth precedes the temporal region occupied by Mary's death. NOTE 1: Each temporal region is its own temporal extent. The temporal extent of a spatiotemporal region is the temporal region it temporally projects onto. The temporal extent of a process or process boundary that occupies temporal region t is t. NOTE 2: Precedes defines a strict partial order on occurrents."@en)
AnnotationAssertion(skos:prefLabel obo:BFO_0000063 "precedes"@en)
TransitiveObjectProperty(obo:BFO_0000063)
ObjectPropertyDomain(obo:BFO_0000063 obo:BFO_0000003)
ObjectPropertyRange(obo:BFO_0000063 obo:BFO_0000003)

# Object Property: obo:BFO_0000066 (occurs in)

AnnotationAssertion(dc:identifier obo:BFO_0000066 "143-BFO")
AnnotationAssertion(rdfs:label obo:BFO_0000066 "occurs in"@en)
AnnotationAssertion(skos:definition obo:BFO_0000066 "b occurs in c =Def b is a process or a process boundary and c is a material entity or immaterial entity & there exists a spatiotemporal region r and b occupies spatiotemporal region r & for all t, if b exists at t then c exists at t & there exist spatial regions s and s' where b spatially projects onto s at t & c occupies spatial region s' at t & s is a continuant part of s' at t"@en)
AnnotationAssertion(skos:example obo:BFO_0000066 "A process of digestion occurs in the interior of an organism, a process of loading artillery rounds into a tank cannon occurs in the interior of the tank."@en)
AnnotationAssertion(skos:prefLabel obo:BFO_0000066 "occurs in"@en)
InverseObjectProperties(obo:BFO_0000066 obo:BFO_0000183)
ObjectPropertyDomain(obo:BFO_0000066 ObjectUnionOf(obo:BFO_0000015 obo:BFO_0000035))
ObjectPropertyRange(obo:BFO_0000066 ObjectUnionOf(obo:BFO_0000029 obo:BFO_0000040))

# Object Property: obo:BFO_0000082 (located in at all times)

AnnotationAssertion(dc:identifier obo:BFO_0000082 "235-BFO")
AnnotationAssertion(rdfs:label obo:BFO_0000082 "located in at all times"@en)
AnnotationAssertion(skos:definition obo:BFO_0000082 "b located in c at all times =Def for all times t, b exists at t implies (b and c are independent continuants and not spatial regions, and the spatial region which b occupies at t is a (proper or improper) continuant part of the spatial region which c occupies at t)"@en)
AnnotationAssertion(skos:prefLabel obo:BFO_0000082 "located in at all times"@en)
SubObjectPropertyOf(obo:BFO_0000082 obo:BFO_0000171)
TransitiveObjectProperty(obo:BFO_0000082)
ObjectPropertyDomain(obo:BFO_0000082 ObjectIntersectionOf(obo:BFO_0000004 ObjectComplementOf(obo:BFO_0000006)))
ObjectPropertyRange(obo:BFO_0000082 ObjectIntersectionOf(obo:BFO_0000004 ObjectComplementOf(obo:BFO_0000006)))

# Object Property: obo:BFO_0000108 (exists at)

AnnotationAssertion(dc:identifier obo:BFO_0000108 "118-BFO")
AnnotationAssertion(rdfs:label obo:BFO_0000108 "exists at"@en)
AnnotationAssertion(skos:definition obo:BFO_0000108 "(Elucidation) exists at is a relation between a particular and some temporal region at which the particular exists"@en)
AnnotationAssertion(skos:example obo:BFO_0000108 "First World War exists at 1914-1916, Mexico exists at January 1, 2000."@en)
AnnotationAssertion(skos:prefLabel obo:BFO_0000108 "exists at"@en)

# Object Property: obo:BFO_0000110 (has continuant part at all times)

AnnotationAssertion(dc:identifier obo:BFO_0000110 "223-BFO")
AnnotationAssertion(rdfs:label obo:BFO_0000110 "has continuant part at all times"@en)
AnnotationAssertion(skos:definition obo:BFO_0000110 "b has continuant part c at all times =Def for all times t, b exists at t implies (b and c are continuants & b is a part of c at t)"@en)
AnnotationAssertion(skos:prefLabel obo:BFO_0000110 "has continuant part at all times"@en)
SubObjectPropertyOf(obo:BFO_0000110 obo:BFO_0000178)
ObjectPropertyDomain(obo:BFO_0000110 obo:BFO_0000002)
ObjectPropertyRange(obo:BFO_0000110 obo:BFO_0000002)

# Object Property: obo:BFO_0000111 (has proper continuant part at all times)

AnnotationAssertion(dc:identifier obo:BFO_0000111 "227-BFO")
AnnotationAssertion(rdfs:label obo:BFO_0000111 "has proper continuant part at all times"@en)
AnnotationAssertion(skos:definition obo:BFO_0000111 "b has proper continuant part c at all times =Def c proper continuant part of b at all times"@en)
AnnotationAssertion(skos:prefLabel obo:BFO_0000111 "has proper continuant part at all times"@en)
SubObjectPropertyOf(obo:BFO_0000111 obo:BFO_0000110)
SubObjectPropertyOf(obo:BFO_0000111 obo:BFO_0000174)
ObjectPropertyDomain(obo:BFO_0000111 obo:BFO_0000002)
ObjectPropertyRange(obo:BFO_0000111 obo:BFO_0000002)

# Object Property: obo:BFO_0000113 (has material basis at all times)

AnnotationAssertion(dc:identifier obo:BFO_0000113 "243-BFO")
AnnotationAssertion(rdfs:label obo:BFO_0000113 "has material basis at all times"@en)
AnnotationAssertion(skos:definition obo:BFO_0000113 "b has material basis c at all times =Def For all times t, b exists at t implies (b is a disposition & c is a material entity & there is some d bearer of b & c continuant part of d at t & d has disposition b because c continuant part of d at t)"@en)
AnnotationAssertion(skos:prefLabel obo:BFO_0000113 "has material basis at all times"@en)
SubObjectPropertyOf(obo:BFO_0000113 obo:BFO_0000218)
ObjectPropertyRange(obo:BFO_0000113 obo:BFO_0000040)

# Object Property: obo:BFO_0000115 (has member part at some time)

AnnotationAssertion(dc:identifier obo:BFO_0000115 "230-BFO")
AnnotationAssertion(rdfs:label obo:BFO_0000115 "has member part at some time"@en)
AnnotationAssertion(skos:definition obo:BFO_0000115 "b has member part c at some time =Def for some time t (c member part of b at t)"@en)
AnnotationAssertion(skos:prefLabel obo:BFO_0000115 "has member part at some time"@en)
SubObjectPropertyOf(obo:BFO_0000115 obo:BFO_0000178)
InverseObjectProperties(obo:BFO_0000115 obo:BFO_0000129)
ObjectPropertyDomain(obo:BFO_0000115 obo:BFO_0000040)
ObjectPropertyRange(obo:BFO_0000115 obo:BFO_0000040)

# Object Property: obo:BFO_0000117 (has occurrent part)

AnnotationAssertion(dc:identifier obo:BFO_0000117 "202-BFO")
AnnotationAssertion(rdfs:label obo:BFO_0000117 "has occurrent part"@en)
AnnotationAssertion(skos:definition obo:BFO_0000117 "(Elucidation) b has occurrent part c means: c is a part of b & b and c are occurrents"@en)
AnnotationAssertion(skos:example obo:BFO_0000117 "Mary's life has occurrent part Mary's 5th birthday."@en)
AnnotationAssertion(skos:prefLabel obo:BFO_0000117 "has occurrent part"@en)
InverseObjectProperties(obo:BFO_0000117 obo:BFO_0000132)
TransitiveObjectProperty(obo:BFO_0000117)
ObjectPropertyDomain(obo:BFO_0000117 obo:BFO_0000003)
ObjectPropertyRange(obo:BFO_0000117 obo:BFO_0000003)

# Object Property: obo:BFO_0000118 (has proper occurrent part)

AnnotationAssertion(dc:identifier obo:BFO_0000118 "154-BFO")
AnnotationAssertion(rdfs:label obo:BFO_0000118 "has proper occurrent part"@en)
AnnotationAssertion(skos:definition obo:BFO_0000118 "b has proper occurrent part c =Def b has occurrent part c & b and c are not identical"@en)
AnnotationAssertion(skos:example obo:BFO_0000118 "As for has occurrent part."@en)
AnnotationAssertion(skos:prefLabel obo:BFO_0000118 "has proper occurrent part"@en)
SubObjectPropertyOf(obo:BFO_0000118 obo:BFO_0000117)
InverseObjectProperties(obo:BFO_0000118 obo:BFO_0000138)
ObjectPropertyDomain(obo:BFO_0000118 obo:BFO_0000003)
ObjectPropertyRange(obo:BFO_0000118 obo:BFO_0000003)

# Object Property: obo:BFO_0000121 (has temporal part)

AnnotationAssertion(dc:identifier obo:BFO_0000121 "211-BFO")
AnnotationAssertion(rdfs:label obo:BFO_0000121 "has temporal part"@en)
AnnotationAssertion(skos:definition obo:BFO_0000121 "b has temporal part c =Def c temporal part of b"@en)
AnnotationAssertion(skos:example obo:BFO_0000121 "Your life has temporal part the first year of your life."@en)
AnnotationAssertion(skos:prefLabel obo:BFO_0000121 "has temporal part"@en)
SubObjectPropertyOf(obo:BFO_0000121 obo:BFO_0000117)
InverseObjectProperties(obo:BFO_0000121 obo:BFO_0000139)
TransitiveObjectProperty(obo:BFO_0000121)
ObjectPropertyDomain(obo:BFO_0000121 obo:BFO_0000003)
ObjectPropertyRange(obo:BFO_0000121 obo:BFO_0000003)

# Object Property: obo:BFO_0000124 (location of at some time)

AnnotationAssertion(dc:identifier obo:BFO_0000124 "236-BFO")
AnnotationAssertion(rdfs:label obo:BFO_0000124 "location of at some time"@en)
AnnotationAssertion(skos:definition obo:BFO_0000124 "b location of c at some time =Def for some time t (c located in b at t)"@en)
AnnotationAssertion(skos:prefLabel obo:BFO_0000124 "location of at some time"@en)
InverseObjectProperties(obo:BFO_0000124 obo:BFO_0000171)
ObjectPropertyDomain(obo:BFO_0000124 ObjectIntersectionOf(obo:BFO_0000004 ObjectComplementOf(obo:BFO_0000006)))
ObjectPropertyRange(obo:BFO_0000124 ObjectIntersectionOf(obo:BFO_0000004 ObjectComplementOf(obo:BFO_0000006)))

# Object Property: obo:BFO_0000129 (member part of at some time)

AnnotationAssertion(dc:identifier obo:BFO_0000129 "228-BFO")
AnnotationAssertion(rdfs:label obo:BFO_0000129 "member part of at some time"@en)
AnnotationAssertion(skos:definition obo:BFO_0000129 "b member part of c at some time =Def for some time t (b is an object & there is at t a mutually exhaustive and pairwise disjoint partition of c into objects x1, ..., xn (for some n ≠ 1) with b = xi (for some 1 <= i <= n))"@en)
AnnotationAssertion(skos:prefLabel obo:BFO_0000129 "member part of at some time"@en)
SubObjectPropertyOf(obo:BFO_0000129 obo:BFO_0000176)
ObjectPropertyDomain(obo:BFO_0000129 obo:BFO_0000040)
ObjectPropertyRange(obo:BFO_0000129 obo:BFO_0000040)

# Object Property: obo:BFO_0000132 (occurrent part of)

AnnotationAssertion(dc:identifier obo:BFO_0000132 "003-BFO")
AnnotationAssertion(rdfs:label obo:BFO_0000132 "occurrent part of"@en)
AnnotationAssertion(skos:definition obo:BFO_0000132 "(Elucidation) b occurrent part of c =Def c has occurrent part b"@en)
AnnotationAssertion(skos:example obo:BFO_0000132 "Mary's 5th birthday is an occurrent part of Mary's life; the first set of the tennis match is an occurrent part of the tennis match."@en)
AnnotationAssertion(skos:prefLabel obo:BFO_0000132 "occurrent part of"@en)
TransitiveObjectProperty(obo:BFO_0000132)
ObjectPropertyDomain(obo:BFO_0000132 obo:BFO_0000003)
ObjectPropertyRange(obo:BFO_0000132 obo:BFO_0000003)

# Object Property: obo:BFO_0000136 (proper temporal part of)

AnnotationAssertion(dc:identifier obo:BFO_0000136 "116-BFO")
AnnotationAssertion(rdfs:label obo:BFO_0000136 "proper temporal part of"@en)
AnnotationAssertion(skos:definition obo:BFO_0000136 "b proper temporal part of c =Def b temporal part of c & not (b = c)"@en)
AnnotationAssertion(skos:example obo:BFO_0000136 "As for temporal part of."@en)
AnnotationAssertion(skos:prefLabel obo:BFO_0000136 "proper temporal part of"@en)
SubObjectPropertyOf(obo:BFO_0000136 obo:BFO_0000139)
InverseObjectProperties(obo:BFO_0000136 obo:BFO_0000181)
ObjectPropertyDomain(obo:BFO_0000136 obo:BFO_0000003)
ObjectPropertyRange(obo:BFO_0000136 obo:BFO_0000003)

# Object Property: obo:BFO_0000137 (proper continuant part of at all times)

AnnotationAssertion(dc:identifier obo:BFO_0000137 "225-BFO")
AnnotationAssertion(rdfs:label obo:BFO_0000137 "proper continuant part of at all times"@en)
AnnotationAssertion(skos:definition obo:BFO_0000137 "b proper continuant part of c at all times =Def for all times t, b exists at t implies (b continuant part of c at t & not (c proper continuant part of b at t))"@en)
AnnotationAssertion(skos:prefLabel obo:BFO_0000137 "proper continuant part of at all times"@en)
SubObjectPropertyOf(obo:BFO_0000137 obo:BFO_0000175)
SubObjectPropertyOf(obo:BFO_0000137 obo:BFO_0000177)
TransitiveObjectProperty(obo:BFO_0000137)
ObjectPropertyDomain(obo:BFO_0000137 obo:BFO_0000002)
ObjectPropertyRange(obo:BFO_0000137 obo:BFO_0000002)

# Object Property: obo:BFO_0000138 (proper occurrent part of)

AnnotationAssertion(dc:identifier obo:BFO_0000138 "005-BFO")
AnnotationAssertion(rdfs:label obo:BFO_0000138 "proper occurrent part of"@en)
AnnotationAssertion(skos:definition obo:BFO_0000138 "b proper occurrent part of c =Def b occurrent part of c & b and c are not identical"@en)
AnnotationAssertion(skos:example obo:BFO_0000138 "As for occurrent part of."@en)
AnnotationAssertion(skos:prefLabel obo:BFO_0000138 "proper occurrent part of"@en)
SubObjectPropertyOf(obo:BFO_0000138 obo:BFO_0000132)
ObjectPropertyDomain(obo:BFO_0000138 obo:BFO_0000003)
ObjectPropertyRange(obo:BFO_0000138 obo:BFO_0000003)

# Object Property: obo:BFO_0000139 (temporal part of)

AnnotationAssertion(dc:identifier obo:BFO_0000139 "078-BFO")
AnnotationAssertion(rdfs:label obo:BFO_0000139 "temporal part of"@en)
AnnotationAssertion(skos:definition obo:BFO_0000139 "b temporal part of c =Def b occurrent part of c & either b and c are temporal regions or b and c are spatiotemporal regions & b temporally projects onto an occurrent part of the temporal region that c temporally projects onto or b and c are processes or process boundaries & b occupies a temporal region that is an occurrent part of the temporal region that c occupies"@en)
AnnotationAssertion(skos:example obo:BFO_0000139 "Your heart beating from 4pm to 5pm today is a temporal part of the process of your heart beating; the 4th year of your life is a temporal part of your life, as is the process boundary which separates the 3rd and 4th years of your life; the first quarter of a game of football is a temporal part of the whole game."@en)
AnnotationAssertion(skos:prefLabel obo:BFO_0000139 "temporal part of"@en)
SubObjectPropertyOf(obo:BFO_0000139 obo:BFO_0000132)
TransitiveObjectProperty(obo:BFO_0000139)
ObjectPropertyDomain(obo:BFO_0000139 obo:BFO_0000003)
ObjectPropertyRange(obo:BFO_0000139 obo:BFO_0000003)

# Object Property: obo:BFO_0000153 (temporally projects onto)

AnnotationAssertion(dc:identifier obo:BFO_0000153 "080-BFO")
AnnotationAssertion(rdfs:label obo:BFO_0000153 "temporally projects onto"@en)
AnnotationAssertion(skos:definition obo:BFO_0000153 "(Elucidation) temporally projects onto is a relation between a spatiotemporal region s and some temporal region which is the temporal extent of s"@en)
AnnotationAssertion(skos:example obo:BFO_0000153 "The world line of a particle temporally projects onto the temporal region extending from the beginning to the end of the existence of the particle."@en)
AnnotationAssertion(skos:prefLabel obo:BFO_0000153 "temporally projects onto"@en)
FunctionalObjectProperty(obo:BFO_0000153)
ObjectPropertyDomain(obo:BFO_0000153 obo:BFO_0000011)
ObjectPropertyRange(obo:BFO_0000153 obo:BFO_0000008)

# Object Property: obo:BFO_0000166 (participates in at all times)

AnnotationAssertion(dc:identifier obo:BFO_0000166 "251-BFO")
AnnotationAssertion(rdfs:label obo:BFO_0000166 "participates in at all times"@en)
AnnotationAssertion(skos:definition obo:BFO_0000166 "b participates in p at all times =Def for all times t, b exists at t implies (p has participant b at t)"@en)
AnnotationAssertion(skos:prefLabel obo:BFO_0000166 "participates in at all times"@en)
SubObjectPropertyOf(obo:BFO_0000166 obo:BFO_0000056)
ObjectPropertyRange(obo:BFO_0000166 obo:BFO_0000015)

# Object Property: obo:BFO_0000167 (has participant at all times)

AnnotationAssertion(dc:identifier obo:BFO_0000167 "249-BFO")
AnnotationAssertion(rdfs:label obo:BFO_0000167 "has participant at all times"@en)
AnnotationAssertion(skos:definition obo:BFO_0000167 "p has participant c at all times =Def for all times t, p exists at t implies (p is a process, c is a continuant, and c participates in p some way at t)"@en)
AnnotationAssertion(skos:prefLabel obo:BFO_0000167 "has participant at all times"@en)
SubObjectPropertyOf(obo:BFO_0000167 obo:BFO_0000057)
ObjectPropertyDomain(obo:BFO_0000167 obo:BFO_0000015)

# Object Property: obo:BFO_0000170 (location of at all times)

AnnotationAssertion(dc:identifier obo:BFO_0000170 "237-BFO")
AnnotationAssertion(rdfs:label obo:BFO_0000170 "location of at all times"@en)
AnnotationAssertion(skos:definition obo:BFO_0000170 "b location of c at all times =Def for all times t, b exists at t implies (c located in b at t)"@en)
AnnotationAssertion(skos:prefLabel obo:BFO_0000170 "location of at all times"@en)
SubObjectPropertyOf(obo:BFO_0000170 obo:BFO_0000124)
ObjectPropertyDomain(obo:BFO_0000170 ObjectIntersectionOf(obo:BFO_0000004 ObjectComplementOf(obo:BFO_0000006)))
ObjectPropertyRange(obo:BFO_0000170 ObjectIntersectionOf(obo:BFO_0000004 ObjectComplementOf(obo:BFO_0000006)))

# Object Property: obo:BFO_0000171 (located in at some time)

AnnotationAssertion(dc:identifier obo:BFO_0000171 "234-BFO")
AnnotationAssertion(rdfs:label obo:BFO_0000171 "located in at some time"@en)
AnnotationAssertion(skos:definition obo:BFO_0000171 "b located in c at some time =Def for some time t (b and c are independent continuants and not spatial regions, and the spatial region which b occupies at t is a (proper or improper) continuant part of the spatial region which c occupies at t)"@en)
AnnotationAssertion(skos:prefLabel obo:BFO_0000171 "located in at some time"@en)
ObjectPropertyDomain(obo:BFO_0000171 ObjectIntersectionOf(obo:BFO_0000004 ObjectComplementOf(obo:BFO_0000006)))
ObjectPropertyRange(obo:BFO_0000171 ObjectIntersectionOf(obo:BFO_0000004 ObjectComplementOf(obo:BFO_0000006)))

# Object Property: obo:BFO_0000172 (has member part at all times)

AnnotationAssertion(dc:identifier obo:BFO_0000172 "231-BFO")
AnnotationAssertion(rdfs:label obo:BFO_0000172 "has member part at all times"@en)
AnnotationAssertion(skos:definition obo:BFO_0000172 "b has member part c at all times =Def for all times t, b exists at t implies (c member part b at t)"@en)
AnnotationAssertion(skos:prefLabel obo:BFO_0000172 "has member part at all times"@en)
SubObjectPropertyOf(obo:BFO_0000172 obo:BFO_0000110)
SubObjectPropertyOf(obo:BFO_0000172 obo:BFO_0000115)
ObjectPropertyDomain(obo:BFO_0000172 obo:BFO_0000040)
ObjectPropertyRange(obo:BFO_0000172 obo:BFO_0000040)

# Object Property: obo:BFO_0000173 (member part of at all times)

AnnotationAssertion(dc:identifier obo:BFO_0000173 "229-BFO")
AnnotationAssertion(rdfs:label obo:BFO_0000173 "member part of at all times"@en)
AnnotationAssertion(skos:definition obo:BFO_0000173 "b member part of c at all times =Def for all times t, b exists at t implies (b is an object & c is an object aggregate & there is at t a mutually exhaustive and pairwise disjoint partition of c into objects x1,..., xn (for some n ≠ 1) with b = xi (for some 1 <= i <= n))"@en)
AnnotationAssertion(skos:prefLabel obo:BFO_0000173 "member part of at all times"@en)
SubObjectPropertyOf(obo:BFO_0000173 obo:BFO_0000129)
SubObjectPropertyOf(obo:BFO_0000173 obo:BFO_0000177)
ObjectPropertyDomain(obo:BFO_0000173 obo:BFO_0000040)
ObjectPropertyRange(obo:BFO_0000173 obo:BFO_0000040)

# Object Property: obo:BFO_0000174 (has proper continuant part at some time)

AnnotationAssertion(dc:identifier obo:BFO_0000174 "226-BFO")
AnnotationAssertion(rdfs:label obo:BFO_0000174 "has proper continuant part at some time"@en)
AnnotationAssertion(skos:definition obo:BFO_0000174 "b has proper continuant part c at some time =Def c proper continuant part of b at some time"@en)
AnnotationAssertion(skos:prefLabel obo:BFO_0000174 "has proper continuant part at some time"@en)
SubObjectPropertyOf(obo:BFO_0000174 obo:BFO_0000178)
InverseObjectProperties(obo:BFO_0000174 obo:BFO_0000175)
ObjectPropertyDomain(obo:BFO_0000174 obo:BFO_0000002)
ObjectPropertyRange(obo:BFO_0000174 obo:BFO_0000002)

# Object Property: obo:BFO_0000175 (proper continuant part of at some time)

AnnotationAssertion(dc:identifier obo:BFO_0000175 "224-BFO")
AnnotationAssertion(rdfs:label obo:BFO_0000175 "proper continuant part of at some time"@en)
AnnotationAssertion(skos:definition obo:BFO_0000175 "b proper continuant part of c at some time =Def for some time t (b continuant part of c at t & not (c continuant part of b at t)"@en)
AnnotationAssertion(skos:prefLabel obo:BFO_0000175 "proper continuant part of at some time"@en)
SubObjectPropertyOf(obo:BFO_0000175 obo:BFO_0000176)
ObjectPropertyDomain(obo:BFO_0000175 obo:BFO_0000002)
ObjectPropertyRange(obo:BFO_0000175 obo:BFO_0000002)

# Object Property: obo:BFO_0000176 (continuant part of at some time)

AnnotationAssertion(dc:identifier obo:BFO_0000176 "221-BFO")
AnnotationAssertion(rdfs:label obo:BFO_0000176 "continuant part of at some time"@en)
AnnotationAssertion(skos:definition obo:BFO_0000176 "b continuant part of c at some time =Def for some time t (b exists at t and c exists at t and b continuant part of c at t & t is a temporal region & b and c are continuants)"@en)
AnnotationAssertion(skos:example obo:BFO_0000176 "Milk teeth continuant part of human at some time; surgically removed tumour continuant part of organism at some time."@en)
AnnotationAssertion(skos:prefLabel obo:BFO_0000176 "continuant part of at some time"@en)
InverseObjectProperties(obo:BFO_0000176 obo:BFO_0000178)
ObjectPropertyDomain(obo:BFO_0000176 obo:BFO_0000002)
ObjectPropertyRange(obo:BFO_0000176 obo:BFO_0000002)

# Object Property: obo:BFO_0000177 (continuant part of at all times)

AnnotationAssertion(dc:identifier obo:BFO_0000177 "222-BFO")
AnnotationAssertion(rdfs:label obo:BFO_0000177 "continuant part of at all times"@en)
AnnotationAssertion(skos:definition obo:BFO_0000177 "b continuant part of c at all times =Def for all times t, (b exists at t, implies b continuant part of c at t & t is a temporal region & b and c are continuants)"@en)
AnnotationAssertion(skos:example obo:BFO_0000177 "Centre of mass of a material entity continuant part of material entity at all times; continuant fiat external boundary of an object continuant part of object at all times."@en)
AnnotationAssertion(skos:prefLabel obo:BFO_0000177 "continuant part of at all times"@en)
SubObjectPropertyOf(obo:BFO_0000177 obo:BFO_0000176)
TransitiveObjectProperty(obo:BFO_0000177)
ObjectPropertyDomain(obo:BFO_0000177 obo:BFO_0000002)
ObjectPropertyRange(obo:BFO_0000177 obo:BFO_0000002)

# Object Property: obo:BFO_0000178 (has continuant part at some time)

AnnotationAssertion(dc:identifier obo:BFO_0000178 "271-BFO")
AnnotationAssertion(rdfs:label obo:BFO_0000178 "has continuant part at some time"@en)
AnnotationAssertion(skos:definition obo:BFO_0000178 "b has continuant part c at some time =Def for some time t (b and c are continuants & b is a part of c at t)"@en)
AnnotationAssertion(skos:prefLabel obo:BFO_0000178 "has continuant part at some time"@en)
ObjectPropertyDomain(obo:BFO_0000178 obo:BFO_0000002)
ObjectPropertyRange(obo:BFO_0000178 obo:BFO_0000002)

# Object Property: obo:BFO_0000181 (has proper temporal part)

AnnotationAssertion(dc:identifier obo:BFO_0000181 "212-BFO")
AnnotationAssertion(rdfs:label obo:BFO_0000181 "has proper temporal part"@en)
AnnotationAssertion(skos:definition obo:BFO_0000181 "b has proper temporal part c =Def c proper temporal part of b"@en)
AnnotationAssertion(skos:example obo:BFO_0000181 "As for has temporal part."@en)
AnnotationAssertion(skos:prefLabel obo:BFO_0000181 "has proper temporal part"@en)
SubObjectPropertyOf(obo:BFO_0000181 obo:BFO_0000121)
ObjectPropertyDomain(obo:BFO_0000181 obo:BFO_0000003)
ObjectPropertyRange(obo:BFO_0000181 obo:BFO_0000003)

# Object Property: obo:BFO_0000183 (environs)

AnnotationAssertion(dc:identifier obo:BFO_0000183 "267-BFO")
AnnotationAssertion(rdfs:label obo:BFO_0000183 "environs"@en)
AnnotationAssertion(skos:definition obo:BFO_0000183 "b environs c =Def c occurs in b"@en)
AnnotationAssertion(skos:example obo:BFO_0000183 "Mouth environs process of mastication, city environs traffic."@en)
AnnotationAssertion(skos:prefLabel obo:BFO_0000183 "environs"@en)
ObjectPropertyDomain(obo:BFO_0000183 ObjectUnionOf(obo:BFO_0000029 obo:BFO_0000040))
ObjectPropertyRange(obo:BFO_0000183 ObjectUnionOf(obo:BFO_0000015 obo:BFO_0000035))

# Object Property: obo:BFO_0000194 (specifically depended on by)

AnnotationAssertion(dc:identifier obo:BFO_0000194 "260-BFO")
AnnotationAssertion(rdfs:label obo:BFO_0000194 "specifically depended on by"@en)
AnnotationAssertion(skos:altLabel obo:BFO_0000194 "s-depended on by"@en)
AnnotationAssertion(skos:definition obo:BFO_0000194 "b s-depended on by c =Def c specifically depends on b"@en)
AnnotationAssertion(skos:example obo:BFO_0000194 "Coloured object s-depended on by colour."@en)
AnnotationAssertion(skos:prefLabel obo:BFO_0000194 "specifically depended on by"@en)
InverseObjectProperties(obo:BFO_0000194 obo:BFO_0000195)
ObjectPropertyDomain(obo:BFO_0000194 ObjectUnionOf(obo:BFO_0000020 ObjectIntersectionOf(obo:BFO_0000004 ObjectComplementOf(obo:BFO_0000006))))
ObjectPropertyRange(obo:BFO_0000194 obo:BFO_0000020)

# Object Property: obo:BFO_0000195 (specifically depends on)

AnnotationAssertion(dc:identifier obo:BFO_0000195 "012-BFO")
AnnotationAssertion(rdfs:label obo:BFO_0000195 "specifically depends on"@en)
AnnotationAssertion(skos:altLabel obo:BFO_0000195 "s-depends on"@en)
AnnotationAssertion(skos:definition obo:BFO_0000195 "(Elucidation) b specifically depends on c means: b and c do not share common parts & b is of a nature such that at all times t it cannot exist at t unless c exists at t & b is not a boundary of c"@en)
AnnotationAssertion(skos:example obo:BFO_0000195 "A shape s-depends on the shaped object, hue, saturation and brightness of a colour sample s-depend on each other."@en)
AnnotationAssertion(skos:prefLabel obo:BFO_0000195 "specifically depends on"@en)
AnnotationAssertion(skos:scopeNote obo:BFO_0000195 "The analogue of s-dependence for occurrents is has participant."@en)
ObjectPropertyDomain(obo:BFO_0000195 obo:BFO_0000020)
ObjectPropertyRange(obo:BFO_0000195 ObjectUnionOf(obo:BFO_0000020 ObjectIntersectionOf(obo:BFO_0000004 ObjectComplementOf(obo:BFO_0000006))))

# Object Property: obo:BFO_0000196 (bearer of)

AnnotationAssertion(dc:identifier obo:BFO_0000196 "053-BFO")
AnnotationAssertion(rdfs:label obo:BFO_0000196 "bearer of"@en)
AnnotationAssertion(skos:definition obo:BFO_0000196 "b bearer of c =Def c inheres in b"@en)
AnnotationAssertion(skos:example obo:BFO_0000196 "A patch of ink is the bearer of a colour quality; an organism is the bearer of a temperature quality."@en)
AnnotationAssertion(skos:prefLabel obo:BFO_0000196 "bearer of"@en)
SubObjectPropertyOf(obo:BFO_0000196 obo:BFO_0000194)
InverseObjectProperties(obo:BFO_0000196 obo:BFO_0000197)
ObjectPropertyDomain(obo:BFO_0000196 ObjectIntersectionOf(obo:BFO_0000004 ObjectComplementOf(obo:BFO_0000006)))
ObjectPropertyRange(obo:BFO_0000196 obo:BFO_0000020)

# Object Property: obo:BFO_0000197 (inheres in)

AnnotationAssertion(dc:identifier obo:BFO_0000197 "051-BFO")
AnnotationAssertion(rdfs:label obo:BFO_0000197 "inheres in"@en)
AnnotationAssertion(skos:definition obo:BFO_0000197 "b inheres in c =Def b is a specifically dependent continuant & c is an independent continuant that is not a spatial region & b s-depends on c"@en)
AnnotationAssertion(skos:example obo:BFO_0000197 "A shape inheres in a shaped object; a mass inheres in a material entity."@en)
AnnotationAssertion(skos:prefLabel obo:BFO_0000197 "inheres in"@en)
SubObjectPropertyOf(obo:BFO_0000197 obo:BFO_0000195)
ObjectPropertyDomain(obo:BFO_0000197 obo:BFO_0000020)
ObjectPropertyRange(obo:BFO_0000197 ObjectIntersectionOf(obo:BFO_0000004 ObjectComplementOf(obo:BFO_0000006)))

# Object Property: obo:BFO_0000199 (occupies temporal region)

AnnotationAssertion(dc:identifier obo:BFO_0000199 "132-BFO")
AnnotationAssertion(rdfs:label obo:BFO_0000199 "occupies temporal region"@en)
AnnotationAssertion(skos:definition obo:BFO_0000199 "p occupies temporal region t =Def the spatiotemporal region occupied by p temporally projects onto t"@en)
AnnotationAssertion(skos:example obo:BFO_0000199 "The Second World War occupies the temporal region September 1, 1939 - September 2, 1945."@en)
AnnotationAssertion(skos:prefLabel obo:BFO_0000199 "occupies temporal region"@en)
FunctionalObjectProperty(obo:BFO_0000199)
ObjectPropertyDomain(obo:BFO_0000199 ObjectUnionOf(obo:BFO_0000015 obo:BFO_0000035))
ObjectPropertyRange(obo:BFO_0000199 obo:BFO_0000008)

# Object Property: obo:BFO_0000200 (occupies spatiotemporal region)

AnnotationAssertion(dc:identifier obo:BFO_0000200 "082-BFO")
AnnotationAssertion(rdfs:label obo:BFO_0000200 "occupies spatiotemporal region"@en)
AnnotationAssertion(skos:definition obo:BFO_0000200 "(Elucidation) p occupies spatiotemporal region s is a relation between an occurrent p and the spatiotemporal region s which is its spatiotemporal extent"@en)
AnnotationAssertion(skos:example obo:BFO_0000200 "A particle emitted by a nuclear reactor occupies the spatiotemporal region which is its trajectory."@en)
AnnotationAssertion(skos:prefLabel obo:BFO_0000200 "occupies spatiotemporal region"@en)
FunctionalObjectProperty(obo:BFO_0000200)
ObjectPropertyDomain(obo:BFO_0000200 ObjectUnionOf(obo:BFO_0000015 obo:BFO_0000035))
ObjectPropertyRange(obo:BFO_0000200 obo:BFO_0000011)

# Object Property: obo:BFO_0000210 (occupies spatial region at some time)

AnnotationAssertion(dc:identifier obo:BFO_0000210 "232-BFO")
AnnotationAssertion(rdfs:label obo:BFO_0000210 "occupies spatial region at some time"@en)
AnnotationAssertion(skos:definition obo:BFO_0000210 "an independent continuant c that is not a spatial region occupies spatial region r at some time =Def for some time t (every continuant part of c occupies some continuant part of r at t and no continuant part of c occupies any spatial region that is not a continuant part of r at t)"@en)
AnnotationAssertion(skos:prefLabel obo:BFO_0000210 "occupies spatial region at some time"@en)
ObjectPropertyDomain(obo:BFO_0000210 ObjectIntersectionOf(obo:BFO_0000004 ObjectComplementOf(obo:BFO_0000006)))
ObjectPropertyRange(obo:BFO_0000210 obo:BFO_0000006)

# Object Property: obo:BFO_0000211 (occupies spatial region at all times)

AnnotationAssertion(dc:identifier obo:BFO_0000211 "233-BFO")
AnnotationAssertion(rdfs:label obo:BFO_0000211 "occupies spatial region at all times"@en)
AnnotationAssertion(skos:definition obo:BFO_0000211 "an independent continuant c that is not a spatial region occupies spatial region r at all times =Def for all times t, b exists at t implies (every continuant part of c occupies some continuant part of r at t and no continuant part of c occupies any spatial region that is not a continuant part of r at t)"@en)
AnnotationAssertion(skos:prefLabel obo:BFO_0000211 "occupies spatial region at all times"@en)
SubObjectPropertyOf(obo:BFO_0000211 obo:BFO_0000210)
FunctionalObjectProperty(obo:BFO_0000211)
ObjectPropertyDomain(obo:BFO_0000211 ObjectIntersectionOf(obo:BFO_0000004 ObjectComplementOf(obo:BFO_0000006)))
ObjectPropertyRange(obo:BFO_0000211 obo:BFO_0000006)

# Object Property: obo:BFO_0000216 (spatially projects onto at some time)

AnnotationAssertion(dc:identifier obo:BFO_0000216 "246-BFO")
AnnotationAssertion(rdfs:label obo:BFO_0000216 "spatially projects onto at some time"@en)
AnnotationAssertion(skos:definition obo:BFO_0000216 "b spatially projects onto c at some time =Def for some time t (b is a spatiotemporal region and c is a spatial region and c is the spatial extent of b at t)"@en)
AnnotationAssertion(skos:prefLabel obo:BFO_0000216 "spatially projects onto at some time"@en)
ObjectPropertyDomain(obo:BFO_0000216 obo:BFO_0000011)
ObjectPropertyRange(obo:BFO_0000216 obo:BFO_0000006)

# Object Property: obo:BFO_0000217 (spatially projects onto at all times)

AnnotationAssertion(dc:identifier obo:BFO_0000217 "247-BFO")
AnnotationAssertion(rdfs:label obo:BFO_0000217 "spatially projects onto at all times"@en)
AnnotationAssertion(skos:definition obo:BFO_0000217 "b spatially projects onto c at all times =Def for all times t, b exists at t implies (b is a spatiotemporal region and c is a spatial region and c is the spatial extent of b at t)"@en)
AnnotationAssertion(skos:prefLabel obo:BFO_0000217 "spatially projects onto at all times"@en)
SubObjectPropertyOf(obo:BFO_0000217 obo:BFO_0000216)
FunctionalObjectProperty(obo:BFO_0000217)
ObjectPropertyDomain(obo:BFO_0000217 obo:BFO_0000011)
ObjectPropertyRange(obo:BFO_0000217 obo:BFO_0000006)

# Object Property: obo:BFO_0000218 (has material basis at some time)

AnnotationAssertion(dc:identifier obo:BFO_0000218 "242-BFO")
AnnotationAssertion(rdfs:label obo:BFO_0000218 "has material basis at some time"@en)
AnnotationAssertion(skos:definition obo:BFO_0000218 "b has material basis c at some time =Def For some time t (b is a disposition & c is a material entity & there is some d bearer of b & c continuant part of d at t & d has disposition b because c continuant part of d at t)"@en)
AnnotationAssertion(skos:prefLabel obo:BFO_0000218 "has material basis at some time"@en)
ObjectPropertyRange(obo:BFO_0000218 obo:BFO_0000040)

# Object Property: :benefits_from (:benefits_from)

AnnotationAssertion(skos:definition :benefits_from "A relationship that holds between an actor or an actor aggregate and the value of a commodity or human activity from which they derive some benefit")
AnnotationAssertion(skos:example :benefits_from "fisher benefits from income")
ObjectPropertyDomain(:benefits_from ObjectUnionOf(:Actor <http://purl.obolibrary.org/obo/eso.owl#Actor_aggregate>))
ObjectPropertyRange(:benefits_from ObjectUnionOf(:Instrumental_value :Relational_value))

# Object Property: :causal_relation_between_entities (:causal_relation_between_entities)

AnnotationAssertion(skos:definition :causal_relation_between_entities "The intent is that the process branch of the causal property hierarchy is primary (causal relations hold between occurrents/processes), and that the material branch is defined in terms of the process branch")
SubObjectPropertyOf(:causal_relation_between_entities :causally_related_to)
ObjectPropertyDomain(:causal_relation_between_entities obo:BFO_0000001)
ObjectPropertyRange(:causal_relation_between_entities obo:BFO_0000001)

# Object Property: :causal_relation_between_processes (:causal_relation_between_processes)

AnnotationAssertion(skos:definition :causal_relation_between_processes "p is causally related to q if and only if p or any part of p and q or any part of q are linked by a chain of events where each event pair is one where the execution of p influences the execution of q. p may be upstream, downstream, part of, or a container of q.")
SubObjectPropertyOf(:causal_relation_between_processes :causally_related_to)
ObjectPropertyDomain(:causal_relation_between_processes obo:BFO_0000015)
ObjectPropertyRange(:causal_relation_between_processes obo:BFO_0000015)

# Object Property: :causally_influences (:causally_influences)

AnnotationAssertion(skos:definition :causally_influences "")
AnnotationAssertion(skos:definition :causally_influences "The entity or characteristic A is causally upstream of the entity or characteristic B, A having an effect on B. An entity corresponds to any biological type of entity as long as a mass is measurable. A characteristic corresponds to a particular specificity of an entity (e.g., phenotype, shape, size).")
SubObjectPropertyOf(:causally_influences :causal_relation_between_entities)
ObjectPropertyDomain(:causally_influences obo:BFO_0000001)
ObjectPropertyRange(:causally_influences obo:BFO_0000001)

# Object Property: :causally_related_to (:causally_related_to)

AnnotationAssertion(skos:definition :causally_related_to "relation that links two events, processes, states, or objects such that one event, process, state, or object (a cause) contributes to the production of another event, process, state, or object (an effect) where the cause is partly or wholly responsible for the effect, and the effect is partly or wholly dependent on the cause.")
AnnotationAssertion(skos:example :causally_related_to "car crash causally related to drunk driving")
TransitiveObjectProperty(:causally_related_to)
ObjectPropertyDomain(:causally_related_to ObjectUnionOf(obo:BFO_0000001 obo:BFO_0000015))
ObjectPropertyRange(:causally_related_to ObjectUnionOf(obo:BFO_0000001 obo:BFO_0000015))

# Object Property: :causally_upstream_of (:causally_upstream_of)

AnnotationAssertion(skos:definition :causally_upstream_of "p is causally upstream of q iff p is causally related to q, the end of p precedes the end of q, and p is not an occurrent part of q.")
SubObjectPropertyOf(:causally_upstream_of :causally_upstream_or_within)
TransitiveObjectProperty(:causally_upstream_of)

# Object Property: :causally_upstream_of_with_negative_effect (:causally_upstream_of_with_negative_effect)

AnnotationAssertion(skos:definition :causally_upstream_of_with_negative_effect "p is causally upstream of, negative effect q iff p is casually upstream of q, and the execution of p decreases the execution of q.")
SubObjectPropertyOf(:causally_upstream_of_with_negative_effect :causally_upstream_of)

# Object Property: :causally_upstream_or_within (:causally_upstream_or_within)

AnnotationAssertion(skos:definition :causally_upstream_or_within "p is 'causally upstream or within' q iff p is causally related to q, and the end of p precedes, or is coincident with, the end of q.")
SubObjectPropertyOf(:causally_upstream_or_within :causal_relation_between_processes)
TransitiveObjectProperty(:causally_upstream_or_within)

# Object Property: :has_output (:has_output)

AnnotationAssertion(rdfs:comment :has_output "Definition from IAO_0000115 taken in ro-eco.owl")
AnnotationAssertion(skos:definition :has_output "p has output c iff c is a participant in p, c is present at the end of p, and c is not present in the same state at the beginning of p.")
AnnotationAssertion(skos:example :has_output "photosynthesis has outpu oxygen")
InverseObjectProperties(:has_output :output_of)
AsymmetricObjectProperty(:has_output)
ObjectPropertyDomain(:has_output obo:BFO_0000015)
ObjectPropertyRange(:has_output ObjectUnionOf(obo:BFO_0000015 obo:BFO_0000030))

# Object Property: :has_quality (:has_quality)

AnnotationAssertion(skos:definition :has_quality "b has quality c =Def c quality of b")
AnnotationAssertion(skos:example :has_quality "tree has quality height, phone has quality price")
ObjectPropertyDomain(:has_quality ObjectUnionOf(obo:BFO_0000015 obo:BFO_0000030))
ObjectPropertyRange(:has_quality obo:BFO_0000019)

# Object Property: :output_of (:output_of)

AnnotationAssertion(skos:definition :output_of "p output of c iff p is a participant in c, p is present at the end of c, and p is not present in the same state at the beginning of c.")
AnnotationAssertion(skos:example :output_of "carbon dioxide output of respiration")
SubObjectPropertyOf(:output_of owl:topObjectProperty)
AsymmetricObjectProperty(:output_of)
ObjectPropertyDomain(:output_of ObjectUnionOf(obo:BFO_0000015 obo:BFO_0000030))
ObjectPropertyRange(:output_of obo:BFO_0000015)

# Object Property: <http://purl.obolibrary.org/obo/eso.owl#measure_of> (<http://purl.obolibrary.org/obo/eso.owl#measure_of>)

AnnotationAssertion(skos:definition <http://purl.obolibrary.org/obo/eso.owl#measure_of> "b measure_of c: b is a BFO entity (usually a process or material entity) that has a data property that can serve as a measure of c some EESV class.")
AnnotationAssertion(skos:example <http://purl.obolibrary.org/obo/eso.owl#measure_of> "The number/mass of wildcaught fish is a measure of the EESV class Use. The abundance of whales in an area is a measure of the EESV class ecological supply.")
ObjectPropertyDomain(<http://purl.obolibrary.org/obo/eso.owl#measure_of> ObjectUnionOf(obo:BFO_0000002 obo:BFO_0000003))
ObjectPropertyRange(<http://purl.obolibrary.org/obo/eso.owl#measure_of> <http://purl.obolibrary.org/obo/eso.owl#Essential_ecosystem_service_variable_class>)


############################
#   Data Properties
############################

# Data Property: :Latitude (:Latitude)

SubDataPropertyOf(:Latitude :Coordinates)

# Data Property: :Longitude (:Longitude)

SubDataPropertyOf(:Longitude :Coordinates)



############################
#   Classes
############################

# Class: obo:BFO_0000001 (entity)

AnnotationAssertion(dc:identifier obo:BFO_0000001 "001-BFO")
AnnotationAssertion(rdfs:label obo:BFO_0000001 "entity"@en)
AnnotationAssertion(skos:definition obo:BFO_0000001 "(Elucidation) An entity is anything that exists or has existed or will exist"@en)
AnnotationAssertion(skos:example obo:BFO_0000001 "Julius Caesar, the Second World War, your body mass index, Verdi's Requiem."@en)
AnnotationAssertion(skos:prefLabel obo:BFO_0000001 "entity"@en)

# Class: obo:BFO_0000002 (continuant)

AnnotationAssertion(dc:identifier obo:BFO_0000002 "008-BFO")
AnnotationAssertion(rdfs:label obo:BFO_0000002 "continuant"@en)
AnnotationAssertion(skos:definition obo:BFO_0000002 "(Elucidation) A continuant is an entity that persists, endures, or continues to exist through time while maintaining its identity"@en)
AnnotationAssertion(skos:example obo:BFO_0000002 "A human being, a tennis ball, a cave, a region of space, someone's temperature."@en)
AnnotationAssertion(skos:prefLabel obo:BFO_0000002 "continuant"@en)
SubClassOf(obo:BFO_0000002 obo:BFO_0000001)
SubClassOf(obo:BFO_0000002 ObjectAllValuesFrom(obo:BFO_0000176 obo:BFO_0000002))
DisjointClasses(obo:BFO_0000002 obo:BFO_0000003)

# Class: obo:BFO_0000003 (occurrent)

AnnotationAssertion(dc:identifier obo:BFO_0000003 "077-BFO")
AnnotationAssertion(rdfs:label obo:BFO_0000003 "occurrent"@en)
AnnotationAssertion(skos:definition obo:BFO_0000003 "(Elucidation) An occurrent is an entity that unfolds itself in time or it is the start or end of such an entity or it is a temporal or spatiotemporal region"@en)
AnnotationAssertion(skos:example obo:BFO_0000003 "As for process, history, process boundary, spatiotemporal region, zero-dimensional temporal region, one-dimensional temporal region, temporal interval, temporal instant."@en)
AnnotationAssertion(skos:prefLabel obo:BFO_0000003 "occurrent"@en)
SubClassOf(obo:BFO_0000003 obo:BFO_0000001)

# Class: obo:BFO_0000004 (independent continuant)

AnnotationAssertion(dc:identifier obo:BFO_0000004 "017-BFO")
AnnotationAssertion(rdfs:label obo:BFO_0000004 "independent continuant"@en)
AnnotationAssertion(skos:definition obo:BFO_0000004 "b is an independent continuant =Def b is a continuant which is such that there is no c such that b s-depends on c and no c such that b g-depends on c"@en)
AnnotationAssertion(skos:example obo:BFO_0000004 "An atom, a molecule, an organism, a heart, a chair, the bottom right portion of a human torso, a leg; the interior of your mouth; a spatial region; an orchestra."@en)
AnnotationAssertion(skos:prefLabel obo:BFO_0000004 "independent continuant"@en)
SubClassOf(obo:BFO_0000004 obo:BFO_0000002)
SubClassOf(obo:BFO_0000004 ObjectAllValuesFrom(obo:BFO_0000176 obo:BFO_0000004))

# Class: obo:BFO_0000006 (spatial region)

AnnotationAssertion(dc:identifier obo:BFO_0000006 "035-BFO")
AnnotationAssertion(rdfs:label obo:BFO_0000006 "spatial region"@en)
AnnotationAssertion(skos:definition obo:BFO_0000006 "(Elucidation) A spatial region is a continuant entity that is a continuant part of the spatial projection of a portion of spacetime at a given time"@en)
AnnotationAssertion(skos:example obo:BFO_0000006 "As for zero-dimensional spatial region, one-dimensional spatial region, two-dimensional spatial region, three-dimensional spatial region."@en)
AnnotationAssertion(skos:prefLabel obo:BFO_0000006 "spatial region"@en)
SubClassOf(obo:BFO_0000006 obo:BFO_0000141)
SubClassOf(obo:BFO_0000006 ObjectAllValuesFrom(obo:BFO_0000176 obo:BFO_0000006))

# Class: obo:BFO_0000008 (temporal region)

AnnotationAssertion(dc:identifier obo:BFO_0000008 "100-BFO")
AnnotationAssertion(rdfs:label obo:BFO_0000008 "temporal region"@en)
AnnotationAssertion(skos:definition obo:BFO_0000008 "(Elucidation) A temporal region is an occurrent over which processes can unfold"@en)
AnnotationAssertion(skos:example obo:BFO_0000008 "As for zero-dimensional temporal region and one-dimensional temporal region."@en)
AnnotationAssertion(skos:prefLabel obo:BFO_0000008 "temporal region"@en)
SubClassOf(obo:BFO_0000008 obo:BFO_0000003)
SubClassOf(obo:BFO_0000008 ObjectAllValuesFrom(obo:BFO_0000132 obo:BFO_0000008))
SubClassOf(obo:BFO_0000008 ObjectAllValuesFrom(obo:BFO_0000139 obo:BFO_0000008))

# Class: obo:BFO_0000009 (two-dimensional spatial region)

AnnotationAssertion(dc:identifier obo:BFO_0000009 "039-BFO")
AnnotationAssertion(rdfs:label obo:BFO_0000009 "two-dimensional spatial region"@en)
AnnotationAssertion(skos:definition obo:BFO_0000009 "(Elucidation) A two-dimensional spatial region is a spatial region that is a whole consisting of a surface together with zero or more surfaces and/or spatial regions of lower dimension as parts"@en)
AnnotationAssertion(skos:example obo:BFO_0000009 "The surface of a sphere-shaped part of space, an infinitely thin plane in space."@en)
AnnotationAssertion(skos:prefLabel obo:BFO_0000009 "two-dimensional spatial region"@en)
SubClassOf(obo:BFO_0000009 obo:BFO_0000006)
SubClassOf(obo:BFO_0000009 ObjectAllValuesFrom(obo:BFO_0000178 ObjectUnionOf(obo:BFO_0000009 obo:BFO_0000018 obo:BFO_0000026)))

# Class: obo:BFO_0000011 (spatiotemporal region)

AnnotationAssertion(dc:identifier obo:BFO_0000011 "095-BFO")
AnnotationAssertion(rdfs:label obo:BFO_0000011 "spatiotemporal region"@en)
AnnotationAssertion(skos:definition obo:BFO_0000011 "(Elucidation) A spatiotemporal region is an occurrent that is an occurrent part of spacetime"@en)
AnnotationAssertion(skos:example obo:BFO_0000011 "The spatiotemporal region occupied by the development of a cancer tumour, the spatiotemporal region occupied by an orbiting satellite."@en)
AnnotationAssertion(skos:prefLabel obo:BFO_0000011 "spatiotemporal region"@en)
AnnotationAssertion(skos:scopeNote obo:BFO_0000011 "'Spacetime' here refers to the maximal instance of the universal spatiotemporal region."@en)
SubClassOf(obo:BFO_0000011 obo:BFO_0000003)
SubClassOf(obo:BFO_0000011 ObjectAllValuesFrom(obo:BFO_0000132 obo:BFO_0000011))
SubClassOf(obo:BFO_0000011 ObjectAllValuesFrom(obo:BFO_0000139 obo:BFO_0000011))

# Class: obo:BFO_0000015 (process)

AnnotationAssertion(dc:identifier obo:BFO_0000015 "083-BFO")
AnnotationAssertion(rdfs:label obo:BFO_0000015 "process"@en)
AnnotationAssertion(skos:definition obo:BFO_0000015 "(Elucidation) p is a process means p is an occurrent that has some temporal proper part and for some time t, p has some material entity as participant at t"@en)
AnnotationAssertion(skos:example obo:BFO_0000015 "An act of selling, the life of an organism, a process of sleeping, a process of cell-division, a beating of the heart, a process of meiosis, the taxiing of an aircraft, the programming of a computer."@en)
AnnotationAssertion(skos:prefLabel obo:BFO_0000015 "process"@en)
SubClassOf(obo:BFO_0000015 obo:BFO_0000003)
SubClassOf(obo:BFO_0000015 ObjectAllValuesFrom(obo:BFO_0000117 ObjectUnionOf(obo:BFO_0000015 obo:BFO_0000035)))
SubClassOf(obo:BFO_0000015 ObjectAllValuesFrom(obo:BFO_0000132 obo:BFO_0000015))
SubClassOf(obo:BFO_0000015 ObjectAllValuesFrom(obo:BFO_0000139 obo:BFO_0000015))

# Class: obo:BFO_0000017 (realizable entity)

AnnotationAssertion(dc:identifier obo:BFO_0000017 "058-BFO")
AnnotationAssertion(rdfs:label obo:BFO_0000017 "realizable entity"@en)
AnnotationAssertion(skos:definition obo:BFO_0000017 "(Elucidation) b is a realizable entity means: b is a specifically dependent continuant that inheres in some independent continuant which is not a spatial region and is of a type some instances of which are realized in processes of a correlated type"@en)
AnnotationAssertion(skos:example obo:BFO_0000017 "The role of being a doctor, the role of this boundary to delineate where Utah and Colorado meet, the function of your reproductive organs, the disposition of your blood to coagulate, the disposition of this piece of metal to conduct electricity."@en)
AnnotationAssertion(skos:prefLabel obo:BFO_0000017 "realizable entity"@en)
SubClassOf(obo:BFO_0000017 obo:BFO_0000020)
DisjointClasses(obo:BFO_0000017 obo:BFO_0000019)

# Class: obo:BFO_0000018 (zero-dimensional spatial region)

AnnotationAssertion(dc:identifier obo:BFO_0000018 "037-BFO")
AnnotationAssertion(rdfs:label obo:BFO_0000018 "zero-dimensional spatial region"@en)
AnnotationAssertion(skos:definition obo:BFO_0000018 "(Elucidation) A zero-dimensional spatial region is one or a collection of more than one spatially disjoint points in space"@en)
AnnotationAssertion(skos:example obo:BFO_0000018 "The spatial region occupied at some time instant by the North Pole."@en)
AnnotationAssertion(skos:prefLabel obo:BFO_0000018 "zero-dimensional spatial region"@en)
SubClassOf(obo:BFO_0000018 obo:BFO_0000006)
SubClassOf(obo:BFO_0000018 ObjectAllValuesFrom(obo:BFO_0000178 obo:BFO_0000018))

# Class: obo:BFO_0000019 (quality)

AnnotationAssertion(dc:identifier obo:BFO_0000019 "055-BFO")
AnnotationAssertion(rdfs:label obo:BFO_0000019 "quality"@en)
AnnotationAssertion(skos:definition obo:BFO_0000019 "(Elucidation) a quality is a specifically dependent continuant that, in contrast to roles and dispositions, does not require any further process in order to be realized"@en)
AnnotationAssertion(skos:example obo:BFO_0000019 "The colour of a tomato, the ambient temperature of this portion of air, the length of the circumference of your waist, the shape of your nose, the shape of your nostril, the mass of this piece of gold."@en)
AnnotationAssertion(skos:prefLabel obo:BFO_0000019 "quality"@en)
SubClassOf(obo:BFO_0000019 obo:BFO_0000020)

# Class: obo:BFO_0000020 (specifically dependent continuant)

AnnotationAssertion(dc:identifier obo:BFO_0000020 "050-BFO")
AnnotationAssertion(rdfs:label obo:BFO_0000020 "specifically dependent continuant"@en)
AnnotationAssertion(skos:definition obo:BFO_0000020 "b is a specifically dependent continuant =Def b is a continuant & there is some independent continuant c which is not a spatial region & which is such that b s-depends on c"@en)
AnnotationAssertion(skos:example obo:BFO_0000020 "(with one bearer) The mass of this tomato, the pink colour of a medium rare piece of grilled filet mignon at its centre, the smell of this portion of mozzarella, the disposition of this fish to decay, the role of being a doctor, the function of this heart: to pump blood, the shape of this hole; (with multiple bearers:) John's love for Mary, the ownership relation between John and this statue, the relation of authority between John and his subordinates."@en)
AnnotationAssertion(skos:prefLabel obo:BFO_0000020 "specifically dependent continuant"@en)
AnnotationAssertion(skos:scopeNote obo:BFO_0000020 "On the multiple bearers case, see relational quality."@en)
SubClassOf(obo:BFO_0000020 obo:BFO_0000002)

# Class: obo:BFO_0000023 (role)

AnnotationAssertion(dc:identifier obo:BFO_0000023 "061-BFO")
AnnotationAssertion(rdfs:label obo:BFO_0000023 "role"@en)
AnnotationAssertion(skos:altLabel obo:BFO_0000023 "externally-grounded realizable entity"@en)
AnnotationAssertion(skos:definition obo:BFO_0000023 "(Elucidation) b is a role means: b is a realizable entity & b exists because there is some single bearer that is in some special physical, social, or institutional set of circumstances in which this bearer does not have to be & b is not such that, if it ceases to exist, then the physical make-up of the bearer is thereby changed"@en)
AnnotationAssertion(skos:example obo:BFO_0000023 "The priest role, the student role, the role of subject in a clinical trial, the role of a stone in marking a property boundary, the role of a boundary to demarcate two neighbouring administrative territories, the role of a building in serving as a military target."@en)
AnnotationAssertion(skos:prefLabel obo:BFO_0000023 "role"@en)
SubClassOf(obo:BFO_0000023 obo:BFO_0000017)

# Class: obo:BFO_0000024 (fiat object part)

AnnotationAssertion(dc:identifier obo:BFO_0000024 "027-BFO")
AnnotationAssertion(rdfs:label obo:BFO_0000024 "fiat object part"@en)
AnnotationAssertion(skos:definition obo:BFO_0000024 "(Elucidation) a fiat object part b is a material entity which is such that for all times t, if b exists at t then there is some object c such that b is a proper continuant part of c at t and b is demarcated from the remainder of c by one or more fiat surfaces"@en)
AnnotationAssertion(skos:example obo:BFO_0000024 "The upper and lower lobes of the left lung, the dorsal and ventral surfaces of the body, the Western hemisphere of the Earth, the FMA:regional parts of an intact human body."@en)
AnnotationAssertion(skos:prefLabel obo:BFO_0000024 "fiat object part"@en)
SubClassOf(obo:BFO_0000024 obo:BFO_0000040)

# Class: obo:BFO_0000026 (one-dimensional spatial region)

AnnotationAssertion(dc:identifier obo:BFO_0000026 "038-BFO")
AnnotationAssertion(rdfs:label obo:BFO_0000026 "one-dimensional spatial region"@en)
AnnotationAssertion(skos:definition obo:BFO_0000026 "(Elucidation) A one-dimensional spatial region is a whole consisting of a line together with zero or more lines and/or points as parts"@en)
AnnotationAssertion(skos:example obo:BFO_0000026 "An edge of a cube-shaped portion of space, a line connecting two points, two parallel lines extended in space."@en)
AnnotationAssertion(skos:prefLabel obo:BFO_0000026 "one-dimensional spatial region"@en)
SubClassOf(obo:BFO_0000026 obo:BFO_0000006)
SubClassOf(obo:BFO_0000026 ObjectAllValuesFrom(obo:BFO_0000178 ObjectUnionOf(obo:BFO_0000018 obo:BFO_0000026)))

# Class: obo:BFO_0000027 (object aggregate)

AnnotationAssertion(dc:identifier obo:BFO_0000027 "025-BFO")
AnnotationAssertion(rdfs:label obo:BFO_0000027 "object aggregate"@en)
AnnotationAssertion(skos:definition obo:BFO_0000027 "(Elucidation) an object aggregate is a material entity consisting exactly of a plurality (≥1) of objects as member parts which together form a unit"@en)
AnnotationAssertion(skos:example obo:BFO_0000027 "The aggregate of the musicians in a symphony orchestra and their instruments, the aggregate of bearings in a constant velocity axle joint, the nitrogen atoms in the atmosphere, a collection of cells in a blood biobank. NOTE 1: 'Exactly' means that there are no parts of the object aggregate other than its member parts. NOTE 2: The unit can, at certain times, consist of exactly one object, for example, when a wolf litter loses all but one of its pups, but it must at some time have a plurality of member parts."@en)
AnnotationAssertion(skos:prefLabel obo:BFO_0000027 "object aggregate"@en)
SubClassOf(obo:BFO_0000027 obo:BFO_0000040)

# Class: obo:BFO_0000028 (three-dimensional spatial region)

AnnotationAssertion(dc:identifier obo:BFO_0000028 "040-BFO")
AnnotationAssertion(rdfs:label obo:BFO_0000028 "three-dimensional spatial region"@en)
AnnotationAssertion(skos:definition obo:BFO_0000028 "(Elucidation) A three-dimensional spatial region is a whole consisting of a spatial volume together with zero or more spatial volumes and/or spatial regions of lower dimension as parts"@en)
AnnotationAssertion(skos:example obo:BFO_0000028 "A cube-shaped region of space, a sphere-shaped region of space, the region of space occupied by all and only the planets in the solar system at some point in time."@en)
AnnotationAssertion(skos:prefLabel obo:BFO_0000028 "three-dimensional spatial region"@en)
SubClassOf(obo:BFO_0000028 obo:BFO_0000006)
SubClassOf(obo:BFO_0000028 ObjectAllValuesFrom(obo:BFO_0000178 obo:BFO_0000006))

# Class: obo:BFO_0000029 (site)

AnnotationAssertion(dc:identifier obo:BFO_0000029 "034-BFO")
AnnotationAssertion(rdfs:label obo:BFO_0000029 "site"@en)
AnnotationAssertion(skos:definition obo:BFO_0000029 "(Elucidation) b is a site means: b is a three-dimensional immaterial entity whose boundaries either (1) (partially or wholly) coincide with the boundaries of one or more material entities or (2) have locations determined in relation to some material entity"@en)
AnnotationAssertion(skos:example obo:BFO_0000029 "A hole in a portion of cheese, a rabbit hole, the Grand Canyon, the Piazza San Marco, the kangaroo-joey-containing hole of a kangaroo pouch, your left nostril (a fiat part - the opening - of your left nasal cavity), the lumen of your gut, the hold of a ship, the interior of the trunk of your car, hole in an engineered floor joist; An air traffic control region of type A is determined in terms of elevation above mean sea level of lower and upper boundaries."@en)
AnnotationAssertion(skos:prefLabel obo:BFO_0000029 "site"@en)
SubClassOf(obo:BFO_0000029 obo:BFO_0000141)
SubClassOf(obo:BFO_0000029 ObjectAllValuesFrom(obo:BFO_0000176 ObjectUnionOf(obo:BFO_0000029 obo:BFO_0000040)))
SubClassOf(obo:BFO_0000029 ObjectAllValuesFrom(obo:BFO_0000210 obo:BFO_0000028))

# Class: obo:BFO_0000030 (object)

AnnotationAssertion(dc:identifier obo:BFO_0000030 "024-BFO")
AnnotationAssertion(rdfs:label obo:BFO_0000030 "object"@en)
AnnotationAssertion(skos:definition obo:BFO_0000030 "(Elucidation) an object is a material entity which manifests causal unity & is of a type instances of which are maximal relative to the sort of causal unity manifested"@en)
AnnotationAssertion(skos:example obo:BFO_0000030 "An organism, a fish tank, a planet, a laptop, a valve, a block of marble, an ice cube."@en)
AnnotationAssertion(skos:prefLabel obo:BFO_0000030 "object"@en)
AnnotationAssertion(skos:scopeNote obo:BFO_0000030 "A description of three primary sorts of causal unity is provided in Basic Formal Ontology 2.0. Specification and User’s Guide"@en)
SubClassOf(obo:BFO_0000030 obo:BFO_0000040)

# Class: obo:BFO_0000035 (process boundary)

AnnotationAssertion(dc:identifier obo:BFO_0000035 "084-BFO")
AnnotationAssertion(rdfs:label obo:BFO_0000035 "process boundary"@en)
AnnotationAssertion(skos:definition obo:BFO_0000035 "p is a process boundary =Def p is a temporal part of a process & p has no proper temporal parts"@en)
AnnotationAssertion(skos:example obo:BFO_0000035 "The boundary between the 2nd and 3rd year of your life."@en)
AnnotationAssertion(skos:prefLabel obo:BFO_0000035 "process boundary"@en)
SubClassOf(obo:BFO_0000035 obo:BFO_0000003)
SubClassOf(obo:BFO_0000035 ObjectAllValuesFrom(obo:BFO_0000117 obo:BFO_0000035))
SubClassOf(obo:BFO_0000035 ObjectAllValuesFrom(obo:BFO_0000121 obo:BFO_0000035))
SubClassOf(obo:BFO_0000035 ObjectAllValuesFrom(obo:BFO_0000132 ObjectUnionOf(obo:BFO_0000015 obo:BFO_0000035)))
SubClassOf(obo:BFO_0000035 ObjectAllValuesFrom(obo:BFO_0000139 ObjectUnionOf(obo:BFO_0000015 obo:BFO_0000035)))

# Class: obo:BFO_0000038 (one-dimensional temporal region)

AnnotationAssertion(dc:identifier obo:BFO_0000038 "103-BFO")
AnnotationAssertion(rdfs:label obo:BFO_0000038 "one-dimensional temporal region"@en)
AnnotationAssertion(skos:definition obo:BFO_0000038 "(Elucidation) A one-dimensional temporal region is a temporal region is a whole that has a temporal interval and zero or more temporal intervals and temporal instants as parts"@en)
AnnotationAssertion(skos:example obo:BFO_0000038 "The temporal region during which a process occurs."@en)
AnnotationAssertion(skos:prefLabel obo:BFO_0000038 "one-dimensional temporal region"@en)
SubClassOf(obo:BFO_0000038 obo:BFO_0000008)
SubClassOf(obo:BFO_0000038 ObjectAllValuesFrom(obo:BFO_0000121 ObjectUnionOf(obo:BFO_0000038 obo:BFO_0000148)))
SubClassOf(obo:BFO_0000038 ObjectAllValuesFrom(obo:BFO_0000139 obo:BFO_0000038))
DisjointClasses(obo:BFO_0000038 obo:BFO_0000148)

# Class: obo:BFO_0000040 (material entity)

AnnotationAssertion(dc:identifier obo:BFO_0000040 "019-BFO")
AnnotationAssertion(rdfs:label obo:BFO_0000040 "material entity"@en)
AnnotationAssertion(skos:definition obo:BFO_0000040 "(Elucidation) A material entity is an independent continuant that at all times at which it exists has some portion of matter as continuant part"@en)
AnnotationAssertion(skos:example obo:BFO_0000040 "A human being, the undetached arm of a human being, an aggregate of human beings."@en)
AnnotationAssertion(skos:prefLabel obo:BFO_0000040 "material entity"@en)
SubClassOf(obo:BFO_0000040 obo:BFO_0000004)
SubClassOf(obo:BFO_0000040 ObjectAllValuesFrom(obo:BFO_0000176 obo:BFO_0000040))
DisjointClasses(obo:BFO_0000040 obo:BFO_0000141)

# Class: obo:BFO_0000141 (immaterial entity)

AnnotationAssertion(dc:identifier obo:BFO_0000141 "028-BFO")
AnnotationAssertion(rdfs:label obo:BFO_0000141 "immaterial entity"@en)
AnnotationAssertion(skos:definition obo:BFO_0000141 "a is an immaterial entity =Def a is an independent continuant which is such that there is no time t when it has a material entity as continuant part at t"@en)
AnnotationAssertion(skos:example obo:BFO_0000141 "As for fiat point, fiat line, fiat surface, site."@en)
AnnotationAssertion(skos:prefLabel obo:BFO_0000141 "immaterial entity"@en)
SubClassOf(obo:BFO_0000141 obo:BFO_0000004)

# Class: obo:BFO_0000148 (zero-dimensional temporal region)

AnnotationAssertion(dc:identifier obo:BFO_0000148 "102-BFO")
AnnotationAssertion(rdfs:label obo:BFO_0000148 "zero-dimensional temporal region"@en)
AnnotationAssertion(skos:definition obo:BFO_0000148 "(Elucidation) A zero-dimensional temporal region is a temporal region that is a whole consisting of one or more separated temporal instants as parts"@en)
AnnotationAssertion(skos:example obo:BFO_0000148 "A temporal region that is occupied by a process boundary; the moment at which a finger is detached in an industrial accident."@en)
AnnotationAssertion(skos:prefLabel obo:BFO_0000148 "zero-dimensional temporal region"@en)
SubClassOf(obo:BFO_0000148 obo:BFO_0000008)
SubClassOf(obo:BFO_0000148 ObjectAllValuesFrom(obo:BFO_0000121 obo:BFO_0000148))

# Class: obo:BFO_0000202 (temporal interval)

AnnotationAssertion(dc:identifier obo:BFO_0000202 "155-BFO")
AnnotationAssertion(rdfs:label obo:BFO_0000202 "temporal interval"@en)
AnnotationAssertion(skos:definition obo:BFO_0000202 "(Elucidation) a temporal interval is a one-dimensional temporal region that is continuous, thus without gaps or breaks"@en)
AnnotationAssertion(skos:example obo:BFO_0000202 "The year 2018."@en)
AnnotationAssertion(skos:prefLabel obo:BFO_0000202 "temporal interval"@en)
AnnotationAssertion(skos:scopeNote obo:BFO_0000202 "A one-dimensional temporal region can include as parts not only temporal intervals but also temporal instants separated from other parts by gaps."@en)
SubClassOf(obo:BFO_0000202 obo:BFO_0000038)

# Class: obo:BFO_0000203 (temporal instant)

AnnotationAssertion(dc:identifier obo:BFO_0000203 "209-BFO")
AnnotationAssertion(rdfs:label obo:BFO_0000203 "temporal instant"@en)
AnnotationAssertion(skos:definition obo:BFO_0000203 "(Elucidation) a temporal instant is a zero-dimensional temporal region that has no proper temporal part"@en)
AnnotationAssertion(skos:example obo:BFO_0000203 "The millennium."@en)
AnnotationAssertion(skos:prefLabel obo:BFO_0000203 "temporal instant"@en)
SubClassOf(obo:BFO_0000203 obo:BFO_0000148)

# Class: :Abiotic_component (:Abiotic_component)

AnnotationAssertion(skos:definition :Abiotic_component "The non-living components that form part of an ecosystem.")
AnnotationAssertion(skos:example :Abiotic_component "A river, a lake, soil")
SubClassOf(:Abiotic_component :Ecosystem_component)

# Class: :Actor (:Actor)

AnnotationAssertion(skos:definition :Actor "An individual entity within a social-ecological system that performs actions or makes decisions impacting the system's dynamics and outcomes.")
SubClassOf(:Actor obo:BFO_0000030)
SubClassOf(:Actor ObjectSomeValuesFrom(obo:BFO_0000166 :Human_activity))
SubClassOf(:Actor ObjectSomeValuesFrom(obo:BFO_0000175 <http://purl.obolibrary.org/obo/eso.owl#Actor_aggregate>))
SubClassOf(:Actor ObjectSomeValuesFrom(:benefits_from :Relational_value))

# Class: :Anthropogenic_asset (:Anthropogenic_asset)

AnnotationAssertion(skos:definition :Anthropogenic_asset "Any human-made or human-influenced object that contributes to human well-being and economic activity.")
AnnotationAssertion(skos:example :Anthropogenic_asset "A fishing boat, fertiliser, infrastructure")
SubClassOf(:Anthropogenic_asset obo:BFO_0000030)
SubClassOf(:Anthropogenic_asset ObjectSomeValuesFrom(obo:BFO_0000166 :Human_activity))
SubClassOf(:Anthropogenic_asset ObjectSomeValuesFrom(obo:BFO_0000175 :Anthropogenic_asset_aggregate))

# Class: :Anthropogenic_asset_aggregate (:Anthropogenic_asset_aggregate)

AnnotationAssertion(skos:definition :Anthropogenic_asset_aggregate "Is a material entity consisting exactly of a plurality (≥1) of anthropogenic assets as member parts which together form a unit.")
AnnotationAssertion(skos:example :Anthropogenic_asset_aggregate "A fishing fleet, all the paths in a provincial park")
SubClassOf(:Anthropogenic_asset_aggregate obo:BFO_0000027)
SubClassOf(:Anthropogenic_asset_aggregate ObjectSomeValuesFrom(obo:BFO_0000056 :Human_activity))
SubClassOf(:Anthropogenic_asset_aggregate ObjectSomeValuesFrom(obo:BFO_0000174 :Anthropogenic_asset))
SubClassOf(:Anthropogenic_asset_aggregate ObjectSomeValuesFrom(<http://purl.obolibrary.org/obo/eso.owl#measure_of> <http://purl.obolibrary.org/obo/eso.owl#EESV_anthropogenic_contribution>))

# Class: :Biotic_component (:Biotic_component)

AnnotationAssertion(skos:definition :Biotic_component "The living components that form part of an ecosystem.")
AnnotationAssertion(skos:example :Biotic_component "A maple tree, a horse")
SubClassOf(:Biotic_component :Ecosystem_component)

# Class: :Commercial_fisher (:Commercial_fisher)

AnnotationAssertion(skos:definition :Commercial_fisher "A type of economic actor who participates in the commercial fishing activity.")
SubClassOf(:Commercial_fisher :Economic_actor)
SubClassOf(:Commercial_fisher ObjectSomeValuesFrom(obo:BFO_0000056 :Commercial_fishing))
SubClassOf(:Commercial_fisher ObjectSomeValuesFrom(:benefits_from :Monetary_instrumental_value))

# Class: :Commercial_fishing (:Commercial_fishing)

AnnotationAssertion(skos:definition :Commercial_fishing "An economic activity that involves the harvesting of wild fish for the purpose of generating economic gain through the sale of catch on the market.")
AnnotationAssertion(skos:example :Commercial_fishing "Commercial cod fishing, commercial salmon fishing")
SubClassOf(:Commercial_fishing :Economic_activity)
SubClassOf(:Commercial_fishing ObjectSomeValuesFrom(obo:BFO_0000055 :Wild_fish_provisioning_service))
SubClassOf(:Commercial_fishing ObjectSomeValuesFrom(obo:BFO_0000167 :Commercial_fisher))
SubClassOf(:Commercial_fishing ObjectSomeValuesFrom(obo:BFO_0000167 :Fishing_fleet))
SubClassOf(:Commercial_fishing ObjectSomeValuesFrom(obo:BFO_0000167 <http://purl.obolibrary.org/obo/eso.owl#Fish_population>))
SubClassOf(:Commercial_fishing ObjectSomeValuesFrom(:causally_upstream_of :Exploitation))
SubClassOf(:Commercial_fishing ObjectSomeValuesFrom(:has_output :Wildcaught_fish))

# Class: :Commodity_aggregate (:Commodity_aggregate)

AnnotationAssertion(skos:definition :Commodity_aggregate "Is a material entity consisting exactly of a plurality (≥1) of commodities as member parts which together form a unit.")
AnnotationAssertion(skos:example :Commodity_aggregate "The wheat of France")
SubClassOf(:Commodity_aggregate obo:BFO_0000027)
SubClassOf(:Commodity_aggregate ObjectSomeValuesFrom(obo:BFO_0000174 <http://purl.obolibrary.org/obo/eso.owl#Commodity>))
SubClassOf(:Commodity_aggregate ObjectSomeValuesFrom(:has_quality :Instrumental_value))
SubClassOf(:Commodity_aggregate ObjectSomeValuesFrom(<http://purl.obolibrary.org/obo/eso.owl#measure_of> <http://purl.obolibrary.org/obo/eso.owl#EESV_use>))

# Class: :Cultural_ecosystem_service (:Cultural_ecosystem_service)

AnnotationAssertion(skos:definition :Cultural_ecosystem_service "These are the services that contribute to the benefits people obtain from ecosystems through spiritual enrichment, cognitive development, reflection, recreation, and aesthetic experiences.")
AnnotationAssertion(skos:example :Cultural_ecosystem_service "Recreation services, aesthetic appreciation")
SubClassOf(:Cultural_ecosystem_service :Ecosystem_service)
SubClassOf(:Cultural_ecosystem_service ObjectSomeValuesFrom(obo:BFO_0000195 :Ecosystem_good))

# Class: :Direct_driver (:Direct_driver)

AnnotationAssertion(skos:definition :Direct_driver "A driver of change that directly and unequivocally influences an ecosystem and its processes.")
AnnotationAssertion(skos:example :Direct_driver "Exploitation")
SubClassOf(:Direct_driver :Driver_of_change)

# Class: :Driver_of_change (:Driver_of_change)

AnnotationAssertion(skos:definition :Driver_of_change "Any natural or human induced factor that directly or indirectly causes a change in an ecosystem.")
AnnotationAssertion(skos:example :Driver_of_change "Global warming, flooding, pollution")
SubClassOf(:Driver_of_change obo:BFO_0000015)
SubClassOf(:Driver_of_change ObjectSomeValuesFrom(:causally_influences :Ecosystem_component))
SubClassOf(:Driver_of_change ObjectSomeValuesFrom(:causally_influences :Ecosystem_good))
SubClassOf(:Driver_of_change ObjectSomeValuesFrom(:causally_upstream_of_with_negative_effect :Ecosystem_process))

# Class: :Economic_activity (:Economic_activity)

AnnotationAssertion(skos:definition :Economic_activity "A human activity involving the production, distribution, exchange or consumption of commodities and services with the goal of meeting human needs and generating monetary instrumental value in the economy.")
AnnotationAssertion(skos:example :Economic_activity "Commercial farming, scuba diving")
SubClassOf(:Economic_activity :Human_activity)
SubClassOf(:Economic_activity ObjectSomeValuesFrom(obo:BFO_0000167 :Economic_actor))

# Class: :Economic_actor (:Economic_actor)

AnnotationAssertion(skos:definition :Economic_actor "An actor who participates in economic activity and who's behaviour and decisions are dependent on economic concerns, ie are tied to monetary considerations.")
AnnotationAssertion(skos:example :Economic_actor "A consumer, a merchant")
SubClassOf(:Economic_actor :Actor)
SubClassOf(:Economic_actor ObjectSomeValuesFrom(obo:BFO_0000166 :Economic_activity))
SubClassOf(:Economic_actor ObjectSomeValuesFrom(:benefits_from :Monetary_instrumental_value))

# Class: :Ecosystem (:Ecosystem)

AnnotationAssertion(skos:definition :Ecosystem "A dynamic complex of plant, animal and micro-organism communities and their non-living environment interacting as a functional unit. Specifically, ecosystems are made up of living components (biotic complexes and assemblages of species), the abiotic environment, the processes and interactions within and between the biotic and abiotic components, and the physical space in which these operate")
SubClassOf(:Ecosystem obo:BFO_0000030)
SubClassOf(:Ecosystem ObjectSomeValuesFrom(obo:BFO_0000183 :Ecosystem_process))
SubClassOf(:Ecosystem ObjectSomeValuesFrom(obo:BFO_0000194 :Ecosystem_service))
SubClassOf(:Ecosystem ObjectSomeValuesFrom(obo:BFO_0000211 :Ecosystem_extent))
SubClassOf(:Ecosystem ObjectSomeValuesFrom(:has_quality :Ecosystem_condition))
SubClassOf(:Ecosystem ObjectSomeValuesFrom(:has_quality :Intrinsic_value))

# Class: :Ecosystem_component (:Ecosystem_component)

AnnotationAssertion(skos:definition :Ecosystem_component "The components that are part of an ecosystem.")
AnnotationAssertion(skos:example :Ecosystem_component "A tree, a fish, a river")
SubClassOf(:Ecosystem_component obo:BFO_0000030)
SubClassOf(:Ecosystem_component ObjectSomeValuesFrom(obo:BFO_0000056 :Ecosystem_process))
SubClassOf(:Ecosystem_component ObjectSomeValuesFrom(obo:BFO_0000137 :Ecosystem))
SubClassOf(:Ecosystem_component ObjectSomeValuesFrom(:has_quality :Intrinsic_value))

# Class: :Ecosystem_condition (:Ecosystem_condition)

AnnotationAssertion(skos:definition :Ecosystem_condition "A measure of the state or health of an ecosystem, characterized by its structure, function, composition, and the ability to sustain biodiversity and provide ecosystem services. It reflects the level of ecological integrity, resilience to disturbances, and the extent to which the ecosystem supports its natural processes and life forms.")
AnnotationAssertion(skos:example :Ecosystem_condition "A healthy ecosystem, a degraded ecosystem")
SubClassOf(:Ecosystem_condition obo:BFO_0000019)
SubClassOf(:Ecosystem_condition ObjectSomeValuesFrom(obo:BFO_0000195 :Ecosystem))

# Class: :Ecosystem_extent (:Ecosystem_extent)

AnnotationAssertion(skos:definition :Ecosystem_extent "The size of an ecosystem, which are contiguous spaces of a specific ecosystem type characterized by a distinct set of biotic and abiotic components and their interactions.")
SubClassOf(:Ecosystem_extent obo:BFO_0000009)

# Class: :Ecosystem_function (:Ecosystem_function)

AnnotationAssertion(skos:definition :Ecosystem_function "They are the subset of ecosystem processes which contribute to human wellbeing through the production of ecosystem goods. Ecosystem functions refer to the broad, overarching roles that ecosystems perform, which support the stability and health of the environment. Functions are often described in terms of their benefits to human societies and the natural world.")
AnnotationAssertion(skos:example :Ecosystem_function "Pollination, primary production")
SubClassOf(:Ecosystem_function :Ecosystem_process)
SubClassOf(:Ecosystem_function ObjectSomeValuesFrom(obo:BFO_0000055 :Ecosystem_service))
SubClassOf(:Ecosystem_function ObjectSomeValuesFrom(:has_output :Ecosystem_good))
SubClassOf(:Ecosystem_function ObjectSomeValuesFrom(:output_of :Ecosystem_process))

# Class: :Ecosystem_good (:Ecosystem_good)

AnnotationAssertion(skos:definition :Ecosystem_good "The output of an ecosystem function before it is used in human activity. Components of nature, directly enjoyed, consumed, or used to yield human well-being. The ecosystem good (i.e., ecological end-product) is a biophysical quality or feature and needs minimal translation for relevance to human well-being.")
AnnotationAssertion(skos:example :Ecosystem_good "Freshwater, harvestable tree, fish")
SubClassOf(:Ecosystem_good obo:BFO_0000030)
SubClassOf(:Ecosystem_good ObjectSomeValuesFrom(obo:BFO_0000056 :Human_activity))
SubClassOf(:Ecosystem_good ObjectSomeValuesFrom(obo:BFO_0000137 <http://purl.obolibrary.org/obo/eso.owl#Ecosystem_good_aggregate>))
SubClassOf(:Ecosystem_good ObjectSomeValuesFrom(:output_of :Ecosystem_process))

# Class: :Ecosystem_process (:Ecosystem_process)

AnnotationAssertion(skos:definition :Ecosystem_process "The flow of energy and materials through the biotic and abiotic components of an ecosystem. Ecosystem processes are the specific mechanisms or actions through which ecosystem functions are achieved. These are the dynamic interactions and transformations that occur within ecosystems, leading to the maintenance and sustainability of ecosystem functions.")
AnnotationAssertion(skos:example :Ecosystem_process "Photosynthesis, predation")
SubClassOf(:Ecosystem_process obo:BFO_0000015)
SubClassOf(:Ecosystem_process ObjectSomeValuesFrom(obo:BFO_0000057 :Ecosystem_component))
SubClassOf(:Ecosystem_process ObjectSomeValuesFrom(obo:BFO_0000066 :Ecosystem))
SubClassOf(:Ecosystem_process ObjectSomeValuesFrom(:has_output :Ecosystem_function))
SubClassOf(:Ecosystem_process ObjectSomeValuesFrom(:has_output <http://purl.obolibrary.org/obo/eso.owl#Ecosystem_good_aggregate>))

# Class: :Ecosystem_service (:Ecosystem_service)

AnnotationAssertion(rdfs:comment :Ecosystem_service "In ESO ecosystem services are roles that ecosystems can bear by virtue of their composition and the processes and functions that arise in them. This role is realised by both the ecosystem function underpinning the service and the human activity that depends on the ecosystem good.")
AnnotationAssertion(skos:definition :Ecosystem_service "A service that is provided by an ecosystem as an intrinsic property of its functionality (e.g. pollination, nutrient cycling, nitrogen fixation, fruit and seed dispersal) contributing to the benefits (and occasionally disbenefits) that people obtain from ecosystems.")
SubClassOf(:Ecosystem_service obo:BFO_0000023)
SubClassOf(:Ecosystem_service ObjectSomeValuesFrom(obo:BFO_0000054 :Ecosystem_function))
SubClassOf(:Ecosystem_service ObjectSomeValuesFrom(obo:BFO_0000054 :Human_activity))
SubClassOf(:Ecosystem_service ObjectSomeValuesFrom(obo:BFO_0000195 :Ecosystem))

# Class: :Enjoyment_value (:Enjoyment_value)

AnnotationAssertion(skos:definition :Enjoyment_value "A non-monetary instrumental value where the achieved end is some form of enjoyment.")
AnnotationAssertion(skos:example :Enjoyment_value "The value of a river in recreational enjoyment")
SubClassOf(:Enjoyment_value :Non_monetary_instrumental_value)

# Class: :Epipelagic_ocean (:Epipelagic_ocean)

AnnotationAssertion(rdfs:comment :Epipelagic_ocean "For additional detailed information refer to Keith, D.A., Ferrer-Paris, J.R., Nicholson, E. and Kingsford, R.T. (eds.) (2020). The IUCN Global Ecosystem Typology 2.0: Descriptive profiles for biomes and ecosystem functional groups. Gland, Switzerland: IUCN.")
AnnotationAssertion(skos:definition :Epipelagic_ocean "The epipelagic or euphotic zone of the open ocean is the uppermost layer that is penetrated by enough light to support photosynthesis.")
AnnotationAssertion(skos:example :Epipelagic_ocean "North Atlantic ocean waters")
SubClassOf(:Epipelagic_ocean :Ecosystem)
SubClassOf(:Epipelagic_ocean ObjectSomeValuesFrom(obo:BFO_0000183 <http://purl.obolibrary.org/obo/eso.owl#Fish_biomass_production>))
SubClassOf(:Epipelagic_ocean ObjectSomeValuesFrom(obo:BFO_0000183 <http://purl.obolibrary.org/obo/eso.owl#Whale_habitat_provisioning>))

# Class: :Exploitation (:Exploitation)

AnnotationAssertion(skos:definition :Exploitation "The consumptive use of any natural resources.")
AnnotationAssertion(skos:example :Exploitation "Overfishing, over hunting")
SubClassOf(:Exploitation :Direct_driver)
SubClassOf(:Exploitation ObjectSomeValuesFrom(:causally_upstream_of_with_negative_effect <http://purl.obolibrary.org/obo/eso.owl#Fish_biomass_production>))

# Class: :Fauna (:Fauna)

AnnotationAssertion(skos:definition :Fauna "Those biotic components that are part of the kingdom Animalia")
AnnotationAssertion(skos:example :Fauna "A dolphin, a chimpanzee, a parrot")
SubClassOf(:Fauna :Biotic_component)

# Class: :Fishing_fleet (:Fishing_fleet)

AnnotationAssertion(skos:example :Fishing_fleet "Is a vessel aggregate where all vessel types are fishing vessels, ie whose primary purpose is to catch fish.")
SubClassOf(:Fishing_fleet :Vessel_fleet)
SubClassOf(:Fishing_fleet ObjectSomeValuesFrom(obo:BFO_0000056 :Commercial_fishing))

# Class: :Flora (:Flora)

AnnotationAssertion(skos:definition :Flora "Those biotic components that are part of the kingdom Plantae")
AnnotationAssertion(skos:example :Flora "A fern, an apple tree")
SubClassOf(:Flora :Biotic_component)

# Class: :Food_value (:Food_value)

AnnotationAssertion(skos:definition :Food_value "A non-monetary instrumental value where the achieved end is a food source.")
AnnotationAssertion(skos:example :Food_value "The value of cereal in contributing to food security, the value of fish as a food source")
SubClassOf(:Food_value :Non_monetary_instrumental_value)

# Class: :Household (:Household)

AnnotationAssertion(skos:definition :Household "A group of individuals residing together and engaging in collective economic activities and decision-making, such as consumption, production, and resource management")
SubClassOf(:Household <http://purl.obolibrary.org/obo/eso.owl#Actor_aggregate>)
SubClassOf(:Household ObjectSomeValuesFrom(:benefits_from :Food_value))

# Class: :Human_activity (:Human_activity)

AnnotationAssertion(skos:definition :Human_activity "Any intentional action or series of actions performed by humans that influence or alter the state of social, economic, or ecological systems, often involving the use of resources, the production of commodities, or the provision of services.")
SubClassOf(:Human_activity obo:BFO_0000015)
SubClassOf(:Human_activity ObjectSomeValuesFrom(obo:BFO_0000055 :Ecosystem_service))
SubClassOf(:Human_activity ObjectSomeValuesFrom(obo:BFO_0000057 :Anthropogenic_asset))
SubClassOf(:Human_activity ObjectSomeValuesFrom(obo:BFO_0000057 :Anthropogenic_asset_aggregate))
SubClassOf(:Human_activity ObjectSomeValuesFrom(obo:BFO_0000057 :Ecosystem_good))
SubClassOf(:Human_activity ObjectSomeValuesFrom(obo:BFO_0000167 :Actor))
SubClassOf(:Human_activity ObjectSomeValuesFrom(:causally_upstream_of :Driver_of_change))
SubClassOf(:Human_activity ObjectSomeValuesFrom(:has_quality ObjectUnionOf(:Instrumental_value :Relational_value)))
SubClassOf(:Human_activity ObjectSomeValuesFrom(<http://purl.obolibrary.org/obo/eso.owl#measure_of> <http://purl.obolibrary.org/obo/eso.owl#EESV_use>))

# Class: :Indirect_driver (:Indirect_driver)

AnnotationAssertion(skos:definition :Indirect_driver "A driver of change that operates diffusely by altering one or more direct drivers.")
AnnotationAssertion(skos:example :Indirect_driver "Climate change")
SubClassOf(:Indirect_driver :Driver_of_change)

# Class: :Instrumental_value (:Instrumental_value)

AnnotationAssertion(rdfs:comment :Instrumental_value "For more, see Pascual, U., Balvanera, P., Díaz, S., Pataki, G., Roth, E., Stenseke, M., Watson, R.T., Dessane, E.B., Islar, M., Kelemen, E. and Maris, V., 2017. Valuing nature’s contributions to people: the IPBES approach. Current opinion in environmental sustainability, 26, pp.7-16.")
AnnotationAssertion(skos:definition :Instrumental_value "The value attributed to something as a means to achieving a particular end")
SubClassOf(:Instrumental_value :Value)
SubClassOf(:Instrumental_value ObjectSomeValuesFrom(<http://purl.obolibrary.org/obo/eso.owl#measure_of> <http://purl.obolibrary.org/obo/eso.owl#EESV_instrumental_value>))

# Class: :Intrinsic_value (:Intrinsic_value)

AnnotationAssertion(rdfs:comment :Intrinsic_value "For more, see Pascual, U., Balvanera, P., Díaz, S., Pataki, G., Roth, E., Stenseke, M., Watson, R.T., Dessane, E.B., Islar, M., Kelemen, E. and Maris, V., 2017. Valuing nature’s contributions to people: the IPBES approach. Current opinion in environmental sustainability, 26, pp.7-16.")
AnnotationAssertion(skos:definition :Intrinsic_value "The inherent value, that is the value something has independent of any human experience or evaluation. Such a value is viewed as an inherent property of the entity and not ascribed or generated by external valuing agents")
AnnotationAssertion(skos:example :Intrinsic_value "Existence value")
SubClassOf(:Intrinsic_value :Value)

# Class: :Monetary_instrumental_value (:Monetary_instrumental_value)

AnnotationAssertion(skos:definition :Monetary_instrumental_value "An instrumental value where the end achieved is monetary gain.")
AnnotationAssertion(skos:example :Monetary_instrumental_value "The value in USD")
SubClassOf(:Monetary_instrumental_value :Instrumental_value)

# Class: :Non_economic_activity (:Non_economic_activity)

AnnotationAssertion(skos:definition :Non_economic_activity "A human activity that serves social, cultural, recreational or environmental purposes and does not involve the production, distribution, or consumption of commodities and services for economic gain.")
AnnotationAssertion(skos:example :Non_economic_activity "Subsistence farming, hiking")
SubClassOf(:Non_economic_activity :Human_activity)
SubClassOf(:Non_economic_activity ObjectSomeValuesFrom(obo:BFO_0000167 :Non_economic_actor))
SubClassOf(:Non_economic_activity ObjectSomeValuesFrom(:has_quality :Non_monetary_instrumental_value))

# Class: :Non_economic_actor (:Non_economic_actor)

AnnotationAssertion(skos:definition :Non_economic_actor "An actor who participates in non-economic activity and who's behaviour and decisions are independent from economic concerns, ie are not tied to monetary considerations.")
SubClassOf(:Non_economic_actor :Actor)
SubClassOf(:Non_economic_actor ObjectSomeValuesFrom(:benefits_from :Non_monetary_instrumental_value))

# Class: :Non_monetary_instrumental_value (:Non_monetary_instrumental_value)

AnnotationAssertion(skos:definition :Non_monetary_instrumental_value "An instrumental value where the end ahieved is not monetary gain.")
SubClassOf(:Non_monetary_instrumental_value :Instrumental_value)

# Class: :Permanent_lowland_rivers (:Permanent_lowland_rivers)

AnnotationAssertion(rdfs:comment :Permanent_lowland_rivers "For additional detailed information refer to Keith, D.A., Ferrer-Paris, J.R., Nicholson, E. and Kingsford, R.T. (eds.) (2020). The IUCN Global Ecosystem Typology 2.0: Descriptive profiles for biomes and ecosystem functional groups. Gland, Switzerland: IUCN.")
AnnotationAssertion(skos:definition :Permanent_lowland_rivers "Small-medium lowland rivers are productive depositional ecosystems with trophic webs that are less diverse than large lowland rivers.")
AnnotationAssertion(skos:example :Permanent_lowland_rivers "Rio Carrao in Venezuela")
SubClassOf(:Permanent_lowland_rivers :Ecosystem)
SubClassOf(:Permanent_lowland_rivers ObjectSomeValuesFrom(obo:BFO_0000183 <http://purl.obolibrary.org/obo/eso.owl#Water_purification>))

# Class: :Pollution (:Pollution)

AnnotationAssertion(skos:definition :Pollution "The introduction of contaminants into the natural environment that cause adverse change.")
AnnotationAssertion(skos:example :Pollution "Heavy metal contamination, air pollution")
SubClassOf(:Pollution :Direct_driver)

# Class: :Provisioning_ecosystem_service (:Provisioning_ecosystem_service)

AnnotationAssertion(skos:definition :Provisioning_ecosystem_service "These are the services that contribute to the products obtained from ecosystems.")
AnnotationAssertion(skos:example :Provisioning_ecosystem_service "Food provisioning services, timber provisioning services, freshwater provisioning services")
SubClassOf(:Provisioning_ecosystem_service :Ecosystem_service)
SubClassOf(:Provisioning_ecosystem_service ObjectSomeValuesFrom(obo:BFO_0000195 :Ecosystem_good))

# Class: :Regulating_ecosystem_service (:Regulating_ecosystem_service)

AnnotationAssertion(skos:definition :Regulating_ecosystem_service "These are the services that contribute to the benefits obtained from the regulation of ecosystem processes.")
AnnotationAssertion(skos:example :Regulating_ecosystem_service "Pollination services, flood prevention services")
SubClassOf(:Regulating_ecosystem_service :Ecosystem_service)

# Class: :Relational_value (:Relational_value)

AnnotationAssertion(rdfs:comment :Relational_value "For more, see Pascual, U., Balvanera, P., Díaz, S., Pataki, G., Roth, E., Stenseke, M., Watson, R.T., Dessane, E.B., Islar, M., Kelemen, E. and Maris, V., 2017. Valuing nature’s contributions to people: the IPBES approach. Current opinion in environmental sustainability, 26, pp.7-16.")
AnnotationAssertion(skos:definition :Relational_value "Values that do not directly emanate from nature but are derivative of our relationships with it and our responsibilities towards it.")
AnnotationAssertion(skos:example :Relational_value "Spiritual value, cultural value")
SubClassOf(:Relational_value :Value)
SubClassOf(:Relational_value ObjectSomeValuesFrom(<http://purl.obolibrary.org/obo/eso.owl#measure_of> <http://purl.obolibrary.org/obo/eso.owl#EESV_relational_value>))

# Class: :Value (:Value)

AnnotationAssertion(skos:definition :Value "A principle associated with a given worldview or cultural context, a preference someone has, the importance of something for itself or for others, or simply as a means to an end.")
SubClassOf(:Value obo:BFO_0000019)

# Class: :Vessel_fleet (:Vessel_fleet)

AnnotationAssertion(skos:definition :Vessel_fleet "Is a material entity consisting exactly of a plurality (≥1) of vessels as member parts which together form a unit.")
AnnotationAssertion(skos:example :Vessel_fleet "A fishing fleet")
SubClassOf(:Vessel_fleet :Anthropogenic_asset_aggregate)

# Class: :Warming (:Warming)

AnnotationAssertion(skos:definition :Warming "The continuous increase in temperature relative to a historical baseline.")
SubClassOf(:Warming :Indirect_driver)

# Class: :Water_quality_regulation_service (:Water_quality_regulation_service)

AnnotationAssertion(skos:definition :Water_quality_regulation_service "The role of an ecosystem in regulating pollutants and excess nutrients to maintain the chemical condition of water to mitigate harmful effects on human health.")
SubClassOf(:Water_quality_regulation_service :Regulating_ecosystem_service)
SubClassOf(:Water_quality_regulation_service ObjectSomeValuesFrom(obo:BFO_0000054 <http://purl.obolibrary.org/obo/eso.owl#Swimming>))
SubClassOf(:Water_quality_regulation_service ObjectSomeValuesFrom(obo:BFO_0000054 <http://purl.obolibrary.org/obo/eso.owl#Water_purification>))

# Class: :Whale_watcher (:Whale_watcher)

AnnotationAssertion(skos:definition :Whale_watcher "A type of economic actor who participates in the whale watching activity as a client.")
SubClassOf(:Whale_watcher :Economic_actor)
SubClassOf(:Whale_watcher ObjectSomeValuesFrom(obo:BFO_0000166 :Whale_watching))
SubClassOf(:Whale_watcher ObjectSomeValuesFrom(:benefits_from :Enjoyment_value))

# Class: :Whale_watching (:Whale_watching)

AnnotationAssertion(skos:definition :Whale_watching "An economic activity that involves the observation of whales.")
SubClassOf(:Whale_watching :Economic_activity)
SubClassOf(:Whale_watching ObjectSomeValuesFrom(obo:BFO_0000055 :Wildlife_viewing_service))
SubClassOf(:Whale_watching ObjectSomeValuesFrom(obo:BFO_0000057 <http://purl.obolibrary.org/obo/eso.owl#Tour_operator>))
SubClassOf(:Whale_watching ObjectSomeValuesFrom(obo:BFO_0000167 :Whalewatching_fleet))
SubClassOf(:Whale_watching ObjectSomeValuesFrom(obo:BFO_0000167 <http://purl.obolibrary.org/obo/eso.owl#Whale_population>))
SubClassOf(:Whale_watching ObjectSomeValuesFrom(:has_quality :Enjoyment_value))
SubClassOf(:Whale_watching ObjectSomeValuesFrom(:has_quality :Monetary_instrumental_value))

# Class: :Whalewatching_fleet (:Whalewatching_fleet)

AnnotationAssertion(skos:example :Whalewatching_fleet "Is a vessel aggregate where all vessel types are whale watching vessels, ie whose primary purpose is to take people to observe whales.")
SubClassOf(:Whalewatching_fleet :Vessel_fleet)
SubClassOf(:Whalewatching_fleet ObjectSomeValuesFrom(obo:BFO_0000056 :Whale_watching))

# Class: :Wild_fish_provisioning_service (:Wild_fish_provisioning_service)

AnnotationAssertion(skos:definition :Wild_fish_provisioning_service "The role of an ecosystem in contributing to the growth of fish and other aquatic biomass that are captured in uncultivated production contexts for various uses, primarily food production.")
SubClassOf(:Wild_fish_provisioning_service :Provisioning_ecosystem_service)
SubClassOf(:Wild_fish_provisioning_service ObjectSomeValuesFrom(obo:BFO_0000054 :Commercial_fishing))
SubClassOf(:Wild_fish_provisioning_service ObjectSomeValuesFrom(obo:BFO_0000054 <http://purl.obolibrary.org/obo/eso.owl#Fish_biomass_production>))

# Class: :Wildcaught_fish (:Wildcaught_fish)

AnnotationAssertion(skos:definition :Wildcaught_fish "Is a material entity consisting exactly of a plurality (≥1) of wild caught fish as member parts which together form a unit.")
AnnotationAssertion(skos:example :Wildcaught_fish "Landed tuna, landed sardines")
SubClassOf(:Wildcaught_fish :Commodity_aggregate)
SubClassOf(:Wildcaught_fish ObjectSomeValuesFrom(:has_quality :Food_value))
SubClassOf(:Wildcaught_fish ObjectSomeValuesFrom(:has_quality :Monetary_instrumental_value))
SubClassOf(:Wildcaught_fish ObjectSomeValuesFrom(:output_of :Commercial_fishing))

# Class: :Wildlife_viewing_service (:Wildlife_viewing_service)

AnnotationAssertion(skos:definition :Wildlife_viewing_service "The role of an ecosystem in enabling people to enjoy wildlife through direct, in-situ, observations.")
SubClassOf(:Wildlife_viewing_service :Cultural_ecosystem_service)
SubClassOf(:Wildlife_viewing_service ObjectSomeValuesFrom(obo:BFO_0000054 :Whale_watching))
SubClassOf(:Wildlife_viewing_service ObjectSomeValuesFrom(obo:BFO_0000054 <http://purl.obolibrary.org/obo/eso.owl#Whale_habitat_provisioning>))

# Class: <http://purl.obolibrary.org/obo/eso.owl#Actor_aggregate> (<http://purl.obolibrary.org/obo/eso.owl#Actor_aggregate>)

AnnotationAssertion(skos:definition <http://purl.obolibrary.org/obo/eso.owl#Actor_aggregate> "Is a material entity consisting exactly of a plurality (≥1) of actors as member parts which together form a unit.")
AnnotationAssertion(skos:example <http://purl.obolibrary.org/obo/eso.owl#Actor_aggregate> "A local community, a group of fishers")
SubClassOf(<http://purl.obolibrary.org/obo/eso.owl#Actor_aggregate> obo:BFO_0000027)
SubClassOf(<http://purl.obolibrary.org/obo/eso.owl#Actor_aggregate> ObjectSomeValuesFrom(obo:BFO_0000174 :Actor))
SubClassOf(<http://purl.obolibrary.org/obo/eso.owl#Actor_aggregate> ObjectSomeValuesFrom(<http://purl.obolibrary.org/obo/eso.owl#measure_of> <http://purl.obolibrary.org/obo/eso.owl#EESV_demand>))

# Class: <http://purl.obolibrary.org/obo/eso.owl#Biological_control> (<http://purl.obolibrary.org/obo/eso.owl#Biological_control>)

AnnotationAssertion(skos:definition <http://purl.obolibrary.org/obo/eso.owl#Biological_control> "The control of pests such as insects, mites, weeds and plant diseases by other organisms.")
SubClassOf(<http://purl.obolibrary.org/obo/eso.owl#Biological_control> :Ecosystem_function)
SubClassOf(<http://purl.obolibrary.org/obo/eso.owl#Biological_control> ObjectSomeValuesFrom(obo:BFO_0000118 <http://purl.obolibrary.org/obo/eso.owl#Predation>))

# Class: <http://purl.obolibrary.org/obo/eso.owl#Biomass_production> (<http://purl.obolibrary.org/obo/eso.owl#Biomass_production>)

AnnotationAssertion(skos:definition <http://purl.obolibrary.org/obo/eso.owl#Biomass_production> "A process involving the generation of organic material through biological growth.")
SubClassOf(<http://purl.obolibrary.org/obo/eso.owl#Biomass_production> :Ecosystem_function)
SubClassOf(<http://purl.obolibrary.org/obo/eso.owl#Biomass_production> ObjectSomeValuesFrom(obo:BFO_0000118 <http://purl.obolibrary.org/obo/eso.owl#Predation>))

# Class: <http://purl.obolibrary.org/obo/eso.owl#Carbon_fixation> (<http://purl.obolibrary.org/obo/eso.owl#Carbon_fixation>)

AnnotationAssertion(skos:definition <http://purl.obolibrary.org/obo/eso.owl#Carbon_fixation> "A biochemical process in which inorganic carbon, typically in the form of carbon dioxide, is converted into organic compounds by living organisms, primarily through photosynthesis.")
SubClassOf(<http://purl.obolibrary.org/obo/eso.owl#Carbon_fixation> :Ecosystem_process)
SubClassOf(<http://purl.obolibrary.org/obo/eso.owl#Carbon_fixation> ObjectSomeValuesFrom(obo:BFO_0000138 <http://purl.obolibrary.org/obo/eso.owl#Net_primary_production>))

# Class: <http://purl.obolibrary.org/obo/eso.owl#Clean_freshwater> (<http://purl.obolibrary.org/obo/eso.owl#Clean_freshwater>)

AnnotationAssertion(skos:definition <http://purl.obolibrary.org/obo/eso.owl#Clean_freshwater> "Water from natural sources, such as rivers, lakes, or aquifers, that is free from harmful contaminants and pollutants, making it safe for consumption, agricultural use, and supporting aquatic ecosystems. It is characterized by low levels of pathogens, chemicals, and physical impurities, ensuring it meets health and environmental standards.")
SubClassOf(<http://purl.obolibrary.org/obo/eso.owl#Clean_freshwater> :Ecosystem_good)
SubClassOf(<http://purl.obolibrary.org/obo/eso.owl#Clean_freshwater> ObjectSomeValuesFrom(obo:BFO_0000056 <http://purl.obolibrary.org/obo/eso.owl#Swimming>))
SubClassOf(<http://purl.obolibrary.org/obo/eso.owl#Clean_freshwater> ObjectSomeValuesFrom(:output_of <http://purl.obolibrary.org/obo/eso.owl#Water_purification>))

# Class: <http://purl.obolibrary.org/obo/eso.owl#Commodity> (<http://purl.obolibrary.org/obo/eso.owl#Commodity>)

AnnotationAssertion(skos:definition <http://purl.obolibrary.org/obo/eso.owl#Commodity> "Marketable product produced as a result of human economic activity.")
AnnotationAssertion(skos:example <http://purl.obolibrary.org/obo/eso.owl#Commodity> "A smoked salmon")
SubClassOf(<http://purl.obolibrary.org/obo/eso.owl#Commodity> obo:BFO_0000030)
SubClassOf(<http://purl.obolibrary.org/obo/eso.owl#Commodity> ObjectSomeValuesFrom(obo:BFO_0000175 :Commodity_aggregate))

# Class: <http://purl.obolibrary.org/obo/eso.owl#Concept> (<http://purl.obolibrary.org/obo/eso.owl#Concept>)

AnnotationAssertion(skos:definition <http://purl.obolibrary.org/obo/eso.owl#Concept> "A concept is an entity that is conceived in the human mind to represent an abstract of generic idea generalised from particular instances.")
AnnotationAssertion(skos:example <http://purl.obolibrary.org/obo/eso.owl#Concept> "A thought, a notion, courage")
SubClassOf(<http://purl.obolibrary.org/obo/eso.owl#Concept> obo:BFO_0000001)

# Class: <http://purl.obolibrary.org/obo/eso.owl#Decomposition> (<http://purl.obolibrary.org/obo/eso.owl#Decomposition>)

AnnotationAssertion(skos:definition <http://purl.obolibrary.org/obo/eso.owl#Decomposition> "Breakdown of complex organic substances into simpler molecules or ions by physical, chemical and/or biological processes.")
SubClassOf(<http://purl.obolibrary.org/obo/eso.owl#Decomposition> :Ecosystem_process)

# Class: <http://purl.obolibrary.org/obo/eso.owl#EESV_anthropogenic_contribution> (<http://purl.obolibrary.org/obo/eso.owl#EESV_anthropogenic_contribution>)

AnnotationAssertion(skos:definition <http://purl.obolibrary.org/obo/eso.owl#EESV_anthropogenic_contribution> "The efforts that humans invest to enhance ecological supply and to make use of ecosystem services.")
AnnotationAssertion(skos:example <http://purl.obolibrary.org/obo/eso.owl#EESV_anthropogenic_contribution> "Infrastructure to access national parks, a fishing fleet, machinery")
SubClassOf(<http://purl.obolibrary.org/obo/eso.owl#EESV_anthropogenic_contribution> <http://purl.obolibrary.org/obo/eso.owl#Essential_ecosystem_service_variable_class>)

# Class: <http://purl.obolibrary.org/obo/eso.owl#EESV_demand> (<http://purl.obolibrary.org/obo/eso.owl#EESV_demand>)

AnnotationAssertion(skos:definition <http://purl.obolibrary.org/obo/eso.owl#EESV_demand> "The explicitly or implicitly expressed human desire or need for an ecosystem service, in terms of its quantity or quality, irrespective of whether awareness exists about such need.")
AnnotationAssertion(skos:example <http://purl.obolibrary.org/obo/eso.owl#EESV_demand> "Population in dependent on a watershed, per capita consumption of a good")
SubClassOf(<http://purl.obolibrary.org/obo/eso.owl#EESV_demand> <http://purl.obolibrary.org/obo/eso.owl#Essential_ecosystem_service_variable_class>)

# Class: <http://purl.obolibrary.org/obo/eso.owl#EESV_ecological_supply> (<http://purl.obolibrary.org/obo/eso.owl#EESV_ecological_supply>)

AnnotationAssertion(skos:definition <http://purl.obolibrary.org/obo/eso.owl#EESV_ecological_supply> "The ecosystem structure and functions that underlie the potential capacity of ecosystems to provide ecosystem services.")
AnnotationAssertion(skos:example <http://purl.obolibrary.org/obo/eso.owl#EESV_ecological_supply> "Fish biomass, pollinator abundance, freshwater supply")
SubClassOf(<http://purl.obolibrary.org/obo/eso.owl#EESV_ecological_supply> <http://purl.obolibrary.org/obo/eso.owl#Essential_ecosystem_service_variable_class>)

# Class: <http://purl.obolibrary.org/obo/eso.owl#EESV_instrumental_value> (<http://purl.obolibrary.org/obo/eso.owl#EESV_instrumental_value>)

AnnotationAssertion(skos:definition <http://purl.obolibrary.org/obo/eso.owl#EESV_instrumental_value> "The importance of an ecosystem service to societies or individuals as a means to achieve a specific end.")
AnnotationAssertion(skos:example <http://purl.obolibrary.org/obo/eso.owl#EESV_instrumental_value> "Income, food, enjoyment")
SubClassOf(<http://purl.obolibrary.org/obo/eso.owl#EESV_instrumental_value> <http://purl.obolibrary.org/obo/eso.owl#Essential_ecosystem_service_variable_class>)

# Class: <http://purl.obolibrary.org/obo/eso.owl#EESV_relational_value> (<http://purl.obolibrary.org/obo/eso.owl#EESV_relational_value>)

AnnotationAssertion(skos:definition <http://purl.obolibrary.org/obo/eso.owl#EESV_relational_value> "The importance ascribed to how ecosystems contribute to desirable and meaningful interactions between humans and nature and between humans in relation to nature.")
AnnotationAssertion(skos:example <http://purl.obolibrary.org/obo/eso.owl#EESV_relational_value> "Cultural practices of stewardship, care, spirituality")
SubClassOf(<http://purl.obolibrary.org/obo/eso.owl#EESV_relational_value> <http://purl.obolibrary.org/obo/eso.owl#Essential_ecosystem_service_variable_class>)

# Class: <http://purl.obolibrary.org/obo/eso.owl#EESV_use> (<http://purl.obolibrary.org/obo/eso.owl#EESV_use>)

AnnotationAssertion(skos:definition <http://purl.obolibrary.org/obo/eso.owl#EESV_use> "The active or passive appropriation of an ecosystem service by people highlights the actual appropriation of benefits from nature.")
AnnotationAssertion(skos:example <http://purl.obolibrary.org/obo/eso.owl#EESV_use> "Harvested crops, recreational experience")
SubClassOf(<http://purl.obolibrary.org/obo/eso.owl#EESV_use> <http://purl.obolibrary.org/obo/eso.owl#Essential_ecosystem_service_variable_class>)

# Class: <http://purl.obolibrary.org/obo/eso.owl#Ecosystem_good_aggregate> (<http://purl.obolibrary.org/obo/eso.owl#Ecosystem_good_aggregate>)

AnnotationAssertion(skos:definition <http://purl.obolibrary.org/obo/eso.owl#Ecosystem_good_aggregate> "Is a material entity consisting exactly of a plurality (≥1) of ecosystem goods as member parts which together form a unit.")
AnnotationAssertion(skos:example <http://purl.obolibrary.org/obo/eso.owl#Ecosystem_good_aggregate> "A population of salmon, a group trees")
SubClassOf(<http://purl.obolibrary.org/obo/eso.owl#Ecosystem_good_aggregate> obo:BFO_0000027)
SubClassOf(<http://purl.obolibrary.org/obo/eso.owl#Ecosystem_good_aggregate> ObjectSomeValuesFrom(obo:BFO_0000056 :Human_activity))
SubClassOf(<http://purl.obolibrary.org/obo/eso.owl#Ecosystem_good_aggregate> ObjectSomeValuesFrom(obo:BFO_0000174 :Ecosystem_good))
SubClassOf(<http://purl.obolibrary.org/obo/eso.owl#Ecosystem_good_aggregate> ObjectSomeValuesFrom(:output_of :Ecosystem_process))
SubClassOf(<http://purl.obolibrary.org/obo/eso.owl#Ecosystem_good_aggregate> ObjectSomeValuesFrom(<http://purl.obolibrary.org/obo/eso.owl#measure_of> <http://purl.obolibrary.org/obo/eso.owl#EESV_ecological_supply>))

# Class: <http://purl.obolibrary.org/obo/eso.owl#Essential_ecosystem_service_variable_class> (<http://purl.obolibrary.org/obo/eso.owl#Essential_ecosystem_service_variable_class>)

AnnotationAssertion(rdfs:comment <http://purl.obolibrary.org/obo/eso.owl#Essential_ecosystem_service_variable_class> "For more see Balvanera, P., Brauman, K.A., Cord, A.F., Drakou, E.G., Geijzendorffer, I.R., Karp, D.S., Martín-López, B., Mwampamba, T.H. and Schröter, M., 2022. Essential ecosystem")
AnnotationAssertion(skos:definition <http://purl.obolibrary.org/obo/eso.owl#Essential_ecosystem_service_variable_class> "EESV classes represent shared and grouped key attributes for all ecosystem services to be monitored across space and time.")
SubClassOf(<http://purl.obolibrary.org/obo/eso.owl#Essential_ecosystem_service_variable_class> <http://purl.obolibrary.org/obo/eso.owl#Concept>)

# Class: <http://purl.obolibrary.org/obo/eso.owl#Fish_biomass_production> (<http://purl.obolibrary.org/obo/eso.owl#Fish_biomass_production>)

AnnotationAssertion(skos:definition <http://purl.obolibrary.org/obo/eso.owl#Fish_biomass_production> "The generation of fish biomass through predation and other ecological processes.")
SubClassOf(<http://purl.obolibrary.org/obo/eso.owl#Fish_biomass_production> <http://purl.obolibrary.org/obo/eso.owl#Biomass_production>)
SubClassOf(<http://purl.obolibrary.org/obo/eso.owl#Fish_biomass_production> ObjectSomeValuesFrom(obo:BFO_0000055 :Wild_fish_provisioning_service))
SubClassOf(<http://purl.obolibrary.org/obo/eso.owl#Fish_biomass_production> ObjectSomeValuesFrom(obo:BFO_0000066 :Epipelagic_ocean))
SubClassOf(<http://purl.obolibrary.org/obo/eso.owl#Fish_biomass_production> ObjectSomeValuesFrom(:has_output <http://purl.obolibrary.org/obo/eso.owl#Fish_population>))

# Class: <http://purl.obolibrary.org/obo/eso.owl#Fish_population> (<http://purl.obolibrary.org/obo/eso.owl#Fish_population>)

AnnotationAssertion(skos:definition <http://purl.obolibrary.org/obo/eso.owl#Fish_population> "Is a material entity consisting exactly of a plurality (≥1) of fish as member parts which together form a unit.")
AnnotationAssertion(skos:example <http://purl.obolibrary.org/obo/eso.owl#Fish_population> "Salmon population")
SubClassOf(<http://purl.obolibrary.org/obo/eso.owl#Fish_population> <http://purl.obolibrary.org/obo/eso.owl#Ecosystem_good_aggregate>)
SubClassOf(<http://purl.obolibrary.org/obo/eso.owl#Fish_population> ObjectSomeValuesFrom(obo:BFO_0000056 :Commercial_fishing))

# Class: <http://purl.obolibrary.org/obo/eso.owl#Habitat_provisioning> (<http://purl.obolibrary.org/obo/eso.owl#Habitat_provisioning>)

AnnotationAssertion(skos:definition <http://purl.obolibrary.org/obo/eso.owl#Habitat_provisioning> "The provision of living space for resident and migratory species.")
SubClassOf(<http://purl.obolibrary.org/obo/eso.owl#Habitat_provisioning> :Ecosystem_function)
SubClassOf(<http://purl.obolibrary.org/obo/eso.owl#Habitat_provisioning> ObjectSomeValuesFrom(obo:BFO_0000118 <http://purl.obolibrary.org/obo/eso.owl#Predation>))

# Class: <http://purl.obolibrary.org/obo/eso.owl#Infrastructure> (<http://purl.obolibrary.org/obo/eso.owl#Infrastructure>)

AnnotationAssertion(skos:definition <http://purl.obolibrary.org/obo/eso.owl#Infrastructure> "A type of anthropogenic asset comprising the physical and organizational systems designed and constructed by humans to support societal functions, economic activities, and the provision of services.")
AnnotationAssertion(skos:example <http://purl.obolibrary.org/obo/eso.owl#Infrastructure> "A road, a sea wall, a bridge")
SubClassOf(<http://purl.obolibrary.org/obo/eso.owl#Infrastructure> :Anthropogenic_asset)

# Class: <http://purl.obolibrary.org/obo/eso.owl#Net_primary_production> (<http://purl.obolibrary.org/obo/eso.owl#Net_primary_production>)

AnnotationAssertion(skos:definition <http://purl.obolibrary.org/obo/eso.owl#Net_primary_production> "The total mass of carbon taken out of the atmosphere by plant photosynthesis (Gross Primary Production) minus return to the atmosphere of carbon due to autotrophic respiration.")
SubClassOf(<http://purl.obolibrary.org/obo/eso.owl#Net_primary_production> :Ecosystem_function)
SubClassOf(<http://purl.obolibrary.org/obo/eso.owl#Net_primary_production> ObjectSomeValuesFrom(obo:BFO_0000118 <http://purl.obolibrary.org/obo/eso.owl#Carbon_fixation>))
SubClassOf(<http://purl.obolibrary.org/obo/eso.owl#Net_primary_production> ObjectSomeValuesFrom(obo:BFO_0000118 <http://purl.obolibrary.org/obo/eso.owl#Photosynthesis>))

# Class: <http://purl.obolibrary.org/obo/eso.owl#Nutrient_cycling> (<http://purl.obolibrary.org/obo/eso.owl#Nutrient_cycling>)

AnnotationAssertion(skos:definition <http://purl.obolibrary.org/obo/eso.owl#Nutrient_cycling> "The processes by which elements are extracted from their mineral, aquatic, or atmospheric sources or recycled from their organic forms, converting them to the ionic form in which biotic uptake occurs and ultimately returning them to the atmosphere, water, or soil.")
SubClassOf(<http://purl.obolibrary.org/obo/eso.owl#Nutrient_cycling> :Ecosystem_function)

# Class: <http://purl.obolibrary.org/obo/eso.owl#Photosynthesis> (<http://purl.obolibrary.org/obo/eso.owl#Photosynthesis>)

AnnotationAssertion(skos:definition <http://purl.obolibrary.org/obo/eso.owl#Photosynthesis> "The metabolic pathways for CO2 fixation by plants.")
SubClassOf(<http://purl.obolibrary.org/obo/eso.owl#Photosynthesis> :Ecosystem_process)
SubClassOf(<http://purl.obolibrary.org/obo/eso.owl#Photosynthesis> ObjectSomeValuesFrom(obo:BFO_0000138 <http://purl.obolibrary.org/obo/eso.owl#Net_primary_production>))

# Class: <http://purl.obolibrary.org/obo/eso.owl#Predation> (<http://purl.obolibrary.org/obo/eso.owl#Predation>)

AnnotationAssertion(skos:definition <http://purl.obolibrary.org/obo/eso.owl#Predation> "A biological process in which one organism, the predator, hunts, captures, and consumes another organism, the prey, as a means of obtaining energy and nutrients.")
SubClassOf(<http://purl.obolibrary.org/obo/eso.owl#Predation> :Ecosystem_process)
SubClassOf(<http://purl.obolibrary.org/obo/eso.owl#Predation> ObjectSomeValuesFrom(obo:BFO_0000138 <http://purl.obolibrary.org/obo/eso.owl#Biological_control>))
SubClassOf(<http://purl.obolibrary.org/obo/eso.owl#Predation> ObjectSomeValuesFrom(obo:BFO_0000138 <http://purl.obolibrary.org/obo/eso.owl#Biomass_production>))
SubClassOf(<http://purl.obolibrary.org/obo/eso.owl#Predation> ObjectSomeValuesFrom(obo:BFO_0000138 <http://purl.obolibrary.org/obo/eso.owl#Habitat_provisioning>))

# Class: <http://purl.obolibrary.org/obo/eso.owl#Reproduction> (<http://purl.obolibrary.org/obo/eso.owl#Reproduction>)

AnnotationAssertion(skos:definition <http://purl.obolibrary.org/obo/eso.owl#Reproduction> "A biological process by which organisms produce offspring, ensuring the continuation of their species to pass on genetic material to the next generation.")
AnnotationAssertion(skos:example <http://purl.obolibrary.org/obo/eso.owl#Reproduction> "Sexual reproduction, asexual reproduction")
SubClassOf(<http://purl.obolibrary.org/obo/eso.owl#Reproduction> :Ecosystem_process)

# Class: <http://purl.obolibrary.org/obo/eso.owl#River_access_infrastructure> (<http://purl.obolibrary.org/obo/eso.owl#River_access_infrastructure>)

AnnotationAssertion(skos:definition <http://purl.obolibrary.org/obo/eso.owl#River_access_infrastructure> "A type of infrastrucure specifically designed to support human activities requiring river access.")
AnnotationAssertion(skos:example <http://purl.obolibrary.org/obo/eso.owl#River_access_infrastructure> "A potoon, a boat launch, a road to the river")
SubClassOf(<http://purl.obolibrary.org/obo/eso.owl#River_access_infrastructure> <http://purl.obolibrary.org/obo/eso.owl#Infrastructure>)
SubClassOf(<http://purl.obolibrary.org/obo/eso.owl#River_access_infrastructure> ObjectSomeValuesFrom(obo:BFO_0000056 <http://purl.obolibrary.org/obo/eso.owl#Swimming>))

# Class: <http://purl.obolibrary.org/obo/eso.owl#Swimmer> (<http://purl.obolibrary.org/obo/eso.owl#Swimmer>)

AnnotationAssertion(skos:definition <http://purl.obolibrary.org/obo/eso.owl#Swimmer> "A type of non-economic actor who participates in the swimming activity.")
SubClassOf(<http://purl.obolibrary.org/obo/eso.owl#Swimmer> :Non_economic_actor)
SubClassOf(<http://purl.obolibrary.org/obo/eso.owl#Swimmer> ObjectSomeValuesFrom(obo:BFO_0000166 <http://purl.obolibrary.org/obo/eso.owl#Swimming>))
SubClassOf(<http://purl.obolibrary.org/obo/eso.owl#Swimmer> ObjectSomeValuesFrom(:benefits_from :Enjoyment_value))

# Class: <http://purl.obolibrary.org/obo/eso.owl#Swimming> (<http://purl.obolibrary.org/obo/eso.owl#Swimming>)

AnnotationAssertion(skos:definition <http://purl.obolibrary.org/obo/eso.owl#Swimming> "A non-economic activity that involves the act of swimming for the purpose of recreation without revenue generation")
SubClassOf(<http://purl.obolibrary.org/obo/eso.owl#Swimming> :Non_economic_activity)
SubClassOf(<http://purl.obolibrary.org/obo/eso.owl#Swimming> ObjectSomeValuesFrom(obo:BFO_0000055 :Water_quality_regulation_service))
SubClassOf(<http://purl.obolibrary.org/obo/eso.owl#Swimming> ObjectSomeValuesFrom(obo:BFO_0000057 <http://purl.obolibrary.org/obo/eso.owl#River_access_infrastructure>))
SubClassOf(<http://purl.obolibrary.org/obo/eso.owl#Swimming> ObjectSomeValuesFrom(obo:BFO_0000167 <http://purl.obolibrary.org/obo/eso.owl#Clean_freshwater>))
SubClassOf(<http://purl.obolibrary.org/obo/eso.owl#Swimming> ObjectSomeValuesFrom(obo:BFO_0000167 <http://purl.obolibrary.org/obo/eso.owl#Swimmer>))
SubClassOf(<http://purl.obolibrary.org/obo/eso.owl#Swimming> ObjectSomeValuesFrom(:has_quality :Enjoyment_value))

# Class: <http://purl.obolibrary.org/obo/eso.owl#Tour_operator> (<http://purl.obolibrary.org/obo/eso.owl#Tour_operator>)

AnnotationAssertion(skos:definition <http://purl.obolibrary.org/obo/eso.owl#Tour_operator> "A type of economic actor who participates in a touristic activity as a provider.")
AnnotationAssertion(skos:example <http://purl.obolibrary.org/obo/eso.owl#Tour_operator> "A whale watching tour operator.")
SubClassOf(<http://purl.obolibrary.org/obo/eso.owl#Tour_operator> :Economic_actor)
SubClassOf(<http://purl.obolibrary.org/obo/eso.owl#Tour_operator> ObjectSomeValuesFrom(obo:BFO_0000056 :Whale_watching))
SubClassOf(<http://purl.obolibrary.org/obo/eso.owl#Tour_operator> ObjectSomeValuesFrom(:benefits_from :Monetary_instrumental_value))

# Class: <http://purl.obolibrary.org/obo/eso.owl#Water_purification> (<http://purl.obolibrary.org/obo/eso.owl#Water_purification>)

AnnotationAssertion(skos:definition <http://purl.obolibrary.org/obo/eso.owl#Water_purification> "The removal of sediments and nutrients and other impurities from water.")
SubClassOf(<http://purl.obolibrary.org/obo/eso.owl#Water_purification> :Ecosystem_function)
SubClassOf(<http://purl.obolibrary.org/obo/eso.owl#Water_purification> ObjectSomeValuesFrom(obo:BFO_0000055 :Water_quality_regulation_service))
SubClassOf(<http://purl.obolibrary.org/obo/eso.owl#Water_purification> ObjectSomeValuesFrom(obo:BFO_0000066 :Permanent_lowland_rivers))
SubClassOf(<http://purl.obolibrary.org/obo/eso.owl#Water_purification> ObjectSomeValuesFrom(:has_output <http://purl.obolibrary.org/obo/eso.owl#Clean_freshwater>))

# Class: <http://purl.obolibrary.org/obo/eso.owl#Whale_habitat_provisioning> (<http://purl.obolibrary.org/obo/eso.owl#Whale_habitat_provisioning>)

AnnotationAssertion(skos:definition <http://purl.obolibrary.org/obo/eso.owl#Whale_habitat_provisioning> "The provision of living space for whale species")
SubClassOf(<http://purl.obolibrary.org/obo/eso.owl#Whale_habitat_provisioning> <http://purl.obolibrary.org/obo/eso.owl#Habitat_provisioning>)
SubClassOf(<http://purl.obolibrary.org/obo/eso.owl#Whale_habitat_provisioning> ObjectSomeValuesFrom(obo:BFO_0000055 :Wildlife_viewing_service))
SubClassOf(<http://purl.obolibrary.org/obo/eso.owl#Whale_habitat_provisioning> ObjectSomeValuesFrom(obo:BFO_0000066 :Epipelagic_ocean))
SubClassOf(<http://purl.obolibrary.org/obo/eso.owl#Whale_habitat_provisioning> ObjectSomeValuesFrom(:has_output <http://purl.obolibrary.org/obo/eso.owl#Whale_population>))

# Class: <http://purl.obolibrary.org/obo/eso.owl#Whale_population> (<http://purl.obolibrary.org/obo/eso.owl#Whale_population>)

AnnotationAssertion(skos:definition <http://purl.obolibrary.org/obo/eso.owl#Whale_population> "Is a material entity consisting exactly of a plurality (≥1) of whales as member parts which together form a unit.")
AnnotationAssertion(skos:example <http://purl.obolibrary.org/obo/eso.owl#Whale_population> "Orca population")
SubClassOf(<http://purl.obolibrary.org/obo/eso.owl#Whale_population> <http://purl.obolibrary.org/obo/eso.owl#Ecosystem_good_aggregate>)
SubClassOf(<http://purl.obolibrary.org/obo/eso.owl#Whale_population> ObjectSomeValuesFrom(obo:BFO_0000056 :Whale_watching))
SubClassOf(<http://purl.obolibrary.org/obo/eso.owl#Whale_population> ObjectSomeValuesFrom(:output_of <http://purl.obolibrary.org/obo/eso.owl#Whale_habitat_provisioning>))


DisjointClasses(obo:BFO_0000008 obo:BFO_0000011 obo:BFO_0000015 obo:BFO_0000035)
DisjointClasses(obo:BFO_0000009 obo:BFO_0000018 obo:BFO_0000026 obo:BFO_0000028)
)