<?xml version="1.0"?>
<rdf:RDF xmlns="http://purl.obolibrary.org/obo/esmo.owl#"
     xml:base="http://purl.obolibrary.org/obo/esmo.owl"
     xmlns:dc="http://purl.org/dc/elements/1.1/"
     xmlns:owl="http://www.w3.org/2002/07/owl#"
     xmlns:rdf="http://www.w3.org/1999/02/22-rdf-syntax-ns#"
     xmlns:xml="http://www.w3.org/XML/1998/namespace"
     xmlns:xsd="http://www.w3.org/2001/XMLSchema#"
     xmlns:rdfs="http://www.w3.org/2000/01/rdf-schema#"
     xmlns:skos="http://www.w3.org/2004/02/skos/core#">
    <owl:Ontology rdf:about="http://purl.obolibrary.org/obo/esmo.owl">
        <owl:versionIRI rdf:resource="http://purl.obolibrary.org/obo/esmo.owl"/>
        <dc:contributor>Flavio Affinito</dc:contributor>
        <dc:license rdf:resource="https://creativecommons.org/licenses/by/4.0/"/>
        <rdfs:label>ESMO 2024</rdfs:label>
    </owl:Ontology>
    


    <!-- 
    ///////////////////////////////////////////////////////////////////////////////////////
    //
    // Annotation properties
    //
    ///////////////////////////////////////////////////////////////////////////////////////
     -->

    


    <!-- http://purl.org/dc/elements/1.1/contributor -->

    <owl:AnnotationProperty rdf:about="http://purl.org/dc/elements/1.1/contributor"/>
    


    <!-- http://purl.org/dc/elements/1.1/identifier -->

    <owl:AnnotationProperty rdf:about="http://purl.org/dc/elements/1.1/identifier"/>
    


    <!-- http://purl.org/dc/elements/1.1/license -->

    <owl:AnnotationProperty rdf:about="http://purl.org/dc/elements/1.1/license"/>
    


    <!-- http://www.w3.org/2004/02/skos/core#altLabel -->

    <owl:AnnotationProperty rdf:about="http://www.w3.org/2004/02/skos/core#altLabel"/>
    


    <!-- http://www.w3.org/2004/02/skos/core#definition -->

    <owl:AnnotationProperty rdf:about="http://www.w3.org/2004/02/skos/core#definition"/>
    


    <!-- http://www.w3.org/2004/02/skos/core#example -->

    <owl:AnnotationProperty rdf:about="http://www.w3.org/2004/02/skos/core#example"/>
    


    <!-- http://www.w3.org/2004/02/skos/core#prefLabel -->

    <owl:AnnotationProperty rdf:about="http://www.w3.org/2004/02/skos/core#prefLabel"/>
    


    <!-- http://www.w3.org/2004/02/skos/core#scopeNote -->

    <owl:AnnotationProperty rdf:about="http://www.w3.org/2004/02/skos/core#scopeNote"/>
    


    <!-- 
    ///////////////////////////////////////////////////////////////////////////////////////
    //
    // Object Properties
    //
    ///////////////////////////////////////////////////////////////////////////////////////
     -->

    


    <!-- http://purl.obolibrary.org/obo/BFO_0000054 -->

    <owl:ObjectProperty rdf:about="http://purl.obolibrary.org/obo/BFO_0000054">
        <owl:inverseOf rdf:resource="http://purl.obolibrary.org/obo/BFO_0000055"/>
        <rdfs:domain rdf:resource="http://purl.obolibrary.org/obo/BFO_0000017"/>
        <rdfs:range rdf:resource="http://purl.obolibrary.org/obo/BFO_0000015"/>
        <dc:identifier>206-BFO</dc:identifier>
        <rdfs:label xml:lang="en">has realization</rdfs:label>
        <skos:definition xml:lang="en">b has realization c =Def c realizes b</skos:definition>
        <skos:example xml:lang="en">As for realizes</skos:example>
        <skos:prefLabel xml:lang="en">has realization</skos:prefLabel>
    </owl:ObjectProperty>
    


    <!-- http://purl.obolibrary.org/obo/BFO_0000055 -->

    <owl:ObjectProperty rdf:about="http://purl.obolibrary.org/obo/BFO_0000055">
        <rdfs:domain rdf:resource="http://purl.obolibrary.org/obo/BFO_0000015"/>
        <rdfs:range rdf:resource="http://purl.obolibrary.org/obo/BFO_0000017"/>
        <dc:identifier>059-BFO</dc:identifier>
        <rdfs:label xml:lang="en">realizes</rdfs:label>
        <skos:definition xml:lang="en">(Elucidation) b realizes c means: b is a process &amp; c is a realizable entity that inheres in d &amp; for all t, if b has participant d at t then c exists at t &amp; the type instantiated by b is correlated with the type instantiated by c</skos:definition>
        <skos:example xml:lang="en">A disposition to go bald is realized in a balding process; a role of student is realized in studying processes; the pumping function of a heart is realized in processes of pumping.</skos:example>
        <skos:prefLabel xml:lang="en">realizes</skos:prefLabel>
    </owl:ObjectProperty>
    


    <!-- http://purl.obolibrary.org/obo/BFO_0000056 -->

    <owl:ObjectProperty rdf:about="http://purl.obolibrary.org/obo/BFO_0000056">
        <owl:inverseOf rdf:resource="http://purl.obolibrary.org/obo/BFO_0000057"/>
        <rdfs:range rdf:resource="http://purl.obolibrary.org/obo/BFO_0000015"/>
        <dc:identifier>250-BFO</dc:identifier>
        <rdfs:label xml:lang="en">participates in at some time</rdfs:label>
        <skos:definition xml:lang="en">b participates in p at some time =Def for some time t (p has participant b at t)</skos:definition>
        <skos:prefLabel xml:lang="en">participates in at some time</skos:prefLabel>
    </owl:ObjectProperty>
    


    <!-- http://purl.obolibrary.org/obo/BFO_0000057 -->

    <owl:ObjectProperty rdf:about="http://purl.obolibrary.org/obo/BFO_0000057">
        <rdfs:domain rdf:resource="http://purl.obolibrary.org/obo/BFO_0000015"/>
        <dc:identifier>248-BFO</dc:identifier>
        <rdfs:label xml:lang="en">has participant at some time</rdfs:label>
        <skos:definition xml:lang="en">p has participant c at some time =Def for some time t (p is a process, c is a continuant, and c participates in p some way at t)</skos:definition>
        <skos:prefLabel xml:lang="en">has participant at some time</skos:prefLabel>
    </owl:ObjectProperty>
    


    <!-- http://purl.obolibrary.org/obo/BFO_0000062 -->

    <owl:ObjectProperty rdf:about="http://purl.obolibrary.org/obo/BFO_0000062">
        <owl:inverseOf rdf:resource="http://purl.obolibrary.org/obo/BFO_0000063"/>
        <rdf:type rdf:resource="http://www.w3.org/2002/07/owl#TransitiveProperty"/>
        <rdfs:domain rdf:resource="http://purl.obolibrary.org/obo/BFO_0000003"/>
        <rdfs:range rdf:resource="http://purl.obolibrary.org/obo/BFO_0000003"/>
        <dc:identifier>213-BFO</dc:identifier>
        <rdfs:label xml:lang="en">preceded by</rdfs:label>
        <skos:definition xml:lang="en">b preceded by c =Def b precedes c</skos:definition>
        <skos:example xml:lang="en">The temporal region occupied by the second half of the match is preceded by the temporal region occupied by the first half of the match.</skos:example>
        <skos:prefLabel xml:lang="en">preceded by</skos:prefLabel>
    </owl:ObjectProperty>
    


    <!-- http://purl.obolibrary.org/obo/BFO_0000063 -->

    <owl:ObjectProperty rdf:about="http://purl.obolibrary.org/obo/BFO_0000063">
        <rdf:type rdf:resource="http://www.w3.org/2002/07/owl#TransitiveProperty"/>
        <rdfs:domain rdf:resource="http://purl.obolibrary.org/obo/BFO_0000003"/>
        <rdfs:range rdf:resource="http://purl.obolibrary.org/obo/BFO_0000003"/>
        <dc:identifier>270-BFO</dc:identifier>
        <rdfs:label xml:lang="en">precedes</rdfs:label>
        <skos:definition xml:lang="en">(Elucidation) If o, o&apos; are occurrents and t is the temporal extent of o and t&apos; is the temporal extent of o&apos; then o precedes o&apos; means: either last instant of o is before first instant of o&apos;  or last instant of o = first instant of o&apos; and neither o nor o&apos; are temporal instants</skos:definition>
        <skos:example xml:lang="en">The temporal region occupied by Mary&apos;s birth precedes the temporal region occupied by Mary&apos;s death. NOTE 1: Each temporal region is its own temporal extent. The temporal extent of a spatiotemporal region is the temporal region it temporally projects onto. The temporal extent of a process or process boundary that occupies temporal region t is t. NOTE 2: Precedes defines a strict partial order on occurrents.</skos:example>
        <skos:prefLabel xml:lang="en">precedes</skos:prefLabel>
    </owl:ObjectProperty>
    


    <!-- http://purl.obolibrary.org/obo/BFO_0000066 -->

    <owl:ObjectProperty rdf:about="http://purl.obolibrary.org/obo/BFO_0000066">
        <owl:inverseOf rdf:resource="http://purl.obolibrary.org/obo/BFO_0000183"/>
        <rdfs:domain>
            <owl:Class>
                <owl:unionOf rdf:parseType="Collection">
                    <rdf:Description rdf:about="http://purl.obolibrary.org/obo/BFO_0000015"/>
                    <rdf:Description rdf:about="http://purl.obolibrary.org/obo/BFO_0000035"/>
                </owl:unionOf>
            </owl:Class>
        </rdfs:domain>
        <rdfs:range>
            <owl:Class>
                <owl:unionOf rdf:parseType="Collection">
                    <rdf:Description rdf:about="http://purl.obolibrary.org/obo/BFO_0000029"/>
                    <rdf:Description rdf:about="http://purl.obolibrary.org/obo/BFO_0000040"/>
                </owl:unionOf>
            </owl:Class>
        </rdfs:range>
        <dc:identifier>143-BFO</dc:identifier>
        <rdfs:label xml:lang="en">occurs in</rdfs:label>
        <skos:definition xml:lang="en">b occurs in c =Def b is a process or a process boundary and c is a material entity or immaterial entity &amp; there exists a spatiotemporal region r and b occupies spatiotemporal region r &amp; for all t, if b exists at t then c exists at t &amp; there exist spatial regions s and s&apos; where b spatially projects onto s at t &amp; c occupies spatial region s&apos; at t &amp; s is a continuant part of s&apos; at t</skos:definition>
        <skos:example xml:lang="en">A process of digestion occurs in the interior of an organism, a process of loading artillery rounds into a tank cannon occurs in the interior of the tank.</skos:example>
        <skos:prefLabel xml:lang="en">occurs in</skos:prefLabel>
    </owl:ObjectProperty>
    


    <!-- http://purl.obolibrary.org/obo/BFO_0000082 -->

    <owl:ObjectProperty rdf:about="http://purl.obolibrary.org/obo/BFO_0000082">
        <rdfs:subPropertyOf rdf:resource="http://purl.obolibrary.org/obo/BFO_0000171"/>
        <rdf:type rdf:resource="http://www.w3.org/2002/07/owl#TransitiveProperty"/>
        <rdfs:domain>
            <owl:Class>
                <owl:intersectionOf rdf:parseType="Collection">
                    <rdf:Description rdf:about="http://purl.obolibrary.org/obo/BFO_0000004"/>
                    <owl:Class>
                        <owl:complementOf rdf:resource="http://purl.obolibrary.org/obo/BFO_0000006"/>
                    </owl:Class>
                </owl:intersectionOf>
            </owl:Class>
        </rdfs:domain>
        <rdfs:range>
            <owl:Class>
                <owl:intersectionOf rdf:parseType="Collection">
                    <rdf:Description rdf:about="http://purl.obolibrary.org/obo/BFO_0000004"/>
                    <owl:Class>
                        <owl:complementOf rdf:resource="http://purl.obolibrary.org/obo/BFO_0000006"/>
                    </owl:Class>
                </owl:intersectionOf>
            </owl:Class>
        </rdfs:range>
        <dc:identifier>235-BFO</dc:identifier>
        <rdfs:label xml:lang="en">located in at all times</rdfs:label>
        <skos:definition xml:lang="en">b located in c at all times =Def for all times t, b exists at t implies (b and c are independent continuants and not spatial regions, and the spatial region which b occupies at t is a (proper or improper) continuant part of the spatial region which c occupies at t)</skos:definition>
        <skos:prefLabel xml:lang="en">located in at all times</skos:prefLabel>
    </owl:ObjectProperty>
    


    <!-- http://purl.obolibrary.org/obo/BFO_0000108 -->

    <owl:ObjectProperty rdf:about="http://purl.obolibrary.org/obo/BFO_0000108">
        <dc:identifier>118-BFO</dc:identifier>
        <rdfs:label xml:lang="en">exists at</rdfs:label>
        <skos:definition xml:lang="en">(Elucidation) exists at is a relation between a particular and some temporal region at which the particular exists</skos:definition>
        <skos:example xml:lang="en">First World War exists at 1914-1916, Mexico exists at January 1, 2000.</skos:example>
        <skos:prefLabel xml:lang="en">exists at</skos:prefLabel>
    </owl:ObjectProperty>
    


    <!-- http://purl.obolibrary.org/obo/BFO_0000110 -->

    <owl:ObjectProperty rdf:about="http://purl.obolibrary.org/obo/BFO_0000110">
        <rdfs:subPropertyOf rdf:resource="http://purl.obolibrary.org/obo/BFO_0000178"/>
        <rdfs:domain rdf:resource="http://purl.obolibrary.org/obo/BFO_0000002"/>
        <rdfs:range rdf:resource="http://purl.obolibrary.org/obo/BFO_0000002"/>
        <dc:identifier>223-BFO</dc:identifier>
        <rdfs:label xml:lang="en">has continuant part at all times</rdfs:label>
        <skos:definition xml:lang="en">b has continuant part c at all times =Def for all times t, b exists at t implies (b and c are continuants &amp; b is a part of c at t)</skos:definition>
        <skos:prefLabel xml:lang="en">has continuant part at all times</skos:prefLabel>
    </owl:ObjectProperty>
    


    <!-- http://purl.obolibrary.org/obo/BFO_0000111 -->

    <owl:ObjectProperty rdf:about="http://purl.obolibrary.org/obo/BFO_0000111">
        <rdfs:subPropertyOf rdf:resource="http://purl.obolibrary.org/obo/BFO_0000110"/>
        <rdfs:subPropertyOf rdf:resource="http://purl.obolibrary.org/obo/BFO_0000174"/>
        <rdfs:domain rdf:resource="http://purl.obolibrary.org/obo/BFO_0000002"/>
        <rdfs:range rdf:resource="http://purl.obolibrary.org/obo/BFO_0000002"/>
        <dc:identifier>227-BFO</dc:identifier>
        <rdfs:label xml:lang="en">has proper continuant part at all times</rdfs:label>
        <skos:definition xml:lang="en">b has proper continuant part c at all times =Def c proper continuant part of b at all times</skos:definition>
        <skos:prefLabel xml:lang="en">has proper continuant part at all times</skos:prefLabel>
    </owl:ObjectProperty>
    


    <!-- http://purl.obolibrary.org/obo/BFO_0000113 -->

    <owl:ObjectProperty rdf:about="http://purl.obolibrary.org/obo/BFO_0000113">
        <rdfs:subPropertyOf rdf:resource="http://purl.obolibrary.org/obo/BFO_0000218"/>
        <rdfs:range rdf:resource="http://purl.obolibrary.org/obo/BFO_0000040"/>
        <dc:identifier>243-BFO</dc:identifier>
        <rdfs:label xml:lang="en">has material basis at all times</rdfs:label>
        <skos:definition xml:lang="en">b has material basis c at all times =Def For all times t, b exists at t implies (b is a disposition &amp; c is a material entity &amp; there is some d bearer of b &amp; c continuant part of d at t &amp; d has disposition b because c continuant part of d at t)</skos:definition>
        <skos:prefLabel xml:lang="en">has material basis at all times</skos:prefLabel>
    </owl:ObjectProperty>
    


    <!-- http://purl.obolibrary.org/obo/BFO_0000115 -->

    <owl:ObjectProperty rdf:about="http://purl.obolibrary.org/obo/BFO_0000115">
        <rdfs:subPropertyOf rdf:resource="http://purl.obolibrary.org/obo/BFO_0000178"/>
        <owl:inverseOf rdf:resource="http://purl.obolibrary.org/obo/BFO_0000129"/>
        <rdfs:domain rdf:resource="http://purl.obolibrary.org/obo/BFO_0000040"/>
        <rdfs:range rdf:resource="http://purl.obolibrary.org/obo/BFO_0000040"/>
        <dc:identifier>230-BFO</dc:identifier>
        <rdfs:label xml:lang="en">has member part at some time</rdfs:label>
        <skos:definition xml:lang="en">b has member part c at some time =Def for some time t (c member part of b at t)</skos:definition>
        <skos:prefLabel xml:lang="en">has member part at some time</skos:prefLabel>
    </owl:ObjectProperty>
    


    <!-- http://purl.obolibrary.org/obo/BFO_0000117 -->

    <owl:ObjectProperty rdf:about="http://purl.obolibrary.org/obo/BFO_0000117">
        <owl:inverseOf rdf:resource="http://purl.obolibrary.org/obo/BFO_0000132"/>
        <rdf:type rdf:resource="http://www.w3.org/2002/07/owl#TransitiveProperty"/>
        <rdfs:domain rdf:resource="http://purl.obolibrary.org/obo/BFO_0000003"/>
        <rdfs:range rdf:resource="http://purl.obolibrary.org/obo/BFO_0000003"/>
        <dc:identifier>202-BFO</dc:identifier>
        <rdfs:label xml:lang="en">has occurrent part</rdfs:label>
        <skos:definition xml:lang="en">(Elucidation) b has occurrent part c means: c is a part of b &amp; b and c are occurrents</skos:definition>
        <skos:example xml:lang="en">Mary&apos;s life has occurrent part Mary&apos;s 5th birthday.</skos:example>
        <skos:prefLabel xml:lang="en">has occurrent part</skos:prefLabel>
    </owl:ObjectProperty>
    


    <!-- http://purl.obolibrary.org/obo/BFO_0000118 -->

    <owl:ObjectProperty rdf:about="http://purl.obolibrary.org/obo/BFO_0000118">
        <rdfs:subPropertyOf rdf:resource="http://purl.obolibrary.org/obo/BFO_0000117"/>
        <owl:inverseOf rdf:resource="http://purl.obolibrary.org/obo/BFO_0000138"/>
        <rdfs:domain rdf:resource="http://purl.obolibrary.org/obo/BFO_0000003"/>
        <rdfs:range rdf:resource="http://purl.obolibrary.org/obo/BFO_0000003"/>
        <dc:identifier>154-BFO</dc:identifier>
        <rdfs:label xml:lang="en">has proper occurrent part</rdfs:label>
        <skos:definition xml:lang="en">b has proper occurrent part c =Def b has occurrent part c &amp; b and c are not identical</skos:definition>
        <skos:example xml:lang="en">As for has occurrent part.</skos:example>
        <skos:prefLabel xml:lang="en">has proper occurrent part</skos:prefLabel>
    </owl:ObjectProperty>
    


    <!-- http://purl.obolibrary.org/obo/BFO_0000121 -->

    <owl:ObjectProperty rdf:about="http://purl.obolibrary.org/obo/BFO_0000121">
        <rdfs:subPropertyOf rdf:resource="http://purl.obolibrary.org/obo/BFO_0000117"/>
        <owl:inverseOf rdf:resource="http://purl.obolibrary.org/obo/BFO_0000139"/>
        <rdf:type rdf:resource="http://www.w3.org/2002/07/owl#TransitiveProperty"/>
        <rdfs:domain rdf:resource="http://purl.obolibrary.org/obo/BFO_0000003"/>
        <rdfs:range rdf:resource="http://purl.obolibrary.org/obo/BFO_0000003"/>
        <dc:identifier>211-BFO</dc:identifier>
        <rdfs:label xml:lang="en">has temporal part</rdfs:label>
        <skos:definition xml:lang="en">b has temporal part c =Def c temporal part of b</skos:definition>
        <skos:example xml:lang="en">Your life has temporal part the first year of your life.</skos:example>
        <skos:prefLabel xml:lang="en">has temporal part</skos:prefLabel>
    </owl:ObjectProperty>
    


    <!-- http://purl.obolibrary.org/obo/BFO_0000124 -->

    <owl:ObjectProperty rdf:about="http://purl.obolibrary.org/obo/BFO_0000124">
        <owl:inverseOf rdf:resource="http://purl.obolibrary.org/obo/BFO_0000171"/>
        <rdfs:domain>
            <owl:Class>
                <owl:intersectionOf rdf:parseType="Collection">
                    <rdf:Description rdf:about="http://purl.obolibrary.org/obo/BFO_0000004"/>
                    <owl:Class>
                        <owl:complementOf rdf:resource="http://purl.obolibrary.org/obo/BFO_0000006"/>
                    </owl:Class>
                </owl:intersectionOf>
            </owl:Class>
        </rdfs:domain>
        <rdfs:range>
            <owl:Class>
                <owl:intersectionOf rdf:parseType="Collection">
                    <rdf:Description rdf:about="http://purl.obolibrary.org/obo/BFO_0000004"/>
                    <owl:Class>
                        <owl:complementOf rdf:resource="http://purl.obolibrary.org/obo/BFO_0000006"/>
                    </owl:Class>
                </owl:intersectionOf>
            </owl:Class>
        </rdfs:range>
        <dc:identifier>236-BFO</dc:identifier>
        <rdfs:label xml:lang="en">location of at some time</rdfs:label>
        <skos:definition xml:lang="en">b location of c at some time =Def for some time t (c located in b at t)</skos:definition>
        <skos:prefLabel xml:lang="en">location of at some time</skos:prefLabel>
    </owl:ObjectProperty>
    


    <!-- http://purl.obolibrary.org/obo/BFO_0000129 -->

    <owl:ObjectProperty rdf:about="http://purl.obolibrary.org/obo/BFO_0000129">
        <rdfs:subPropertyOf rdf:resource="http://purl.obolibrary.org/obo/BFO_0000176"/>
        <rdfs:domain rdf:resource="http://purl.obolibrary.org/obo/BFO_0000040"/>
        <rdfs:range rdf:resource="http://purl.obolibrary.org/obo/BFO_0000040"/>
        <dc:identifier>228-BFO</dc:identifier>
        <rdfs:label xml:lang="en">member part of at some time</rdfs:label>
        <skos:definition xml:lang="en">b member part of c at some time =Def for some time t (b is an object &amp; there is at t a mutually exhaustive and pairwise disjoint partition of c into objects x1, ..., xn (for some n ≠ 1) with b = xi (for some 1 &lt;= i &lt;= n))</skos:definition>
        <skos:prefLabel xml:lang="en">member part of at some time</skos:prefLabel>
    </owl:ObjectProperty>
    


    <!-- http://purl.obolibrary.org/obo/BFO_0000132 -->

    <owl:ObjectProperty rdf:about="http://purl.obolibrary.org/obo/BFO_0000132">
        <rdf:type rdf:resource="http://www.w3.org/2002/07/owl#TransitiveProperty"/>
        <rdfs:domain rdf:resource="http://purl.obolibrary.org/obo/BFO_0000003"/>
        <rdfs:range rdf:resource="http://purl.obolibrary.org/obo/BFO_0000003"/>
        <dc:identifier>003-BFO</dc:identifier>
        <rdfs:label xml:lang="en">occurrent part of</rdfs:label>
        <skos:definition xml:lang="en">(Elucidation) b occurrent part of c =Def c has occurrent part b</skos:definition>
        <skos:example xml:lang="en">Mary&apos;s 5th birthday is an occurrent part of Mary&apos;s life; the first set of the tennis match is an occurrent part of the tennis match.</skos:example>
        <skos:prefLabel xml:lang="en">occurrent part of</skos:prefLabel>
    </owl:ObjectProperty>
    


    <!-- http://purl.obolibrary.org/obo/BFO_0000136 -->

    <owl:ObjectProperty rdf:about="http://purl.obolibrary.org/obo/BFO_0000136">
        <rdfs:subPropertyOf rdf:resource="http://purl.obolibrary.org/obo/BFO_0000139"/>
        <owl:inverseOf rdf:resource="http://purl.obolibrary.org/obo/BFO_0000181"/>
        <rdfs:domain rdf:resource="http://purl.obolibrary.org/obo/BFO_0000003"/>
        <rdfs:range rdf:resource="http://purl.obolibrary.org/obo/BFO_0000003"/>
        <dc:identifier>116-BFO</dc:identifier>
        <rdfs:label xml:lang="en">proper temporal part of</rdfs:label>
        <skos:definition xml:lang="en">b proper temporal part of c =Def b temporal part of c &amp; not (b = c)</skos:definition>
        <skos:example xml:lang="en">As for temporal part of.</skos:example>
        <skos:prefLabel xml:lang="en">proper temporal part of</skos:prefLabel>
    </owl:ObjectProperty>
    


    <!-- http://purl.obolibrary.org/obo/BFO_0000137 -->

    <owl:ObjectProperty rdf:about="http://purl.obolibrary.org/obo/BFO_0000137">
        <rdfs:subPropertyOf rdf:resource="http://purl.obolibrary.org/obo/BFO_0000175"/>
        <rdfs:subPropertyOf rdf:resource="http://purl.obolibrary.org/obo/BFO_0000177"/>
        <rdf:type rdf:resource="http://www.w3.org/2002/07/owl#TransitiveProperty"/>
        <rdfs:domain rdf:resource="http://purl.obolibrary.org/obo/BFO_0000002"/>
        <rdfs:range rdf:resource="http://purl.obolibrary.org/obo/BFO_0000002"/>
        <dc:identifier>225-BFO</dc:identifier>
        <rdfs:label xml:lang="en">proper continuant part of at all times</rdfs:label>
        <skos:definition xml:lang="en">b proper continuant part of c at all times =Def for all times t, b exists at t implies (b continuant part of c at t &amp; not (c proper continuant part of b at t))</skos:definition>
        <skos:prefLabel xml:lang="en">proper continuant part of at all times</skos:prefLabel>
    </owl:ObjectProperty>
    


    <!-- http://purl.obolibrary.org/obo/BFO_0000138 -->

    <owl:ObjectProperty rdf:about="http://purl.obolibrary.org/obo/BFO_0000138">
        <rdfs:subPropertyOf rdf:resource="http://purl.obolibrary.org/obo/BFO_0000132"/>
        <rdfs:domain rdf:resource="http://purl.obolibrary.org/obo/BFO_0000003"/>
        <rdfs:range rdf:resource="http://purl.obolibrary.org/obo/BFO_0000003"/>
        <dc:identifier>005-BFO</dc:identifier>
        <rdfs:label xml:lang="en">proper occurrent part of</rdfs:label>
        <skos:definition xml:lang="en">b proper occurrent part of c =Def b occurrent part of c &amp; b and c are not identical</skos:definition>
        <skos:example xml:lang="en">As for occurrent part of.</skos:example>
        <skos:prefLabel xml:lang="en">proper occurrent part of</skos:prefLabel>
    </owl:ObjectProperty>
    


    <!-- http://purl.obolibrary.org/obo/BFO_0000139 -->

    <owl:ObjectProperty rdf:about="http://purl.obolibrary.org/obo/BFO_0000139">
        <rdfs:subPropertyOf rdf:resource="http://purl.obolibrary.org/obo/BFO_0000132"/>
        <rdf:type rdf:resource="http://www.w3.org/2002/07/owl#TransitiveProperty"/>
        <rdfs:domain rdf:resource="http://purl.obolibrary.org/obo/BFO_0000003"/>
        <rdfs:range rdf:resource="http://purl.obolibrary.org/obo/BFO_0000003"/>
        <dc:identifier>078-BFO</dc:identifier>
        <rdfs:label xml:lang="en">temporal part of</rdfs:label>
        <skos:definition xml:lang="en">b temporal part of c =Def b occurrent part of c &amp; either b and c are temporal regions or b and c are spatiotemporal regions &amp; b temporally projects onto an occurrent part of the temporal region that c temporally projects onto or b and c are processes or process boundaries &amp; b occupies a temporal region that is an occurrent part of the temporal region that c occupies</skos:definition>
        <skos:example xml:lang="en">Your heart beating from 4pm to 5pm today is a temporal part of the process of your heart beating; the 4th year of your life is a temporal part of your life, as is the process boundary which separates the 3rd and 4th years of your life; the first quarter of a game of football is a temporal part of the whole game.</skos:example>
        <skos:prefLabel xml:lang="en">temporal part of</skos:prefLabel>
    </owl:ObjectProperty>
    


    <!-- http://purl.obolibrary.org/obo/BFO_0000153 -->

    <owl:ObjectProperty rdf:about="http://purl.obolibrary.org/obo/BFO_0000153">
        <rdf:type rdf:resource="http://www.w3.org/2002/07/owl#FunctionalProperty"/>
        <rdfs:domain rdf:resource="http://purl.obolibrary.org/obo/BFO_0000011"/>
        <rdfs:range rdf:resource="http://purl.obolibrary.org/obo/BFO_0000008"/>
        <dc:identifier>080-BFO</dc:identifier>
        <rdfs:label xml:lang="en">temporally projects onto</rdfs:label>
        <skos:definition xml:lang="en">(Elucidation) temporally projects onto is a relation between a spatiotemporal region s and some temporal region which is the temporal extent of s</skos:definition>
        <skos:example xml:lang="en">The world line of a particle temporally projects onto the temporal region extending from the beginning to the end of the existence of the particle.</skos:example>
        <skos:prefLabel xml:lang="en">temporally projects onto</skos:prefLabel>
    </owl:ObjectProperty>
    


    <!-- http://purl.obolibrary.org/obo/BFO_0000166 -->

    <owl:ObjectProperty rdf:about="http://purl.obolibrary.org/obo/BFO_0000166">
        <rdfs:subPropertyOf rdf:resource="http://purl.obolibrary.org/obo/BFO_0000056"/>
        <rdfs:range rdf:resource="http://purl.obolibrary.org/obo/BFO_0000015"/>
        <dc:identifier>251-BFO</dc:identifier>
        <rdfs:label xml:lang="en">participates in at all times</rdfs:label>
        <skos:definition xml:lang="en">b participates in p at all times =Def for all times t, b exists at t implies (p has participant b at t)</skos:definition>
        <skos:prefLabel xml:lang="en">participates in at all times</skos:prefLabel>
    </owl:ObjectProperty>
    


    <!-- http://purl.obolibrary.org/obo/BFO_0000167 -->

    <owl:ObjectProperty rdf:about="http://purl.obolibrary.org/obo/BFO_0000167">
        <rdfs:subPropertyOf rdf:resource="http://purl.obolibrary.org/obo/BFO_0000057"/>
        <rdfs:domain rdf:resource="http://purl.obolibrary.org/obo/BFO_0000015"/>
        <dc:identifier>249-BFO</dc:identifier>
        <rdfs:label xml:lang="en">has participant at all times</rdfs:label>
        <skos:definition xml:lang="en">p has participant c at all times =Def for all times t, p exists at t implies (p is a process, c is a continuant, and c participates in p some way at t)</skos:definition>
        <skos:prefLabel xml:lang="en">has participant at all times</skos:prefLabel>
    </owl:ObjectProperty>
    


    <!-- http://purl.obolibrary.org/obo/BFO_0000170 -->

    <owl:ObjectProperty rdf:about="http://purl.obolibrary.org/obo/BFO_0000170">
        <rdfs:subPropertyOf rdf:resource="http://purl.obolibrary.org/obo/BFO_0000124"/>
        <rdfs:domain>
            <owl:Class>
                <owl:intersectionOf rdf:parseType="Collection">
                    <rdf:Description rdf:about="http://purl.obolibrary.org/obo/BFO_0000004"/>
                    <owl:Class>
                        <owl:complementOf rdf:resource="http://purl.obolibrary.org/obo/BFO_0000006"/>
                    </owl:Class>
                </owl:intersectionOf>
            </owl:Class>
        </rdfs:domain>
        <rdfs:range>
            <owl:Class>
                <owl:intersectionOf rdf:parseType="Collection">
                    <rdf:Description rdf:about="http://purl.obolibrary.org/obo/BFO_0000004"/>
                    <owl:Class>
                        <owl:complementOf rdf:resource="http://purl.obolibrary.org/obo/BFO_0000006"/>
                    </owl:Class>
                </owl:intersectionOf>
            </owl:Class>
        </rdfs:range>
        <dc:identifier>237-BFO</dc:identifier>
        <rdfs:label xml:lang="en">location of at all times</rdfs:label>
        <skos:definition xml:lang="en">b location of c at all times =Def for all times t, b exists at t implies (c located in b at t)</skos:definition>
        <skos:prefLabel xml:lang="en">location of at all times</skos:prefLabel>
    </owl:ObjectProperty>
    


    <!-- http://purl.obolibrary.org/obo/BFO_0000171 -->

    <owl:ObjectProperty rdf:about="http://purl.obolibrary.org/obo/BFO_0000171">
        <rdfs:domain>
            <owl:Class>
                <owl:intersectionOf rdf:parseType="Collection">
                    <rdf:Description rdf:about="http://purl.obolibrary.org/obo/BFO_0000004"/>
                    <owl:Class>
                        <owl:complementOf rdf:resource="http://purl.obolibrary.org/obo/BFO_0000006"/>
                    </owl:Class>
                </owl:intersectionOf>
            </owl:Class>
        </rdfs:domain>
        <rdfs:range>
            <owl:Class>
                <owl:intersectionOf rdf:parseType="Collection">
                    <rdf:Description rdf:about="http://purl.obolibrary.org/obo/BFO_0000004"/>
                    <owl:Class>
                        <owl:complementOf rdf:resource="http://purl.obolibrary.org/obo/BFO_0000006"/>
                    </owl:Class>
                </owl:intersectionOf>
            </owl:Class>
        </rdfs:range>
        <dc:identifier>234-BFO</dc:identifier>
        <rdfs:label xml:lang="en">located in at some time</rdfs:label>
        <skos:definition xml:lang="en">b located in c at some time =Def for some time t (b and c are independent continuants and not spatial regions, and the spatial region which b occupies at t is a (proper or improper) continuant part of the spatial region which c occupies at t)</skos:definition>
        <skos:prefLabel xml:lang="en">located in at some time</skos:prefLabel>
    </owl:ObjectProperty>
    


    <!-- http://purl.obolibrary.org/obo/BFO_0000172 -->

    <owl:ObjectProperty rdf:about="http://purl.obolibrary.org/obo/BFO_0000172">
        <rdfs:subPropertyOf rdf:resource="http://purl.obolibrary.org/obo/BFO_0000110"/>
        <rdfs:subPropertyOf rdf:resource="http://purl.obolibrary.org/obo/BFO_0000115"/>
        <rdfs:domain rdf:resource="http://purl.obolibrary.org/obo/BFO_0000040"/>
        <rdfs:range rdf:resource="http://purl.obolibrary.org/obo/BFO_0000040"/>
        <dc:identifier>231-BFO</dc:identifier>
        <rdfs:label xml:lang="en">has member part at all times</rdfs:label>
        <skos:definition xml:lang="en">b has member part c at all times =Def for all times t, b exists at t implies (c member part b at t)</skos:definition>
        <skos:prefLabel xml:lang="en">has member part at all times</skos:prefLabel>
    </owl:ObjectProperty>
    


    <!-- http://purl.obolibrary.org/obo/BFO_0000173 -->

    <owl:ObjectProperty rdf:about="http://purl.obolibrary.org/obo/BFO_0000173">
        <rdfs:subPropertyOf rdf:resource="http://purl.obolibrary.org/obo/BFO_0000129"/>
        <rdfs:subPropertyOf rdf:resource="http://purl.obolibrary.org/obo/BFO_0000177"/>
        <rdfs:domain rdf:resource="http://purl.obolibrary.org/obo/BFO_0000040"/>
        <rdfs:range rdf:resource="http://purl.obolibrary.org/obo/BFO_0000040"/>
        <dc:identifier>229-BFO</dc:identifier>
        <rdfs:label xml:lang="en">member part of at all times</rdfs:label>
        <skos:definition xml:lang="en">b member part of c at all times =Def for all times t, b exists at t implies (b is an object &amp; c is an object aggregate &amp; there is at t a mutually exhaustive and pairwise disjoint partition of c into objects x1,..., xn (for some n ≠ 1) with b = xi (for some 1 &lt;= i &lt;= n))</skos:definition>
        <skos:prefLabel xml:lang="en">member part of at all times</skos:prefLabel>
    </owl:ObjectProperty>
    


    <!-- http://purl.obolibrary.org/obo/BFO_0000174 -->

    <owl:ObjectProperty rdf:about="http://purl.obolibrary.org/obo/BFO_0000174">
        <rdfs:subPropertyOf rdf:resource="http://purl.obolibrary.org/obo/BFO_0000178"/>
        <owl:inverseOf rdf:resource="http://purl.obolibrary.org/obo/BFO_0000175"/>
        <rdfs:domain rdf:resource="http://purl.obolibrary.org/obo/BFO_0000002"/>
        <rdfs:range rdf:resource="http://purl.obolibrary.org/obo/BFO_0000002"/>
        <dc:identifier>226-BFO</dc:identifier>
        <rdfs:label xml:lang="en">has proper continuant part at some time</rdfs:label>
        <skos:definition xml:lang="en">b has proper continuant part c at some time =Def c proper continuant part of b at some time</skos:definition>
        <skos:prefLabel xml:lang="en">has proper continuant part at some time</skos:prefLabel>
    </owl:ObjectProperty>
    


    <!-- http://purl.obolibrary.org/obo/BFO_0000175 -->

    <owl:ObjectProperty rdf:about="http://purl.obolibrary.org/obo/BFO_0000175">
        <rdfs:subPropertyOf rdf:resource="http://purl.obolibrary.org/obo/BFO_0000176"/>
        <rdfs:domain rdf:resource="http://purl.obolibrary.org/obo/BFO_0000002"/>
        <rdfs:range rdf:resource="http://purl.obolibrary.org/obo/BFO_0000002"/>
        <dc:identifier>224-BFO</dc:identifier>
        <rdfs:label xml:lang="en">proper continuant part of at some time</rdfs:label>
        <skos:definition xml:lang="en">b proper continuant part of c at some time =Def for some time t (b continuant part of c at t &amp; not (c continuant part of b at t)</skos:definition>
        <skos:prefLabel xml:lang="en">proper continuant part of at some time</skos:prefLabel>
    </owl:ObjectProperty>
    


    <!-- http://purl.obolibrary.org/obo/BFO_0000176 -->

    <owl:ObjectProperty rdf:about="http://purl.obolibrary.org/obo/BFO_0000176">
        <owl:inverseOf rdf:resource="http://purl.obolibrary.org/obo/BFO_0000178"/>
        <rdfs:domain rdf:resource="http://purl.obolibrary.org/obo/BFO_0000002"/>
        <rdfs:range rdf:resource="http://purl.obolibrary.org/obo/BFO_0000002"/>
        <dc:identifier>221-BFO</dc:identifier>
        <rdfs:label xml:lang="en">continuant part of at some time</rdfs:label>
        <skos:definition xml:lang="en">b continuant part of c at some time =Def for some time t (b exists at t and c exists at t and b continuant part of c at t &amp; t is a temporal region &amp; b and c are continuants)</skos:definition>
        <skos:example xml:lang="en">Milk teeth continuant part of human at some time; surgically removed tumour continuant part of organism at some time.</skos:example>
        <skos:prefLabel xml:lang="en">continuant part of at some time</skos:prefLabel>
    </owl:ObjectProperty>
    


    <!-- http://purl.obolibrary.org/obo/BFO_0000177 -->

    <owl:ObjectProperty rdf:about="http://purl.obolibrary.org/obo/BFO_0000177">
        <rdfs:subPropertyOf rdf:resource="http://purl.obolibrary.org/obo/BFO_0000176"/>
        <rdf:type rdf:resource="http://www.w3.org/2002/07/owl#TransitiveProperty"/>
        <rdfs:domain rdf:resource="http://purl.obolibrary.org/obo/BFO_0000002"/>
        <rdfs:range rdf:resource="http://purl.obolibrary.org/obo/BFO_0000002"/>
        <dc:identifier>222-BFO</dc:identifier>
        <rdfs:label xml:lang="en">continuant part of at all times</rdfs:label>
        <skos:definition xml:lang="en">b continuant part of c at all times =Def for all times t, (b exists at t, implies b continuant part of c at t &amp; t is a temporal region &amp; b and c are continuants)</skos:definition>
        <skos:example xml:lang="en">Centre of mass of a material entity continuant part of material entity at all times; continuant fiat external boundary of an object continuant part of object at all times.</skos:example>
        <skos:prefLabel xml:lang="en">continuant part of at all times</skos:prefLabel>
    </owl:ObjectProperty>
    


    <!-- http://purl.obolibrary.org/obo/BFO_0000178 -->

    <owl:ObjectProperty rdf:about="http://purl.obolibrary.org/obo/BFO_0000178">
        <rdfs:domain rdf:resource="http://purl.obolibrary.org/obo/BFO_0000002"/>
        <rdfs:range rdf:resource="http://purl.obolibrary.org/obo/BFO_0000002"/>
        <dc:identifier>271-BFO</dc:identifier>
        <rdfs:label xml:lang="en">has continuant part at some time</rdfs:label>
        <skos:definition xml:lang="en">b has continuant part c at some time =Def for some time t (b and c are continuants &amp; b is a part of c at t)</skos:definition>
        <skos:prefLabel xml:lang="en">has continuant part at some time</skos:prefLabel>
    </owl:ObjectProperty>
    


    <!-- http://purl.obolibrary.org/obo/BFO_0000181 -->

    <owl:ObjectProperty rdf:about="http://purl.obolibrary.org/obo/BFO_0000181">
        <rdfs:subPropertyOf rdf:resource="http://purl.obolibrary.org/obo/BFO_0000121"/>
        <rdfs:domain rdf:resource="http://purl.obolibrary.org/obo/BFO_0000003"/>
        <rdfs:range rdf:resource="http://purl.obolibrary.org/obo/BFO_0000003"/>
        <dc:identifier>212-BFO</dc:identifier>
        <rdfs:label xml:lang="en">has proper temporal part</rdfs:label>
        <skos:definition xml:lang="en">b has proper temporal part c =Def c proper temporal part of b</skos:definition>
        <skos:example xml:lang="en">As for has temporal part.</skos:example>
        <skos:prefLabel xml:lang="en">has proper temporal part</skos:prefLabel>
    </owl:ObjectProperty>
    


    <!-- http://purl.obolibrary.org/obo/BFO_0000183 -->

    <owl:ObjectProperty rdf:about="http://purl.obolibrary.org/obo/BFO_0000183">
        <rdfs:domain>
            <owl:Class>
                <owl:unionOf rdf:parseType="Collection">
                    <rdf:Description rdf:about="http://purl.obolibrary.org/obo/BFO_0000029"/>
                    <rdf:Description rdf:about="http://purl.obolibrary.org/obo/BFO_0000040"/>
                </owl:unionOf>
            </owl:Class>
        </rdfs:domain>
        <rdfs:range>
            <owl:Class>
                <owl:unionOf rdf:parseType="Collection">
                    <rdf:Description rdf:about="http://purl.obolibrary.org/obo/BFO_0000015"/>
                    <rdf:Description rdf:about="http://purl.obolibrary.org/obo/BFO_0000035"/>
                </owl:unionOf>
            </owl:Class>
        </rdfs:range>
        <dc:identifier>267-BFO</dc:identifier>
        <rdfs:label xml:lang="en">environs</rdfs:label>
        <skos:definition xml:lang="en">b environs c =Def c occurs in b</skos:definition>
        <skos:example xml:lang="en">Mouth environs process of mastication, city environs traffic.</skos:example>
        <skos:prefLabel xml:lang="en">environs</skos:prefLabel>
    </owl:ObjectProperty>
    


    <!-- http://purl.obolibrary.org/obo/BFO_0000194 -->

    <owl:ObjectProperty rdf:about="http://purl.obolibrary.org/obo/BFO_0000194">
        <owl:inverseOf rdf:resource="http://purl.obolibrary.org/obo/BFO_0000195"/>
        <rdfs:domain>
            <owl:Class>
                <owl:unionOf rdf:parseType="Collection">
                    <rdf:Description rdf:about="http://purl.obolibrary.org/obo/BFO_0000020"/>
                    <owl:Class>
                        <owl:intersectionOf rdf:parseType="Collection">
                            <rdf:Description rdf:about="http://purl.obolibrary.org/obo/BFO_0000004"/>
                            <owl:Class>
                                <owl:complementOf rdf:resource="http://purl.obolibrary.org/obo/BFO_0000006"/>
                            </owl:Class>
                        </owl:intersectionOf>
                    </owl:Class>
                </owl:unionOf>
            </owl:Class>
        </rdfs:domain>
        <rdfs:range rdf:resource="http://purl.obolibrary.org/obo/BFO_0000020"/>
        <dc:identifier>260-BFO</dc:identifier>
        <rdfs:label xml:lang="en">specifically depended on by</rdfs:label>
        <skos:altLabel xml:lang="en">s-depended on by</skos:altLabel>
        <skos:definition xml:lang="en">b s-depended on by c =Def c specifically depends on b</skos:definition>
        <skos:example xml:lang="en">Coloured object s-depended on by colour.</skos:example>
        <skos:prefLabel xml:lang="en">specifically depended on by</skos:prefLabel>
    </owl:ObjectProperty>
    


    <!-- http://purl.obolibrary.org/obo/BFO_0000195 -->

    <owl:ObjectProperty rdf:about="http://purl.obolibrary.org/obo/BFO_0000195">
        <rdfs:domain rdf:resource="http://purl.obolibrary.org/obo/BFO_0000020"/>
        <rdfs:range>
            <owl:Class>
                <owl:unionOf rdf:parseType="Collection">
                    <rdf:Description rdf:about="http://purl.obolibrary.org/obo/BFO_0000020"/>
                    <owl:Class>
                        <owl:intersectionOf rdf:parseType="Collection">
                            <rdf:Description rdf:about="http://purl.obolibrary.org/obo/BFO_0000004"/>
                            <owl:Class>
                                <owl:complementOf rdf:resource="http://purl.obolibrary.org/obo/BFO_0000006"/>
                            </owl:Class>
                        </owl:intersectionOf>
                    </owl:Class>
                </owl:unionOf>
            </owl:Class>
        </rdfs:range>
        <dc:identifier>012-BFO</dc:identifier>
        <rdfs:label xml:lang="en">specifically depends on</rdfs:label>
        <skos:altLabel xml:lang="en">s-depends on</skos:altLabel>
        <skos:definition xml:lang="en">(Elucidation) b specifically depends on c means: b and c do not share common parts &amp; b is of a nature such that at all times t it cannot exist at t unless c exists at t &amp; b is not a boundary of c</skos:definition>
        <skos:example xml:lang="en">A shape s-depends on the shaped object, hue, saturation and brightness of a colour sample s-depend on each other.</skos:example>
        <skos:prefLabel xml:lang="en">specifically depends on</skos:prefLabel>
        <skos:scopeNote xml:lang="en">The analogue of s-dependence for occurrents is has participant.</skos:scopeNote>
    </owl:ObjectProperty>
    


    <!-- http://purl.obolibrary.org/obo/BFO_0000196 -->

    <owl:ObjectProperty rdf:about="http://purl.obolibrary.org/obo/BFO_0000196">
        <rdfs:subPropertyOf rdf:resource="http://purl.obolibrary.org/obo/BFO_0000194"/>
        <owl:inverseOf rdf:resource="http://purl.obolibrary.org/obo/BFO_0000197"/>
        <rdfs:domain>
            <owl:Class>
                <owl:intersectionOf rdf:parseType="Collection">
                    <rdf:Description rdf:about="http://purl.obolibrary.org/obo/BFO_0000004"/>
                    <owl:Class>
                        <owl:complementOf rdf:resource="http://purl.obolibrary.org/obo/BFO_0000006"/>
                    </owl:Class>
                </owl:intersectionOf>
            </owl:Class>
        </rdfs:domain>
        <rdfs:range rdf:resource="http://purl.obolibrary.org/obo/BFO_0000020"/>
        <dc:identifier>053-BFO</dc:identifier>
        <rdfs:label xml:lang="en">bearer of</rdfs:label>
        <skos:definition xml:lang="en">b bearer of c =Def c inheres in b</skos:definition>
        <skos:example xml:lang="en">A patch of ink is the bearer of a colour quality; an organism is the bearer of a temperature quality.</skos:example>
        <skos:prefLabel xml:lang="en">bearer of</skos:prefLabel>
    </owl:ObjectProperty>
    


    <!-- http://purl.obolibrary.org/obo/BFO_0000197 -->

    <owl:ObjectProperty rdf:about="http://purl.obolibrary.org/obo/BFO_0000197">
        <rdfs:subPropertyOf rdf:resource="http://purl.obolibrary.org/obo/BFO_0000195"/>
        <rdfs:domain rdf:resource="http://purl.obolibrary.org/obo/BFO_0000020"/>
        <rdfs:range>
            <owl:Class>
                <owl:intersectionOf rdf:parseType="Collection">
                    <rdf:Description rdf:about="http://purl.obolibrary.org/obo/BFO_0000004"/>
                    <owl:Class>
                        <owl:complementOf rdf:resource="http://purl.obolibrary.org/obo/BFO_0000006"/>
                    </owl:Class>
                </owl:intersectionOf>
            </owl:Class>
        </rdfs:range>
        <dc:identifier>051-BFO</dc:identifier>
        <rdfs:label xml:lang="en">inheres in</rdfs:label>
        <skos:definition xml:lang="en">b inheres in c =Def b is a specifically dependent continuant &amp; c is an independent continuant that is not a spatial region &amp; b s-depends on c</skos:definition>
        <skos:example xml:lang="en">A shape inheres in a shaped object; a mass inheres in a material entity.</skos:example>
        <skos:prefLabel xml:lang="en">inheres in</skos:prefLabel>
    </owl:ObjectProperty>
    


    <!-- http://purl.obolibrary.org/obo/BFO_0000199 -->

    <owl:ObjectProperty rdf:about="http://purl.obolibrary.org/obo/BFO_0000199">
        <rdf:type rdf:resource="http://www.w3.org/2002/07/owl#FunctionalProperty"/>
        <rdfs:domain>
            <owl:Class>
                <owl:unionOf rdf:parseType="Collection">
                    <rdf:Description rdf:about="http://purl.obolibrary.org/obo/BFO_0000015"/>
                    <rdf:Description rdf:about="http://purl.obolibrary.org/obo/BFO_0000035"/>
                </owl:unionOf>
            </owl:Class>
        </rdfs:domain>
        <rdfs:range rdf:resource="http://purl.obolibrary.org/obo/BFO_0000008"/>
        <dc:identifier>132-BFO</dc:identifier>
        <rdfs:label xml:lang="en">occupies temporal region</rdfs:label>
        <skos:definition xml:lang="en">p occupies temporal region t =Def the spatiotemporal region occupied by p temporally projects onto t</skos:definition>
        <skos:example xml:lang="en">The Second World War occupies the temporal region September 1, 1939 - September 2, 1945.</skos:example>
        <skos:prefLabel xml:lang="en">occupies temporal region</skos:prefLabel>
    </owl:ObjectProperty>
    


    <!-- http://purl.obolibrary.org/obo/BFO_0000200 -->

    <owl:ObjectProperty rdf:about="http://purl.obolibrary.org/obo/BFO_0000200">
        <rdf:type rdf:resource="http://www.w3.org/2002/07/owl#FunctionalProperty"/>
        <rdfs:domain>
            <owl:Class>
                <owl:unionOf rdf:parseType="Collection">
                    <rdf:Description rdf:about="http://purl.obolibrary.org/obo/BFO_0000015"/>
                    <rdf:Description rdf:about="http://purl.obolibrary.org/obo/BFO_0000035"/>
                </owl:unionOf>
            </owl:Class>
        </rdfs:domain>
        <rdfs:range rdf:resource="http://purl.obolibrary.org/obo/BFO_0000011"/>
        <dc:identifier>082-BFO</dc:identifier>
        <rdfs:label xml:lang="en">occupies spatiotemporal region</rdfs:label>
        <skos:definition xml:lang="en">(Elucidation) p occupies spatiotemporal region s is a relation between an occurrent p and the spatiotemporal region s which is its spatiotemporal extent</skos:definition>
        <skos:example xml:lang="en">A particle emitted by a nuclear reactor occupies the spatiotemporal region which is its trajectory.</skos:example>
        <skos:prefLabel xml:lang="en">occupies spatiotemporal region</skos:prefLabel>
    </owl:ObjectProperty>
    


    <!-- http://purl.obolibrary.org/obo/BFO_0000210 -->

    <owl:ObjectProperty rdf:about="http://purl.obolibrary.org/obo/BFO_0000210">
        <rdfs:domain>
            <owl:Class>
                <owl:intersectionOf rdf:parseType="Collection">
                    <rdf:Description rdf:about="http://purl.obolibrary.org/obo/BFO_0000004"/>
                    <owl:Class>
                        <owl:complementOf rdf:resource="http://purl.obolibrary.org/obo/BFO_0000006"/>
                    </owl:Class>
                </owl:intersectionOf>
            </owl:Class>
        </rdfs:domain>
        <rdfs:range rdf:resource="http://purl.obolibrary.org/obo/BFO_0000006"/>
        <dc:identifier>232-BFO</dc:identifier>
        <rdfs:label xml:lang="en">occupies spatial region at some time</rdfs:label>
        <skos:definition xml:lang="en">an independent continuant c that is not a spatial region occupies spatial region r at some time =Def for some time t (every continuant part of c occupies some continuant part of r at t and no continuant part of c occupies any spatial region that is not a continuant part of r at t)</skos:definition>
        <skos:prefLabel xml:lang="en">occupies spatial region at some time</skos:prefLabel>
    </owl:ObjectProperty>
    


    <!-- http://purl.obolibrary.org/obo/BFO_0000211 -->

    <owl:ObjectProperty rdf:about="http://purl.obolibrary.org/obo/BFO_0000211">
        <rdfs:subPropertyOf rdf:resource="http://purl.obolibrary.org/obo/BFO_0000210"/>
        <rdf:type rdf:resource="http://www.w3.org/2002/07/owl#FunctionalProperty"/>
        <rdfs:domain>
            <owl:Class>
                <owl:intersectionOf rdf:parseType="Collection">
                    <rdf:Description rdf:about="http://purl.obolibrary.org/obo/BFO_0000004"/>
                    <owl:Class>
                        <owl:complementOf rdf:resource="http://purl.obolibrary.org/obo/BFO_0000006"/>
                    </owl:Class>
                </owl:intersectionOf>
            </owl:Class>
        </rdfs:domain>
        <rdfs:range rdf:resource="http://purl.obolibrary.org/obo/BFO_0000006"/>
        <dc:identifier>233-BFO</dc:identifier>
        <rdfs:label xml:lang="en">occupies spatial region at all times</rdfs:label>
        <skos:definition xml:lang="en">an independent continuant c that is not a spatial region occupies spatial region r at all times =Def for all times t, b exists at t implies (every continuant part of c occupies some continuant part of r at t and no continuant part of c occupies any spatial region that is not a continuant part of r at t)</skos:definition>
        <skos:prefLabel xml:lang="en">occupies spatial region at all times</skos:prefLabel>
    </owl:ObjectProperty>
    


    <!-- http://purl.obolibrary.org/obo/BFO_0000216 -->

    <owl:ObjectProperty rdf:about="http://purl.obolibrary.org/obo/BFO_0000216">
        <rdfs:domain rdf:resource="http://purl.obolibrary.org/obo/BFO_0000011"/>
        <rdfs:range rdf:resource="http://purl.obolibrary.org/obo/BFO_0000006"/>
        <dc:identifier>246-BFO</dc:identifier>
        <rdfs:label xml:lang="en">spatially projects onto at some time</rdfs:label>
        <skos:definition xml:lang="en">b spatially projects onto c at some time =Def for some time t (b is a spatiotemporal region and c is a spatial region and c is the spatial extent of b at t)</skos:definition>
        <skos:prefLabel xml:lang="en">spatially projects onto at some time</skos:prefLabel>
    </owl:ObjectProperty>
    


    <!-- http://purl.obolibrary.org/obo/BFO_0000217 -->

    <owl:ObjectProperty rdf:about="http://purl.obolibrary.org/obo/BFO_0000217">
        <rdfs:subPropertyOf rdf:resource="http://purl.obolibrary.org/obo/BFO_0000216"/>
        <rdf:type rdf:resource="http://www.w3.org/2002/07/owl#FunctionalProperty"/>
        <rdfs:domain rdf:resource="http://purl.obolibrary.org/obo/BFO_0000011"/>
        <rdfs:range rdf:resource="http://purl.obolibrary.org/obo/BFO_0000006"/>
        <dc:identifier>247-BFO</dc:identifier>
        <rdfs:label xml:lang="en">spatially projects onto at all times</rdfs:label>
        <skos:definition xml:lang="en">b spatially projects onto c at all times =Def for all times t, b exists at t implies (b is a spatiotemporal region and c is a spatial region and c is the spatial extent of b at t)</skos:definition>
        <skos:prefLabel xml:lang="en">spatially projects onto at all times</skos:prefLabel>
    </owl:ObjectProperty>
    


    <!-- http://purl.obolibrary.org/obo/BFO_0000218 -->

    <owl:ObjectProperty rdf:about="http://purl.obolibrary.org/obo/BFO_0000218">
        <rdfs:range rdf:resource="http://purl.obolibrary.org/obo/BFO_0000040"/>
        <dc:identifier>242-BFO</dc:identifier>
        <rdfs:label xml:lang="en">has material basis at some time</rdfs:label>
        <skos:definition xml:lang="en">b has material basis c at some time =Def For some time t (b is a disposition &amp; c is a material entity &amp; there is some d bearer of b &amp; c continuant part of d at t &amp; d has disposition b because c continuant part of d at t)</skos:definition>
        <skos:prefLabel xml:lang="en">has material basis at some time</skos:prefLabel>
    </owl:ObjectProperty>
    


    <!-- http://purl.obolibrary.org/obo/esmo.owl#benefits_from -->

    <owl:ObjectProperty rdf:about="http://purl.obolibrary.org/obo/esmo.owl#benefits_from">
        <rdfs:domain>
            <owl:Class>
                <owl:unionOf rdf:parseType="Collection">
                    <rdf:Description rdf:about="http://purl.obolibrary.org/obo/esmo.owl#Actor"/>
                    <rdf:Description rdf:about="http://purl.obolibrary.org/obo/esmo.owl#Actor_aggregate"/>
                </owl:unionOf>
            </owl:Class>
        </rdfs:domain>
        <rdfs:range>
            <owl:Class>
                <owl:unionOf rdf:parseType="Collection">
                    <rdf:Description rdf:about="http://purl.obolibrary.org/obo/esmo.owl#Instrumental_value"/>
                    <rdf:Description rdf:about="http://purl.obolibrary.org/obo/esmo.owl#Relational_value"/>
                </owl:unionOf>
            </owl:Class>
        </rdfs:range>
        <skos:definition>A relationship that holds between an actor or an actor aggregate and the value of a commodity or human activity from which they derive some benefit</skos:definition>
        <skos:example>fisher benefits from income</skos:example>
    </owl:ObjectProperty>
    


    <!-- http://purl.obolibrary.org/obo/esmo.owl#causal_relation_between_entities -->

    <owl:ObjectProperty rdf:about="http://purl.obolibrary.org/obo/esmo.owl#causal_relation_between_entities">
        <rdfs:subPropertyOf rdf:resource="http://purl.obolibrary.org/obo/esmo.owl#causally_related_to"/>
        <rdfs:domain rdf:resource="http://purl.obolibrary.org/obo/BFO_0000001"/>
        <rdfs:range rdf:resource="http://purl.obolibrary.org/obo/BFO_0000001"/>
        <skos:definition>The intent is that the process branch of the causal property hierarchy is primary (causal relations hold between occurrents/processes), and that the material branch is defined in terms of the process branch</skos:definition>
    </owl:ObjectProperty>
    


    <!-- http://purl.obolibrary.org/obo/esmo.owl#causal_relation_between_processes -->

    <owl:ObjectProperty rdf:about="http://purl.obolibrary.org/obo/esmo.owl#causal_relation_between_processes">
        <rdfs:subPropertyOf rdf:resource="http://purl.obolibrary.org/obo/esmo.owl#causally_related_to"/>
        <rdfs:domain rdf:resource="http://purl.obolibrary.org/obo/BFO_0000015"/>
        <rdfs:range rdf:resource="http://purl.obolibrary.org/obo/BFO_0000015"/>
        <skos:definition>p is causally related to q if and only if p or any part of p and q or any part of q are linked by a chain of events where each event pair is one where the execution of p influences the execution of q. p may be upstream, downstream, part of, or a container of q.</skos:definition>
    </owl:ObjectProperty>
    


    <!-- http://purl.obolibrary.org/obo/esmo.owl#causally_influences -->

    <owl:ObjectProperty rdf:about="http://purl.obolibrary.org/obo/esmo.owl#causally_influences">
        <rdfs:subPropertyOf rdf:resource="http://purl.obolibrary.org/obo/esmo.owl#causal_relation_between_entities"/>
        <rdfs:domain rdf:resource="http://purl.obolibrary.org/obo/BFO_0000001"/>
        <rdfs:range rdf:resource="http://purl.obolibrary.org/obo/BFO_0000001"/>
        <skos:definition></skos:definition>
        <skos:definition>The entity or characteristic A is causally upstream of the entity or characteristic B, A having an effect on B. An entity corresponds to any biological type of entity as long as a mass is measurable. A characteristic corresponds to a particular specificity of an entity (e.g., phenotype, shape, size).</skos:definition>
    </owl:ObjectProperty>
    


    <!-- http://purl.obolibrary.org/obo/esmo.owl#causally_related_to -->

    <owl:ObjectProperty rdf:about="http://purl.obolibrary.org/obo/esmo.owl#causally_related_to">
        <rdf:type rdf:resource="http://www.w3.org/2002/07/owl#TransitiveProperty"/>
        <rdfs:domain>
            <owl:Class>
                <owl:unionOf rdf:parseType="Collection">
                    <rdf:Description rdf:about="http://purl.obolibrary.org/obo/BFO_0000001"/>
                    <rdf:Description rdf:about="http://purl.obolibrary.org/obo/BFO_0000015"/>
                </owl:unionOf>
            </owl:Class>
        </rdfs:domain>
        <rdfs:range>
            <owl:Class>
                <owl:unionOf rdf:parseType="Collection">
                    <rdf:Description rdf:about="http://purl.obolibrary.org/obo/BFO_0000001"/>
                    <rdf:Description rdf:about="http://purl.obolibrary.org/obo/BFO_0000015"/>
                </owl:unionOf>
            </owl:Class>
        </rdfs:range>
        <skos:definition>relation that links two events, processes, states, or objects such that one event, process, state, or object (a cause) contributes to the production of another event, process, state, or object (an effect) where the cause is partly or wholly responsible for the effect, and the effect is partly or wholly dependent on the cause.</skos:definition>
        <skos:example>car crash causally related to drunk driving</skos:example>
    </owl:ObjectProperty>
    


    <!-- http://purl.obolibrary.org/obo/esmo.owl#causally_upstream_of -->

    <owl:ObjectProperty rdf:about="http://purl.obolibrary.org/obo/esmo.owl#causally_upstream_of">
        <rdfs:subPropertyOf rdf:resource="http://purl.obolibrary.org/obo/esmo.owl#causally_upstream_or_within"/>
        <rdf:type rdf:resource="http://www.w3.org/2002/07/owl#TransitiveProperty"/>
        <skos:definition>p is causally upstream of q iff p is causally related to q, the end of p precedes the end of q, and p is not an occurrent part of q.</skos:definition>
    </owl:ObjectProperty>
    


    <!-- http://purl.obolibrary.org/obo/esmo.owl#causally_upstream_of_with_negative_effect -->

    <owl:ObjectProperty rdf:about="http://purl.obolibrary.org/obo/esmo.owl#causally_upstream_of_with_negative_effect">
        <rdfs:subPropertyOf rdf:resource="http://purl.obolibrary.org/obo/esmo.owl#causally_upstream_of"/>
        <skos:definition>p is causally upstream of, negative effect q iff p is casually upstream of q, and the execution of p decreases the execution of q.</skos:definition>
    </owl:ObjectProperty>
    


    <!-- http://purl.obolibrary.org/obo/esmo.owl#causally_upstream_or_within -->

    <owl:ObjectProperty rdf:about="http://purl.obolibrary.org/obo/esmo.owl#causally_upstream_or_within">
        <rdfs:subPropertyOf rdf:resource="http://purl.obolibrary.org/obo/esmo.owl#causal_relation_between_processes"/>
        <rdf:type rdf:resource="http://www.w3.org/2002/07/owl#TransitiveProperty"/>
        <skos:definition>p is &apos;causally upstream or within&apos; q iff p is causally related to q, and the end of p precedes, or is coincident with, the end of q.</skos:definition>
    </owl:ObjectProperty>
    


    <!-- http://purl.obolibrary.org/obo/esmo.owl#has_output -->

    <owl:ObjectProperty rdf:about="http://purl.obolibrary.org/obo/esmo.owl#has_output">
        <owl:inverseOf rdf:resource="http://purl.obolibrary.org/obo/esmo.owl#output_of"/>
        <rdf:type rdf:resource="http://www.w3.org/2002/07/owl#AsymmetricProperty"/>
        <rdfs:domain rdf:resource="http://purl.obolibrary.org/obo/BFO_0000015"/>
        <rdfs:range>
            <owl:Class>
                <owl:unionOf rdf:parseType="Collection">
                    <rdf:Description rdf:about="http://purl.obolibrary.org/obo/BFO_0000015"/>
                    <rdf:Description rdf:about="http://purl.obolibrary.org/obo/BFO_0000027"/>
                    <rdf:Description rdf:about="http://purl.obolibrary.org/obo/BFO_0000030"/>
                </owl:unionOf>
            </owl:Class>
        </rdfs:range>
        <rdfs:comment>Definition from IAO_0000115 taken in ro-eco.owl</rdfs:comment>
        <skos:definition>p has output c iff c is a participant in p, c is present at the end of p, and c is not present in the same state at the beginning of p.</skos:definition>
        <skos:example>photosynthesis has outpu oxygen</skos:example>
    </owl:ObjectProperty>
    


    <!-- http://purl.obolibrary.org/obo/esmo.owl#has_quality -->

    <owl:ObjectProperty rdf:about="http://purl.obolibrary.org/obo/esmo.owl#has_quality">
        <rdfs:domain>
            <owl:Class>
                <owl:unionOf rdf:parseType="Collection">
                    <rdf:Description rdf:about="http://purl.obolibrary.org/obo/BFO_0000015"/>
                    <rdf:Description rdf:about="http://purl.obolibrary.org/obo/BFO_0000040"/>
                </owl:unionOf>
            </owl:Class>
        </rdfs:domain>
        <rdfs:range rdf:resource="http://purl.obolibrary.org/obo/BFO_0000019"/>
        <skos:definition>b has quality c =Def c quality of b</skos:definition>
        <skos:example>tree has quality height, phone has quality price</skos:example>
    </owl:ObjectProperty>
    


    <!-- http://purl.obolibrary.org/obo/esmo.owl#measure_of -->

    <owl:ObjectProperty rdf:about="http://purl.obolibrary.org/obo/esmo.owl#measure_of">
        <rdf:type rdf:resource="http://www.w3.org/2002/07/owl#IrreflexiveProperty"/>
        <rdfs:domain>
            <owl:Class>
                <owl:unionOf rdf:parseType="Collection">
                    <rdf:Description rdf:about="http://purl.obolibrary.org/obo/BFO_0000002"/>
                    <rdf:Description rdf:about="http://purl.obolibrary.org/obo/BFO_0000003"/>
                </owl:unionOf>
            </owl:Class>
        </rdfs:domain>
        <rdfs:range rdf:resource="http://purl.obolibrary.org/obo/esmo.owl#Essential_ecosystem_service_variable_class"/>
        <skos:definition>b measure_of c: b is a BFO entity (usually a process or material entity) that has a data property that can serve as a measure of c some EESV class.</skos:definition>
        <skos:example>The number/mass of wildcaught fish is a measure of the EESV class Use. The abundance of whales in an area is a measure of the EESV class ecological supply.</skos:example>
    </owl:ObjectProperty>
    


    <!-- http://purl.obolibrary.org/obo/esmo.owl#output_of -->

    <owl:ObjectProperty rdf:about="http://purl.obolibrary.org/obo/esmo.owl#output_of">
        <rdfs:subPropertyOf rdf:resource="http://www.w3.org/2002/07/owl#topObjectProperty"/>
        <rdf:type rdf:resource="http://www.w3.org/2002/07/owl#AsymmetricProperty"/>
        <rdfs:domain>
            <owl:Class>
                <owl:unionOf rdf:parseType="Collection">
                    <rdf:Description rdf:about="http://purl.obolibrary.org/obo/BFO_0000015"/>
                    <rdf:Description rdf:about="http://purl.obolibrary.org/obo/BFO_0000027"/>
                    <rdf:Description rdf:about="http://purl.obolibrary.org/obo/BFO_0000030"/>
                </owl:unionOf>
            </owl:Class>
        </rdfs:domain>
        <rdfs:range rdf:resource="http://purl.obolibrary.org/obo/BFO_0000015"/>
        <skos:definition>p output of c iff p is a participant in c, p is present at the end of c, and p is not present in the same state at the beginning of c.</skos:definition>
        <skos:example>carbon dioxide output of respiration</skos:example>
    </owl:ObjectProperty>
    


    <!-- 
    ///////////////////////////////////////////////////////////////////////////////////////
    //
    // Data properties
    //
    ///////////////////////////////////////////////////////////////////////////////////////
     -->

    


    <!-- http://purl.obolibrary.org/obo/esmo.owl#hasAbundance -->

    <owl:DatatypeProperty rdf:about="http://purl.obolibrary.org/obo/esmo.owl#hasAbundance"/>
    


    <!-- http://purl.obolibrary.org/obo/esmo.owl#hasArea -->

    <owl:DatatypeProperty rdf:about="http://purl.obolibrary.org/obo/esmo.owl#hasArea"/>
    


    <!-- http://purl.obolibrary.org/obo/esmo.owl#hasConcentration -->

    <owl:DatatypeProperty rdf:about="http://purl.obolibrary.org/obo/esmo.owl#hasConcentration"/>
    


    <!-- http://purl.obolibrary.org/obo/esmo.owl#hasCoordinates -->

    <owl:DatatypeProperty rdf:about="http://purl.obolibrary.org/obo/esmo.owl#hasCoordinates">
        <rdfs:subPropertyOf rdf:resource="http://www.w3.org/2002/07/owl#topDataProperty"/>
    </owl:DatatypeProperty>
    


    <!-- http://purl.obolibrary.org/obo/esmo.owl#hasCount -->

    <owl:DatatypeProperty rdf:about="http://purl.obolibrary.org/obo/esmo.owl#hasCount"/>
    


    <!-- http://purl.obolibrary.org/obo/esmo.owl#hasLatitude -->

    <owl:DatatypeProperty rdf:about="http://purl.obolibrary.org/obo/esmo.owl#hasLatitude">
        <rdfs:subPropertyOf rdf:resource="http://purl.obolibrary.org/obo/esmo.owl#hasCoordinates"/>
    </owl:DatatypeProperty>
    


    <!-- http://purl.obolibrary.org/obo/esmo.owl#hasLongitude -->

    <owl:DatatypeProperty rdf:about="http://purl.obolibrary.org/obo/esmo.owl#hasLongitude">
        <rdfs:subPropertyOf rdf:resource="http://purl.obolibrary.org/obo/esmo.owl#hasCoordinates"/>
    </owl:DatatypeProperty>
    


    <!-- http://purl.obolibrary.org/obo/esmo.owl#hasWholesaleValue -->

    <owl:DatatypeProperty rdf:about="http://purl.obolibrary.org/obo/esmo.owl#hasWholesaleValue"/>
    


    <!-- http://purl.obolibrary.org/obo/esmo.owl#hasYear -->

    <owl:DatatypeProperty rdf:about="http://purl.obolibrary.org/obo/esmo.owl#hasYear"/>
    


    <!-- 
    ///////////////////////////////////////////////////////////////////////////////////////
    //
    // Classes
    //
    ///////////////////////////////////////////////////////////////////////////////////////
     -->

    


    <!-- http://purl.obolibrary.org/obo/BFO_0000001 -->

    <owl:Class rdf:about="http://purl.obolibrary.org/obo/BFO_0000001">
        <dc:identifier>001-BFO</dc:identifier>
        <rdfs:label xml:lang="en">entity</rdfs:label>
        <skos:definition xml:lang="en">(Elucidation) An entity is anything that exists or has existed or will exist</skos:definition>
        <skos:example xml:lang="en">Julius Caesar, the Second World War, your body mass index, Verdi&apos;s Requiem.</skos:example>
        <skos:prefLabel xml:lang="en">entity</skos:prefLabel>
    </owl:Class>
    


    <!-- http://purl.obolibrary.org/obo/BFO_0000002 -->

    <owl:Class rdf:about="http://purl.obolibrary.org/obo/BFO_0000002">
        <rdfs:subClassOf rdf:resource="http://purl.obolibrary.org/obo/BFO_0000001"/>
        <rdfs:subClassOf>
            <owl:Restriction>
                <owl:onProperty rdf:resource="http://purl.obolibrary.org/obo/BFO_0000176"/>
                <owl:allValuesFrom rdf:resource="http://purl.obolibrary.org/obo/BFO_0000002"/>
            </owl:Restriction>
        </rdfs:subClassOf>
        <owl:disjointWith rdf:resource="http://purl.obolibrary.org/obo/BFO_0000003"/>
        <dc:identifier>008-BFO</dc:identifier>
        <rdfs:label xml:lang="en">continuant</rdfs:label>
        <skos:definition xml:lang="en">(Elucidation) A continuant is an entity that persists, endures, or continues to exist through time while maintaining its identity</skos:definition>
        <skos:example xml:lang="en">A human being, a tennis ball, a cave, a region of space, someone&apos;s temperature.</skos:example>
        <skos:prefLabel xml:lang="en">continuant</skos:prefLabel>
    </owl:Class>
    


    <!-- http://purl.obolibrary.org/obo/BFO_0000003 -->

    <owl:Class rdf:about="http://purl.obolibrary.org/obo/BFO_0000003">
        <rdfs:subClassOf rdf:resource="http://purl.obolibrary.org/obo/BFO_0000001"/>
        <dc:identifier>077-BFO</dc:identifier>
        <rdfs:label xml:lang="en">occurrent</rdfs:label>
        <skos:definition xml:lang="en">(Elucidation) An occurrent is an entity that unfolds itself in time or it is the start or end of such an entity or it is a temporal or spatiotemporal region</skos:definition>
        <skos:example xml:lang="en">As for process, history, process boundary, spatiotemporal region, zero-dimensional temporal region, one-dimensional temporal region, temporal interval, temporal instant.</skos:example>
        <skos:prefLabel xml:lang="en">occurrent</skos:prefLabel>
    </owl:Class>
    


    <!-- http://purl.obolibrary.org/obo/BFO_0000004 -->

    <owl:Class rdf:about="http://purl.obolibrary.org/obo/BFO_0000004">
        <rdfs:subClassOf rdf:resource="http://purl.obolibrary.org/obo/BFO_0000002"/>
        <rdfs:subClassOf>
            <owl:Restriction>
                <owl:onProperty rdf:resource="http://purl.obolibrary.org/obo/BFO_0000176"/>
                <owl:allValuesFrom rdf:resource="http://purl.obolibrary.org/obo/BFO_0000004"/>
            </owl:Restriction>
        </rdfs:subClassOf>
        <dc:identifier>017-BFO</dc:identifier>
        <rdfs:label xml:lang="en">independent continuant</rdfs:label>
        <skos:definition xml:lang="en">b is an independent continuant =Def b is a continuant which is such that there is no c such that b s-depends on c and no c such that b g-depends on c</skos:definition>
        <skos:example xml:lang="en">An atom, a molecule, an organism, a heart, a chair, the bottom right portion of a human torso, a leg; the interior of your mouth; a spatial region; an orchestra.</skos:example>
        <skos:prefLabel xml:lang="en">independent continuant</skos:prefLabel>
    </owl:Class>
    


    <!-- http://purl.obolibrary.org/obo/BFO_0000006 -->

    <owl:Class rdf:about="http://purl.obolibrary.org/obo/BFO_0000006">
        <rdfs:subClassOf rdf:resource="http://purl.obolibrary.org/obo/BFO_0000141"/>
        <rdfs:subClassOf>
            <owl:Restriction>
                <owl:onProperty rdf:resource="http://purl.obolibrary.org/obo/BFO_0000176"/>
                <owl:allValuesFrom rdf:resource="http://purl.obolibrary.org/obo/BFO_0000006"/>
            </owl:Restriction>
        </rdfs:subClassOf>
        <dc:identifier>035-BFO</dc:identifier>
        <rdfs:label xml:lang="en">spatial region</rdfs:label>
        <skos:definition xml:lang="en">(Elucidation) A spatial region is a continuant entity that is a continuant part of the spatial projection of a portion of spacetime at a given time</skos:definition>
        <skos:example xml:lang="en">As for zero-dimensional spatial region, one-dimensional spatial region, two-dimensional spatial region, three-dimensional spatial region.</skos:example>
        <skos:prefLabel xml:lang="en">spatial region</skos:prefLabel>
    </owl:Class>
    


    <!-- http://purl.obolibrary.org/obo/BFO_0000008 -->

    <owl:Class rdf:about="http://purl.obolibrary.org/obo/BFO_0000008">
        <rdfs:subClassOf rdf:resource="http://purl.obolibrary.org/obo/BFO_0000003"/>
        <rdfs:subClassOf>
            <owl:Restriction>
                <owl:onProperty rdf:resource="http://purl.obolibrary.org/obo/BFO_0000132"/>
                <owl:allValuesFrom rdf:resource="http://purl.obolibrary.org/obo/BFO_0000008"/>
            </owl:Restriction>
        </rdfs:subClassOf>
        <rdfs:subClassOf>
            <owl:Restriction>
                <owl:onProperty rdf:resource="http://purl.obolibrary.org/obo/BFO_0000139"/>
                <owl:allValuesFrom rdf:resource="http://purl.obolibrary.org/obo/BFO_0000008"/>
            </owl:Restriction>
        </rdfs:subClassOf>
        <dc:identifier>100-BFO</dc:identifier>
        <rdfs:label xml:lang="en">temporal region</rdfs:label>
        <skos:definition xml:lang="en">(Elucidation) A temporal region is an occurrent over which processes can unfold</skos:definition>
        <skos:example xml:lang="en">As for zero-dimensional temporal region and one-dimensional temporal region.</skos:example>
        <skos:prefLabel xml:lang="en">temporal region</skos:prefLabel>
    </owl:Class>
    


    <!-- http://purl.obolibrary.org/obo/BFO_0000009 -->

    <owl:Class rdf:about="http://purl.obolibrary.org/obo/BFO_0000009">
        <rdfs:subClassOf rdf:resource="http://purl.obolibrary.org/obo/BFO_0000006"/>
        <rdfs:subClassOf>
            <owl:Restriction>
                <owl:onProperty rdf:resource="http://purl.obolibrary.org/obo/BFO_0000178"/>
                <owl:allValuesFrom>
                    <owl:Class>
                        <owl:unionOf rdf:parseType="Collection">
                            <rdf:Description rdf:about="http://purl.obolibrary.org/obo/BFO_0000009"/>
                            <rdf:Description rdf:about="http://purl.obolibrary.org/obo/BFO_0000018"/>
                            <rdf:Description rdf:about="http://purl.obolibrary.org/obo/BFO_0000026"/>
                        </owl:unionOf>
                    </owl:Class>
                </owl:allValuesFrom>
            </owl:Restriction>
        </rdfs:subClassOf>
        <dc:identifier>039-BFO</dc:identifier>
        <rdfs:label xml:lang="en">two-dimensional spatial region</rdfs:label>
        <skos:definition xml:lang="en">(Elucidation) A two-dimensional spatial region is a spatial region that is a whole consisting of a surface together with zero or more surfaces and/or spatial regions of lower dimension as parts</skos:definition>
        <skos:example xml:lang="en">The surface of a sphere-shaped part of space, an infinitely thin plane in space.</skos:example>
        <skos:prefLabel xml:lang="en">two-dimensional spatial region</skos:prefLabel>
    </owl:Class>
    


    <!-- http://purl.obolibrary.org/obo/BFO_0000011 -->

    <owl:Class rdf:about="http://purl.obolibrary.org/obo/BFO_0000011">
        <rdfs:subClassOf rdf:resource="http://purl.obolibrary.org/obo/BFO_0000003"/>
        <rdfs:subClassOf>
            <owl:Restriction>
                <owl:onProperty rdf:resource="http://purl.obolibrary.org/obo/BFO_0000132"/>
                <owl:allValuesFrom rdf:resource="http://purl.obolibrary.org/obo/BFO_0000011"/>
            </owl:Restriction>
        </rdfs:subClassOf>
        <rdfs:subClassOf>
            <owl:Restriction>
                <owl:onProperty rdf:resource="http://purl.obolibrary.org/obo/BFO_0000139"/>
                <owl:allValuesFrom rdf:resource="http://purl.obolibrary.org/obo/BFO_0000011"/>
            </owl:Restriction>
        </rdfs:subClassOf>
        <dc:identifier>095-BFO</dc:identifier>
        <rdfs:label xml:lang="en">spatiotemporal region</rdfs:label>
        <skos:definition xml:lang="en">(Elucidation) A spatiotemporal region is an occurrent that is an occurrent part of spacetime</skos:definition>
        <skos:example xml:lang="en">The spatiotemporal region occupied by the development of a cancer tumour, the spatiotemporal region occupied by an orbiting satellite.</skos:example>
        <skos:prefLabel xml:lang="en">spatiotemporal region</skos:prefLabel>
        <skos:scopeNote xml:lang="en">&apos;Spacetime&apos; here refers to the maximal instance of the universal spatiotemporal region.</skos:scopeNote>
    </owl:Class>
    


    <!-- http://purl.obolibrary.org/obo/BFO_0000015 -->

    <owl:Class rdf:about="http://purl.obolibrary.org/obo/BFO_0000015">
        <rdfs:subClassOf rdf:resource="http://purl.obolibrary.org/obo/BFO_0000003"/>
        <rdfs:subClassOf>
            <owl:Restriction>
                <owl:onProperty rdf:resource="http://purl.obolibrary.org/obo/BFO_0000117"/>
                <owl:allValuesFrom>
                    <owl:Class>
                        <owl:unionOf rdf:parseType="Collection">
                            <rdf:Description rdf:about="http://purl.obolibrary.org/obo/BFO_0000015"/>
                            <rdf:Description rdf:about="http://purl.obolibrary.org/obo/BFO_0000035"/>
                        </owl:unionOf>
                    </owl:Class>
                </owl:allValuesFrom>
            </owl:Restriction>
        </rdfs:subClassOf>
        <rdfs:subClassOf>
            <owl:Restriction>
                <owl:onProperty rdf:resource="http://purl.obolibrary.org/obo/BFO_0000132"/>
                <owl:allValuesFrom rdf:resource="http://purl.obolibrary.org/obo/BFO_0000015"/>
            </owl:Restriction>
        </rdfs:subClassOf>
        <rdfs:subClassOf>
            <owl:Restriction>
                <owl:onProperty rdf:resource="http://purl.obolibrary.org/obo/BFO_0000139"/>
                <owl:allValuesFrom rdf:resource="http://purl.obolibrary.org/obo/BFO_0000015"/>
            </owl:Restriction>
        </rdfs:subClassOf>
        <dc:identifier>083-BFO</dc:identifier>
        <rdfs:label xml:lang="en">process</rdfs:label>
        <skos:definition xml:lang="en">(Elucidation) p is a process means p is an occurrent that has some temporal proper part and for some time t, p has some material entity as participant at t</skos:definition>
        <skos:example xml:lang="en">An act of selling, the life of an organism, a process of sleeping, a process of cell-division, a beating of the heart, a process of meiosis, the taxiing of an aircraft, the programming of a computer.</skos:example>
        <skos:prefLabel xml:lang="en">process</skos:prefLabel>
    </owl:Class>
    


    <!-- http://purl.obolibrary.org/obo/BFO_0000017 -->

    <owl:Class rdf:about="http://purl.obolibrary.org/obo/BFO_0000017">
        <rdfs:subClassOf rdf:resource="http://purl.obolibrary.org/obo/BFO_0000020"/>
        <owl:disjointWith rdf:resource="http://purl.obolibrary.org/obo/BFO_0000019"/>
        <dc:identifier>058-BFO</dc:identifier>
        <rdfs:label xml:lang="en">realizable entity</rdfs:label>
        <skos:definition xml:lang="en">(Elucidation) b is a realizable entity means: b is a specifically dependent continuant that inheres in some independent continuant which is not a spatial region and is of a type some instances of which are realized in processes of a correlated type</skos:definition>
        <skos:example xml:lang="en">The role of being a doctor, the role of this boundary to delineate where Utah and Colorado meet, the function of your reproductive organs, the disposition of your blood to coagulate, the disposition of this piece of metal to conduct electricity.</skos:example>
        <skos:prefLabel xml:lang="en">realizable entity</skos:prefLabel>
    </owl:Class>
    


    <!-- http://purl.obolibrary.org/obo/BFO_0000018 -->

    <owl:Class rdf:about="http://purl.obolibrary.org/obo/BFO_0000018">
        <rdfs:subClassOf rdf:resource="http://purl.obolibrary.org/obo/BFO_0000006"/>
        <rdfs:subClassOf>
            <owl:Restriction>
                <owl:onProperty rdf:resource="http://purl.obolibrary.org/obo/BFO_0000178"/>
                <owl:allValuesFrom rdf:resource="http://purl.obolibrary.org/obo/BFO_0000018"/>
            </owl:Restriction>
        </rdfs:subClassOf>
        <dc:identifier>037-BFO</dc:identifier>
        <rdfs:label xml:lang="en">zero-dimensional spatial region</rdfs:label>
        <skos:definition xml:lang="en">(Elucidation) A zero-dimensional spatial region is one or a collection of more than one spatially disjoint points in space</skos:definition>
        <skos:example xml:lang="en">The spatial region occupied at some time instant by the North Pole.</skos:example>
        <skos:prefLabel xml:lang="en">zero-dimensional spatial region</skos:prefLabel>
    </owl:Class>
    


    <!-- http://purl.obolibrary.org/obo/BFO_0000019 -->

    <owl:Class rdf:about="http://purl.obolibrary.org/obo/BFO_0000019">
        <rdfs:subClassOf rdf:resource="http://purl.obolibrary.org/obo/BFO_0000020"/>
        <dc:identifier>055-BFO</dc:identifier>
        <rdfs:label xml:lang="en">quality</rdfs:label>
        <skos:definition xml:lang="en">(Elucidation) a quality is a specifically dependent continuant that, in contrast to roles and dispositions, does not require any further process in order to be realized</skos:definition>
        <skos:example xml:lang="en">The colour of a tomato, the ambient temperature of this portion of air, the length of the circumference of your waist, the shape of your nose, the shape of your nostril, the mass of this piece of gold.</skos:example>
        <skos:prefLabel xml:lang="en">quality</skos:prefLabel>
    </owl:Class>
    


    <!-- http://purl.obolibrary.org/obo/BFO_0000020 -->

    <owl:Class rdf:about="http://purl.obolibrary.org/obo/BFO_0000020">
        <rdfs:subClassOf rdf:resource="http://purl.obolibrary.org/obo/BFO_0000002"/>
        <dc:identifier>050-BFO</dc:identifier>
        <rdfs:label xml:lang="en">specifically dependent continuant</rdfs:label>
        <skos:definition xml:lang="en">b is a specifically dependent continuant =Def b is a continuant &amp; there is some independent continuant c which is not a spatial region &amp; which is such that b s-depends on c</skos:definition>
        <skos:example xml:lang="en">(with one bearer) The mass of this tomato, the pink colour of a medium rare piece of grilled filet mignon at its centre, the smell of this portion of mozzarella, the disposition of this fish to decay, the role of being a doctor, the function of this heart: to pump blood, the shape of this hole; (with multiple bearers:) John&apos;s love for Mary, the ownership relation between John and this statue, the relation of authority between John and his subordinates.</skos:example>
        <skos:prefLabel xml:lang="en">specifically dependent continuant</skos:prefLabel>
        <skos:scopeNote xml:lang="en">On the multiple bearers case, see relational quality.</skos:scopeNote>
    </owl:Class>
    


    <!-- http://purl.obolibrary.org/obo/BFO_0000023 -->

    <owl:Class rdf:about="http://purl.obolibrary.org/obo/BFO_0000023">
        <rdfs:subClassOf rdf:resource="http://purl.obolibrary.org/obo/BFO_0000017"/>
        <dc:identifier>061-BFO</dc:identifier>
        <rdfs:label xml:lang="en">role</rdfs:label>
        <skos:altLabel xml:lang="en">externally-grounded realizable entity</skos:altLabel>
        <skos:definition xml:lang="en">(Elucidation) b is a role means: b is a realizable entity &amp; b exists because there is some single bearer that is in some special physical, social, or institutional set of circumstances in which this bearer does not have to be &amp; b is not such that, if it ceases to exist, then the physical make-up of the bearer is thereby changed</skos:definition>
        <skos:example xml:lang="en">The priest role, the student role, the role of subject in a clinical trial, the role of a stone in marking a property boundary, the role of a boundary to demarcate two neighbouring administrative territories, the role of a building in serving as a military target.</skos:example>
        <skos:prefLabel xml:lang="en">role</skos:prefLabel>
    </owl:Class>
    


    <!-- http://purl.obolibrary.org/obo/BFO_0000024 -->

    <owl:Class rdf:about="http://purl.obolibrary.org/obo/BFO_0000024">
        <rdfs:subClassOf rdf:resource="http://purl.obolibrary.org/obo/BFO_0000040"/>
        <dc:identifier>027-BFO</dc:identifier>
        <rdfs:label xml:lang="en">fiat object part</rdfs:label>
        <skos:definition xml:lang="en">(Elucidation) a fiat object part b is a material entity which is such that for all times t, if b exists at t then there is some object c such that b is a proper continuant part of c at t and b is demarcated from the remainder of c by one or more fiat surfaces</skos:definition>
        <skos:example xml:lang="en">The upper and lower lobes of the left lung, the dorsal and ventral surfaces of the body, the Western hemisphere of the Earth, the FMA:regional parts of an intact human body.</skos:example>
        <skos:prefLabel xml:lang="en">fiat object part</skos:prefLabel>
    </owl:Class>
    


    <!-- http://purl.obolibrary.org/obo/BFO_0000026 -->

    <owl:Class rdf:about="http://purl.obolibrary.org/obo/BFO_0000026">
        <rdfs:subClassOf rdf:resource="http://purl.obolibrary.org/obo/BFO_0000006"/>
        <rdfs:subClassOf>
            <owl:Restriction>
                <owl:onProperty rdf:resource="http://purl.obolibrary.org/obo/BFO_0000178"/>
                <owl:allValuesFrom>
                    <owl:Class>
                        <owl:unionOf rdf:parseType="Collection">
                            <rdf:Description rdf:about="http://purl.obolibrary.org/obo/BFO_0000018"/>
                            <rdf:Description rdf:about="http://purl.obolibrary.org/obo/BFO_0000026"/>
                        </owl:unionOf>
                    </owl:Class>
                </owl:allValuesFrom>
            </owl:Restriction>
        </rdfs:subClassOf>
        <dc:identifier>038-BFO</dc:identifier>
        <rdfs:label xml:lang="en">one-dimensional spatial region</rdfs:label>
        <skos:definition xml:lang="en">(Elucidation) A one-dimensional spatial region is a whole consisting of a line together with zero or more lines and/or points as parts</skos:definition>
        <skos:example xml:lang="en">An edge of a cube-shaped portion of space, a line connecting two points, two parallel lines extended in space.</skos:example>
        <skos:prefLabel xml:lang="en">one-dimensional spatial region</skos:prefLabel>
    </owl:Class>
    


    <!-- http://purl.obolibrary.org/obo/BFO_0000027 -->

    <owl:Class rdf:about="http://purl.obolibrary.org/obo/BFO_0000027">
        <rdfs:subClassOf rdf:resource="http://purl.obolibrary.org/obo/BFO_0000040"/>
        <dc:identifier>025-BFO</dc:identifier>
        <rdfs:label xml:lang="en">object aggregate</rdfs:label>
        <skos:definition xml:lang="en">(Elucidation) an object aggregate is a material entity consisting exactly of a plurality (≥1) of objects as member parts which together form a unit</skos:definition>
        <skos:example xml:lang="en">The aggregate of the musicians in a symphony orchestra and their instruments, the aggregate of bearings in a constant velocity axle joint, the nitrogen atoms in the atmosphere, a collection of cells in a blood biobank. NOTE 1: &apos;Exactly&apos; means that there are no parts of the object aggregate other than its member parts. NOTE 2: The unit can, at certain times, consist of exactly one object, for example, when a wolf litter loses all but one of its pups, but it must at some time have a plurality of member parts.</skos:example>
        <skos:prefLabel xml:lang="en">object aggregate</skos:prefLabel>
    </owl:Class>
    


    <!-- http://purl.obolibrary.org/obo/BFO_0000028 -->

    <owl:Class rdf:about="http://purl.obolibrary.org/obo/BFO_0000028">
        <rdfs:subClassOf rdf:resource="http://purl.obolibrary.org/obo/BFO_0000006"/>
        <rdfs:subClassOf>
            <owl:Restriction>
                <owl:onProperty rdf:resource="http://purl.obolibrary.org/obo/BFO_0000178"/>
                <owl:allValuesFrom rdf:resource="http://purl.obolibrary.org/obo/BFO_0000006"/>
            </owl:Restriction>
        </rdfs:subClassOf>
        <dc:identifier>040-BFO</dc:identifier>
        <rdfs:label xml:lang="en">three-dimensional spatial region</rdfs:label>
        <skos:definition xml:lang="en">(Elucidation) A three-dimensional spatial region is a whole consisting of a spatial volume together with zero or more spatial volumes and/or spatial regions of lower dimension as parts</skos:definition>
        <skos:example xml:lang="en">A cube-shaped region of space, a sphere-shaped region of space, the region of space occupied by all and only the planets in the solar system at some point in time.</skos:example>
        <skos:prefLabel xml:lang="en">three-dimensional spatial region</skos:prefLabel>
    </owl:Class>
    


    <!-- http://purl.obolibrary.org/obo/BFO_0000029 -->

    <owl:Class rdf:about="http://purl.obolibrary.org/obo/BFO_0000029">
        <rdfs:subClassOf rdf:resource="http://purl.obolibrary.org/obo/BFO_0000141"/>
        <rdfs:subClassOf>
            <owl:Restriction>
                <owl:onProperty rdf:resource="http://purl.obolibrary.org/obo/BFO_0000176"/>
                <owl:allValuesFrom>
                    <owl:Class>
                        <owl:unionOf rdf:parseType="Collection">
                            <rdf:Description rdf:about="http://purl.obolibrary.org/obo/BFO_0000029"/>
                            <rdf:Description rdf:about="http://purl.obolibrary.org/obo/BFO_0000040"/>
                        </owl:unionOf>
                    </owl:Class>
                </owl:allValuesFrom>
            </owl:Restriction>
        </rdfs:subClassOf>
        <rdfs:subClassOf>
            <owl:Restriction>
                <owl:onProperty rdf:resource="http://purl.obolibrary.org/obo/BFO_0000210"/>
                <owl:allValuesFrom rdf:resource="http://purl.obolibrary.org/obo/BFO_0000028"/>
            </owl:Restriction>
        </rdfs:subClassOf>
        <dc:identifier>034-BFO</dc:identifier>
        <rdfs:label xml:lang="en">site</rdfs:label>
        <skos:definition xml:lang="en">(Elucidation) b is a site means: b is a three-dimensional immaterial entity whose boundaries either (1) (partially or wholly) coincide with the boundaries of one or more material entities or (2) have locations determined in relation to some material entity</skos:definition>
        <skos:example xml:lang="en">A hole in a portion of cheese, a rabbit hole, the Grand Canyon, the Piazza San Marco, the kangaroo-joey-containing hole of a kangaroo pouch, your left nostril (a fiat part - the opening - of your left nasal cavity), the lumen of your gut, the hold of a ship, the interior of the trunk of your car, hole in an engineered floor joist; An air traffic control region of type A is determined in terms of elevation above mean sea level of lower and upper boundaries.</skos:example>
        <skos:prefLabel xml:lang="en">site</skos:prefLabel>
    </owl:Class>
    


    <!-- http://purl.obolibrary.org/obo/BFO_0000030 -->

    <owl:Class rdf:about="http://purl.obolibrary.org/obo/BFO_0000030">
        <rdfs:subClassOf rdf:resource="http://purl.obolibrary.org/obo/BFO_0000040"/>
        <dc:identifier>024-BFO</dc:identifier>
        <rdfs:label xml:lang="en">object</rdfs:label>
        <skos:definition xml:lang="en">(Elucidation) an object is a material entity which manifests causal unity &amp; is of a type instances of which are maximal relative to the sort of causal unity manifested</skos:definition>
        <skos:example xml:lang="en">An organism, a fish tank, a planet, a laptop, a valve, a block of marble, an ice cube.</skos:example>
        <skos:prefLabel xml:lang="en">object</skos:prefLabel>
        <skos:scopeNote xml:lang="en">A description of three primary sorts of causal unity is provided in Basic Formal Ontology 2.0. Specification and User’s Guide</skos:scopeNote>
    </owl:Class>
    


    <!-- http://purl.obolibrary.org/obo/BFO_0000035 -->

    <owl:Class rdf:about="http://purl.obolibrary.org/obo/BFO_0000035">
        <rdfs:subClassOf rdf:resource="http://purl.obolibrary.org/obo/BFO_0000003"/>
        <rdfs:subClassOf>
            <owl:Restriction>
                <owl:onProperty rdf:resource="http://purl.obolibrary.org/obo/BFO_0000117"/>
                <owl:allValuesFrom rdf:resource="http://purl.obolibrary.org/obo/BFO_0000035"/>
            </owl:Restriction>
        </rdfs:subClassOf>
        <rdfs:subClassOf>
            <owl:Restriction>
                <owl:onProperty rdf:resource="http://purl.obolibrary.org/obo/BFO_0000121"/>
                <owl:allValuesFrom rdf:resource="http://purl.obolibrary.org/obo/BFO_0000035"/>
            </owl:Restriction>
        </rdfs:subClassOf>
        <rdfs:subClassOf>
            <owl:Restriction>
                <owl:onProperty rdf:resource="http://purl.obolibrary.org/obo/BFO_0000132"/>
                <owl:allValuesFrom>
                    <owl:Class>
                        <owl:unionOf rdf:parseType="Collection">
                            <rdf:Description rdf:about="http://purl.obolibrary.org/obo/BFO_0000015"/>
                            <rdf:Description rdf:about="http://purl.obolibrary.org/obo/BFO_0000035"/>
                        </owl:unionOf>
                    </owl:Class>
                </owl:allValuesFrom>
            </owl:Restriction>
        </rdfs:subClassOf>
        <rdfs:subClassOf>
            <owl:Restriction>
                <owl:onProperty rdf:resource="http://purl.obolibrary.org/obo/BFO_0000139"/>
                <owl:allValuesFrom>
                    <owl:Class>
                        <owl:unionOf rdf:parseType="Collection">
                            <rdf:Description rdf:about="http://purl.obolibrary.org/obo/BFO_0000015"/>
                            <rdf:Description rdf:about="http://purl.obolibrary.org/obo/BFO_0000035"/>
                        </owl:unionOf>
                    </owl:Class>
                </owl:allValuesFrom>
            </owl:Restriction>
        </rdfs:subClassOf>
        <dc:identifier>084-BFO</dc:identifier>
        <rdfs:label xml:lang="en">process boundary</rdfs:label>
        <skos:definition xml:lang="en">p is a process boundary =Def p is a temporal part of a process &amp; p has no proper temporal parts</skos:definition>
        <skos:example xml:lang="en">The boundary between the 2nd and 3rd year of your life.</skos:example>
        <skos:prefLabel xml:lang="en">process boundary</skos:prefLabel>
    </owl:Class>
    


    <!-- http://purl.obolibrary.org/obo/BFO_0000038 -->

    <owl:Class rdf:about="http://purl.obolibrary.org/obo/BFO_0000038">
        <rdfs:subClassOf rdf:resource="http://purl.obolibrary.org/obo/BFO_0000008"/>
        <rdfs:subClassOf>
            <owl:Restriction>
                <owl:onProperty rdf:resource="http://purl.obolibrary.org/obo/BFO_0000121"/>
                <owl:allValuesFrom>
                    <owl:Class>
                        <owl:unionOf rdf:parseType="Collection">
                            <rdf:Description rdf:about="http://purl.obolibrary.org/obo/BFO_0000038"/>
                            <rdf:Description rdf:about="http://purl.obolibrary.org/obo/BFO_0000148"/>
                        </owl:unionOf>
                    </owl:Class>
                </owl:allValuesFrom>
            </owl:Restriction>
        </rdfs:subClassOf>
        <rdfs:subClassOf>
            <owl:Restriction>
                <owl:onProperty rdf:resource="http://purl.obolibrary.org/obo/BFO_0000139"/>
                <owl:allValuesFrom rdf:resource="http://purl.obolibrary.org/obo/BFO_0000038"/>
            </owl:Restriction>
        </rdfs:subClassOf>
        <owl:disjointWith rdf:resource="http://purl.obolibrary.org/obo/BFO_0000148"/>
        <dc:identifier>103-BFO</dc:identifier>
        <rdfs:label xml:lang="en">one-dimensional temporal region</rdfs:label>
        <skos:definition xml:lang="en">(Elucidation) A one-dimensional temporal region is a temporal region is a whole that has a temporal interval and zero or more temporal intervals and temporal instants as parts</skos:definition>
        <skos:example xml:lang="en">The temporal region during which a process occurs.</skos:example>
        <skos:prefLabel xml:lang="en">one-dimensional temporal region</skos:prefLabel>
    </owl:Class>
    


    <!-- http://purl.obolibrary.org/obo/BFO_0000040 -->

    <owl:Class rdf:about="http://purl.obolibrary.org/obo/BFO_0000040">
        <rdfs:subClassOf rdf:resource="http://purl.obolibrary.org/obo/BFO_0000004"/>
        <rdfs:subClassOf>
            <owl:Restriction>
                <owl:onProperty rdf:resource="http://purl.obolibrary.org/obo/BFO_0000176"/>
                <owl:allValuesFrom rdf:resource="http://purl.obolibrary.org/obo/BFO_0000040"/>
            </owl:Restriction>
        </rdfs:subClassOf>
        <owl:disjointWith rdf:resource="http://purl.obolibrary.org/obo/BFO_0000141"/>
        <dc:identifier>019-BFO</dc:identifier>
        <rdfs:label xml:lang="en">material entity</rdfs:label>
        <skos:definition xml:lang="en">(Elucidation) A material entity is an independent continuant that at all times at which it exists has some portion of matter as continuant part</skos:definition>
        <skos:example xml:lang="en">A human being, the undetached arm of a human being, an aggregate of human beings.</skos:example>
        <skos:prefLabel xml:lang="en">material entity</skos:prefLabel>
    </owl:Class>
    


    <!-- http://purl.obolibrary.org/obo/BFO_0000141 -->

    <owl:Class rdf:about="http://purl.obolibrary.org/obo/BFO_0000141">
        <rdfs:subClassOf rdf:resource="http://purl.obolibrary.org/obo/BFO_0000004"/>
        <dc:identifier>028-BFO</dc:identifier>
        <rdfs:label xml:lang="en">immaterial entity</rdfs:label>
        <skos:definition xml:lang="en">a is an immaterial entity =Def a is an independent continuant which is such that there is no time t when it has a material entity as continuant part at t</skos:definition>
        <skos:example xml:lang="en">As for fiat point, fiat line, fiat surface, site.</skos:example>
        <skos:prefLabel xml:lang="en">immaterial entity</skos:prefLabel>
    </owl:Class>
    


    <!-- http://purl.obolibrary.org/obo/BFO_0000148 -->

    <owl:Class rdf:about="http://purl.obolibrary.org/obo/BFO_0000148">
        <rdfs:subClassOf rdf:resource="http://purl.obolibrary.org/obo/BFO_0000008"/>
        <rdfs:subClassOf>
            <owl:Restriction>
                <owl:onProperty rdf:resource="http://purl.obolibrary.org/obo/BFO_0000121"/>
                <owl:allValuesFrom rdf:resource="http://purl.obolibrary.org/obo/BFO_0000148"/>
            </owl:Restriction>
        </rdfs:subClassOf>
        <dc:identifier>102-BFO</dc:identifier>
        <rdfs:label xml:lang="en">zero-dimensional temporal region</rdfs:label>
        <skos:definition xml:lang="en">(Elucidation) A zero-dimensional temporal region is a temporal region that is a whole consisting of one or more separated temporal instants as parts</skos:definition>
        <skos:example xml:lang="en">A temporal region that is occupied by a process boundary; the moment at which a finger is detached in an industrial accident.</skos:example>
        <skos:prefLabel xml:lang="en">zero-dimensional temporal region</skos:prefLabel>
    </owl:Class>
    


    <!-- http://purl.obolibrary.org/obo/BFO_0000202 -->

    <owl:Class rdf:about="http://purl.obolibrary.org/obo/BFO_0000202">
        <rdfs:subClassOf rdf:resource="http://purl.obolibrary.org/obo/BFO_0000038"/>
        <dc:identifier>155-BFO</dc:identifier>
        <rdfs:label xml:lang="en">temporal interval</rdfs:label>
        <skos:definition xml:lang="en">(Elucidation) a temporal interval is a one-dimensional temporal region that is continuous, thus without gaps or breaks</skos:definition>
        <skos:example xml:lang="en">The year 2018.</skos:example>
        <skos:prefLabel xml:lang="en">temporal interval</skos:prefLabel>
        <skos:scopeNote xml:lang="en">A one-dimensional temporal region can include as parts not only temporal intervals but also temporal instants separated from other parts by gaps.</skos:scopeNote>
    </owl:Class>
    


    <!-- http://purl.obolibrary.org/obo/BFO_0000203 -->

    <owl:Class rdf:about="http://purl.obolibrary.org/obo/BFO_0000203">
        <rdfs:subClassOf rdf:resource="http://purl.obolibrary.org/obo/BFO_0000148"/>
        <dc:identifier>209-BFO</dc:identifier>
        <rdfs:label xml:lang="en">temporal instant</rdfs:label>
        <skos:definition xml:lang="en">(Elucidation) a temporal instant is a zero-dimensional temporal region that has no proper temporal part</skos:definition>
        <skos:example xml:lang="en">The millennium.</skos:example>
        <skos:prefLabel xml:lang="en">temporal instant</skos:prefLabel>
    </owl:Class>
    


    <!-- http://purl.obolibrary.org/obo/esmo.owl#Abiotic_component -->

    <owl:Class rdf:about="http://purl.obolibrary.org/obo/esmo.owl#Abiotic_component">
        <rdfs:subClassOf rdf:resource="http://purl.obolibrary.org/obo/esmo.owl#Ecosystem_component"/>
        <skos:definition>The non-living components that form part of an ecosystem.</skos:definition>
        <skos:example>A river, a lake, soil</skos:example>
    </owl:Class>
    


    <!-- http://purl.obolibrary.org/obo/esmo.owl#Abiotic_component_aggregate -->

    <owl:Class rdf:about="http://purl.obolibrary.org/obo/esmo.owl#Abiotic_component_aggregate">
        <rdfs:subClassOf rdf:resource="http://purl.obolibrary.org/obo/esmo.owl#Ecosystem_component_aggregate"/>
    </owl:Class>
    


    <!-- http://purl.obolibrary.org/obo/esmo.owl#Actor -->

    <owl:Class rdf:about="http://purl.obolibrary.org/obo/esmo.owl#Actor">
        <rdfs:subClassOf rdf:resource="http://purl.obolibrary.org/obo/BFO_0000030"/>
        <rdfs:subClassOf>
            <owl:Restriction>
                <owl:onProperty rdf:resource="http://purl.obolibrary.org/obo/BFO_0000166"/>
                <owl:someValuesFrom rdf:resource="http://purl.obolibrary.org/obo/esmo.owl#Human_activity"/>
            </owl:Restriction>
        </rdfs:subClassOf>
        <rdfs:subClassOf>
            <owl:Restriction>
                <owl:onProperty rdf:resource="http://purl.obolibrary.org/obo/BFO_0000175"/>
                <owl:someValuesFrom rdf:resource="http://purl.obolibrary.org/obo/esmo.owl#Actor_aggregate"/>
            </owl:Restriction>
        </rdfs:subClassOf>
        <rdfs:subClassOf>
            <owl:Restriction>
                <owl:onProperty rdf:resource="http://purl.obolibrary.org/obo/esmo.owl#benefits_from"/>
                <owl:someValuesFrom rdf:resource="http://purl.obolibrary.org/obo/esmo.owl#Relational_value"/>
            </owl:Restriction>
        </rdfs:subClassOf>
        <skos:definition>An individual entity within a social-ecological system that performs actions or makes decisions impacting the system&apos;s dynamics and outcomes.</skos:definition>
    </owl:Class>
    


    <!-- http://purl.obolibrary.org/obo/esmo.owl#Actor_aggregate -->

    <owl:Class rdf:about="http://purl.obolibrary.org/obo/esmo.owl#Actor_aggregate">
        <rdfs:subClassOf rdf:resource="http://purl.obolibrary.org/obo/BFO_0000027"/>
        <rdfs:subClassOf>
            <owl:Restriction>
                <owl:onProperty rdf:resource="http://purl.obolibrary.org/obo/BFO_0000174"/>
                <owl:someValuesFrom rdf:resource="http://purl.obolibrary.org/obo/esmo.owl#Actor"/>
            </owl:Restriction>
        </rdfs:subClassOf>
        <skos:definition>Is a material entity consisting exactly of a plurality (≥1) of actors as member parts which together form a unit.</skos:definition>
        <skos:example>A local community, a group of fishers</skos:example>
    </owl:Class>
    


    <!-- http://purl.obolibrary.org/obo/esmo.owl#Anthropogenic_asset -->

    <owl:Class rdf:about="http://purl.obolibrary.org/obo/esmo.owl#Anthropogenic_asset">
        <rdfs:subClassOf rdf:resource="http://purl.obolibrary.org/obo/BFO_0000030"/>
        <rdfs:subClassOf>
            <owl:Restriction>
                <owl:onProperty rdf:resource="http://purl.obolibrary.org/obo/BFO_0000166"/>
                <owl:someValuesFrom rdf:resource="http://purl.obolibrary.org/obo/esmo.owl#Human_activity"/>
            </owl:Restriction>
        </rdfs:subClassOf>
        <rdfs:subClassOf>
            <owl:Restriction>
                <owl:onProperty rdf:resource="http://purl.obolibrary.org/obo/BFO_0000175"/>
                <owl:someValuesFrom rdf:resource="http://purl.obolibrary.org/obo/esmo.owl#Anthropogenic_asset_aggregate"/>
            </owl:Restriction>
        </rdfs:subClassOf>
        <skos:definition>Any human-made or human-influenced object that contributes to human well-being and economic activity.</skos:definition>
        <skos:example>A fishing boat, fertiliser, infrastructure</skos:example>
    </owl:Class>
    


    <!-- http://purl.obolibrary.org/obo/esmo.owl#Anthropogenic_asset_aggregate -->

    <owl:Class rdf:about="http://purl.obolibrary.org/obo/esmo.owl#Anthropogenic_asset_aggregate">
        <rdfs:subClassOf rdf:resource="http://purl.obolibrary.org/obo/BFO_0000027"/>
        <rdfs:subClassOf>
            <owl:Restriction>
                <owl:onProperty rdf:resource="http://purl.obolibrary.org/obo/BFO_0000056"/>
                <owl:someValuesFrom rdf:resource="http://purl.obolibrary.org/obo/esmo.owl#Human_activity"/>
            </owl:Restriction>
        </rdfs:subClassOf>
        <rdfs:subClassOf>
            <owl:Restriction>
                <owl:onProperty rdf:resource="http://purl.obolibrary.org/obo/BFO_0000174"/>
                <owl:someValuesFrom rdf:resource="http://purl.obolibrary.org/obo/esmo.owl#Anthropogenic_asset"/>
            </owl:Restriction>
        </rdfs:subClassOf>
        <skos:definition>Is a material entity consisting exactly of a plurality (≥1) of anthropogenic assets as member parts which together form a unit.</skos:definition>
        <skos:example>A fishing fleet, all the paths in a provincial park</skos:example>
    </owl:Class>
    


    <!-- http://purl.obolibrary.org/obo/esmo.owl#Biological_control -->

    <owl:Class rdf:about="http://purl.obolibrary.org/obo/esmo.owl#Biological_control">
        <rdfs:subClassOf rdf:resource="http://purl.obolibrary.org/obo/esmo.owl#Ecosystem_function"/>
        <rdfs:subClassOf>
            <owl:Restriction>
                <owl:onProperty rdf:resource="http://purl.obolibrary.org/obo/BFO_0000118"/>
                <owl:someValuesFrom rdf:resource="http://purl.obolibrary.org/obo/esmo.owl#Predation"/>
            </owl:Restriction>
        </rdfs:subClassOf>
        <skos:definition>The control of pests such as insects, mites, weeds and plant diseases by other organisms.</skos:definition>
    </owl:Class>
    


    <!-- http://purl.obolibrary.org/obo/esmo.owl#Biomass_production -->

    <owl:Class rdf:about="http://purl.obolibrary.org/obo/esmo.owl#Biomass_production">
        <rdfs:subClassOf rdf:resource="http://purl.obolibrary.org/obo/esmo.owl#Ecosystem_function"/>
        <rdfs:subClassOf>
            <owl:Restriction>
                <owl:onProperty rdf:resource="http://purl.obolibrary.org/obo/BFO_0000118"/>
                <owl:someValuesFrom rdf:resource="http://purl.obolibrary.org/obo/esmo.owl#Predation"/>
            </owl:Restriction>
        </rdfs:subClassOf>
        <skos:definition>A process involving the generation of organic material through biological growth.</skos:definition>
    </owl:Class>
    


    <!-- http://purl.obolibrary.org/obo/esmo.owl#Biotic_component -->

    <owl:Class rdf:about="http://purl.obolibrary.org/obo/esmo.owl#Biotic_component">
        <rdfs:subClassOf rdf:resource="http://purl.obolibrary.org/obo/esmo.owl#Ecosystem_component"/>
        <skos:definition>The living components that form part of an ecosystem.</skos:definition>
        <skos:example>A maple tree, a horse</skos:example>
    </owl:Class>
    


    <!-- http://purl.obolibrary.org/obo/esmo.owl#Biotic_component_aggregate -->

    <owl:Class rdf:about="http://purl.obolibrary.org/obo/esmo.owl#Biotic_component_aggregate">
        <rdfs:subClassOf rdf:resource="http://purl.obolibrary.org/obo/esmo.owl#Ecosystem_component_aggregate"/>
    </owl:Class>
    


    <!-- http://purl.obolibrary.org/obo/esmo.owl#Carbon_fixation -->

    <owl:Class rdf:about="http://purl.obolibrary.org/obo/esmo.owl#Carbon_fixation">
        <rdfs:subClassOf rdf:resource="http://purl.obolibrary.org/obo/esmo.owl#Ecosystem_process"/>
        <rdfs:subClassOf>
            <owl:Restriction>
                <owl:onProperty rdf:resource="http://purl.obolibrary.org/obo/BFO_0000138"/>
                <owl:someValuesFrom rdf:resource="http://purl.obolibrary.org/obo/esmo.owl#Net_primary_production"/>
            </owl:Restriction>
        </rdfs:subClassOf>
        <skos:definition>A biochemical process in which inorganic carbon, typically in the form of carbon dioxide, is converted into organic compounds by living organisms, primarily through photosynthesis.</skos:definition>
    </owl:Class>
    


    <!-- http://purl.obolibrary.org/obo/esmo.owl#Clean_freshwater -->

    <owl:Class rdf:about="http://purl.obolibrary.org/obo/esmo.owl#Clean_freshwater">
        <rdfs:subClassOf rdf:resource="http://purl.obolibrary.org/obo/esmo.owl#Ecosystem_good"/>
        <rdfs:subClassOf>
            <owl:Restriction>
                <owl:onProperty rdf:resource="http://purl.obolibrary.org/obo/BFO_0000056"/>
                <owl:someValuesFrom rdf:resource="http://purl.obolibrary.org/obo/esmo.owl#Swimming"/>
            </owl:Restriction>
        </rdfs:subClassOf>
        <rdfs:subClassOf>
            <owl:Restriction>
                <owl:onProperty rdf:resource="http://purl.obolibrary.org/obo/esmo.owl#output_of"/>
                <owl:someValuesFrom rdf:resource="http://purl.obolibrary.org/obo/esmo.owl#Water_purification"/>
            </owl:Restriction>
        </rdfs:subClassOf>
        <skos:definition>Water from natural sources, such as rivers, lakes, or aquifers, that is free from harmful contaminants and pollutants, making it safe for consumption, agricultural use, and supporting aquatic ecosystems. It is characterized by low levels of pathogens, chemicals, and physical impurities, ensuring it meets health and environmental standards.</skos:definition>
    </owl:Class>
    


    <!-- http://purl.obolibrary.org/obo/esmo.owl#Commercial_fisher -->

    <owl:Class rdf:about="http://purl.obolibrary.org/obo/esmo.owl#Commercial_fisher">
        <rdfs:subClassOf rdf:resource="http://purl.obolibrary.org/obo/esmo.owl#Economic_actor"/>
        <rdfs:subClassOf>
            <owl:Restriction>
                <owl:onProperty rdf:resource="http://purl.obolibrary.org/obo/BFO_0000056"/>
                <owl:someValuesFrom rdf:resource="http://purl.obolibrary.org/obo/esmo.owl#Commercial_fishing"/>
            </owl:Restriction>
        </rdfs:subClassOf>
        <rdfs:subClassOf>
            <owl:Restriction>
                <owl:onProperty rdf:resource="http://purl.obolibrary.org/obo/esmo.owl#benefits_from"/>
                <owl:someValuesFrom rdf:resource="http://purl.obolibrary.org/obo/esmo.owl#Monetary_instrumental_value"/>
            </owl:Restriction>
        </rdfs:subClassOf>
        <skos:definition>A type of economic actor who participates in the commercial fishing activity.</skos:definition>
    </owl:Class>
    


    <!-- http://purl.obolibrary.org/obo/esmo.owl#Commercial_fishing -->

    <owl:Class rdf:about="http://purl.obolibrary.org/obo/esmo.owl#Commercial_fishing">
        <rdfs:subClassOf rdf:resource="http://purl.obolibrary.org/obo/esmo.owl#Economic_activity"/>
        <rdfs:subClassOf>
            <owl:Restriction>
                <owl:onProperty rdf:resource="http://purl.obolibrary.org/obo/BFO_0000055"/>
                <owl:someValuesFrom rdf:resource="http://purl.obolibrary.org/obo/esmo.owl#Wild_fish_provisioning_service"/>
            </owl:Restriction>
        </rdfs:subClassOf>
        <rdfs:subClassOf>
            <owl:Restriction>
                <owl:onProperty rdf:resource="http://purl.obolibrary.org/obo/BFO_0000167"/>
                <owl:someValuesFrom rdf:resource="http://purl.obolibrary.org/obo/esmo.owl#Commercial_fisher"/>
            </owl:Restriction>
        </rdfs:subClassOf>
        <rdfs:subClassOf>
            <owl:Restriction>
                <owl:onProperty rdf:resource="http://purl.obolibrary.org/obo/BFO_0000167"/>
                <owl:someValuesFrom rdf:resource="http://purl.obolibrary.org/obo/esmo.owl#Fish_population"/>
            </owl:Restriction>
        </rdfs:subClassOf>
        <rdfs:subClassOf>
            <owl:Restriction>
                <owl:onProperty rdf:resource="http://purl.obolibrary.org/obo/BFO_0000167"/>
                <owl:someValuesFrom rdf:resource="http://purl.obolibrary.org/obo/esmo.owl#Fishing_fleet"/>
            </owl:Restriction>
        </rdfs:subClassOf>
        <rdfs:subClassOf>
            <owl:Restriction>
                <owl:onProperty rdf:resource="http://purl.obolibrary.org/obo/esmo.owl#causally_upstream_of"/>
                <owl:someValuesFrom rdf:resource="http://purl.obolibrary.org/obo/esmo.owl#Exploitation"/>
            </owl:Restriction>
        </rdfs:subClassOf>
        <rdfs:subClassOf>
            <owl:Restriction>
                <owl:onProperty rdf:resource="http://purl.obolibrary.org/obo/esmo.owl#has_output"/>
                <owl:someValuesFrom rdf:resource="http://purl.obolibrary.org/obo/esmo.owl#Wildcaught_fish"/>
            </owl:Restriction>
        </rdfs:subClassOf>
        <skos:definition>An economic activity that involves the harvesting of wild fish for the purpose of generating economic gain through the sale of catch on the market.</skos:definition>
        <skos:example>Commercial cod fishing, commercial salmon fishing</skos:example>
    </owl:Class>
    


    <!-- http://purl.obolibrary.org/obo/esmo.owl#Commodity -->

    <owl:Class rdf:about="http://purl.obolibrary.org/obo/esmo.owl#Commodity">
        <rdfs:subClassOf rdf:resource="http://purl.obolibrary.org/obo/BFO_0000030"/>
        <rdfs:subClassOf>
            <owl:Restriction>
                <owl:onProperty rdf:resource="http://purl.obolibrary.org/obo/BFO_0000175"/>
                <owl:someValuesFrom rdf:resource="http://purl.obolibrary.org/obo/esmo.owl#Commodity_aggregate"/>
            </owl:Restriction>
        </rdfs:subClassOf>
        <skos:definition>Marketable product produced as a result of human economic activity.</skos:definition>
        <skos:example>A smoked salmon</skos:example>
    </owl:Class>
    


    <!-- http://purl.obolibrary.org/obo/esmo.owl#Commodity_aggregate -->

    <owl:Class rdf:about="http://purl.obolibrary.org/obo/esmo.owl#Commodity_aggregate">
        <rdfs:subClassOf rdf:resource="http://purl.obolibrary.org/obo/BFO_0000027"/>
        <rdfs:subClassOf>
            <owl:Restriction>
                <owl:onProperty rdf:resource="http://purl.obolibrary.org/obo/BFO_0000174"/>
                <owl:someValuesFrom rdf:resource="http://purl.obolibrary.org/obo/esmo.owl#Commodity"/>
            </owl:Restriction>
        </rdfs:subClassOf>
        <rdfs:subClassOf>
            <owl:Restriction>
                <owl:onProperty rdf:resource="http://purl.obolibrary.org/obo/esmo.owl#has_quality"/>
                <owl:someValuesFrom rdf:resource="http://purl.obolibrary.org/obo/esmo.owl#Instrumental_value"/>
            </owl:Restriction>
        </rdfs:subClassOf>
        <skos:definition>Is a material entity consisting exactly of a plurality (≥1) of commodities as member parts which together form a unit.</skos:definition>
        <skos:example>The wheat of France</skos:example>
    </owl:Class>
    


    <!-- http://purl.obolibrary.org/obo/esmo.owl#Concept -->

    <owl:Class rdf:about="http://purl.obolibrary.org/obo/esmo.owl#Concept">
        <rdfs:subClassOf rdf:resource="http://purl.obolibrary.org/obo/BFO_0000001"/>
        <skos:definition>A concept is an entity that is conceived in the human mind to represent an abstract of generic idea generalised from particular instances.</skos:definition>
        <skos:example>A thought, a notion, courage</skos:example>
    </owl:Class>
    


    <!-- http://purl.obolibrary.org/obo/esmo.owl#Cultural_ecosystem_service -->

    <owl:Class rdf:about="http://purl.obolibrary.org/obo/esmo.owl#Cultural_ecosystem_service">
        <rdfs:subClassOf rdf:resource="http://purl.obolibrary.org/obo/esmo.owl#Ecosystem_service"/>
        <rdfs:subClassOf>
            <owl:Restriction>
                <owl:onProperty rdf:resource="http://purl.obolibrary.org/obo/BFO_0000195"/>
                <owl:someValuesFrom rdf:resource="http://purl.obolibrary.org/obo/esmo.owl#Ecosystem_good"/>
            </owl:Restriction>
        </rdfs:subClassOf>
        <skos:definition>These are the services that contribute to the benefits people obtain from ecosystems through spiritual enrichment, cognitive development, reflection, recreation, and aesthetic experiences.</skos:definition>
        <skos:example>Recreation services, aesthetic appreciation</skos:example>
    </owl:Class>
    


    <!-- http://purl.obolibrary.org/obo/esmo.owl#Cultural_value -->

    <owl:Class rdf:about="http://purl.obolibrary.org/obo/esmo.owl#Cultural_value">
        <rdfs:subClassOf rdf:resource="http://purl.obolibrary.org/obo/esmo.owl#Relational_value"/>
        <rdfs:subClassOf>
            <owl:Restriction>
                <owl:onProperty rdf:resource="http://purl.obolibrary.org/obo/esmo.owl#measure_of"/>
                <owl:someValuesFrom rdf:resource="http://purl.obolibrary.org/obo/esmo.owl#EESV_instrumental_value"/>
            </owl:Restriction>
        </rdfs:subClassOf>
        <skos:definition>Those types of relational values that are associated with a local culture and context.</skos:definition>
    </owl:Class>
    


    <!-- http://purl.obolibrary.org/obo/esmo.owl#Decomposition -->

    <owl:Class rdf:about="http://purl.obolibrary.org/obo/esmo.owl#Decomposition">
        <rdfs:subClassOf rdf:resource="http://purl.obolibrary.org/obo/esmo.owl#Ecosystem_process"/>
        <skos:definition>Breakdown of complex organic substances into simpler molecules or ions by physical, chemical and/or biological processes.</skos:definition>
    </owl:Class>
    


    <!-- http://purl.obolibrary.org/obo/esmo.owl#Direct_driver -->

    <owl:Class rdf:about="http://purl.obolibrary.org/obo/esmo.owl#Direct_driver">
        <rdfs:subClassOf rdf:resource="http://purl.obolibrary.org/obo/esmo.owl#Driver_of_change"/>
        <skos:definition>A driver of change that directly and unequivocally influences an ecosystem and its processes.</skos:definition>
        <skos:example>Exploitation</skos:example>
    </owl:Class>
    


    <!-- http://purl.obolibrary.org/obo/esmo.owl#Driver_of_change -->

    <owl:Class rdf:about="http://purl.obolibrary.org/obo/esmo.owl#Driver_of_change">
        <rdfs:subClassOf rdf:resource="http://purl.obolibrary.org/obo/BFO_0000015"/>
        <rdfs:subClassOf>
            <owl:Restriction>
                <owl:onProperty rdf:resource="http://purl.obolibrary.org/obo/esmo.owl#causally_influences"/>
                <owl:someValuesFrom rdf:resource="http://purl.obolibrary.org/obo/esmo.owl#Ecosystem_component"/>
            </owl:Restriction>
        </rdfs:subClassOf>
        <rdfs:subClassOf>
            <owl:Restriction>
                <owl:onProperty rdf:resource="http://purl.obolibrary.org/obo/esmo.owl#causally_influences"/>
                <owl:someValuesFrom rdf:resource="http://purl.obolibrary.org/obo/esmo.owl#Ecosystem_good"/>
            </owl:Restriction>
        </rdfs:subClassOf>
        <rdfs:subClassOf>
            <owl:Restriction>
                <owl:onProperty rdf:resource="http://purl.obolibrary.org/obo/esmo.owl#causally_upstream_of_with_negative_effect"/>
                <owl:someValuesFrom rdf:resource="http://purl.obolibrary.org/obo/esmo.owl#Ecosystem_process"/>
            </owl:Restriction>
        </rdfs:subClassOf>
        <skos:definition>Any natural or human induced factor that directly or indirectly causes a change in an ecosystem.</skos:definition>
        <skos:example>Global warming, flooding, pollution</skos:example>
    </owl:Class>
    


    <!-- http://purl.obolibrary.org/obo/esmo.owl#EESV_anthropogenic_contribution -->

    <owl:Class rdf:about="http://purl.obolibrary.org/obo/esmo.owl#EESV_anthropogenic_contribution">
        <rdfs:subClassOf rdf:resource="http://purl.obolibrary.org/obo/esmo.owl#Essential_ecosystem_service_variable_class"/>
        <skos:definition>The efforts that humans invest to enhance ecological supply and to make use of ecosystem services.</skos:definition>
        <skos:example>Infrastructure to access national parks, a fishing fleet, machinery</skos:example>
    </owl:Class>
    


    <!-- http://purl.obolibrary.org/obo/esmo.owl#EESV_demand -->

    <owl:Class rdf:about="http://purl.obolibrary.org/obo/esmo.owl#EESV_demand">
        <rdfs:subClassOf rdf:resource="http://purl.obolibrary.org/obo/esmo.owl#Essential_ecosystem_service_variable_class"/>
        <skos:definition>The explicitly or implicitly expressed human desire or need for an ecosystem service, in terms of its quantity or quality, irrespective of whether awareness exists about such need.</skos:definition>
        <skos:example>Population in dependent on a watershed, per capita consumption of a good</skos:example>
    </owl:Class>
    


    <!-- http://purl.obolibrary.org/obo/esmo.owl#EESV_ecological_supply -->

    <owl:Class rdf:about="http://purl.obolibrary.org/obo/esmo.owl#EESV_ecological_supply">
        <rdfs:subClassOf rdf:resource="http://purl.obolibrary.org/obo/esmo.owl#Essential_ecosystem_service_variable_class"/>
        <skos:definition>The ecosystem structure and functions that underlie the potential capacity of ecosystems to provide ecosystem services.</skos:definition>
        <skos:example>Fish biomass, pollinator abundance, freshwater supply</skos:example>
    </owl:Class>
    


    <!-- http://purl.obolibrary.org/obo/esmo.owl#EESV_instrumental_value -->

    <owl:Class rdf:about="http://purl.obolibrary.org/obo/esmo.owl#EESV_instrumental_value">
        <rdfs:subClassOf rdf:resource="http://purl.obolibrary.org/obo/esmo.owl#Essential_ecosystem_service_variable_class"/>
        <skos:definition>The importance of an ecosystem service to societies or individuals as a means to achieve a specific end.</skos:definition>
        <skos:example>Income, food, enjoyment</skos:example>
    </owl:Class>
    


    <!-- http://purl.obolibrary.org/obo/esmo.owl#EESV_relational_value -->

    <owl:Class rdf:about="http://purl.obolibrary.org/obo/esmo.owl#EESV_relational_value">
        <rdfs:subClassOf rdf:resource="http://purl.obolibrary.org/obo/esmo.owl#Essential_ecosystem_service_variable_class"/>
        <skos:definition>The importance ascribed to how ecosystems contribute to desirable and meaningful interactions between humans and nature and between humans in relation to nature.</skos:definition>
        <skos:example>Cultural practices of stewardship, care, spirituality</skos:example>
    </owl:Class>
    


    <!-- http://purl.obolibrary.org/obo/esmo.owl#EESV_use -->

    <owl:Class rdf:about="http://purl.obolibrary.org/obo/esmo.owl#EESV_use">
        <rdfs:subClassOf rdf:resource="http://purl.obolibrary.org/obo/esmo.owl#Essential_ecosystem_service_variable_class"/>
        <skos:definition>The active or passive appropriation of an ecosystem service by people highlights the actual appropriation of benefits from nature.</skos:definition>
        <skos:example>Harvested crops, recreational experience</skos:example>
    </owl:Class>
    


    <!-- http://purl.obolibrary.org/obo/esmo.owl#Economic_activity -->

    <owl:Class rdf:about="http://purl.obolibrary.org/obo/esmo.owl#Economic_activity">
        <rdfs:subClassOf rdf:resource="http://purl.obolibrary.org/obo/esmo.owl#Human_activity"/>
        <rdfs:subClassOf>
            <owl:Restriction>
                <owl:onProperty rdf:resource="http://purl.obolibrary.org/obo/BFO_0000167"/>
                <owl:someValuesFrom rdf:resource="http://purl.obolibrary.org/obo/esmo.owl#Economic_actor"/>
            </owl:Restriction>
        </rdfs:subClassOf>
        <skos:definition>A human activity involving the production, distribution, exchange or consumption of commodities and services with the goal of meeting human needs and generating monetary instrumental value in the economy.</skos:definition>
        <skos:example>Commercial farming, scuba diving</skos:example>
    </owl:Class>
    


    <!-- http://purl.obolibrary.org/obo/esmo.owl#Economic_actor -->

    <owl:Class rdf:about="http://purl.obolibrary.org/obo/esmo.owl#Economic_actor">
        <rdfs:subClassOf rdf:resource="http://purl.obolibrary.org/obo/esmo.owl#Actor"/>
        <rdfs:subClassOf>
            <owl:Restriction>
                <owl:onProperty rdf:resource="http://purl.obolibrary.org/obo/BFO_0000166"/>
                <owl:someValuesFrom rdf:resource="http://purl.obolibrary.org/obo/esmo.owl#Economic_activity"/>
            </owl:Restriction>
        </rdfs:subClassOf>
        <rdfs:subClassOf>
            <owl:Restriction>
                <owl:onProperty rdf:resource="http://purl.obolibrary.org/obo/esmo.owl#benefits_from"/>
                <owl:someValuesFrom rdf:resource="http://purl.obolibrary.org/obo/esmo.owl#Monetary_instrumental_value"/>
            </owl:Restriction>
        </rdfs:subClassOf>
        <skos:definition>An actor who participates in economic activity and who&apos;s behaviour and decisions are dependent on economic concerns, ie are tied to monetary considerations.</skos:definition>
        <skos:example>A consumer, a merchant</skos:example>
    </owl:Class>
    


    <!-- http://purl.obolibrary.org/obo/esmo.owl#Ecosystem -->

    <owl:Class rdf:about="http://purl.obolibrary.org/obo/esmo.owl#Ecosystem">
        <rdfs:subClassOf rdf:resource="http://purl.obolibrary.org/obo/BFO_0000027"/>
        <rdfs:subClassOf>
            <owl:Restriction>
                <owl:onProperty rdf:resource="http://purl.obolibrary.org/obo/BFO_0000183"/>
                <owl:someValuesFrom rdf:resource="http://purl.obolibrary.org/obo/esmo.owl#Ecosystem_process"/>
            </owl:Restriction>
        </rdfs:subClassOf>
        <rdfs:subClassOf>
            <owl:Restriction>
                <owl:onProperty rdf:resource="http://purl.obolibrary.org/obo/BFO_0000194"/>
                <owl:someValuesFrom rdf:resource="http://purl.obolibrary.org/obo/esmo.owl#Ecosystem_service"/>
            </owl:Restriction>
        </rdfs:subClassOf>
        <rdfs:subClassOf>
            <owl:Restriction>
                <owl:onProperty rdf:resource="http://purl.obolibrary.org/obo/BFO_0000211"/>
                <owl:someValuesFrom rdf:resource="http://purl.obolibrary.org/obo/esmo.owl#Ecosystem_extent"/>
            </owl:Restriction>
        </rdfs:subClassOf>
        <rdfs:subClassOf>
            <owl:Restriction>
                <owl:onProperty rdf:resource="http://purl.obolibrary.org/obo/esmo.owl#has_quality"/>
                <owl:someValuesFrom rdf:resource="http://purl.obolibrary.org/obo/esmo.owl#Ecosystem_condition"/>
            </owl:Restriction>
        </rdfs:subClassOf>
        <rdfs:subClassOf>
            <owl:Restriction>
                <owl:onProperty rdf:resource="http://purl.obolibrary.org/obo/esmo.owl#has_quality"/>
                <owl:someValuesFrom rdf:resource="http://purl.obolibrary.org/obo/esmo.owl#Intrinsic_value"/>
            </owl:Restriction>
        </rdfs:subClassOf>
        <skos:definition>A dynamic complex of plant, animal and micro-organism communities and their non-living environment interacting as a functional unit. Specifically, ecosystems are made up of living components (biotic complexes and assemblages of species), the abiotic environment, the processes and interactions within and between the biotic and abiotic components, and the physical space in which these operate</skos:definition>
    </owl:Class>
    


    <!-- http://purl.obolibrary.org/obo/esmo.owl#Ecosystem_component -->

    <owl:Class rdf:about="http://purl.obolibrary.org/obo/esmo.owl#Ecosystem_component">
        <rdfs:subClassOf rdf:resource="http://purl.obolibrary.org/obo/BFO_0000030"/>
        <rdfs:subClassOf>
            <owl:Restriction>
                <owl:onProperty rdf:resource="http://purl.obolibrary.org/obo/BFO_0000056"/>
                <owl:someValuesFrom rdf:resource="http://purl.obolibrary.org/obo/esmo.owl#Ecosystem_process"/>
            </owl:Restriction>
        </rdfs:subClassOf>
        <rdfs:subClassOf>
            <owl:Restriction>
                <owl:onProperty rdf:resource="http://purl.obolibrary.org/obo/BFO_0000137"/>
                <owl:someValuesFrom rdf:resource="http://purl.obolibrary.org/obo/esmo.owl#Ecosystem"/>
            </owl:Restriction>
        </rdfs:subClassOf>
        <rdfs:subClassOf>
            <owl:Restriction>
                <owl:onProperty rdf:resource="http://purl.obolibrary.org/obo/esmo.owl#has_quality"/>
                <owl:someValuesFrom rdf:resource="http://purl.obolibrary.org/obo/esmo.owl#Intrinsic_value"/>
            </owl:Restriction>
        </rdfs:subClassOf>
        <skos:definition>The components that are part of an ecosystem.</skos:definition>
        <skos:example>A tree, a fish, a river</skos:example>
    </owl:Class>
    


    <!-- http://purl.obolibrary.org/obo/esmo.owl#Ecosystem_component_aggregate -->

    <owl:Class rdf:about="http://purl.obolibrary.org/obo/esmo.owl#Ecosystem_component_aggregate">
        <rdfs:subClassOf rdf:resource="http://purl.obolibrary.org/obo/BFO_0000027"/>
        <rdfs:subClassOf>
            <owl:Restriction>
                <owl:onProperty rdf:resource="http://purl.obolibrary.org/obo/BFO_0000056"/>
                <owl:someValuesFrom rdf:resource="http://purl.obolibrary.org/obo/esmo.owl#Ecosystem_process"/>
            </owl:Restriction>
        </rdfs:subClassOf>
        <rdfs:subClassOf>
            <owl:Restriction>
                <owl:onProperty rdf:resource="http://purl.obolibrary.org/obo/BFO_0000137"/>
                <owl:someValuesFrom rdf:resource="http://purl.obolibrary.org/obo/esmo.owl#Ecosystem"/>
            </owl:Restriction>
        </rdfs:subClassOf>
        <rdfs:subClassOf>
            <owl:Restriction>
                <owl:onProperty rdf:resource="http://purl.obolibrary.org/obo/esmo.owl#has_quality"/>
                <owl:someValuesFrom rdf:resource="http://purl.obolibrary.org/obo/esmo.owl#Intrinsic_value"/>
            </owl:Restriction>
        </rdfs:subClassOf>
    </owl:Class>
    


    <!-- http://purl.obolibrary.org/obo/esmo.owl#Ecosystem_condition -->

    <owl:Class rdf:about="http://purl.obolibrary.org/obo/esmo.owl#Ecosystem_condition">
        <rdfs:subClassOf rdf:resource="http://purl.obolibrary.org/obo/BFO_0000019"/>
        <rdfs:subClassOf>
            <owl:Restriction>
                <owl:onProperty rdf:resource="http://purl.obolibrary.org/obo/BFO_0000195"/>
                <owl:someValuesFrom rdf:resource="http://purl.obolibrary.org/obo/esmo.owl#Ecosystem"/>
            </owl:Restriction>
        </rdfs:subClassOf>
        <skos:definition>A measure of the state or health of an ecosystem, characterized by its structure, function, composition, and the ability to sustain biodiversity and provide ecosystem services. It reflects the level of ecological integrity, resilience to disturbances, and the extent to which the ecosystem supports its natural processes and life forms.</skos:definition>
        <skos:example>A healthy ecosystem, a degraded ecosystem</skos:example>
    </owl:Class>
    


    <!-- http://purl.obolibrary.org/obo/esmo.owl#Ecosystem_extent -->

    <owl:Class rdf:about="http://purl.obolibrary.org/obo/esmo.owl#Ecosystem_extent">
        <rdfs:subClassOf rdf:resource="http://purl.obolibrary.org/obo/BFO_0000009"/>
        <skos:definition>The size of an ecosystem, which are contiguous spaces of a specific ecosystem type characterized by a distinct set of biotic and abiotic components and their interactions.</skos:definition>
    </owl:Class>
    


    <!-- http://purl.obolibrary.org/obo/esmo.owl#Ecosystem_function -->

    <owl:Class rdf:about="http://purl.obolibrary.org/obo/esmo.owl#Ecosystem_function">
        <rdfs:subClassOf rdf:resource="http://purl.obolibrary.org/obo/esmo.owl#Ecosystem_process"/>
        <rdfs:subClassOf>
            <owl:Restriction>
                <owl:onProperty rdf:resource="http://purl.obolibrary.org/obo/BFO_0000055"/>
                <owl:someValuesFrom rdf:resource="http://purl.obolibrary.org/obo/esmo.owl#Ecosystem_service"/>
            </owl:Restriction>
        </rdfs:subClassOf>
        <rdfs:subClassOf>
            <owl:Restriction>
                <owl:onProperty rdf:resource="http://purl.obolibrary.org/obo/esmo.owl#has_output"/>
                <owl:someValuesFrom rdf:resource="http://purl.obolibrary.org/obo/esmo.owl#Ecosystem_good"/>
            </owl:Restriction>
        </rdfs:subClassOf>
        <rdfs:subClassOf>
            <owl:Restriction>
                <owl:onProperty rdf:resource="http://purl.obolibrary.org/obo/esmo.owl#output_of"/>
                <owl:someValuesFrom rdf:resource="http://purl.obolibrary.org/obo/esmo.owl#Ecosystem_process"/>
            </owl:Restriction>
        </rdfs:subClassOf>
        <skos:definition>They are the subset of ecosystem processes which contribute to human wellbeing through the production of ecosystem goods. Ecosystem functions refer to the broad, overarching roles that ecosystems perform, which support the stability and health of the environment. Functions are often described in terms of their benefits to human societies and the natural world.</skos:definition>
        <skos:example>Pollination, primary production</skos:example>
    </owl:Class>
    


    <!-- http://purl.obolibrary.org/obo/esmo.owl#Ecosystem_good -->

    <owl:Class rdf:about="http://purl.obolibrary.org/obo/esmo.owl#Ecosystem_good">
        <rdfs:subClassOf rdf:resource="http://purl.obolibrary.org/obo/BFO_0000030"/>
        <rdfs:subClassOf>
            <owl:Restriction>
                <owl:onProperty rdf:resource="http://purl.obolibrary.org/obo/BFO_0000056"/>
                <owl:someValuesFrom rdf:resource="http://purl.obolibrary.org/obo/esmo.owl#Human_activity"/>
            </owl:Restriction>
        </rdfs:subClassOf>
        <rdfs:subClassOf>
            <owl:Restriction>
                <owl:onProperty rdf:resource="http://purl.obolibrary.org/obo/BFO_0000137"/>
                <owl:someValuesFrom rdf:resource="http://purl.obolibrary.org/obo/esmo.owl#Ecosystem_good_aggregate"/>
            </owl:Restriction>
        </rdfs:subClassOf>
        <rdfs:subClassOf>
            <owl:Restriction>
                <owl:onProperty rdf:resource="http://purl.obolibrary.org/obo/esmo.owl#output_of"/>
                <owl:someValuesFrom rdf:resource="http://purl.obolibrary.org/obo/esmo.owl#Ecosystem_process"/>
            </owl:Restriction>
        </rdfs:subClassOf>
        <skos:definition>The output of an ecosystem function before it is used in human activity. Components of nature, directly enjoyed, consumed, or used to yield human well-being. The ecosystem good (i.e., ecological end-product) is a biophysical quality and needs minimal translation for relevance to human well-being.</skos:definition>
        <skos:example>Freshwater, harvestable tree, fish</skos:example>
    </owl:Class>
    


    <!-- http://purl.obolibrary.org/obo/esmo.owl#Ecosystem_good_aggregate -->

    <owl:Class rdf:about="http://purl.obolibrary.org/obo/esmo.owl#Ecosystem_good_aggregate">
        <rdfs:subClassOf rdf:resource="http://purl.obolibrary.org/obo/BFO_0000027"/>
        <rdfs:subClassOf>
            <owl:Restriction>
                <owl:onProperty rdf:resource="http://purl.obolibrary.org/obo/BFO_0000056"/>
                <owl:someValuesFrom rdf:resource="http://purl.obolibrary.org/obo/esmo.owl#Human_activity"/>
            </owl:Restriction>
        </rdfs:subClassOf>
        <rdfs:subClassOf>
            <owl:Restriction>
                <owl:onProperty rdf:resource="http://purl.obolibrary.org/obo/BFO_0000174"/>
                <owl:someValuesFrom rdf:resource="http://purl.obolibrary.org/obo/esmo.owl#Ecosystem_good"/>
            </owl:Restriction>
        </rdfs:subClassOf>
        <rdfs:subClassOf>
            <owl:Restriction>
                <owl:onProperty rdf:resource="http://purl.obolibrary.org/obo/esmo.owl#output_of"/>
                <owl:someValuesFrom rdf:resource="http://purl.obolibrary.org/obo/esmo.owl#Ecosystem_process"/>
            </owl:Restriction>
        </rdfs:subClassOf>
        <skos:definition>Is a material entity consisting exactly of a plurality (≥1) of ecosystem goods as member parts which together form a unit.</skos:definition>
        <skos:example>A population of salmon, a group trees</skos:example>
    </owl:Class>
    


    <!-- http://purl.obolibrary.org/obo/esmo.owl#Ecosystem_process -->

    <owl:Class rdf:about="http://purl.obolibrary.org/obo/esmo.owl#Ecosystem_process">
        <rdfs:subClassOf rdf:resource="http://purl.obolibrary.org/obo/BFO_0000015"/>
        <rdfs:subClassOf>
            <owl:Restriction>
                <owl:onProperty rdf:resource="http://purl.obolibrary.org/obo/BFO_0000057"/>
                <owl:someValuesFrom rdf:resource="http://purl.obolibrary.org/obo/esmo.owl#Ecosystem_component"/>
            </owl:Restriction>
        </rdfs:subClassOf>
        <rdfs:subClassOf>
            <owl:Restriction>
                <owl:onProperty rdf:resource="http://purl.obolibrary.org/obo/BFO_0000066"/>
                <owl:someValuesFrom rdf:resource="http://purl.obolibrary.org/obo/esmo.owl#Ecosystem"/>
            </owl:Restriction>
        </rdfs:subClassOf>
        <rdfs:subClassOf>
            <owl:Restriction>
                <owl:onProperty rdf:resource="http://purl.obolibrary.org/obo/esmo.owl#has_output"/>
                <owl:someValuesFrom rdf:resource="http://purl.obolibrary.org/obo/esmo.owl#Ecosystem_function"/>
            </owl:Restriction>
        </rdfs:subClassOf>
        <rdfs:subClassOf>
            <owl:Restriction>
                <owl:onProperty rdf:resource="http://purl.obolibrary.org/obo/esmo.owl#has_output"/>
                <owl:someValuesFrom rdf:resource="http://purl.obolibrary.org/obo/esmo.owl#Ecosystem_good_aggregate"/>
            </owl:Restriction>
        </rdfs:subClassOf>
        <skos:definition>The flow of energy and materials through the biotic and abiotic components of an ecosystem. Ecosystem processes are the specific mechanisms or actions through which ecosystem functions are achieved. These are the dynamic interactions and transformations that occur within ecosystems, leading to the maintenance and sustainability of ecosystem functions.</skos:definition>
        <skos:example>Photosynthesis, predation</skos:example>
    </owl:Class>
    


    <!-- http://purl.obolibrary.org/obo/esmo.owl#Ecosystem_service -->

    <owl:Class rdf:about="http://purl.obolibrary.org/obo/esmo.owl#Ecosystem_service">
        <rdfs:subClassOf rdf:resource="http://purl.obolibrary.org/obo/BFO_0000023"/>
        <rdfs:subClassOf>
            <owl:Restriction>
                <owl:onProperty rdf:resource="http://purl.obolibrary.org/obo/BFO_0000054"/>
                <owl:someValuesFrom rdf:resource="http://purl.obolibrary.org/obo/esmo.owl#Ecosystem_function"/>
            </owl:Restriction>
        </rdfs:subClassOf>
        <rdfs:subClassOf>
            <owl:Restriction>
                <owl:onProperty rdf:resource="http://purl.obolibrary.org/obo/BFO_0000054"/>
                <owl:someValuesFrom rdf:resource="http://purl.obolibrary.org/obo/esmo.owl#Human_activity"/>
            </owl:Restriction>
        </rdfs:subClassOf>
        <rdfs:subClassOf>
            <owl:Restriction>
                <owl:onProperty rdf:resource="http://purl.obolibrary.org/obo/BFO_0000195"/>
                <owl:someValuesFrom rdf:resource="http://purl.obolibrary.org/obo/esmo.owl#Ecosystem"/>
            </owl:Restriction>
        </rdfs:subClassOf>
        <rdfs:comment>In ESMO ecosystem services are roles that ecosystems can bear by virtue of their composition and the processes and functions that arise in them. This role is realised by both the ecosystem function underpinning the service and the human activity that depends on the ecosystem good.</rdfs:comment>
        <skos:definition>A service that is provided by an ecosystem as an intrinsic property of its functionality (e.g. pollination, nutrient cycling, nitrogen fixation, fruit and seed dispersal) contributing to the benefits (and occasionally disbenefits) that people obtain from ecosystems.</skos:definition>
    </owl:Class>
    


    <!-- http://purl.obolibrary.org/obo/esmo.owl#Enjoyment_value -->

    <owl:Class rdf:about="http://purl.obolibrary.org/obo/esmo.owl#Enjoyment_value">
        <rdfs:subClassOf rdf:resource="http://purl.obolibrary.org/obo/esmo.owl#Non_monetary_instrumental_value"/>
        <rdfs:subClassOf>
            <owl:Restriction>
                <owl:onProperty rdf:resource="http://purl.obolibrary.org/obo/esmo.owl#measure_of"/>
                <owl:someValuesFrom rdf:resource="http://purl.obolibrary.org/obo/esmo.owl#EESV_instrumental_value"/>
            </owl:Restriction>
        </rdfs:subClassOf>
        <skos:definition>A non-monetary instrumental value where the achieved end is some form of enjoyment.</skos:definition>
        <skos:example>The value of a river in recreational enjoyment</skos:example>
    </owl:Class>
    


    <!-- http://purl.obolibrary.org/obo/esmo.owl#Epipelagic_ocean -->

    <owl:Class rdf:about="http://purl.obolibrary.org/obo/esmo.owl#Epipelagic_ocean">
        <rdfs:subClassOf rdf:resource="http://purl.obolibrary.org/obo/esmo.owl#Ecosystem"/>
        <rdfs:subClassOf>
            <owl:Restriction>
                <owl:onProperty rdf:resource="http://purl.obolibrary.org/obo/BFO_0000183"/>
                <owl:someValuesFrom rdf:resource="http://purl.obolibrary.org/obo/esmo.owl#Fish_biomass_production"/>
            </owl:Restriction>
        </rdfs:subClassOf>
        <rdfs:subClassOf>
            <owl:Restriction>
                <owl:onProperty rdf:resource="http://purl.obolibrary.org/obo/BFO_0000183"/>
                <owl:someValuesFrom rdf:resource="http://purl.obolibrary.org/obo/esmo.owl#Whale_habitat_provisioning"/>
            </owl:Restriction>
        </rdfs:subClassOf>
        <rdfs:comment>For additional detailed information refer to Keith, D.A., Ferrer-Paris, J.R., Nicholson, E. and Kingsford, R.T. (eds.) (2020). The IUCN Global Ecosystem Typology 2.0: Descriptive profiles for biomes and ecosystem functional groups. Gland, Switzerland: IUCN.</rdfs:comment>
        <skos:definition>The epipelagic or euphotic zone of the open ocean is the uppermost layer that is penetrated by enough light to support photosynthesis.</skos:definition>
        <skos:example>North Atlantic ocean waters</skos:example>
    </owl:Class>
    


    <!-- http://purl.obolibrary.org/obo/esmo.owl#Essential_ecosystem_service_variable_class -->

    <owl:Class rdf:about="http://purl.obolibrary.org/obo/esmo.owl#Essential_ecosystem_service_variable_class">
        <rdfs:subClassOf rdf:resource="http://purl.obolibrary.org/obo/esmo.owl#Concept"/>
        <rdfs:comment>For more see Balvanera, P., Brauman, K.A., Cord, A.F., Drakou, E.G., Geijzendorffer, I.R., Karp, D.S., Martín-López, B., Mwampamba, T.H. and Schröter, M., 2022. Essential ecosystem</rdfs:comment>
        <skos:definition>EESV classes represent shared and grouped key attributes for all ecosystem services to be monitored across space and time.</skos:definition>
    </owl:Class>
    


    <!-- http://purl.obolibrary.org/obo/esmo.owl#Exploitation -->

    <owl:Class rdf:about="http://purl.obolibrary.org/obo/esmo.owl#Exploitation">
        <rdfs:subClassOf rdf:resource="http://purl.obolibrary.org/obo/esmo.owl#Direct_driver"/>
        <rdfs:subClassOf>
            <owl:Restriction>
                <owl:onProperty rdf:resource="http://purl.obolibrary.org/obo/esmo.owl#causally_upstream_of_with_negative_effect"/>
                <owl:someValuesFrom rdf:resource="http://purl.obolibrary.org/obo/esmo.owl#Fish_biomass_production"/>
            </owl:Restriction>
        </rdfs:subClassOf>
        <skos:definition>The consumptive use of any natural resources.</skos:definition>
        <skos:example>Overfishing, over hunting</skos:example>
    </owl:Class>
    


    <!-- http://purl.obolibrary.org/obo/esmo.owl#Fauna_aggregate -->

    <owl:Class rdf:about="http://purl.obolibrary.org/obo/esmo.owl#Fauna_aggregate">
        <rdfs:subClassOf rdf:resource="http://purl.obolibrary.org/obo/esmo.owl#Biotic_component_aggregate"/>
    </owl:Class>
    


    <!-- http://purl.obolibrary.org/obo/esmo.owl#Fauna_component -->

    <owl:Class rdf:about="http://purl.obolibrary.org/obo/esmo.owl#Fauna_component">
        <rdfs:subClassOf rdf:resource="http://purl.obolibrary.org/obo/esmo.owl#Biotic_component"/>
        <skos:definition>Those biotic components that are part of the kingdom Animalia</skos:definition>
        <skos:example>A dolphin, a chimpanzee, a parrot</skos:example>
    </owl:Class>
    


    <!-- http://purl.obolibrary.org/obo/esmo.owl#Fish_biomass_production -->

    <owl:Class rdf:about="http://purl.obolibrary.org/obo/esmo.owl#Fish_biomass_production">
        <rdfs:subClassOf rdf:resource="http://purl.obolibrary.org/obo/esmo.owl#Biomass_production"/>
        <rdfs:subClassOf>
            <owl:Restriction>
                <owl:onProperty rdf:resource="http://purl.obolibrary.org/obo/BFO_0000055"/>
                <owl:someValuesFrom rdf:resource="http://purl.obolibrary.org/obo/esmo.owl#Wild_fish_provisioning_service"/>
            </owl:Restriction>
        </rdfs:subClassOf>
        <rdfs:subClassOf>
            <owl:Restriction>
                <owl:onProperty rdf:resource="http://purl.obolibrary.org/obo/BFO_0000066"/>
                <owl:someValuesFrom rdf:resource="http://purl.obolibrary.org/obo/esmo.owl#Epipelagic_ocean"/>
            </owl:Restriction>
        </rdfs:subClassOf>
        <rdfs:subClassOf>
            <owl:Restriction>
                <owl:onProperty rdf:resource="http://purl.obolibrary.org/obo/esmo.owl#has_output"/>
                <owl:someValuesFrom rdf:resource="http://purl.obolibrary.org/obo/esmo.owl#Fish_population"/>
            </owl:Restriction>
        </rdfs:subClassOf>
        <skos:definition>The generation of fish biomass through predation and other ecological processes.</skos:definition>
    </owl:Class>
    


    <!-- http://purl.obolibrary.org/obo/esmo.owl#Fish_population -->

    <owl:Class rdf:about="http://purl.obolibrary.org/obo/esmo.owl#Fish_population">
        <rdfs:subClassOf rdf:resource="http://purl.obolibrary.org/obo/esmo.owl#Ecosystem_good_aggregate"/>
        <rdfs:subClassOf>
            <owl:Restriction>
                <owl:onProperty rdf:resource="http://purl.obolibrary.org/obo/BFO_0000056"/>
                <owl:someValuesFrom rdf:resource="http://purl.obolibrary.org/obo/esmo.owl#Commercial_fishing"/>
            </owl:Restriction>
        </rdfs:subClassOf>
        <rdfs:subClassOf>
            <owl:Restriction>
                <owl:onProperty rdf:resource="http://purl.obolibrary.org/obo/esmo.owl#measure_of"/>
                <owl:someValuesFrom rdf:resource="http://purl.obolibrary.org/obo/esmo.owl#EESV_ecological_supply"/>
            </owl:Restriction>
        </rdfs:subClassOf>
        <skos:definition>Is a material entity consisting exactly of a plurality (≥1) of fish as member parts which together form a unit.</skos:definition>
        <skos:example>Salmon population</skos:example>
    </owl:Class>
    


    <!-- http://purl.obolibrary.org/obo/esmo.owl#Fishing_fleet -->

    <owl:Class rdf:about="http://purl.obolibrary.org/obo/esmo.owl#Fishing_fleet">
        <rdfs:subClassOf rdf:resource="http://purl.obolibrary.org/obo/esmo.owl#Vessel_fleet"/>
        <rdfs:subClassOf>
            <owl:Restriction>
                <owl:onProperty rdf:resource="http://purl.obolibrary.org/obo/BFO_0000056"/>
                <owl:someValuesFrom rdf:resource="http://purl.obolibrary.org/obo/esmo.owl#Commercial_fishing"/>
            </owl:Restriction>
        </rdfs:subClassOf>
        <rdfs:subClassOf>
            <owl:Restriction>
                <owl:onProperty rdf:resource="http://purl.obolibrary.org/obo/esmo.owl#measure_of"/>
                <owl:someValuesFrom rdf:resource="http://purl.obolibrary.org/obo/esmo.owl#EESV_anthropogenic_contribution"/>
            </owl:Restriction>
        </rdfs:subClassOf>
        <skos:example>Is a vessel aggregate where all vessel types are fishing vessels, ie whose primary purpose is to catch fish.</skos:example>
    </owl:Class>
    


    <!-- http://purl.obolibrary.org/obo/esmo.owl#Flora_aggregate -->

    <owl:Class rdf:about="http://purl.obolibrary.org/obo/esmo.owl#Flora_aggregate">
        <rdfs:subClassOf rdf:resource="http://purl.obolibrary.org/obo/esmo.owl#Biotic_component_aggregate"/>
    </owl:Class>
    


    <!-- http://purl.obolibrary.org/obo/esmo.owl#Flora_component -->

    <owl:Class rdf:about="http://purl.obolibrary.org/obo/esmo.owl#Flora_component">
        <rdfs:subClassOf rdf:resource="http://purl.obolibrary.org/obo/esmo.owl#Biotic_component"/>
        <skos:definition>Those biotic components that are part of the kingdom Plantae</skos:definition>
        <skos:example>A fern, an apple tree</skos:example>
    </owl:Class>
    


    <!-- http://purl.obolibrary.org/obo/esmo.owl#Food_value -->

    <owl:Class rdf:about="http://purl.obolibrary.org/obo/esmo.owl#Food_value">
        <rdfs:subClassOf rdf:resource="http://purl.obolibrary.org/obo/esmo.owl#Non_monetary_instrumental_value"/>
        <rdfs:subClassOf>
            <owl:Restriction>
                <owl:onProperty rdf:resource="http://purl.obolibrary.org/obo/esmo.owl#measure_of"/>
                <owl:someValuesFrom rdf:resource="http://purl.obolibrary.org/obo/esmo.owl#EESV_instrumental_value"/>
            </owl:Restriction>
        </rdfs:subClassOf>
        <skos:definition>A non-monetary instrumental value where the achieved end is a food source.</skos:definition>
        <skos:example>The value of cereal in contributing to food security, the value of fish as a food source</skos:example>
    </owl:Class>
    


    <!-- http://purl.obolibrary.org/obo/esmo.owl#Habitat_provisioning -->

    <owl:Class rdf:about="http://purl.obolibrary.org/obo/esmo.owl#Habitat_provisioning">
        <rdfs:subClassOf rdf:resource="http://purl.obolibrary.org/obo/esmo.owl#Ecosystem_function"/>
        <rdfs:subClassOf>
            <owl:Restriction>
                <owl:onProperty rdf:resource="http://purl.obolibrary.org/obo/BFO_0000118"/>
                <owl:someValuesFrom rdf:resource="http://purl.obolibrary.org/obo/esmo.owl#Predation"/>
            </owl:Restriction>
        </rdfs:subClassOf>
        <skos:definition>The provision of living space for resident and migratory species.</skos:definition>
    </owl:Class>
    


    <!-- http://purl.obolibrary.org/obo/esmo.owl#Household -->

    <owl:Class rdf:about="http://purl.obolibrary.org/obo/esmo.owl#Household">
        <rdfs:subClassOf rdf:resource="http://purl.obolibrary.org/obo/esmo.owl#Actor_aggregate"/>
        <rdfs:subClassOf>
            <owl:Restriction>
                <owl:onProperty rdf:resource="http://purl.obolibrary.org/obo/esmo.owl#benefits_from"/>
                <owl:someValuesFrom rdf:resource="http://purl.obolibrary.org/obo/esmo.owl#Food_value"/>
            </owl:Restriction>
        </rdfs:subClassOf>
        <rdfs:subClassOf>
            <owl:Restriction>
                <owl:onProperty rdf:resource="http://purl.obolibrary.org/obo/esmo.owl#measure_of"/>
                <owl:someValuesFrom rdf:resource="http://purl.obolibrary.org/obo/esmo.owl#EESV_demand"/>
            </owl:Restriction>
        </rdfs:subClassOf>
        <skos:definition>A group of individuals residing together and engaging in collective economic activities and decision-making, such as consumption, production, and resource management</skos:definition>
    </owl:Class>
    


    <!-- http://purl.obolibrary.org/obo/esmo.owl#Human_activity -->

    <owl:Class rdf:about="http://purl.obolibrary.org/obo/esmo.owl#Human_activity">
        <rdfs:subClassOf rdf:resource="http://purl.obolibrary.org/obo/BFO_0000015"/>
        <rdfs:subClassOf>
            <owl:Restriction>
                <owl:onProperty rdf:resource="http://purl.obolibrary.org/obo/BFO_0000055"/>
                <owl:someValuesFrom rdf:resource="http://purl.obolibrary.org/obo/esmo.owl#Ecosystem_service"/>
            </owl:Restriction>
        </rdfs:subClassOf>
        <rdfs:subClassOf>
            <owl:Restriction>
                <owl:onProperty rdf:resource="http://purl.obolibrary.org/obo/BFO_0000057"/>
                <owl:someValuesFrom rdf:resource="http://purl.obolibrary.org/obo/esmo.owl#Anthropogenic_asset"/>
            </owl:Restriction>
        </rdfs:subClassOf>
        <rdfs:subClassOf>
            <owl:Restriction>
                <owl:onProperty rdf:resource="http://purl.obolibrary.org/obo/BFO_0000057"/>
                <owl:someValuesFrom rdf:resource="http://purl.obolibrary.org/obo/esmo.owl#Anthropogenic_asset_aggregate"/>
            </owl:Restriction>
        </rdfs:subClassOf>
        <rdfs:subClassOf>
            <owl:Restriction>
                <owl:onProperty rdf:resource="http://purl.obolibrary.org/obo/BFO_0000057"/>
                <owl:someValuesFrom rdf:resource="http://purl.obolibrary.org/obo/esmo.owl#Ecosystem_good"/>
            </owl:Restriction>
        </rdfs:subClassOf>
        <rdfs:subClassOf>
            <owl:Restriction>
                <owl:onProperty rdf:resource="http://purl.obolibrary.org/obo/BFO_0000167"/>
                <owl:someValuesFrom rdf:resource="http://purl.obolibrary.org/obo/esmo.owl#Actor"/>
            </owl:Restriction>
        </rdfs:subClassOf>
        <rdfs:subClassOf>
            <owl:Restriction>
                <owl:onProperty rdf:resource="http://purl.obolibrary.org/obo/esmo.owl#causally_upstream_of"/>
                <owl:someValuesFrom rdf:resource="http://purl.obolibrary.org/obo/esmo.owl#Driver_of_change"/>
            </owl:Restriction>
        </rdfs:subClassOf>
        <rdfs:subClassOf>
            <owl:Restriction>
                <owl:onProperty rdf:resource="http://purl.obolibrary.org/obo/esmo.owl#has_quality"/>
                <owl:someValuesFrom>
                    <owl:Class>
                        <owl:unionOf rdf:parseType="Collection">
                            <rdf:Description rdf:about="http://purl.obolibrary.org/obo/esmo.owl#Instrumental_value"/>
                            <rdf:Description rdf:about="http://purl.obolibrary.org/obo/esmo.owl#Relational_value"/>
                        </owl:unionOf>
                    </owl:Class>
                </owl:someValuesFrom>
            </owl:Restriction>
        </rdfs:subClassOf>
        <skos:definition>Any intentional action or series of actions performed by humans that influence or alter the state of social, economic, or ecological systems, often involving the use of resources, the production of commodities, or the provision of services.</skos:definition>
    </owl:Class>
    


    <!-- http://purl.obolibrary.org/obo/esmo.owl#Indirect_driver -->

    <owl:Class rdf:about="http://purl.obolibrary.org/obo/esmo.owl#Indirect_driver">
        <rdfs:subClassOf rdf:resource="http://purl.obolibrary.org/obo/esmo.owl#Driver_of_change"/>
        <skos:definition>A driver of change that operates diffusely by altering one or more direct drivers.</skos:definition>
        <skos:example>Climate change</skos:example>
    </owl:Class>
    


    <!-- http://purl.obolibrary.org/obo/esmo.owl#Infrastructure -->

    <owl:Class rdf:about="http://purl.obolibrary.org/obo/esmo.owl#Infrastructure">
        <rdfs:subClassOf rdf:resource="http://purl.obolibrary.org/obo/esmo.owl#Anthropogenic_asset"/>
        <skos:definition>A type of anthropogenic asset comprising the physical and organizational systems designed and constructed by humans to support societal functions, economic activities, and the provision of services.</skos:definition>
        <skos:example>A road, a sea wall, a bridge</skos:example>
    </owl:Class>
    


    <!-- http://purl.obolibrary.org/obo/esmo.owl#Instrumental_value -->

    <owl:Class rdf:about="http://purl.obolibrary.org/obo/esmo.owl#Instrumental_value">
        <rdfs:subClassOf rdf:resource="http://purl.obolibrary.org/obo/esmo.owl#Value"/>
        <rdfs:comment>For more, see Pascual, U., Balvanera, P., Díaz, S., Pataki, G., Roth, E., Stenseke, M., Watson, R.T., Dessane, E.B., Islar, M., Kelemen, E. and Maris, V., 2017. Valuing nature’s contributions to people: the IPBES approach. Current opinion in environmental sustainability, 26, pp.7-16.</rdfs:comment>
        <skos:definition>The value attributed to something as a means to achieving a particular end</skos:definition>
    </owl:Class>
    


    <!-- http://purl.obolibrary.org/obo/esmo.owl#Intrinsic_value -->

    <owl:Class rdf:about="http://purl.obolibrary.org/obo/esmo.owl#Intrinsic_value">
        <rdfs:subClassOf rdf:resource="http://purl.obolibrary.org/obo/esmo.owl#Value"/>
        <rdfs:comment>For more, see Pascual, U., Balvanera, P., Díaz, S., Pataki, G., Roth, E., Stenseke, M., Watson, R.T., Dessane, E.B., Islar, M., Kelemen, E. and Maris, V., 2017. Valuing nature’s contributions to people: the IPBES approach. Current opinion in environmental sustainability, 26, pp.7-16.</rdfs:comment>
        <skos:definition>The inherent value, that is the value something has independent of any human experience or evaluation. Such a value is viewed as an inherent property of the entity and not ascribed or generated by external valuing agents</skos:definition>
        <skos:example>Existence value</skos:example>
    </owl:Class>
    


    <!-- http://purl.obolibrary.org/obo/esmo.owl#Monetary_instrumental_value -->

    <owl:Class rdf:about="http://purl.obolibrary.org/obo/esmo.owl#Monetary_instrumental_value">
        <rdfs:subClassOf rdf:resource="http://purl.obolibrary.org/obo/esmo.owl#Instrumental_value"/>
        <skos:definition>An instrumental value where the end achieved is monetary gain.</skos:definition>
        <skos:example>The value in USD</skos:example>
    </owl:Class>
    


    <!-- http://purl.obolibrary.org/obo/esmo.owl#Net_primary_production -->

    <owl:Class rdf:about="http://purl.obolibrary.org/obo/esmo.owl#Net_primary_production">
        <rdfs:subClassOf rdf:resource="http://purl.obolibrary.org/obo/esmo.owl#Ecosystem_function"/>
        <rdfs:subClassOf>
            <owl:Restriction>
                <owl:onProperty rdf:resource="http://purl.obolibrary.org/obo/BFO_0000118"/>
                <owl:someValuesFrom rdf:resource="http://purl.obolibrary.org/obo/esmo.owl#Carbon_fixation"/>
            </owl:Restriction>
        </rdfs:subClassOf>
        <rdfs:subClassOf>
            <owl:Restriction>
                <owl:onProperty rdf:resource="http://purl.obolibrary.org/obo/BFO_0000118"/>
                <owl:someValuesFrom rdf:resource="http://purl.obolibrary.org/obo/esmo.owl#Photosynthesis"/>
            </owl:Restriction>
        </rdfs:subClassOf>
        <skos:definition>The total mass of carbon taken out of the atmosphere by plant photosynthesis (Gross Primary Production) minus return to the atmosphere of carbon due to autotrophic respiration.</skos:definition>
    </owl:Class>
    


    <!-- http://purl.obolibrary.org/obo/esmo.owl#Non_economic_activity -->

    <owl:Class rdf:about="http://purl.obolibrary.org/obo/esmo.owl#Non_economic_activity">
        <rdfs:subClassOf rdf:resource="http://purl.obolibrary.org/obo/esmo.owl#Human_activity"/>
        <rdfs:subClassOf>
            <owl:Restriction>
                <owl:onProperty rdf:resource="http://purl.obolibrary.org/obo/BFO_0000167"/>
                <owl:someValuesFrom rdf:resource="http://purl.obolibrary.org/obo/esmo.owl#Non_economic_actor"/>
            </owl:Restriction>
        </rdfs:subClassOf>
        <rdfs:subClassOf>
            <owl:Restriction>
                <owl:onProperty rdf:resource="http://purl.obolibrary.org/obo/esmo.owl#has_quality"/>
                <owl:someValuesFrom rdf:resource="http://purl.obolibrary.org/obo/esmo.owl#Non_monetary_instrumental_value"/>
            </owl:Restriction>
        </rdfs:subClassOf>
        <skos:definition>A human activity that serves social, cultural, recreational or environmental purposes and does not involve the production, distribution, or consumption of commodities and services for economic gain.</skos:definition>
        <skos:example>Subsistence farming, hiking</skos:example>
    </owl:Class>
    


    <!-- http://purl.obolibrary.org/obo/esmo.owl#Non_economic_actor -->

    <owl:Class rdf:about="http://purl.obolibrary.org/obo/esmo.owl#Non_economic_actor">
        <rdfs:subClassOf rdf:resource="http://purl.obolibrary.org/obo/esmo.owl#Actor"/>
        <rdfs:subClassOf>
            <owl:Restriction>
                <owl:onProperty rdf:resource="http://purl.obolibrary.org/obo/esmo.owl#benefits_from"/>
                <owl:someValuesFrom rdf:resource="http://purl.obolibrary.org/obo/esmo.owl#Non_monetary_instrumental_value"/>
            </owl:Restriction>
        </rdfs:subClassOf>
        <skos:definition>An actor who participates in non-economic activity and who&apos;s behaviour and decisions are independent from economic concerns, ie are not tied to monetary considerations.</skos:definition>
    </owl:Class>
    


    <!-- http://purl.obolibrary.org/obo/esmo.owl#Non_monetary_instrumental_value -->

    <owl:Class rdf:about="http://purl.obolibrary.org/obo/esmo.owl#Non_monetary_instrumental_value">
        <rdfs:subClassOf rdf:resource="http://purl.obolibrary.org/obo/esmo.owl#Instrumental_value"/>
        <skos:definition>An instrumental value where the end achieved is not monetary gain.</skos:definition>
    </owl:Class>
    


    <!-- http://purl.obolibrary.org/obo/esmo.owl#Nutrient_cycling -->

    <owl:Class rdf:about="http://purl.obolibrary.org/obo/esmo.owl#Nutrient_cycling">
        <rdfs:subClassOf rdf:resource="http://purl.obolibrary.org/obo/esmo.owl#Ecosystem_function"/>
        <skos:definition>The processes by which elements are extracted from their mineral, aquatic, or atmospheric sources or recycled from their organic forms, converting them to the ionic form in which biotic uptake occurs and ultimately returning them to the atmosphere, water, or soil.</skos:definition>
    </owl:Class>
    


    <!-- http://purl.obolibrary.org/obo/esmo.owl#Permanent_lowland_rivers -->

    <owl:Class rdf:about="http://purl.obolibrary.org/obo/esmo.owl#Permanent_lowland_rivers">
        <rdfs:subClassOf rdf:resource="http://purl.obolibrary.org/obo/esmo.owl#Ecosystem"/>
        <rdfs:subClassOf>
            <owl:Restriction>
                <owl:onProperty rdf:resource="http://purl.obolibrary.org/obo/BFO_0000183"/>
                <owl:someValuesFrom rdf:resource="http://purl.obolibrary.org/obo/esmo.owl#Water_purification"/>
            </owl:Restriction>
        </rdfs:subClassOf>
        <rdfs:comment>For additional detailed information refer to Keith, D.A., Ferrer-Paris, J.R., Nicholson, E. and Kingsford, R.T. (eds.) (2020). The IUCN Global Ecosystem Typology 2.0: Descriptive profiles for biomes and ecosystem functional groups. Gland, Switzerland: IUCN.</rdfs:comment>
        <skos:definition>Small-medium lowland rivers are productive depositional ecosystems with trophic webs that are less diverse than large lowland rivers.</skos:definition>
        <skos:example>Rio Carrao in Venezuela</skos:example>
    </owl:Class>
    


    <!-- http://purl.obolibrary.org/obo/esmo.owl#Photosynthesis -->

    <owl:Class rdf:about="http://purl.obolibrary.org/obo/esmo.owl#Photosynthesis">
        <rdfs:subClassOf rdf:resource="http://purl.obolibrary.org/obo/esmo.owl#Ecosystem_process"/>
        <rdfs:subClassOf>
            <owl:Restriction>
                <owl:onProperty rdf:resource="http://purl.obolibrary.org/obo/BFO_0000138"/>
                <owl:someValuesFrom rdf:resource="http://purl.obolibrary.org/obo/esmo.owl#Net_primary_production"/>
            </owl:Restriction>
        </rdfs:subClassOf>
        <skos:definition>The metabolic pathways for CO2 fixation by plants.</skos:definition>
    </owl:Class>
    


    <!-- http://purl.obolibrary.org/obo/esmo.owl#Pollution -->

    <owl:Class rdf:about="http://purl.obolibrary.org/obo/esmo.owl#Pollution">
        <rdfs:subClassOf rdf:resource="http://purl.obolibrary.org/obo/esmo.owl#Direct_driver"/>
        <skos:definition>The introduction of contaminants into the natural environment that cause adverse change.</skos:definition>
        <skos:example>Heavy metal contamination, air pollution</skos:example>
    </owl:Class>
    


    <!-- http://purl.obolibrary.org/obo/esmo.owl#Predation -->

    <owl:Class rdf:about="http://purl.obolibrary.org/obo/esmo.owl#Predation">
        <rdfs:subClassOf rdf:resource="http://purl.obolibrary.org/obo/esmo.owl#Ecosystem_process"/>
        <rdfs:subClassOf>
            <owl:Restriction>
                <owl:onProperty rdf:resource="http://purl.obolibrary.org/obo/BFO_0000138"/>
                <owl:someValuesFrom rdf:resource="http://purl.obolibrary.org/obo/esmo.owl#Biological_control"/>
            </owl:Restriction>
        </rdfs:subClassOf>
        <rdfs:subClassOf>
            <owl:Restriction>
                <owl:onProperty rdf:resource="http://purl.obolibrary.org/obo/BFO_0000138"/>
                <owl:someValuesFrom rdf:resource="http://purl.obolibrary.org/obo/esmo.owl#Biomass_production"/>
            </owl:Restriction>
        </rdfs:subClassOf>
        <rdfs:subClassOf>
            <owl:Restriction>
                <owl:onProperty rdf:resource="http://purl.obolibrary.org/obo/BFO_0000138"/>
                <owl:someValuesFrom rdf:resource="http://purl.obolibrary.org/obo/esmo.owl#Habitat_provisioning"/>
            </owl:Restriction>
        </rdfs:subClassOf>
        <skos:definition>A biological process in which one organism, the predator, hunts, captures, and consumes another organism, the prey, as a means of obtaining energy and nutrients.</skos:definition>
    </owl:Class>
    


    <!-- http://purl.obolibrary.org/obo/esmo.owl#Provisioning_ecosystem_service -->

    <owl:Class rdf:about="http://purl.obolibrary.org/obo/esmo.owl#Provisioning_ecosystem_service">
        <rdfs:subClassOf rdf:resource="http://purl.obolibrary.org/obo/esmo.owl#Ecosystem_service"/>
        <rdfs:subClassOf>
            <owl:Restriction>
                <owl:onProperty rdf:resource="http://purl.obolibrary.org/obo/BFO_0000195"/>
                <owl:someValuesFrom rdf:resource="http://purl.obolibrary.org/obo/esmo.owl#Ecosystem_good"/>
            </owl:Restriction>
        </rdfs:subClassOf>
        <skos:definition>These are the services that contribute to the products obtained from ecosystems.</skos:definition>
        <skos:example>Food provisioning services, timber provisioning services, freshwater provisioning services</skos:example>
    </owl:Class>
    


    <!-- http://purl.obolibrary.org/obo/esmo.owl#Regulating_ecosystem_service -->

    <owl:Class rdf:about="http://purl.obolibrary.org/obo/esmo.owl#Regulating_ecosystem_service">
        <rdfs:subClassOf rdf:resource="http://purl.obolibrary.org/obo/esmo.owl#Ecosystem_service"/>
        <skos:definition>These are the services that contribute to the benefits obtained from the regulation of ecosystem processes.</skos:definition>
        <skos:example>Pollination services, flood prevention services</skos:example>
    </owl:Class>
    


    <!-- http://purl.obolibrary.org/obo/esmo.owl#Relational_value -->

    <owl:Class rdf:about="http://purl.obolibrary.org/obo/esmo.owl#Relational_value">
        <rdfs:subClassOf rdf:resource="http://purl.obolibrary.org/obo/esmo.owl#Value"/>
        <rdfs:comment>For more, see Pascual, U., Balvanera, P., Díaz, S., Pataki, G., Roth, E., Stenseke, M., Watson, R.T., Dessane, E.B., Islar, M., Kelemen, E. and Maris, V., 2017. Valuing nature’s contributions to people: the IPBES approach. Current opinion in environmental sustainability, 26, pp.7-16.</rdfs:comment>
        <skos:definition>Values that do not directly emanate from nature but are derivative of our relationships with it and our responsibilities towards it.</skos:definition>
        <skos:example>Spiritual value, cultural value</skos:example>
    </owl:Class>
    


    <!-- http://purl.obolibrary.org/obo/esmo.owl#Reproduction -->

    <owl:Class rdf:about="http://purl.obolibrary.org/obo/esmo.owl#Reproduction">
        <rdfs:subClassOf rdf:resource="http://purl.obolibrary.org/obo/esmo.owl#Ecosystem_process"/>
        <skos:definition>A biological process by which organisms produce offspring, ensuring the continuation of their species to pass on genetic material to the next generation.</skos:definition>
        <skos:example>Sexual reproduction, asexual reproduction</skos:example>
    </owl:Class>
    


    <!-- http://purl.obolibrary.org/obo/esmo.owl#River_access_infrastructure -->

    <owl:Class rdf:about="http://purl.obolibrary.org/obo/esmo.owl#River_access_infrastructure">
        <rdfs:subClassOf rdf:resource="http://purl.obolibrary.org/obo/esmo.owl#Infrastructure"/>
        <rdfs:subClassOf>
            <owl:Restriction>
                <owl:onProperty rdf:resource="http://purl.obolibrary.org/obo/BFO_0000056"/>
                <owl:someValuesFrom rdf:resource="http://purl.obolibrary.org/obo/esmo.owl#Swimming"/>
            </owl:Restriction>
        </rdfs:subClassOf>
        <rdfs:subClassOf>
            <owl:Restriction>
                <owl:onProperty rdf:resource="http://purl.obolibrary.org/obo/esmo.owl#measure_of"/>
                <owl:someValuesFrom rdf:resource="http://purl.obolibrary.org/obo/esmo.owl#EESV_anthropogenic_contribution"/>
            </owl:Restriction>
        </rdfs:subClassOf>
        <skos:definition>A type of infrastrucure specifically designed to support human activities requiring river access.</skos:definition>
        <skos:example>A potoon, a boat launch, a road to the river</skos:example>
    </owl:Class>
    


    <!-- http://purl.obolibrary.org/obo/esmo.owl#Swimmer -->

    <owl:Class rdf:about="http://purl.obolibrary.org/obo/esmo.owl#Swimmer">
        <rdfs:subClassOf rdf:resource="http://purl.obolibrary.org/obo/esmo.owl#Non_economic_actor"/>
        <rdfs:subClassOf>
            <owl:Restriction>
                <owl:onProperty rdf:resource="http://purl.obolibrary.org/obo/BFO_0000166"/>
                <owl:someValuesFrom rdf:resource="http://purl.obolibrary.org/obo/esmo.owl#Swimming"/>
            </owl:Restriction>
        </rdfs:subClassOf>
        <rdfs:subClassOf>
            <owl:Restriction>
                <owl:onProperty rdf:resource="http://purl.obolibrary.org/obo/esmo.owl#benefits_from"/>
                <owl:someValuesFrom rdf:resource="http://purl.obolibrary.org/obo/esmo.owl#Enjoyment_value"/>
            </owl:Restriction>
        </rdfs:subClassOf>
        <skos:definition>A type of non-economic actor who participates in the swimming activity.</skos:definition>
    </owl:Class>
    


    <!-- http://purl.obolibrary.org/obo/esmo.owl#Swimming -->

    <owl:Class rdf:about="http://purl.obolibrary.org/obo/esmo.owl#Swimming">
        <rdfs:subClassOf rdf:resource="http://purl.obolibrary.org/obo/esmo.owl#Non_economic_activity"/>
        <rdfs:subClassOf>
            <owl:Restriction>
                <owl:onProperty rdf:resource="http://purl.obolibrary.org/obo/BFO_0000055"/>
                <owl:someValuesFrom rdf:resource="http://purl.obolibrary.org/obo/esmo.owl#Water_quality_regulation_service"/>
            </owl:Restriction>
        </rdfs:subClassOf>
        <rdfs:subClassOf>
            <owl:Restriction>
                <owl:onProperty rdf:resource="http://purl.obolibrary.org/obo/BFO_0000057"/>
                <owl:someValuesFrom rdf:resource="http://purl.obolibrary.org/obo/esmo.owl#River_access_infrastructure"/>
            </owl:Restriction>
        </rdfs:subClassOf>
        <rdfs:subClassOf>
            <owl:Restriction>
                <owl:onProperty rdf:resource="http://purl.obolibrary.org/obo/BFO_0000167"/>
                <owl:someValuesFrom rdf:resource="http://purl.obolibrary.org/obo/esmo.owl#Clean_freshwater"/>
            </owl:Restriction>
        </rdfs:subClassOf>
        <rdfs:subClassOf>
            <owl:Restriction>
                <owl:onProperty rdf:resource="http://purl.obolibrary.org/obo/BFO_0000167"/>
                <owl:someValuesFrom rdf:resource="http://purl.obolibrary.org/obo/esmo.owl#Swimmer"/>
            </owl:Restriction>
        </rdfs:subClassOf>
        <rdfs:subClassOf>
            <owl:Restriction>
                <owl:onProperty rdf:resource="http://purl.obolibrary.org/obo/esmo.owl#has_quality"/>
                <owl:someValuesFrom rdf:resource="http://purl.obolibrary.org/obo/esmo.owl#Enjoyment_value"/>
            </owl:Restriction>
        </rdfs:subClassOf>
        <rdfs:subClassOf>
            <owl:Restriction>
                <owl:onProperty rdf:resource="http://purl.obolibrary.org/obo/esmo.owl#measure_of"/>
                <owl:someValuesFrom rdf:resource="http://purl.obolibrary.org/obo/esmo.owl#EESV_use"/>
            </owl:Restriction>
        </rdfs:subClassOf>
        <skos:definition>A non-economic activity that involves the act of swimming for the purpose of recreation without revenue generation</skos:definition>
    </owl:Class>
    


    <!-- http://purl.obolibrary.org/obo/esmo.owl#Tour_operator -->

    <owl:Class rdf:about="http://purl.obolibrary.org/obo/esmo.owl#Tour_operator">
        <rdfs:subClassOf rdf:resource="http://purl.obolibrary.org/obo/esmo.owl#Economic_actor"/>
        <rdfs:subClassOf>
            <owl:Restriction>
                <owl:onProperty rdf:resource="http://purl.obolibrary.org/obo/BFO_0000056"/>
                <owl:someValuesFrom rdf:resource="http://purl.obolibrary.org/obo/esmo.owl#Whale_watching"/>
            </owl:Restriction>
        </rdfs:subClassOf>
        <rdfs:subClassOf>
            <owl:Restriction>
                <owl:onProperty rdf:resource="http://purl.obolibrary.org/obo/esmo.owl#benefits_from"/>
                <owl:someValuesFrom rdf:resource="http://purl.obolibrary.org/obo/esmo.owl#Monetary_instrumental_value"/>
            </owl:Restriction>
        </rdfs:subClassOf>
        <skos:definition>A type of economic actor who participates in a touristic activity as a provider.</skos:definition>
        <skos:example>A whale watching tour operator.</skos:example>
    </owl:Class>
    


    <!-- http://purl.obolibrary.org/obo/esmo.owl#Value -->

    <owl:Class rdf:about="http://purl.obolibrary.org/obo/esmo.owl#Value">
        <rdfs:subClassOf rdf:resource="http://purl.obolibrary.org/obo/BFO_0000019"/>
        <skos:definition>A principle associated with a given worldview or cultural context, a preference someone has, the importance of something for itself or for others, or simply as a means to an end.</skos:definition>
    </owl:Class>
    


    <!-- http://purl.obolibrary.org/obo/esmo.owl#Vessel_fleet -->

    <owl:Class rdf:about="http://purl.obolibrary.org/obo/esmo.owl#Vessel_fleet">
        <rdfs:subClassOf rdf:resource="http://purl.obolibrary.org/obo/esmo.owl#Anthropogenic_asset_aggregate"/>
        <skos:definition>Is a material entity consisting exactly of a plurality (≥1) of vessels as member parts which together form a unit.</skos:definition>
        <skos:example>A fishing fleet</skos:example>
    </owl:Class>
    


    <!-- http://purl.obolibrary.org/obo/esmo.owl#Vessel_strike -->

    <owl:Class rdf:about="http://purl.obolibrary.org/obo/esmo.owl#Vessel_strike">
        <rdfs:subClassOf rdf:resource="http://purl.obolibrary.org/obo/esmo.owl#Direct_driver"/>
        <rdfs:subClassOf>
            <owl:Restriction>
                <owl:onProperty rdf:resource="http://purl.obolibrary.org/obo/esmo.owl#causally_influences"/>
                <owl:someValuesFrom rdf:resource="http://purl.obolibrary.org/obo/esmo.owl#Whale_population"/>
            </owl:Restriction>
        </rdfs:subClassOf>
        <skos:definition>A vessel strike is a collision between any type of boat and a marine animal in the ocean.</skos:definition>
    </owl:Class>
    


    <!-- http://purl.obolibrary.org/obo/esmo.owl#Warming -->

    <owl:Class rdf:about="http://purl.obolibrary.org/obo/esmo.owl#Warming">
        <rdfs:subClassOf rdf:resource="http://purl.obolibrary.org/obo/esmo.owl#Indirect_driver"/>
        <skos:definition>The continuous increase in temperature relative to a historical baseline.</skos:definition>
    </owl:Class>
    


    <!-- http://purl.obolibrary.org/obo/esmo.owl#Water_purification -->

    <owl:Class rdf:about="http://purl.obolibrary.org/obo/esmo.owl#Water_purification">
        <rdfs:subClassOf rdf:resource="http://purl.obolibrary.org/obo/esmo.owl#Ecosystem_function"/>
        <rdfs:subClassOf>
            <owl:Restriction>
                <owl:onProperty rdf:resource="http://purl.obolibrary.org/obo/BFO_0000055"/>
                <owl:someValuesFrom rdf:resource="http://purl.obolibrary.org/obo/esmo.owl#Water_quality_regulation_service"/>
            </owl:Restriction>
        </rdfs:subClassOf>
        <rdfs:subClassOf>
            <owl:Restriction>
                <owl:onProperty rdf:resource="http://purl.obolibrary.org/obo/BFO_0000066"/>
                <owl:someValuesFrom rdf:resource="http://purl.obolibrary.org/obo/esmo.owl#Permanent_lowland_rivers"/>
            </owl:Restriction>
        </rdfs:subClassOf>
        <rdfs:subClassOf>
            <owl:Restriction>
                <owl:onProperty rdf:resource="http://purl.obolibrary.org/obo/esmo.owl#has_output"/>
                <owl:someValuesFrom rdf:resource="http://purl.obolibrary.org/obo/esmo.owl#Clean_freshwater"/>
            </owl:Restriction>
        </rdfs:subClassOf>
        <skos:definition>The removal of sediments and nutrients and other impurities from water.</skos:definition>
    </owl:Class>
    


    <!-- http://purl.obolibrary.org/obo/esmo.owl#Water_quality_regulation_service -->

    <owl:Class rdf:about="http://purl.obolibrary.org/obo/esmo.owl#Water_quality_regulation_service">
        <rdfs:subClassOf rdf:resource="http://purl.obolibrary.org/obo/esmo.owl#Regulating_ecosystem_service"/>
        <rdfs:subClassOf>
            <owl:Restriction>
                <owl:onProperty rdf:resource="http://purl.obolibrary.org/obo/BFO_0000054"/>
                <owl:someValuesFrom rdf:resource="http://purl.obolibrary.org/obo/esmo.owl#Swimming"/>
            </owl:Restriction>
        </rdfs:subClassOf>
        <rdfs:subClassOf>
            <owl:Restriction>
                <owl:onProperty rdf:resource="http://purl.obolibrary.org/obo/BFO_0000054"/>
                <owl:someValuesFrom rdf:resource="http://purl.obolibrary.org/obo/esmo.owl#Water_purification"/>
            </owl:Restriction>
        </rdfs:subClassOf>
        <skos:definition>The role of an ecosystem in regulating pollutants and excess nutrients to maintain the chemical condition of water to mitigate harmful effects on human health.</skos:definition>
    </owl:Class>
    


    <!-- http://purl.obolibrary.org/obo/esmo.owl#Whale_habitat_provisioning -->

    <owl:Class rdf:about="http://purl.obolibrary.org/obo/esmo.owl#Whale_habitat_provisioning">
        <rdfs:subClassOf rdf:resource="http://purl.obolibrary.org/obo/esmo.owl#Habitat_provisioning"/>
        <rdfs:subClassOf>
            <owl:Restriction>
                <owl:onProperty rdf:resource="http://purl.obolibrary.org/obo/BFO_0000055"/>
                <owl:someValuesFrom rdf:resource="http://purl.obolibrary.org/obo/esmo.owl#Wildlife_viewing_service"/>
            </owl:Restriction>
        </rdfs:subClassOf>
        <rdfs:subClassOf>
            <owl:Restriction>
                <owl:onProperty rdf:resource="http://purl.obolibrary.org/obo/BFO_0000066"/>
                <owl:someValuesFrom rdf:resource="http://purl.obolibrary.org/obo/esmo.owl#Epipelagic_ocean"/>
            </owl:Restriction>
        </rdfs:subClassOf>
        <rdfs:subClassOf>
            <owl:Restriction>
                <owl:onProperty rdf:resource="http://purl.obolibrary.org/obo/esmo.owl#has_output"/>
                <owl:someValuesFrom rdf:resource="http://purl.obolibrary.org/obo/esmo.owl#Whale_population"/>
            </owl:Restriction>
        </rdfs:subClassOf>
        <skos:definition>The provision of living space for whale species</skos:definition>
    </owl:Class>
    


    <!-- http://purl.obolibrary.org/obo/esmo.owl#Whale_population -->

    <owl:Class rdf:about="http://purl.obolibrary.org/obo/esmo.owl#Whale_population">
        <rdfs:subClassOf rdf:resource="http://purl.obolibrary.org/obo/esmo.owl#Ecosystem_good_aggregate"/>
        <rdfs:subClassOf>
            <owl:Restriction>
                <owl:onProperty rdf:resource="http://purl.obolibrary.org/obo/BFO_0000056"/>
                <owl:someValuesFrom rdf:resource="http://purl.obolibrary.org/obo/esmo.owl#Whale_watching"/>
            </owl:Restriction>
        </rdfs:subClassOf>
        <rdfs:subClassOf>
            <owl:Restriction>
                <owl:onProperty rdf:resource="http://purl.obolibrary.org/obo/esmo.owl#measure_of"/>
                <owl:someValuesFrom rdf:resource="http://purl.obolibrary.org/obo/esmo.owl#EESV_ecological_supply"/>
            </owl:Restriction>
        </rdfs:subClassOf>
        <rdfs:subClassOf>
            <owl:Restriction>
                <owl:onProperty rdf:resource="http://purl.obolibrary.org/obo/esmo.owl#output_of"/>
                <owl:someValuesFrom rdf:resource="http://purl.obolibrary.org/obo/esmo.owl#Whale_habitat_provisioning"/>
            </owl:Restriction>
        </rdfs:subClassOf>
        <skos:definition>Is a material entity consisting exactly of a plurality (≥1) of whales as member parts which together form a unit.</skos:definition>
        <skos:example>Orca population</skos:example>
    </owl:Class>
    


    <!-- http://purl.obolibrary.org/obo/esmo.owl#Whale_watcher -->

    <owl:Class rdf:about="http://purl.obolibrary.org/obo/esmo.owl#Whale_watcher">
        <rdfs:subClassOf rdf:resource="http://purl.obolibrary.org/obo/esmo.owl#Economic_actor"/>
        <rdfs:subClassOf>
            <owl:Restriction>
                <owl:onProperty rdf:resource="http://purl.obolibrary.org/obo/BFO_0000166"/>
                <owl:someValuesFrom rdf:resource="http://purl.obolibrary.org/obo/esmo.owl#Whale_watching"/>
            </owl:Restriction>
        </rdfs:subClassOf>
        <rdfs:subClassOf>
            <owl:Restriction>
                <owl:onProperty rdf:resource="http://purl.obolibrary.org/obo/esmo.owl#benefits_from"/>
                <owl:someValuesFrom rdf:resource="http://purl.obolibrary.org/obo/esmo.owl#Enjoyment_value"/>
            </owl:Restriction>
        </rdfs:subClassOf>
        <skos:definition>A type of economic actor who participates in the whale watching activity as a client.</skos:definition>
    </owl:Class>
    


    <!-- http://purl.obolibrary.org/obo/esmo.owl#Whale_watching -->

    <owl:Class rdf:about="http://purl.obolibrary.org/obo/esmo.owl#Whale_watching">
        <rdfs:subClassOf rdf:resource="http://purl.obolibrary.org/obo/esmo.owl#Economic_activity"/>
        <rdfs:subClassOf>
            <owl:Restriction>
                <owl:onProperty rdf:resource="http://purl.obolibrary.org/obo/BFO_0000055"/>
                <owl:someValuesFrom rdf:resource="http://purl.obolibrary.org/obo/esmo.owl#Wildlife_viewing_service"/>
            </owl:Restriction>
        </rdfs:subClassOf>
        <rdfs:subClassOf>
            <owl:Restriction>
                <owl:onProperty rdf:resource="http://purl.obolibrary.org/obo/BFO_0000057"/>
                <owl:someValuesFrom rdf:resource="http://purl.obolibrary.org/obo/esmo.owl#Tour_operator"/>
            </owl:Restriction>
        </rdfs:subClassOf>
        <rdfs:subClassOf>
            <owl:Restriction>
                <owl:onProperty rdf:resource="http://purl.obolibrary.org/obo/BFO_0000167"/>
                <owl:someValuesFrom rdf:resource="http://purl.obolibrary.org/obo/esmo.owl#Whale_population"/>
            </owl:Restriction>
        </rdfs:subClassOf>
        <rdfs:subClassOf>
            <owl:Restriction>
                <owl:onProperty rdf:resource="http://purl.obolibrary.org/obo/BFO_0000167"/>
                <owl:someValuesFrom rdf:resource="http://purl.obolibrary.org/obo/esmo.owl#Whalewatching_fleet"/>
            </owl:Restriction>
        </rdfs:subClassOf>
        <rdfs:subClassOf>
            <owl:Restriction>
                <owl:onProperty rdf:resource="http://purl.obolibrary.org/obo/esmo.owl#has_quality"/>
                <owl:someValuesFrom rdf:resource="http://purl.obolibrary.org/obo/esmo.owl#Enjoyment_value"/>
            </owl:Restriction>
        </rdfs:subClassOf>
        <rdfs:subClassOf>
            <owl:Restriction>
                <owl:onProperty rdf:resource="http://purl.obolibrary.org/obo/esmo.owl#has_quality"/>
                <owl:someValuesFrom rdf:resource="http://purl.obolibrary.org/obo/esmo.owl#Monetary_instrumental_value"/>
            </owl:Restriction>
        </rdfs:subClassOf>
        <rdfs:subClassOf>
            <owl:Restriction>
                <owl:onProperty rdf:resource="http://purl.obolibrary.org/obo/esmo.owl#measure_of"/>
                <owl:someValuesFrom rdf:resource="http://purl.obolibrary.org/obo/esmo.owl#EESV_use"/>
            </owl:Restriction>
        </rdfs:subClassOf>
        <skos:definition>An economic activity that involves the observation of whales.</skos:definition>
    </owl:Class>
    


    <!-- http://purl.obolibrary.org/obo/esmo.owl#Whalewatching_fleet -->

    <owl:Class rdf:about="http://purl.obolibrary.org/obo/esmo.owl#Whalewatching_fleet">
        <rdfs:subClassOf rdf:resource="http://purl.obolibrary.org/obo/esmo.owl#Vessel_fleet"/>
        <rdfs:subClassOf>
            <owl:Restriction>
                <owl:onProperty rdf:resource="http://purl.obolibrary.org/obo/BFO_0000056"/>
                <owl:someValuesFrom rdf:resource="http://purl.obolibrary.org/obo/esmo.owl#Whale_watching"/>
            </owl:Restriction>
        </rdfs:subClassOf>
        <rdfs:subClassOf>
            <owl:Restriction>
                <owl:onProperty rdf:resource="http://purl.obolibrary.org/obo/esmo.owl#measure_of"/>
                <owl:someValuesFrom rdf:resource="http://purl.obolibrary.org/obo/esmo.owl#EESV_anthropogenic_contribution"/>
            </owl:Restriction>
        </rdfs:subClassOf>
        <skos:example>Is a vessel aggregate where all vessel types are whale watching vessels, ie whose primary purpose is to take people to observe whales.</skos:example>
    </owl:Class>
    


    <!-- http://purl.obolibrary.org/obo/esmo.owl#Wholesale_value -->

    <owl:Class rdf:about="http://purl.obolibrary.org/obo/esmo.owl#Wholesale_value">
        <rdfs:subClassOf rdf:resource="http://purl.obolibrary.org/obo/esmo.owl#Monetary_instrumental_value"/>
        <rdfs:subClassOf>
            <owl:Restriction>
                <owl:onProperty rdf:resource="http://purl.obolibrary.org/obo/esmo.owl#measure_of"/>
                <owl:someValuesFrom rdf:resource="http://purl.obolibrary.org/obo/esmo.owl#EESV_instrumental_value"/>
            </owl:Restriction>
        </rdfs:subClassOf>
        <skos:definition>The monetary value of a product paid by retailers before being marked up and sold to consumers.</skos:definition>
    </owl:Class>
    


    <!-- http://purl.obolibrary.org/obo/esmo.owl#Wild_fish_provisioning_service -->

    <owl:Class rdf:about="http://purl.obolibrary.org/obo/esmo.owl#Wild_fish_provisioning_service">
        <rdfs:subClassOf rdf:resource="http://purl.obolibrary.org/obo/esmo.owl#Provisioning_ecosystem_service"/>
        <rdfs:subClassOf>
            <owl:Restriction>
                <owl:onProperty rdf:resource="http://purl.obolibrary.org/obo/BFO_0000054"/>
                <owl:someValuesFrom rdf:resource="http://purl.obolibrary.org/obo/esmo.owl#Commercial_fishing"/>
            </owl:Restriction>
        </rdfs:subClassOf>
        <rdfs:subClassOf>
            <owl:Restriction>
                <owl:onProperty rdf:resource="http://purl.obolibrary.org/obo/BFO_0000054"/>
                <owl:someValuesFrom rdf:resource="http://purl.obolibrary.org/obo/esmo.owl#Fish_biomass_production"/>
            </owl:Restriction>
        </rdfs:subClassOf>
        <skos:definition>The role of an ecosystem in contributing to the growth of fish and other aquatic biomass that are captured in uncultivated production contexts for various uses, primarily food production.</skos:definition>
    </owl:Class>
    


    <!-- http://purl.obolibrary.org/obo/esmo.owl#Wildcaught_fish -->

    <owl:Class rdf:about="http://purl.obolibrary.org/obo/esmo.owl#Wildcaught_fish">
        <rdfs:subClassOf rdf:resource="http://purl.obolibrary.org/obo/esmo.owl#Commodity_aggregate"/>
        <rdfs:subClassOf>
            <owl:Restriction>
                <owl:onProperty rdf:resource="http://purl.obolibrary.org/obo/esmo.owl#has_quality"/>
                <owl:someValuesFrom rdf:resource="http://purl.obolibrary.org/obo/esmo.owl#Food_value"/>
            </owl:Restriction>
        </rdfs:subClassOf>
        <rdfs:subClassOf>
            <owl:Restriction>
                <owl:onProperty rdf:resource="http://purl.obolibrary.org/obo/esmo.owl#has_quality"/>
                <owl:someValuesFrom rdf:resource="http://purl.obolibrary.org/obo/esmo.owl#Wholesale_value"/>
            </owl:Restriction>
        </rdfs:subClassOf>
        <rdfs:subClassOf>
            <owl:Restriction>
                <owl:onProperty rdf:resource="http://purl.obolibrary.org/obo/esmo.owl#measure_of"/>
                <owl:someValuesFrom rdf:resource="http://purl.obolibrary.org/obo/esmo.owl#EESV_use"/>
            </owl:Restriction>
        </rdfs:subClassOf>
        <rdfs:subClassOf>
            <owl:Restriction>
                <owl:onProperty rdf:resource="http://purl.obolibrary.org/obo/esmo.owl#output_of"/>
                <owl:someValuesFrom rdf:resource="http://purl.obolibrary.org/obo/esmo.owl#Commercial_fishing"/>
            </owl:Restriction>
        </rdfs:subClassOf>
        <skos:definition>Is a material entity consisting exactly of a plurality (≥1) of wild caught fish as member parts which together form a unit.</skos:definition>
        <skos:example>Landed tuna, landed sardines</skos:example>
    </owl:Class>
    


    <!-- http://purl.obolibrary.org/obo/esmo.owl#Wildlife_viewing_service -->

    <owl:Class rdf:about="http://purl.obolibrary.org/obo/esmo.owl#Wildlife_viewing_service">
        <rdfs:subClassOf rdf:resource="http://purl.obolibrary.org/obo/esmo.owl#Cultural_ecosystem_service"/>
        <rdfs:subClassOf>
            <owl:Restriction>
                <owl:onProperty rdf:resource="http://purl.obolibrary.org/obo/BFO_0000054"/>
                <owl:someValuesFrom rdf:resource="http://purl.obolibrary.org/obo/esmo.owl#Whale_habitat_provisioning"/>
            </owl:Restriction>
        </rdfs:subClassOf>
        <rdfs:subClassOf>
            <owl:Restriction>
                <owl:onProperty rdf:resource="http://purl.obolibrary.org/obo/BFO_0000054"/>
                <owl:someValuesFrom rdf:resource="http://purl.obolibrary.org/obo/esmo.owl#Whale_watching"/>
            </owl:Restriction>
        </rdfs:subClassOf>
        <skos:definition>The role of an ecosystem in enabling people to enjoy wildlife through direct, in-situ, observations.</skos:definition>
    </owl:Class>
    


    <!-- 
    ///////////////////////////////////////////////////////////////////////////////////////
    //
    // Individuals
    //
    ///////////////////////////////////////////////////////////////////////////////////////
     -->

    


    <!-- http://purl.obolibrary.org/obo/esmo.owl#Chin00 -->

    <owl:NamedIndividual rdf:about="http://purl.obolibrary.org/obo/esmo.owl#Chin00">
        <rdf:type rdf:resource="http://purl.obolibrary.org/obo/esmo.owl#Fish_population"/>
        <hasAbundance rdf:datatype="http://www.w3.org/2001/XMLSchema#double">51907.9043</hasAbundance>
        <hasYear rdf:datatype="http://www.w3.org/2001/XMLSchema#integer">2000</hasYear>
    </owl:NamedIndividual>
    


    <!-- http://purl.obolibrary.org/obo/esmo.owl#Chin01 -->

    <owl:NamedIndividual rdf:about="http://purl.obolibrary.org/obo/esmo.owl#Chin01">
        <rdf:type rdf:resource="http://purl.obolibrary.org/obo/esmo.owl#Fish_population"/>
        <hasAbundance rdf:datatype="http://www.w3.org/2001/XMLSchema#double">66245.72922</hasAbundance>
        <hasYear rdf:datatype="http://www.w3.org/2001/XMLSchema#integer">2001</hasYear>
    </owl:NamedIndividual>
    


    <!-- http://purl.obolibrary.org/obo/esmo.owl#Chin02 -->

    <owl:NamedIndividual rdf:about="http://purl.obolibrary.org/obo/esmo.owl#Chin02">
        <rdf:type rdf:resource="http://purl.obolibrary.org/obo/esmo.owl#Fish_population"/>
        <hasAbundance rdf:datatype="http://www.w3.org/2001/XMLSchema#double">57899.99048</hasAbundance>
        <hasYear rdf:datatype="http://www.w3.org/2001/XMLSchema#integer">2002</hasYear>
    </owl:NamedIndividual>
    


    <!-- http://purl.obolibrary.org/obo/esmo.owl#Chin03 -->

    <owl:NamedIndividual rdf:about="http://purl.obolibrary.org/obo/esmo.owl#Chin03">
        <rdf:type rdf:resource="http://purl.obolibrary.org/obo/esmo.owl#Fish_population"/>
        <hasAbundance rdf:datatype="http://www.w3.org/2001/XMLSchema#double">78181.28889</hasAbundance>
        <hasYear rdf:datatype="http://www.w3.org/2001/XMLSchema#integer">2003</hasYear>
    </owl:NamedIndividual>
    


    <!-- http://purl.obolibrary.org/obo/esmo.owl#Chin04 -->

    <owl:NamedIndividual rdf:about="http://purl.obolibrary.org/obo/esmo.owl#Chin04">
        <rdf:type rdf:resource="http://purl.obolibrary.org/obo/esmo.owl#Fish_population"/>
        <hasAbundance rdf:datatype="http://www.w3.org/2001/XMLSchema#double">57974.43614</hasAbundance>
        <hasYear rdf:datatype="http://www.w3.org/2001/XMLSchema#integer">2004</hasYear>
    </owl:NamedIndividual>
    


    <!-- http://purl.obolibrary.org/obo/esmo.owl#Chin05 -->

    <owl:NamedIndividual rdf:about="http://purl.obolibrary.org/obo/esmo.owl#Chin05">
        <rdf:type rdf:resource="http://purl.obolibrary.org/obo/esmo.owl#Fish_population"/>
        <hasAbundance rdf:datatype="http://www.w3.org/2001/XMLSchema#double">52715.09282</hasAbundance>
        <hasYear rdf:datatype="http://www.w3.org/2001/XMLSchema#integer">2005</hasYear>
    </owl:NamedIndividual>
    


    <!-- http://purl.obolibrary.org/obo/esmo.owl#Chin06 -->

    <owl:NamedIndividual rdf:about="http://purl.obolibrary.org/obo/esmo.owl#Chin06">
        <rdf:type rdf:resource="http://purl.obolibrary.org/obo/esmo.owl#Fish_population"/>
        <hasAbundance rdf:datatype="http://www.w3.org/2001/XMLSchema#double">69591.42064</hasAbundance>
        <hasYear rdf:datatype="http://www.w3.org/2001/XMLSchema#integer">2006</hasYear>
    </owl:NamedIndividual>
    


    <!-- http://purl.obolibrary.org/obo/esmo.owl#Chin07 -->

    <owl:NamedIndividual rdf:about="http://purl.obolibrary.org/obo/esmo.owl#Chin07">
        <rdf:type rdf:resource="http://purl.obolibrary.org/obo/esmo.owl#Fish_population"/>
        <hasAbundance rdf:datatype="http://www.w3.org/2001/XMLSchema#double">47915.13832</hasAbundance>
        <hasYear rdf:datatype="http://www.w3.org/2001/XMLSchema#integer">2007</hasYear>
    </owl:NamedIndividual>
    


    <!-- http://purl.obolibrary.org/obo/esmo.owl#Chin08 -->

    <owl:NamedIndividual rdf:about="http://purl.obolibrary.org/obo/esmo.owl#Chin08">
        <rdf:type rdf:resource="http://purl.obolibrary.org/obo/esmo.owl#Fish_population"/>
        <hasAbundance rdf:datatype="http://www.w3.org/2001/XMLSchema#double">46286.44842</hasAbundance>
        <hasYear rdf:datatype="http://www.w3.org/2001/XMLSchema#integer">2008</hasYear>
    </owl:NamedIndividual>
    


    <!-- http://purl.obolibrary.org/obo/esmo.owl#Chin09 -->

    <owl:NamedIndividual rdf:about="http://purl.obolibrary.org/obo/esmo.owl#Chin09">
        <rdf:type rdf:resource="http://purl.obolibrary.org/obo/esmo.owl#Fish_population"/>
        <hasAbundance rdf:datatype="http://www.w3.org/2001/XMLSchema#double">49749.82983</hasAbundance>
        <hasYear rdf:datatype="http://www.w3.org/2001/XMLSchema#integer">2009</hasYear>
    </owl:NamedIndividual>
    


    <!-- http://purl.obolibrary.org/obo/esmo.owl#Chin10 -->

    <owl:NamedIndividual rdf:about="http://purl.obolibrary.org/obo/esmo.owl#Chin10">
        <rdf:type rdf:resource="http://purl.obolibrary.org/obo/esmo.owl#Fish_population"/>
        <hasAbundance rdf:datatype="http://www.w3.org/2001/XMLSchema#double">52486.05582</hasAbundance>
        <hasYear rdf:datatype="http://www.w3.org/2001/XMLSchema#integer">2010</hasYear>
    </owl:NamedIndividual>
    


    <!-- http://purl.obolibrary.org/obo/esmo.owl#Chin11 -->

    <owl:NamedIndividual rdf:about="http://purl.obolibrary.org/obo/esmo.owl#Chin11">
        <rdf:type rdf:resource="http://purl.obolibrary.org/obo/esmo.owl#Fish_population"/>
        <hasAbundance rdf:datatype="http://www.w3.org/2001/XMLSchema#double">43185.58947</hasAbundance>
        <hasYear rdf:datatype="http://www.w3.org/2001/XMLSchema#integer">2011</hasYear>
    </owl:NamedIndividual>
    


    <!-- http://purl.obolibrary.org/obo/esmo.owl#Chin12 -->

    <owl:NamedIndividual rdf:about="http://purl.obolibrary.org/obo/esmo.owl#Chin12">
        <rdf:type rdf:resource="http://purl.obolibrary.org/obo/esmo.owl#Fish_population"/>
        <hasAbundance rdf:datatype="http://www.w3.org/2001/XMLSchema#double">31571.89075</hasAbundance>
        <hasYear rdf:datatype="http://www.w3.org/2001/XMLSchema#integer">2012</hasYear>
    </owl:NamedIndividual>
    


    <!-- http://purl.obolibrary.org/obo/esmo.owl#Chin13 -->

    <owl:NamedIndividual rdf:about="http://purl.obolibrary.org/obo/esmo.owl#Chin13">
        <rdf:type rdf:resource="http://purl.obolibrary.org/obo/esmo.owl#Fish_population"/>
        <hasAbundance rdf:datatype="http://www.w3.org/2001/XMLSchema#double">45522.46667</hasAbundance>
        <hasYear rdf:datatype="http://www.w3.org/2001/XMLSchema#integer">2013</hasYear>
    </owl:NamedIndividual>
    


    <!-- http://purl.obolibrary.org/obo/esmo.owl#Chin14 -->

    <owl:NamedIndividual rdf:about="http://purl.obolibrary.org/obo/esmo.owl#Chin14">
        <rdf:type rdf:resource="http://purl.obolibrary.org/obo/esmo.owl#Fish_population"/>
        <hasAbundance rdf:datatype="http://www.w3.org/2001/XMLSchema#double">46031.24747</hasAbundance>
        <hasYear rdf:datatype="http://www.w3.org/2001/XMLSchema#integer">2014</hasYear>
    </owl:NamedIndividual>
    


    <!-- http://purl.obolibrary.org/obo/esmo.owl#Chin15 -->

    <owl:NamedIndividual rdf:about="http://purl.obolibrary.org/obo/esmo.owl#Chin15">
        <rdf:type rdf:resource="http://purl.obolibrary.org/obo/esmo.owl#Fish_population"/>
        <hasAbundance rdf:datatype="http://www.w3.org/2001/XMLSchema#double">69967.76381</hasAbundance>
        <hasYear rdf:datatype="http://www.w3.org/2001/XMLSchema#integer">2015</hasYear>
    </owl:NamedIndividual>
    


    <!-- http://purl.obolibrary.org/obo/esmo.owl#Chin16 -->

    <owl:NamedIndividual rdf:about="http://purl.obolibrary.org/obo/esmo.owl#Chin16">
        <rdf:type rdf:resource="http://purl.obolibrary.org/obo/esmo.owl#Fish_population"/>
        <hasAbundance rdf:datatype="http://www.w3.org/2001/XMLSchema#double">49724.60707</hasAbundance>
        <hasYear rdf:datatype="http://www.w3.org/2001/XMLSchema#integer">2016</hasYear>
    </owl:NamedIndividual>
    


    <!-- http://purl.obolibrary.org/obo/esmo.owl#Chin17 -->

    <owl:NamedIndividual rdf:about="http://purl.obolibrary.org/obo/esmo.owl#Chin17">
        <rdf:type rdf:resource="http://purl.obolibrary.org/obo/esmo.owl#Fish_population"/>
        <hasAbundance rdf:datatype="http://www.w3.org/2001/XMLSchema#double">31383.07576</hasAbundance>
        <hasYear rdf:datatype="http://www.w3.org/2001/XMLSchema#integer">2017</hasYear>
    </owl:NamedIndividual>
    


    <!-- http://purl.obolibrary.org/obo/esmo.owl#Chin18 -->

    <owl:NamedIndividual rdf:about="http://purl.obolibrary.org/obo/esmo.owl#Chin18">
        <rdf:type rdf:resource="http://purl.obolibrary.org/obo/esmo.owl#Fish_population"/>
        <hasAbundance rdf:datatype="http://www.w3.org/2001/XMLSchema#double">19946.05556</hasAbundance>
        <hasYear rdf:datatype="http://www.w3.org/2001/XMLSchema#integer">2018</hasYear>
    </owl:NamedIndividual>
    


    <!-- http://purl.obolibrary.org/obo/esmo.owl#Chin19 -->

    <owl:NamedIndividual rdf:about="http://purl.obolibrary.org/obo/esmo.owl#Chin19">
        <rdf:type rdf:resource="http://purl.obolibrary.org/obo/esmo.owl#Fish_population"/>
        <hasAbundance rdf:datatype="http://www.w3.org/2001/XMLSchema#double">686.0</hasAbundance>
        <hasYear rdf:datatype="http://www.w3.org/2001/XMLSchema#integer">2019</hasYear>
    </owl:NamedIndividual>
    


    <!-- http://purl.obolibrary.org/obo/esmo.owl#Chin20 -->

    <owl:NamedIndividual rdf:about="http://purl.obolibrary.org/obo/esmo.owl#Chin20">
        <rdf:type rdf:resource="http://purl.obolibrary.org/obo/esmo.owl#Fish_population"/>
        <hasAbundance rdf:datatype="http://www.w3.org/2001/XMLSchema#double">1922.0</hasAbundance>
        <hasYear rdf:datatype="http://www.w3.org/2001/XMLSchema#integer">2020</hasYear>
    </owl:NamedIndividual>
    


    <!-- http://purl.obolibrary.org/obo/esmo.owl#Chin21 -->

    <owl:NamedIndividual rdf:about="http://purl.obolibrary.org/obo/esmo.owl#Chin21">
        <rdf:type rdf:resource="http://purl.obolibrary.org/obo/esmo.owl#Fish_population"/>
        <hasAbundance rdf:datatype="http://www.w3.org/2001/XMLSchema#double">0.0</hasAbundance>
        <hasYear rdf:datatype="http://www.w3.org/2001/XMLSchema#integer">2021</hasYear>
    </owl:NamedIndividual>
    


    <!-- http://purl.obolibrary.org/obo/esmo.owl#Chin97 -->

    <owl:NamedIndividual rdf:about="http://purl.obolibrary.org/obo/esmo.owl#Chin97">
        <rdf:type rdf:resource="http://purl.obolibrary.org/obo/esmo.owl#Fish_population"/>
        <hasAbundance rdf:datatype="http://www.w3.org/2001/XMLSchema#double">nan</hasAbundance>
        <hasYear rdf:datatype="http://www.w3.org/2001/XMLSchema#integer">1997</hasYear>
    </owl:NamedIndividual>
    


    <!-- http://purl.obolibrary.org/obo/esmo.owl#Chin98 -->

    <owl:NamedIndividual rdf:about="http://purl.obolibrary.org/obo/esmo.owl#Chin98">
        <rdf:type rdf:resource="http://purl.obolibrary.org/obo/esmo.owl#Fish_population"/>
        <hasAbundance rdf:datatype="http://www.w3.org/2001/XMLSchema#double">nan</hasAbundance>
        <hasYear rdf:datatype="http://www.w3.org/2001/XMLSchema#integer">1998</hasYear>
    </owl:NamedIndividual>
    


    <!-- http://purl.obolibrary.org/obo/esmo.owl#Chin99 -->

    <owl:NamedIndividual rdf:about="http://purl.obolibrary.org/obo/esmo.owl#Chin99">
        <rdf:type rdf:resource="http://purl.obolibrary.org/obo/esmo.owl#Fish_population"/>
        <hasAbundance rdf:datatype="http://www.w3.org/2001/XMLSchema#double">54575.67143</hasAbundance>
        <hasYear rdf:datatype="http://www.w3.org/2001/XMLSchema#integer">1999</hasYear>
    </owl:NamedIndividual>
    


    <!-- http://purl.obolibrary.org/obo/esmo.owl#ChinC00 -->

    <owl:NamedIndividual rdf:about="http://purl.obolibrary.org/obo/esmo.owl#ChinC00">
        <rdf:type rdf:resource="http://purl.obolibrary.org/obo/esmo.owl#Wildcaught_fish"/>
        <has_quality rdf:resource="http://purl.obolibrary.org/obo/esmo.owl#WholeSale00"/>
        <hasCount rdf:datatype="http://www.w3.org/2001/XMLSchema#double">72581.0</hasCount>
        <hasYear rdf:datatype="http://www.w3.org/2001/XMLSchema#integer">2000</hasYear>
    </owl:NamedIndividual>
    


    <!-- http://purl.obolibrary.org/obo/esmo.owl#ChinC01 -->

    <owl:NamedIndividual rdf:about="http://purl.obolibrary.org/obo/esmo.owl#ChinC01">
        <rdf:type rdf:resource="http://purl.obolibrary.org/obo/esmo.owl#Wildcaught_fish"/>
        <has_quality rdf:resource="http://purl.obolibrary.org/obo/esmo.owl#WholeSale01"/>
        <hasCount rdf:datatype="http://www.w3.org/2001/XMLSchema#double">102048.0</hasCount>
        <hasYear rdf:datatype="http://www.w3.org/2001/XMLSchema#integer">2001</hasYear>
    </owl:NamedIndividual>
    


    <!-- http://purl.obolibrary.org/obo/esmo.owl#ChinC02 -->

    <owl:NamedIndividual rdf:about="http://purl.obolibrary.org/obo/esmo.owl#ChinC02">
        <rdf:type rdf:resource="http://purl.obolibrary.org/obo/esmo.owl#Wildcaught_fish"/>
        <has_quality rdf:resource="http://purl.obolibrary.org/obo/esmo.owl#WholeSale02"/>
        <hasCount rdf:datatype="http://www.w3.org/2001/XMLSchema#double">261938.0</hasCount>
        <hasYear rdf:datatype="http://www.w3.org/2001/XMLSchema#integer">2002</hasYear>
    </owl:NamedIndividual>
    


    <!-- http://purl.obolibrary.org/obo/esmo.owl#ChinC03 -->

    <owl:NamedIndividual rdf:about="http://purl.obolibrary.org/obo/esmo.owl#ChinC03">
        <rdf:type rdf:resource="http://purl.obolibrary.org/obo/esmo.owl#Wildcaught_fish"/>
        <has_quality rdf:resource="http://purl.obolibrary.org/obo/esmo.owl#WholeSale03"/>
        <hasCount rdf:datatype="http://www.w3.org/2001/XMLSchema#double">326606.0</hasCount>
        <hasYear rdf:datatype="http://www.w3.org/2001/XMLSchema#integer">2003</hasYear>
    </owl:NamedIndividual>
    


    <!-- http://purl.obolibrary.org/obo/esmo.owl#ChinC04 -->

    <owl:NamedIndividual rdf:about="http://purl.obolibrary.org/obo/esmo.owl#ChinC04">
        <rdf:type rdf:resource="http://purl.obolibrary.org/obo/esmo.owl#Wildcaught_fish"/>
        <has_quality rdf:resource="http://purl.obolibrary.org/obo/esmo.owl#WholeSale04"/>
        <hasCount rdf:datatype="http://www.w3.org/2001/XMLSchema#double">376769.0</hasCount>
        <hasYear rdf:datatype="http://www.w3.org/2001/XMLSchema#integer">2004</hasYear>
    </owl:NamedIndividual>
    


    <!-- http://purl.obolibrary.org/obo/esmo.owl#ChinC05 -->

    <owl:NamedIndividual rdf:about="http://purl.obolibrary.org/obo/esmo.owl#ChinC05">
        <rdf:type rdf:resource="http://purl.obolibrary.org/obo/esmo.owl#Wildcaught_fish"/>
        <has_quality rdf:resource="http://purl.obolibrary.org/obo/esmo.owl#WholeSale05"/>
        <hasCount rdf:datatype="http://www.w3.org/2001/XMLSchema#double">330606.0001</hasCount>
        <hasYear rdf:datatype="http://www.w3.org/2001/XMLSchema#integer">2005</hasYear>
    </owl:NamedIndividual>
    


    <!-- http://purl.obolibrary.org/obo/esmo.owl#ChinC06 -->

    <owl:NamedIndividual rdf:about="http://purl.obolibrary.org/obo/esmo.owl#ChinC06">
        <rdf:type rdf:resource="http://purl.obolibrary.org/obo/esmo.owl#Wildcaught_fish"/>
        <has_quality rdf:resource="http://purl.obolibrary.org/obo/esmo.owl#WholeSale06"/>
        <hasCount rdf:datatype="http://www.w3.org/2001/XMLSchema#double">274170.0</hasCount>
        <hasYear rdf:datatype="http://www.w3.org/2001/XMLSchema#integer">2006</hasYear>
    </owl:NamedIndividual>
    


    <!-- http://purl.obolibrary.org/obo/esmo.owl#ChinC07 -->

    <owl:NamedIndividual rdf:about="http://purl.obolibrary.org/obo/esmo.owl#ChinC07">
        <rdf:type rdf:resource="http://purl.obolibrary.org/obo/esmo.owl#Wildcaught_fish"/>
        <has_quality rdf:resource="http://purl.obolibrary.org/obo/esmo.owl#WholeSale07"/>
        <hasCount rdf:datatype="http://www.w3.org/2001/XMLSchema#double">193289.0</hasCount>
        <hasYear rdf:datatype="http://www.w3.org/2001/XMLSchema#integer">2007</hasYear>
    </owl:NamedIndividual>
    


    <!-- http://purl.obolibrary.org/obo/esmo.owl#ChinC08 -->

    <owl:NamedIndividual rdf:about="http://purl.obolibrary.org/obo/esmo.owl#ChinC08">
        <rdf:type rdf:resource="http://purl.obolibrary.org/obo/esmo.owl#Wildcaught_fish"/>
        <has_quality rdf:resource="http://purl.obolibrary.org/obo/esmo.owl#WholeSale08"/>
        <hasCount rdf:datatype="http://www.w3.org/2001/XMLSchema#double">152176.0</hasCount>
        <hasYear rdf:datatype="http://www.w3.org/2001/XMLSchema#integer">2008</hasYear>
    </owl:NamedIndividual>
    


    <!-- http://purl.obolibrary.org/obo/esmo.owl#ChinC09 -->

    <owl:NamedIndividual rdf:about="http://purl.obolibrary.org/obo/esmo.owl#ChinC09">
        <rdf:type rdf:resource="http://purl.obolibrary.org/obo/esmo.owl#Wildcaught_fish"/>
        <has_quality rdf:resource="http://purl.obolibrary.org/obo/esmo.owl#WholeSale09"/>
        <hasCount rdf:datatype="http://www.w3.org/2001/XMLSchema#double">138064.0</hasCount>
        <hasYear rdf:datatype="http://www.w3.org/2001/XMLSchema#integer">2009</hasYear>
    </owl:NamedIndividual>
    


    <!-- http://purl.obolibrary.org/obo/esmo.owl#ChinC10 -->

    <owl:NamedIndividual rdf:about="http://purl.obolibrary.org/obo/esmo.owl#ChinC10">
        <rdf:type rdf:resource="http://purl.obolibrary.org/obo/esmo.owl#Wildcaught_fish"/>
        <has_quality rdf:resource="http://purl.obolibrary.org/obo/esmo.owl#WholeSale10"/>
        <hasCount rdf:datatype="http://www.w3.org/2001/XMLSchema#double">174981.0</hasCount>
        <hasYear rdf:datatype="http://www.w3.org/2001/XMLSchema#integer">2010</hasYear>
    </owl:NamedIndividual>
    


    <!-- http://purl.obolibrary.org/obo/esmo.owl#ChinC11 -->

    <owl:NamedIndividual rdf:about="http://purl.obolibrary.org/obo/esmo.owl#ChinC11">
        <rdf:type rdf:resource="http://purl.obolibrary.org/obo/esmo.owl#Wildcaught_fish"/>
        <has_quality rdf:resource="http://purl.obolibrary.org/obo/esmo.owl#WholeSale11"/>
        <hasCount rdf:datatype="http://www.w3.org/2001/XMLSchema#double">227292.0</hasCount>
        <hasYear rdf:datatype="http://www.w3.org/2001/XMLSchema#integer">2011</hasYear>
    </owl:NamedIndividual>
    


    <!-- http://purl.obolibrary.org/obo/esmo.owl#ChinC12 -->

    <owl:NamedIndividual rdf:about="http://purl.obolibrary.org/obo/esmo.owl#ChinC12">
        <rdf:type rdf:resource="http://purl.obolibrary.org/obo/esmo.owl#Wildcaught_fish"/>
        <has_quality rdf:resource="http://purl.obolibrary.org/obo/esmo.owl#WholeSale12"/>
        <hasCount rdf:datatype="http://www.w3.org/2001/XMLSchema#double">154506.0</hasCount>
        <hasYear rdf:datatype="http://www.w3.org/2001/XMLSchema#integer">2012</hasYear>
    </owl:NamedIndividual>
    


    <!-- http://purl.obolibrary.org/obo/esmo.owl#ChinC13 -->

    <owl:NamedIndividual rdf:about="http://purl.obolibrary.org/obo/esmo.owl#ChinC13">
        <rdf:type rdf:resource="http://purl.obolibrary.org/obo/esmo.owl#Wildcaught_fish"/>
        <has_quality rdf:resource="http://purl.obolibrary.org/obo/esmo.owl#WholeSale13"/>
        <hasCount rdf:datatype="http://www.w3.org/2001/XMLSchema#double">119619.0</hasCount>
        <hasYear rdf:datatype="http://www.w3.org/2001/XMLSchema#integer">2013</hasYear>
    </owl:NamedIndividual>
    


    <!-- http://purl.obolibrary.org/obo/esmo.owl#ChinC14 -->

    <owl:NamedIndividual rdf:about="http://purl.obolibrary.org/obo/esmo.owl#ChinC14">
        <rdf:type rdf:resource="http://purl.obolibrary.org/obo/esmo.owl#Wildcaught_fish"/>
        <has_quality rdf:resource="http://purl.obolibrary.org/obo/esmo.owl#WholeSale14"/>
        <hasCount rdf:datatype="http://www.w3.org/2001/XMLSchema#double">310649.0</hasCount>
        <hasYear rdf:datatype="http://www.w3.org/2001/XMLSchema#integer">2014</hasYear>
    </owl:NamedIndividual>
    


    <!-- http://purl.obolibrary.org/obo/esmo.owl#ChinC15 -->

    <owl:NamedIndividual rdf:about="http://purl.obolibrary.org/obo/esmo.owl#ChinC15">
        <rdf:type rdf:resource="http://purl.obolibrary.org/obo/esmo.owl#Wildcaught_fish"/>
        <has_quality rdf:resource="http://purl.obolibrary.org/obo/esmo.owl#WholeSale15"/>
        <hasCount rdf:datatype="http://www.w3.org/2001/XMLSchema#double">177568.0</hasCount>
        <hasYear rdf:datatype="http://www.w3.org/2001/XMLSchema#integer">2015</hasYear>
    </owl:NamedIndividual>
    


    <!-- http://purl.obolibrary.org/obo/esmo.owl#ChinC16 -->

    <owl:NamedIndividual rdf:about="http://purl.obolibrary.org/obo/esmo.owl#ChinC16">
        <rdf:type rdf:resource="http://purl.obolibrary.org/obo/esmo.owl#Wildcaught_fish"/>
        <has_quality rdf:resource="http://purl.obolibrary.org/obo/esmo.owl#WholeSale16"/>
        <hasCount rdf:datatype="http://www.w3.org/2001/XMLSchema#double">207932.0</hasCount>
        <hasYear rdf:datatype="http://www.w3.org/2001/XMLSchema#integer">2016</hasYear>
    </owl:NamedIndividual>
    


    <!-- http://purl.obolibrary.org/obo/esmo.owl#ChinC17 -->

    <owl:NamedIndividual rdf:about="http://purl.obolibrary.org/obo/esmo.owl#ChinC17">
        <rdf:type rdf:resource="http://purl.obolibrary.org/obo/esmo.owl#Wildcaught_fish"/>
        <has_quality rdf:resource="http://purl.obolibrary.org/obo/esmo.owl#WholeSale17"/>
        <hasCount rdf:datatype="http://www.w3.org/2001/XMLSchema#double">179413.0</hasCount>
        <hasYear rdf:datatype="http://www.w3.org/2001/XMLSchema#integer">2017</hasYear>
    </owl:NamedIndividual>
    


    <!-- http://purl.obolibrary.org/obo/esmo.owl#ChinC18 -->

    <owl:NamedIndividual rdf:about="http://purl.obolibrary.org/obo/esmo.owl#ChinC18">
        <rdf:type rdf:resource="http://purl.obolibrary.org/obo/esmo.owl#Wildcaught_fish"/>
        <has_quality rdf:resource="http://purl.obolibrary.org/obo/esmo.owl#WholeSale18"/>
        <hasCount rdf:datatype="http://www.w3.org/2001/XMLSchema#double">116051.0</hasCount>
        <hasYear rdf:datatype="http://www.w3.org/2001/XMLSchema#integer">2018</hasYear>
    </owl:NamedIndividual>
    


    <!-- http://purl.obolibrary.org/obo/esmo.owl#ChinC19 -->

    <owl:NamedIndividual rdf:about="http://purl.obolibrary.org/obo/esmo.owl#ChinC19">
        <rdf:type rdf:resource="http://purl.obolibrary.org/obo/esmo.owl#Wildcaught_fish"/>
        <has_quality rdf:resource="http://purl.obolibrary.org/obo/esmo.owl#WholeSale19"/>
        <hasCount rdf:datatype="http://www.w3.org/2001/XMLSchema#double">117593.0</hasCount>
        <hasYear rdf:datatype="http://www.w3.org/2001/XMLSchema#integer">2019</hasYear>
    </owl:NamedIndividual>
    


    <!-- http://purl.obolibrary.org/obo/esmo.owl#ChinC20 -->

    <owl:NamedIndividual rdf:about="http://purl.obolibrary.org/obo/esmo.owl#ChinC20">
        <rdf:type rdf:resource="http://purl.obolibrary.org/obo/esmo.owl#Wildcaught_fish"/>
        <has_quality rdf:resource="http://purl.obolibrary.org/obo/esmo.owl#WholeSale20"/>
        <hasCount rdf:datatype="http://www.w3.org/2001/XMLSchema#double">88414.0</hasCount>
        <hasYear rdf:datatype="http://www.w3.org/2001/XMLSchema#integer">2020</hasYear>
    </owl:NamedIndividual>
    


    <!-- http://purl.obolibrary.org/obo/esmo.owl#ChinC21 -->

    <owl:NamedIndividual rdf:about="http://purl.obolibrary.org/obo/esmo.owl#ChinC21">
        <rdf:type rdf:resource="http://purl.obolibrary.org/obo/esmo.owl#Wildcaught_fish"/>
        <has_quality rdf:resource="http://purl.obolibrary.org/obo/esmo.owl#WholeSale21"/>
        <hasCount rdf:datatype="http://www.w3.org/2001/XMLSchema#double">92385.0</hasCount>
        <hasYear rdf:datatype="http://www.w3.org/2001/XMLSchema#integer">2021</hasYear>
    </owl:NamedIndividual>
    


    <!-- http://purl.obolibrary.org/obo/esmo.owl#ChinC97 -->

    <owl:NamedIndividual rdf:about="http://purl.obolibrary.org/obo/esmo.owl#ChinC97">
        <rdf:type rdf:resource="http://purl.obolibrary.org/obo/esmo.owl#Wildcaught_fish"/>
        <has_quality rdf:resource="http://purl.obolibrary.org/obo/esmo.owl#Wholesale97"/>
        <hasCount rdf:datatype="http://www.w3.org/2001/XMLSchema#double">nan</hasCount>
        <hasYear rdf:datatype="http://www.w3.org/2001/XMLSchema#integer">1997</hasYear>
    </owl:NamedIndividual>
    


    <!-- http://purl.obolibrary.org/obo/esmo.owl#ChinC98 -->

    <owl:NamedIndividual rdf:about="http://purl.obolibrary.org/obo/esmo.owl#ChinC98">
        <rdf:type rdf:resource="http://purl.obolibrary.org/obo/esmo.owl#Wildcaught_fish"/>
        <has_quality rdf:resource="http://purl.obolibrary.org/obo/esmo.owl#Wholesale98"/>
        <hasCount rdf:datatype="http://www.w3.org/2001/XMLSchema#double">nan</hasCount>
        <hasYear rdf:datatype="http://www.w3.org/2001/XMLSchema#integer">1998</hasYear>
    </owl:NamedIndividual>
    


    <!-- http://purl.obolibrary.org/obo/esmo.owl#ChinC99 -->

    <owl:NamedIndividual rdf:about="http://purl.obolibrary.org/obo/esmo.owl#ChinC99">
        <rdf:type rdf:resource="http://purl.obolibrary.org/obo/esmo.owl#Wildcaught_fish"/>
        <has_quality rdf:resource="http://purl.obolibrary.org/obo/esmo.owl#Wholesale99"/>
        <hasCount rdf:datatype="http://www.w3.org/2001/XMLSchema#double">116815.0</hasCount>
        <hasYear rdf:datatype="http://www.w3.org/2001/XMLSchema#integer">1999</hasYear>
    </owl:NamedIndividual>
    


    <!-- http://purl.obolibrary.org/obo/esmo.owl#Orca00 -->

    <owl:NamedIndividual rdf:about="http://purl.obolibrary.org/obo/esmo.owl#Orca00">
        <rdf:type rdf:resource="http://purl.obolibrary.org/obo/esmo.owl#Whale_population"/>
        <hasAbundance rdf:datatype="http://www.w3.org/2001/XMLSchema#integer">164</hasAbundance>
        <hasYear rdf:datatype="http://www.w3.org/2001/XMLSchema#integer">2000</hasYear>
    </owl:NamedIndividual>
    


    <!-- http://purl.obolibrary.org/obo/esmo.owl#Orca01 -->

    <owl:NamedIndividual rdf:about="http://purl.obolibrary.org/obo/esmo.owl#Orca01">
        <rdf:type rdf:resource="http://purl.obolibrary.org/obo/esmo.owl#Whale_population"/>
        <hasAbundance rdf:datatype="http://www.w3.org/2001/XMLSchema#integer">156</hasAbundance>
        <hasYear rdf:datatype="http://www.w3.org/2001/XMLSchema#integer">2001</hasYear>
    </owl:NamedIndividual>
    


    <!-- http://purl.obolibrary.org/obo/esmo.owl#Orca02 -->

    <owl:NamedIndividual rdf:about="http://purl.obolibrary.org/obo/esmo.owl#Orca02">
        <rdf:type rdf:resource="http://purl.obolibrary.org/obo/esmo.owl#Whale_population"/>
        <hasAbundance rdf:datatype="http://www.w3.org/2001/XMLSchema#integer">158</hasAbundance>
        <hasYear rdf:datatype="http://www.w3.org/2001/XMLSchema#integer">2002</hasYear>
    </owl:NamedIndividual>
    


    <!-- http://purl.obolibrary.org/obo/esmo.owl#Orca03 -->

    <owl:NamedIndividual rdf:about="http://purl.obolibrary.org/obo/esmo.owl#Orca03">
        <rdf:type rdf:resource="http://purl.obolibrary.org/obo/esmo.owl#Whale_population"/>
        <hasAbundance rdf:datatype="http://www.w3.org/2001/XMLSchema#integer">164</hasAbundance>
        <hasYear rdf:datatype="http://www.w3.org/2001/XMLSchema#integer">2003</hasYear>
    </owl:NamedIndividual>
    


    <!-- http://purl.obolibrary.org/obo/esmo.owl#Orca04 -->

    <owl:NamedIndividual rdf:about="http://purl.obolibrary.org/obo/esmo.owl#Orca04">
        <rdf:type rdf:resource="http://purl.obolibrary.org/obo/esmo.owl#Whale_population"/>
        <hasAbundance rdf:datatype="http://www.w3.org/2001/XMLSchema#integer">166</hasAbundance>
        <hasYear rdf:datatype="http://www.w3.org/2001/XMLSchema#integer">2004</hasYear>
    </owl:NamedIndividual>
    


    <!-- http://purl.obolibrary.org/obo/esmo.owl#Orca05 -->

    <owl:NamedIndividual rdf:about="http://purl.obolibrary.org/obo/esmo.owl#Orca05">
        <rdf:type rdf:resource="http://purl.obolibrary.org/obo/esmo.owl#Whale_population"/>
        <hasAbundance rdf:datatype="http://www.w3.org/2001/XMLSchema#integer">176</hasAbundance>
        <hasYear rdf:datatype="http://www.w3.org/2001/XMLSchema#integer">2005</hasYear>
    </owl:NamedIndividual>
    


    <!-- http://purl.obolibrary.org/obo/esmo.owl#Orca06 -->

    <owl:NamedIndividual rdf:about="http://purl.obolibrary.org/obo/esmo.owl#Orca06">
        <rdf:type rdf:resource="http://purl.obolibrary.org/obo/esmo.owl#Whale_population"/>
        <hasAbundance rdf:datatype="http://www.w3.org/2001/XMLSchema#integer">178</hasAbundance>
        <hasYear rdf:datatype="http://www.w3.org/2001/XMLSchema#integer">2006</hasYear>
    </owl:NamedIndividual>
    


    <!-- http://purl.obolibrary.org/obo/esmo.owl#Orca07 -->

    <owl:NamedIndividual rdf:about="http://purl.obolibrary.org/obo/esmo.owl#Orca07">
        <rdf:type rdf:resource="http://purl.obolibrary.org/obo/esmo.owl#Whale_population"/>
        <hasAbundance rdf:datatype="http://www.w3.org/2001/XMLSchema#integer">172</hasAbundance>
        <hasYear rdf:datatype="http://www.w3.org/2001/XMLSchema#integer">2007</hasYear>
    </owl:NamedIndividual>
    


    <!-- http://purl.obolibrary.org/obo/esmo.owl#Orca08 -->

    <owl:NamedIndividual rdf:about="http://purl.obolibrary.org/obo/esmo.owl#Orca08">
        <rdf:type rdf:resource="http://purl.obolibrary.org/obo/esmo.owl#Whale_population"/>
        <hasAbundance rdf:datatype="http://www.w3.org/2001/XMLSchema#integer">170</hasAbundance>
        <hasYear rdf:datatype="http://www.w3.org/2001/XMLSchema#integer">2008</hasYear>
    </owl:NamedIndividual>
    


    <!-- http://purl.obolibrary.org/obo/esmo.owl#Orca09 -->

    <owl:NamedIndividual rdf:about="http://purl.obolibrary.org/obo/esmo.owl#Orca09">
        <rdf:type rdf:resource="http://purl.obolibrary.org/obo/esmo.owl#Whale_population"/>
        <hasAbundance rdf:datatype="http://www.w3.org/2001/XMLSchema#integer">170</hasAbundance>
        <hasYear rdf:datatype="http://www.w3.org/2001/XMLSchema#integer">2009</hasYear>
    </owl:NamedIndividual>
    


    <!-- http://purl.obolibrary.org/obo/esmo.owl#Orca10 -->

    <owl:NamedIndividual rdf:about="http://purl.obolibrary.org/obo/esmo.owl#Orca10">
        <rdf:type rdf:resource="http://purl.obolibrary.org/obo/esmo.owl#Whale_population"/>
        <hasAbundance rdf:datatype="http://www.w3.org/2001/XMLSchema#integer">172</hasAbundance>
        <hasYear rdf:datatype="http://www.w3.org/2001/XMLSchema#integer">2010</hasYear>
    </owl:NamedIndividual>
    


    <!-- http://purl.obolibrary.org/obo/esmo.owl#Orca11 -->

    <owl:NamedIndividual rdf:about="http://purl.obolibrary.org/obo/esmo.owl#Orca11">
        <rdf:type rdf:resource="http://purl.obolibrary.org/obo/esmo.owl#Whale_population"/>
        <hasAbundance rdf:datatype="http://www.w3.org/2001/XMLSchema#integer">174</hasAbundance>
        <hasYear rdf:datatype="http://www.w3.org/2001/XMLSchema#integer">2011</hasYear>
    </owl:NamedIndividual>
    


    <!-- http://purl.obolibrary.org/obo/esmo.owl#Orca12 -->

    <owl:NamedIndividual rdf:about="http://purl.obolibrary.org/obo/esmo.owl#Orca12">
        <rdf:type rdf:resource="http://purl.obolibrary.org/obo/esmo.owl#Whale_population"/>
        <hasAbundance rdf:datatype="http://www.w3.org/2001/XMLSchema#integer">168</hasAbundance>
        <hasYear rdf:datatype="http://www.w3.org/2001/XMLSchema#integer">2012</hasYear>
    </owl:NamedIndividual>
    


    <!-- http://purl.obolibrary.org/obo/esmo.owl#Orca13 -->

    <owl:NamedIndividual rdf:about="http://purl.obolibrary.org/obo/esmo.owl#Orca13">
        <rdf:type rdf:resource="http://purl.obolibrary.org/obo/esmo.owl#Whale_population"/>
        <hasAbundance rdf:datatype="http://www.w3.org/2001/XMLSchema#integer">165</hasAbundance>
        <hasYear rdf:datatype="http://www.w3.org/2001/XMLSchema#integer">2013</hasYear>
    </owl:NamedIndividual>
    


    <!-- http://purl.obolibrary.org/obo/esmo.owl#Orca14 -->

    <owl:NamedIndividual rdf:about="http://purl.obolibrary.org/obo/esmo.owl#Orca14">
        <rdf:type rdf:resource="http://purl.obolibrary.org/obo/esmo.owl#Whale_population"/>
        <hasAbundance rdf:datatype="http://www.w3.org/2001/XMLSchema#integer">156</hasAbundance>
        <hasYear rdf:datatype="http://www.w3.org/2001/XMLSchema#integer">2014</hasYear>
    </owl:NamedIndividual>
    


    <!-- http://purl.obolibrary.org/obo/esmo.owl#Orca15 -->

    <owl:NamedIndividual rdf:about="http://purl.obolibrary.org/obo/esmo.owl#Orca15">
        <rdf:type rdf:resource="http://purl.obolibrary.org/obo/esmo.owl#Whale_population"/>
        <hasAbundance rdf:datatype="http://www.w3.org/2001/XMLSchema#integer">162</hasAbundance>
        <hasYear rdf:datatype="http://www.w3.org/2001/XMLSchema#integer">2015</hasYear>
    </owl:NamedIndividual>
    


    <!-- http://purl.obolibrary.org/obo/esmo.owl#Orca16 -->

    <owl:NamedIndividual rdf:about="http://purl.obolibrary.org/obo/esmo.owl#Orca16">
        <rdf:type rdf:resource="http://purl.obolibrary.org/obo/esmo.owl#Whale_population"/>
        <hasAbundance rdf:datatype="http://www.w3.org/2001/XMLSchema#integer">166</hasAbundance>
        <hasYear rdf:datatype="http://www.w3.org/2001/XMLSchema#integer">2016</hasYear>
    </owl:NamedIndividual>
    


    <!-- http://purl.obolibrary.org/obo/esmo.owl#Orca17 -->

    <owl:NamedIndividual rdf:about="http://purl.obolibrary.org/obo/esmo.owl#Orca17">
        <rdf:type rdf:resource="http://purl.obolibrary.org/obo/esmo.owl#Whale_population"/>
        <hasAbundance rdf:datatype="http://www.w3.org/2001/XMLSchema#integer">154</hasAbundance>
        <hasYear rdf:datatype="http://www.w3.org/2001/XMLSchema#integer">2017</hasYear>
    </owl:NamedIndividual>
    


    <!-- http://purl.obolibrary.org/obo/esmo.owl#Orca18 -->

    <owl:NamedIndividual rdf:about="http://purl.obolibrary.org/obo/esmo.owl#Orca18">
        <rdf:type rdf:resource="http://purl.obolibrary.org/obo/esmo.owl#Whale_population"/>
        <hasAbundance rdf:datatype="http://www.w3.org/2001/XMLSchema#integer">150</hasAbundance>
        <hasYear rdf:datatype="http://www.w3.org/2001/XMLSchema#integer">2018</hasYear>
    </owl:NamedIndividual>
    


    <!-- http://purl.obolibrary.org/obo/esmo.owl#Orca19 -->

    <owl:NamedIndividual rdf:about="http://purl.obolibrary.org/obo/esmo.owl#Orca19">
        <rdf:type rdf:resource="http://purl.obolibrary.org/obo/esmo.owl#Whale_population"/>
        <hasAbundance rdf:datatype="http://www.w3.org/2001/XMLSchema#integer">146</hasAbundance>
        <hasYear rdf:datatype="http://www.w3.org/2001/XMLSchema#integer">2019</hasYear>
    </owl:NamedIndividual>
    


    <!-- http://purl.obolibrary.org/obo/esmo.owl#Orca20 -->

    <owl:NamedIndividual rdf:about="http://purl.obolibrary.org/obo/esmo.owl#Orca20">
        <rdf:type rdf:resource="http://purl.obolibrary.org/obo/esmo.owl#Whale_population"/>
        <hasAbundance rdf:datatype="http://www.w3.org/2001/XMLSchema#integer">144</hasAbundance>
        <hasYear rdf:datatype="http://www.w3.org/2001/XMLSchema#integer">2020</hasYear>
    </owl:NamedIndividual>
    


    <!-- http://purl.obolibrary.org/obo/esmo.owl#Orca21 -->

    <owl:NamedIndividual rdf:about="http://purl.obolibrary.org/obo/esmo.owl#Orca21">
        <rdf:type rdf:resource="http://purl.obolibrary.org/obo/esmo.owl#Whale_population"/>
        <hasAbundance rdf:datatype="http://www.w3.org/2001/XMLSchema#integer">148</hasAbundance>
        <hasYear rdf:datatype="http://www.w3.org/2001/XMLSchema#integer">2021</hasYear>
    </owl:NamedIndividual>
    


    <!-- http://purl.obolibrary.org/obo/esmo.owl#Orca98 -->

    <owl:NamedIndividual rdf:about="http://purl.obolibrary.org/obo/esmo.owl#Orca98">
        <rdf:type rdf:resource="http://purl.obolibrary.org/obo/esmo.owl#Whale_population"/>
        <hasAbundance rdf:datatype="http://www.w3.org/2001/XMLSchema#integer">178</hasAbundance>
        <hasYear rdf:datatype="http://www.w3.org/2001/XMLSchema#integer">1998</hasYear>
    </owl:NamedIndividual>
    


    <!-- http://purl.obolibrary.org/obo/esmo.owl#Orca99 -->

    <owl:NamedIndividual rdf:about="http://purl.obolibrary.org/obo/esmo.owl#Orca99">
        <rdf:type rdf:resource="http://purl.obolibrary.org/obo/esmo.owl#Whale_population"/>
        <hasAbundance rdf:datatype="http://www.w3.org/2001/XMLSchema#integer">170</hasAbundance>
        <hasYear rdf:datatype="http://www.w3.org/2001/XMLSchema#integer">1999</hasYear>
    </owl:NamedIndividual>
    


    <!-- http://purl.obolibrary.org/obo/esmo.owl#SalmonFleet00 -->

    <owl:NamedIndividual rdf:about="http://purl.obolibrary.org/obo/esmo.owl#SalmonFleet00">
        <rdf:type rdf:resource="http://purl.obolibrary.org/obo/esmo.owl#Fishing_fleet"/>
        <hasCount rdf:datatype="http://www.w3.org/2001/XMLSchema#double">nan</hasCount>
        <hasYear rdf:datatype="http://www.w3.org/2001/XMLSchema#integer">2000</hasYear>
    </owl:NamedIndividual>
    


    <!-- http://purl.obolibrary.org/obo/esmo.owl#SalmonFleet01 -->

    <owl:NamedIndividual rdf:about="http://purl.obolibrary.org/obo/esmo.owl#SalmonFleet01">
        <rdf:type rdf:resource="http://purl.obolibrary.org/obo/esmo.owl#Fishing_fleet"/>
        <hasCount rdf:datatype="http://www.w3.org/2001/XMLSchema#double">nan</hasCount>
        <hasYear rdf:datatype="http://www.w3.org/2001/XMLSchema#integer">2001</hasYear>
    </owl:NamedIndividual>
    


    <!-- http://purl.obolibrary.org/obo/esmo.owl#SalmonFleet02 -->

    <owl:NamedIndividual rdf:about="http://purl.obolibrary.org/obo/esmo.owl#SalmonFleet02">
        <rdf:type rdf:resource="http://purl.obolibrary.org/obo/esmo.owl#Fishing_fleet"/>
        <hasCount rdf:datatype="http://www.w3.org/2001/XMLSchema#double">nan</hasCount>
        <hasYear rdf:datatype="http://www.w3.org/2001/XMLSchema#integer">2002</hasYear>
    </owl:NamedIndividual>
    


    <!-- http://purl.obolibrary.org/obo/esmo.owl#SalmonFleet03 -->

    <owl:NamedIndividual rdf:about="http://purl.obolibrary.org/obo/esmo.owl#SalmonFleet03">
        <rdf:type rdf:resource="http://purl.obolibrary.org/obo/esmo.owl#Fishing_fleet"/>
        <hasCount rdf:datatype="http://www.w3.org/2001/XMLSchema#double">nan</hasCount>
        <hasYear rdf:datatype="http://www.w3.org/2001/XMLSchema#integer">2003</hasYear>
    </owl:NamedIndividual>
    


    <!-- http://purl.obolibrary.org/obo/esmo.owl#SalmonFleet04 -->

    <owl:NamedIndividual rdf:about="http://purl.obolibrary.org/obo/esmo.owl#SalmonFleet04">
        <rdf:type rdf:resource="http://purl.obolibrary.org/obo/esmo.owl#Fishing_fleet"/>
        <hasCount rdf:datatype="http://www.w3.org/2001/XMLSchema#double">nan</hasCount>
        <hasYear rdf:datatype="http://www.w3.org/2001/XMLSchema#integer">2004</hasYear>
    </owl:NamedIndividual>
    


    <!-- http://purl.obolibrary.org/obo/esmo.owl#SalmonFleet05 -->

    <owl:NamedIndividual rdf:about="http://purl.obolibrary.org/obo/esmo.owl#SalmonFleet05">
        <rdf:type rdf:resource="http://purl.obolibrary.org/obo/esmo.owl#Fishing_fleet"/>
        <hasCount rdf:datatype="http://www.w3.org/2001/XMLSchema#double">4593.0</hasCount>
        <hasYear rdf:datatype="http://www.w3.org/2001/XMLSchema#integer">2005</hasYear>
    </owl:NamedIndividual>
    


    <!-- http://purl.obolibrary.org/obo/esmo.owl#SalmonFleet06 -->

    <owl:NamedIndividual rdf:about="http://purl.obolibrary.org/obo/esmo.owl#SalmonFleet06">
        <rdf:type rdf:resource="http://purl.obolibrary.org/obo/esmo.owl#Fishing_fleet"/>
        <hasCount rdf:datatype="http://www.w3.org/2001/XMLSchema#double">6280.0</hasCount>
        <hasYear rdf:datatype="http://www.w3.org/2001/XMLSchema#integer">2006</hasYear>
    </owl:NamedIndividual>
    


    <!-- http://purl.obolibrary.org/obo/esmo.owl#SalmonFleet07 -->

    <owl:NamedIndividual rdf:about="http://purl.obolibrary.org/obo/esmo.owl#SalmonFleet07">
        <rdf:type rdf:resource="http://purl.obolibrary.org/obo/esmo.owl#Fishing_fleet"/>
        <hasCount rdf:datatype="http://www.w3.org/2001/XMLSchema#double">4911.0</hasCount>
        <hasYear rdf:datatype="http://www.w3.org/2001/XMLSchema#integer">2007</hasYear>
    </owl:NamedIndividual>
    


    <!-- http://purl.obolibrary.org/obo/esmo.owl#SalmonFleet08 -->

    <owl:NamedIndividual rdf:about="http://purl.obolibrary.org/obo/esmo.owl#SalmonFleet08">
        <rdf:type rdf:resource="http://purl.obolibrary.org/obo/esmo.owl#Fishing_fleet"/>
        <hasCount rdf:datatype="http://www.w3.org/2001/XMLSchema#double">3926.0</hasCount>
        <hasYear rdf:datatype="http://www.w3.org/2001/XMLSchema#integer">2008</hasYear>
    </owl:NamedIndividual>
    


    <!-- http://purl.obolibrary.org/obo/esmo.owl#SalmonFleet09 -->

    <owl:NamedIndividual rdf:about="http://purl.obolibrary.org/obo/esmo.owl#SalmonFleet09">
        <rdf:type rdf:resource="http://purl.obolibrary.org/obo/esmo.owl#Fishing_fleet"/>
        <hasCount rdf:datatype="http://www.w3.org/2001/XMLSchema#double">3705.0</hasCount>
        <hasYear rdf:datatype="http://www.w3.org/2001/XMLSchema#integer">2009</hasYear>
    </owl:NamedIndividual>
    


    <!-- http://purl.obolibrary.org/obo/esmo.owl#SalmonFleet10 -->

    <owl:NamedIndividual rdf:about="http://purl.obolibrary.org/obo/esmo.owl#SalmonFleet10">
        <rdf:type rdf:resource="http://purl.obolibrary.org/obo/esmo.owl#Fishing_fleet"/>
        <hasCount rdf:datatype="http://www.w3.org/2001/XMLSchema#double">3959.0</hasCount>
        <hasYear rdf:datatype="http://www.w3.org/2001/XMLSchema#integer">2010</hasYear>
    </owl:NamedIndividual>
    


    <!-- http://purl.obolibrary.org/obo/esmo.owl#SalmonFleet11 -->

    <owl:NamedIndividual rdf:about="http://purl.obolibrary.org/obo/esmo.owl#SalmonFleet11">
        <rdf:type rdf:resource="http://purl.obolibrary.org/obo/esmo.owl#Fishing_fleet"/>
        <hasCount rdf:datatype="http://www.w3.org/2001/XMLSchema#double">4559.0</hasCount>
        <hasYear rdf:datatype="http://www.w3.org/2001/XMLSchema#integer">2011</hasYear>
    </owl:NamedIndividual>
    


    <!-- http://purl.obolibrary.org/obo/esmo.owl#SalmonFleet12 -->

    <owl:NamedIndividual rdf:about="http://purl.obolibrary.org/obo/esmo.owl#SalmonFleet12">
        <rdf:type rdf:resource="http://purl.obolibrary.org/obo/esmo.owl#Fishing_fleet"/>
        <hasCount rdf:datatype="http://www.w3.org/2001/XMLSchema#double">4359.0</hasCount>
        <hasYear rdf:datatype="http://www.w3.org/2001/XMLSchema#integer">2012</hasYear>
    </owl:NamedIndividual>
    


    <!-- http://purl.obolibrary.org/obo/esmo.owl#SalmonFleet13 -->

    <owl:NamedIndividual rdf:about="http://purl.obolibrary.org/obo/esmo.owl#SalmonFleet13">
        <rdf:type rdf:resource="http://purl.obolibrary.org/obo/esmo.owl#Fishing_fleet"/>
        <hasCount rdf:datatype="http://www.w3.org/2001/XMLSchema#double">3312.0</hasCount>
        <hasYear rdf:datatype="http://www.w3.org/2001/XMLSchema#integer">2013</hasYear>
    </owl:NamedIndividual>
    


    <!-- http://purl.obolibrary.org/obo/esmo.owl#SalmonFleet14 -->

    <owl:NamedIndividual rdf:about="http://purl.obolibrary.org/obo/esmo.owl#SalmonFleet14">
        <rdf:type rdf:resource="http://purl.obolibrary.org/obo/esmo.owl#Fishing_fleet"/>
        <hasCount rdf:datatype="http://www.w3.org/2001/XMLSchema#double">4681.0</hasCount>
        <hasYear rdf:datatype="http://www.w3.org/2001/XMLSchema#integer">2014</hasYear>
    </owl:NamedIndividual>
    


    <!-- http://purl.obolibrary.org/obo/esmo.owl#SalmonFleet15 -->

    <owl:NamedIndividual rdf:about="http://purl.obolibrary.org/obo/esmo.owl#SalmonFleet15">
        <rdf:type rdf:resource="http://purl.obolibrary.org/obo/esmo.owl#Fishing_fleet"/>
        <hasCount rdf:datatype="http://www.w3.org/2001/XMLSchema#double">3959.0</hasCount>
        <hasYear rdf:datatype="http://www.w3.org/2001/XMLSchema#integer">2015</hasYear>
    </owl:NamedIndividual>
    


    <!-- http://purl.obolibrary.org/obo/esmo.owl#SalmonFleet16 -->

    <owl:NamedIndividual rdf:about="http://purl.obolibrary.org/obo/esmo.owl#SalmonFleet16">
        <rdf:type rdf:resource="http://purl.obolibrary.org/obo/esmo.owl#Fishing_fleet"/>
        <hasCount rdf:datatype="http://www.w3.org/2001/XMLSchema#double">4698.0</hasCount>
        <hasYear rdf:datatype="http://www.w3.org/2001/XMLSchema#integer">2016</hasYear>
    </owl:NamedIndividual>
    


    <!-- http://purl.obolibrary.org/obo/esmo.owl#SalmonFleet17 -->

    <owl:NamedIndividual rdf:about="http://purl.obolibrary.org/obo/esmo.owl#SalmonFleet17">
        <rdf:type rdf:resource="http://purl.obolibrary.org/obo/esmo.owl#Fishing_fleet"/>
        <hasCount rdf:datatype="http://www.w3.org/2001/XMLSchema#double">3266.0</hasCount>
        <hasYear rdf:datatype="http://www.w3.org/2001/XMLSchema#integer">2017</hasYear>
    </owl:NamedIndividual>
    


    <!-- http://purl.obolibrary.org/obo/esmo.owl#SalmonFleet18 -->

    <owl:NamedIndividual rdf:about="http://purl.obolibrary.org/obo/esmo.owl#SalmonFleet18">
        <rdf:type rdf:resource="http://purl.obolibrary.org/obo/esmo.owl#Fishing_fleet"/>
        <hasCount rdf:datatype="http://www.w3.org/2001/XMLSchema#double">3881.0</hasCount>
        <hasYear rdf:datatype="http://www.w3.org/2001/XMLSchema#integer">2018</hasYear>
    </owl:NamedIndividual>
    


    <!-- http://purl.obolibrary.org/obo/esmo.owl#SalmonFleet19 -->

    <owl:NamedIndividual rdf:about="http://purl.obolibrary.org/obo/esmo.owl#SalmonFleet19">
        <rdf:type rdf:resource="http://purl.obolibrary.org/obo/esmo.owl#Fishing_fleet"/>
        <hasCount rdf:datatype="http://www.w3.org/2001/XMLSchema#double">1545.0</hasCount>
        <hasYear rdf:datatype="http://www.w3.org/2001/XMLSchema#integer">2019</hasYear>
    </owl:NamedIndividual>
    


    <!-- http://purl.obolibrary.org/obo/esmo.owl#SalmonFleet20 -->

    <owl:NamedIndividual rdf:about="http://purl.obolibrary.org/obo/esmo.owl#SalmonFleet20">
        <rdf:type rdf:resource="http://purl.obolibrary.org/obo/esmo.owl#Fishing_fleet"/>
        <hasCount rdf:datatype="http://www.w3.org/2001/XMLSchema#double">2239.0</hasCount>
        <hasYear rdf:datatype="http://www.w3.org/2001/XMLSchema#integer">2020</hasYear>
    </owl:NamedIndividual>
    


    <!-- http://purl.obolibrary.org/obo/esmo.owl#SalmonFleet21 -->

    <owl:NamedIndividual rdf:about="http://purl.obolibrary.org/obo/esmo.owl#SalmonFleet21">
        <rdf:type rdf:resource="http://purl.obolibrary.org/obo/esmo.owl#Fishing_fleet"/>
        <hasCount rdf:datatype="http://www.w3.org/2001/XMLSchema#double">921.0</hasCount>
        <hasYear rdf:datatype="http://www.w3.org/2001/XMLSchema#integer">2021</hasYear>
    </owl:NamedIndividual>
    


    <!-- http://purl.obolibrary.org/obo/esmo.owl#SalmonFleet97 -->

    <owl:NamedIndividual rdf:about="http://purl.obolibrary.org/obo/esmo.owl#SalmonFleet97">
        <rdf:type rdf:resource="http://purl.obolibrary.org/obo/esmo.owl#Fishing_fleet"/>
        <hasCount rdf:datatype="http://www.w3.org/2001/XMLSchema#double">nan</hasCount>
        <hasYear rdf:datatype="http://www.w3.org/2001/XMLSchema#integer">1997</hasYear>
    </owl:NamedIndividual>
    


    <!-- http://purl.obolibrary.org/obo/esmo.owl#SalmonFleet98 -->

    <owl:NamedIndividual rdf:about="http://purl.obolibrary.org/obo/esmo.owl#SalmonFleet98">
        <rdf:type rdf:resource="http://purl.obolibrary.org/obo/esmo.owl#Fishing_fleet"/>
        <hasCount rdf:datatype="http://www.w3.org/2001/XMLSchema#double">nan</hasCount>
        <hasYear rdf:datatype="http://www.w3.org/2001/XMLSchema#integer">1998</hasYear>
    </owl:NamedIndividual>
    


    <!-- http://purl.obolibrary.org/obo/esmo.owl#SalmonFleet99 -->

    <owl:NamedIndividual rdf:about="http://purl.obolibrary.org/obo/esmo.owl#SalmonFleet99">
        <rdf:type rdf:resource="http://purl.obolibrary.org/obo/esmo.owl#Fishing_fleet"/>
        <hasCount rdf:datatype="http://www.w3.org/2001/XMLSchema#double">nan</hasCount>
        <hasYear rdf:datatype="http://www.w3.org/2001/XMLSchema#integer">1999</hasYear>
    </owl:NamedIndividual>
    


    <!-- http://purl.obolibrary.org/obo/esmo.owl#Water00 -->

    <owl:NamedIndividual rdf:about="http://purl.obolibrary.org/obo/esmo.owl#Water00">
        <rdf:type rdf:resource="http://purl.obolibrary.org/obo/esmo.owl#Clean_freshwater"/>
        <hasConcentration rdf:datatype="http://www.w3.org/2001/XMLSchema#double">0.014</hasConcentration>
        <hasYear rdf:datatype="http://www.w3.org/2001/XMLSchema#integer">2000</hasYear>
    </owl:NamedIndividual>
    


    <!-- http://purl.obolibrary.org/obo/esmo.owl#Water01 -->

    <owl:NamedIndividual rdf:about="http://purl.obolibrary.org/obo/esmo.owl#Water01">
        <rdf:type rdf:resource="http://purl.obolibrary.org/obo/esmo.owl#Clean_freshwater"/>
        <hasConcentration rdf:datatype="http://www.w3.org/2001/XMLSchema#double">0.013</hasConcentration>
        <hasYear rdf:datatype="http://www.w3.org/2001/XMLSchema#integer">2001</hasYear>
    </owl:NamedIndividual>
    


    <!-- http://purl.obolibrary.org/obo/esmo.owl#Water02 -->

    <owl:NamedIndividual rdf:about="http://purl.obolibrary.org/obo/esmo.owl#Water02">
        <rdf:type rdf:resource="http://purl.obolibrary.org/obo/esmo.owl#Clean_freshwater"/>
        <hasConcentration rdf:datatype="http://www.w3.org/2001/XMLSchema#double">0.018</hasConcentration>
        <hasYear rdf:datatype="http://www.w3.org/2001/XMLSchema#integer">2002</hasYear>
    </owl:NamedIndividual>
    


    <!-- http://purl.obolibrary.org/obo/esmo.owl#Water04 -->

    <owl:NamedIndividual rdf:about="http://purl.obolibrary.org/obo/esmo.owl#Water04">
        <rdf:type rdf:resource="http://purl.obolibrary.org/obo/esmo.owl#Clean_freshwater"/>
        <hasConcentration rdf:datatype="http://www.w3.org/2001/XMLSchema#double">0.004</hasConcentration>
        <hasYear rdf:datatype="http://www.w3.org/2001/XMLSchema#integer">2004</hasYear>
    </owl:NamedIndividual>
    


    <!-- http://purl.obolibrary.org/obo/esmo.owl#Water05 -->

    <owl:NamedIndividual rdf:about="http://purl.obolibrary.org/obo/esmo.owl#Water05">
        <rdf:type rdf:resource="http://purl.obolibrary.org/obo/esmo.owl#Clean_freshwater"/>
        <hasConcentration rdf:datatype="http://www.w3.org/2001/XMLSchema#double">0.006333333</hasConcentration>
        <hasYear rdf:datatype="http://www.w3.org/2001/XMLSchema#integer">2005</hasYear>
    </owl:NamedIndividual>
    


    <!-- http://purl.obolibrary.org/obo/esmo.owl#Water06 -->

    <owl:NamedIndividual rdf:about="http://purl.obolibrary.org/obo/esmo.owl#Water06">
        <rdf:type rdf:resource="http://purl.obolibrary.org/obo/esmo.owl#Clean_freshwater"/>
        <hasConcentration rdf:datatype="http://www.w3.org/2001/XMLSchema#double">0.006</hasConcentration>
        <hasYear rdf:datatype="http://www.w3.org/2001/XMLSchema#integer">2006</hasYear>
    </owl:NamedIndividual>
    


    <!-- http://purl.obolibrary.org/obo/esmo.owl#Water07 -->

    <owl:NamedIndividual rdf:about="http://purl.obolibrary.org/obo/esmo.owl#Water07">
        <rdf:type rdf:resource="http://purl.obolibrary.org/obo/esmo.owl#Clean_freshwater"/>
        <hasConcentration rdf:datatype="http://www.w3.org/2001/XMLSchema#double">0.009</hasConcentration>
        <hasYear rdf:datatype="http://www.w3.org/2001/XMLSchema#integer">2007</hasYear>
    </owl:NamedIndividual>
    


    <!-- http://purl.obolibrary.org/obo/esmo.owl#Water08 -->

    <owl:NamedIndividual rdf:about="http://purl.obolibrary.org/obo/esmo.owl#Water08">
        <rdf:type rdf:resource="http://purl.obolibrary.org/obo/esmo.owl#Clean_freshwater"/>
        <hasConcentration rdf:datatype="http://www.w3.org/2001/XMLSchema#double">0.016</hasConcentration>
        <hasYear rdf:datatype="http://www.w3.org/2001/XMLSchema#integer">2008</hasYear>
    </owl:NamedIndividual>
    


    <!-- http://purl.obolibrary.org/obo/esmo.owl#Water10 -->

    <owl:NamedIndividual rdf:about="http://purl.obolibrary.org/obo/esmo.owl#Water10">
        <rdf:type rdf:resource="http://purl.obolibrary.org/obo/esmo.owl#Clean_freshwater"/>
        <hasConcentration rdf:datatype="http://www.w3.org/2001/XMLSchema#double">0.00675</hasConcentration>
        <hasYear rdf:datatype="http://www.w3.org/2001/XMLSchema#integer">2010</hasYear>
    </owl:NamedIndividual>
    


    <!-- http://purl.obolibrary.org/obo/esmo.owl#Water11 -->

    <owl:NamedIndividual rdf:about="http://purl.obolibrary.org/obo/esmo.owl#Water11">
        <rdf:type rdf:resource="http://purl.obolibrary.org/obo/esmo.owl#Clean_freshwater"/>
        <hasConcentration rdf:datatype="http://www.w3.org/2001/XMLSchema#double">0.009125</hasConcentration>
        <hasYear rdf:datatype="http://www.w3.org/2001/XMLSchema#integer">2011</hasYear>
    </owl:NamedIndividual>
    


    <!-- http://purl.obolibrary.org/obo/esmo.owl#Water12 -->

    <owl:NamedIndividual rdf:about="http://purl.obolibrary.org/obo/esmo.owl#Water12">
        <rdf:type rdf:resource="http://purl.obolibrary.org/obo/esmo.owl#Clean_freshwater"/>
        <hasConcentration rdf:datatype="http://www.w3.org/2001/XMLSchema#double">0.0164875</hasConcentration>
        <hasYear rdf:datatype="http://www.w3.org/2001/XMLSchema#integer">2012</hasYear>
    </owl:NamedIndividual>
    


    <!-- http://purl.obolibrary.org/obo/esmo.owl#Water13 -->

    <owl:NamedIndividual rdf:about="http://purl.obolibrary.org/obo/esmo.owl#Water13">
        <rdf:type rdf:resource="http://purl.obolibrary.org/obo/esmo.owl#Clean_freshwater"/>
        <hasConcentration rdf:datatype="http://www.w3.org/2001/XMLSchema#double">0.0127</hasConcentration>
        <hasYear rdf:datatype="http://www.w3.org/2001/XMLSchema#integer">2013</hasYear>
    </owl:NamedIndividual>
    


    <!-- http://purl.obolibrary.org/obo/esmo.owl#Water14 -->

    <owl:NamedIndividual rdf:about="http://purl.obolibrary.org/obo/esmo.owl#Water14">
        <rdf:type rdf:resource="http://purl.obolibrary.org/obo/esmo.owl#Clean_freshwater"/>
        <hasConcentration rdf:datatype="http://www.w3.org/2001/XMLSchema#double">0.01095</hasConcentration>
        <hasYear rdf:datatype="http://www.w3.org/2001/XMLSchema#integer">2014</hasYear>
    </owl:NamedIndividual>
    


    <!-- http://purl.obolibrary.org/obo/esmo.owl#Water15 -->

    <owl:NamedIndividual rdf:about="http://purl.obolibrary.org/obo/esmo.owl#Water15">
        <rdf:type rdf:resource="http://purl.obolibrary.org/obo/esmo.owl#Clean_freshwater"/>
        <hasConcentration rdf:datatype="http://www.w3.org/2001/XMLSchema#double">0.005475</hasConcentration>
        <hasYear rdf:datatype="http://www.w3.org/2001/XMLSchema#integer">2015</hasYear>
    </owl:NamedIndividual>
    


    <!-- http://purl.obolibrary.org/obo/esmo.owl#Water16 -->

    <owl:NamedIndividual rdf:about="http://purl.obolibrary.org/obo/esmo.owl#Water16">
        <rdf:type rdf:resource="http://purl.obolibrary.org/obo/esmo.owl#Clean_freshwater"/>
        <hasConcentration rdf:datatype="http://www.w3.org/2001/XMLSchema#double">0.0072</hasConcentration>
        <hasYear rdf:datatype="http://www.w3.org/2001/XMLSchema#integer">2016</hasYear>
    </owl:NamedIndividual>
    


    <!-- http://purl.obolibrary.org/obo/esmo.owl#Water17 -->

    <owl:NamedIndividual rdf:about="http://purl.obolibrary.org/obo/esmo.owl#Water17">
        <rdf:type rdf:resource="http://purl.obolibrary.org/obo/esmo.owl#Clean_freshwater"/>
        <hasConcentration rdf:datatype="http://www.w3.org/2001/XMLSchema#double">0.012785714</hasConcentration>
        <hasYear rdf:datatype="http://www.w3.org/2001/XMLSchema#integer">2017</hasYear>
    </owl:NamedIndividual>
    


    <!-- http://purl.obolibrary.org/obo/esmo.owl#Water18 -->

    <owl:NamedIndividual rdf:about="http://purl.obolibrary.org/obo/esmo.owl#Water18">
        <rdf:type rdf:resource="http://purl.obolibrary.org/obo/esmo.owl#Clean_freshwater"/>
        <hasConcentration rdf:datatype="http://www.w3.org/2001/XMLSchema#double">0.014014286</hasConcentration>
        <hasYear rdf:datatype="http://www.w3.org/2001/XMLSchema#integer">2018</hasYear>
    </owl:NamedIndividual>
    


    <!-- http://purl.obolibrary.org/obo/esmo.owl#Water19 -->

    <owl:NamedIndividual rdf:about="http://purl.obolibrary.org/obo/esmo.owl#Water19">
        <rdf:type rdf:resource="http://purl.obolibrary.org/obo/esmo.owl#Clean_freshwater"/>
        <hasConcentration rdf:datatype="http://www.w3.org/2001/XMLSchema#double">0.006666667</hasConcentration>
        <hasYear rdf:datatype="http://www.w3.org/2001/XMLSchema#integer">2019</hasYear>
    </owl:NamedIndividual>
    


    <!-- http://purl.obolibrary.org/obo/esmo.owl#Water20 -->

    <owl:NamedIndividual rdf:about="http://purl.obolibrary.org/obo/esmo.owl#Water20">
        <rdf:type rdf:resource="http://purl.obolibrary.org/obo/esmo.owl#Clean_freshwater"/>
        <hasConcentration rdf:datatype="http://www.w3.org/2001/XMLSchema#double">0.0194</hasConcentration>
        <hasYear rdf:datatype="http://www.w3.org/2001/XMLSchema#integer">2020</hasYear>
    </owl:NamedIndividual>
    


    <!-- http://purl.obolibrary.org/obo/esmo.owl#Water87 -->

    <owl:NamedIndividual rdf:about="http://purl.obolibrary.org/obo/esmo.owl#Water87">
        <rdf:type rdf:resource="http://purl.obolibrary.org/obo/esmo.owl#Clean_freshwater"/>
        <hasConcentration rdf:datatype="http://www.w3.org/2001/XMLSchema#double">0.010333333</hasConcentration>
        <hasYear rdf:datatype="http://www.w3.org/2001/XMLSchema#integer">1987</hasYear>
    </owl:NamedIndividual>
    


    <!-- http://purl.obolibrary.org/obo/esmo.owl#Water88 -->

    <owl:NamedIndividual rdf:about="http://purl.obolibrary.org/obo/esmo.owl#Water88">
        <rdf:type rdf:resource="http://purl.obolibrary.org/obo/esmo.owl#Clean_freshwater"/>
        <hasConcentration rdf:datatype="http://www.w3.org/2001/XMLSchema#double">0.013</hasConcentration>
        <hasYear rdf:datatype="http://www.w3.org/2001/XMLSchema#integer">1988</hasYear>
    </owl:NamedIndividual>
    


    <!-- http://purl.obolibrary.org/obo/esmo.owl#Water89 -->

    <owl:NamedIndividual rdf:about="http://purl.obolibrary.org/obo/esmo.owl#Water89">
        <rdf:type rdf:resource="http://purl.obolibrary.org/obo/esmo.owl#Clean_freshwater"/>
        <hasConcentration rdf:datatype="http://www.w3.org/2001/XMLSchema#double">0.01175</hasConcentration>
        <hasYear rdf:datatype="http://www.w3.org/2001/XMLSchema#integer">1989</hasYear>
    </owl:NamedIndividual>
    


    <!-- http://purl.obolibrary.org/obo/esmo.owl#Water90 -->

    <owl:NamedIndividual rdf:about="http://purl.obolibrary.org/obo/esmo.owl#Water90">
        <rdf:type rdf:resource="http://purl.obolibrary.org/obo/esmo.owl#Clean_freshwater"/>
        <hasConcentration rdf:datatype="http://www.w3.org/2001/XMLSchema#double">0.016333333</hasConcentration>
        <hasYear rdf:datatype="http://www.w3.org/2001/XMLSchema#integer">1990</hasYear>
    </owl:NamedIndividual>
    


    <!-- http://purl.obolibrary.org/obo/esmo.owl#Water91 -->

    <owl:NamedIndividual rdf:about="http://purl.obolibrary.org/obo/esmo.owl#Water91">
        <rdf:type rdf:resource="http://purl.obolibrary.org/obo/esmo.owl#Clean_freshwater"/>
        <hasConcentration rdf:datatype="http://www.w3.org/2001/XMLSchema#double">0.009166667</hasConcentration>
        <hasYear rdf:datatype="http://www.w3.org/2001/XMLSchema#integer">1991</hasYear>
    </owl:NamedIndividual>
    


    <!-- http://purl.obolibrary.org/obo/esmo.owl#Water92 -->

    <owl:NamedIndividual rdf:about="http://purl.obolibrary.org/obo/esmo.owl#Water92">
        <rdf:type rdf:resource="http://purl.obolibrary.org/obo/esmo.owl#Clean_freshwater"/>
        <hasConcentration rdf:datatype="http://www.w3.org/2001/XMLSchema#double">0.0085</hasConcentration>
        <hasYear rdf:datatype="http://www.w3.org/2001/XMLSchema#integer">1992</hasYear>
    </owl:NamedIndividual>
    


    <!-- http://purl.obolibrary.org/obo/esmo.owl#Water93 -->

    <owl:NamedIndividual rdf:about="http://purl.obolibrary.org/obo/esmo.owl#Water93">
        <rdf:type rdf:resource="http://purl.obolibrary.org/obo/esmo.owl#Clean_freshwater"/>
        <hasConcentration rdf:datatype="http://www.w3.org/2001/XMLSchema#double">0.013</hasConcentration>
        <hasYear rdf:datatype="http://www.w3.org/2001/XMLSchema#integer">1993</hasYear>
    </owl:NamedIndividual>
    


    <!-- http://purl.obolibrary.org/obo/esmo.owl#Water94 -->

    <owl:NamedIndividual rdf:about="http://purl.obolibrary.org/obo/esmo.owl#Water94">
        <rdf:type rdf:resource="http://purl.obolibrary.org/obo/esmo.owl#Clean_freshwater"/>
        <hasConcentration rdf:datatype="http://www.w3.org/2001/XMLSchema#double">0.008</hasConcentration>
        <hasYear rdf:datatype="http://www.w3.org/2001/XMLSchema#integer">1994</hasYear>
    </owl:NamedIndividual>
    


    <!-- http://purl.obolibrary.org/obo/esmo.owl#Water95 -->

    <owl:NamedIndividual rdf:about="http://purl.obolibrary.org/obo/esmo.owl#Water95">
        <rdf:type rdf:resource="http://purl.obolibrary.org/obo/esmo.owl#Clean_freshwater"/>
        <hasConcentration rdf:datatype="http://www.w3.org/2001/XMLSchema#double">0.007</hasConcentration>
        <hasYear rdf:datatype="http://www.w3.org/2001/XMLSchema#integer">1995</hasYear>
    </owl:NamedIndividual>
    


    <!-- http://purl.obolibrary.org/obo/esmo.owl#Water96 -->

    <owl:NamedIndividual rdf:about="http://purl.obolibrary.org/obo/esmo.owl#Water96">
        <rdf:type rdf:resource="http://purl.obolibrary.org/obo/esmo.owl#Clean_freshwater"/>
        <hasConcentration rdf:datatype="http://www.w3.org/2001/XMLSchema#double">0.024</hasConcentration>
        <hasYear rdf:datatype="http://www.w3.org/2001/XMLSchema#integer">1997</hasYear>
    </owl:NamedIndividual>
    


    <!-- http://purl.obolibrary.org/obo/esmo.owl#Water97 -->

    <owl:NamedIndividual rdf:about="http://purl.obolibrary.org/obo/esmo.owl#Water97">
        <rdf:type rdf:resource="http://purl.obolibrary.org/obo/esmo.owl#Clean_freshwater"/>
        <hasConcentration rdf:datatype="http://www.w3.org/2001/XMLSchema#double">0.016</hasConcentration>
        <hasYear rdf:datatype="http://www.w3.org/2001/XMLSchema#integer">1998</hasYear>
    </owl:NamedIndividual>
    


    <!-- http://purl.obolibrary.org/obo/esmo.owl#Water98 -->

    <owl:NamedIndividual rdf:about="http://purl.obolibrary.org/obo/esmo.owl#Water98">
        <rdf:type rdf:resource="http://purl.obolibrary.org/obo/esmo.owl#Clean_freshwater"/>
        <hasConcentration rdf:datatype="http://www.w3.org/2001/XMLSchema#double">0.016</hasConcentration>
        <hasYear rdf:datatype="http://www.w3.org/2001/XMLSchema#integer">1999</hasYear>
    </owl:NamedIndividual>
    


    <!-- http://purl.obolibrary.org/obo/esmo.owl#WholeSale00 -->

    <owl:NamedIndividual rdf:about="http://purl.obolibrary.org/obo/esmo.owl#WholeSale00">
        <rdf:type rdf:resource="http://purl.obolibrary.org/obo/esmo.owl#Wholesale_value"/>
        <hasWholesaleValue rdf:datatype="http://www.w3.org/2001/XMLSchema#double">5.3</hasWholesaleValue>
        <hasYear rdf:datatype="http://www.w3.org/2001/XMLSchema#integer">2000</hasYear>
    </owl:NamedIndividual>
    


    <!-- http://purl.obolibrary.org/obo/esmo.owl#WholeSale01 -->

    <owl:NamedIndividual rdf:about="http://purl.obolibrary.org/obo/esmo.owl#WholeSale01">
        <rdf:type rdf:resource="http://purl.obolibrary.org/obo/esmo.owl#Wholesale_value"/>
        <hasWholesaleValue rdf:datatype="http://www.w3.org/2001/XMLSchema#double">5.1</hasWholesaleValue>
        <hasYear rdf:datatype="http://www.w3.org/2001/XMLSchema#integer">2001</hasYear>
    </owl:NamedIndividual>
    


    <!-- http://purl.obolibrary.org/obo/esmo.owl#WholeSale02 -->

    <owl:NamedIndividual rdf:about="http://purl.obolibrary.org/obo/esmo.owl#WholeSale02">
        <rdf:type rdf:resource="http://purl.obolibrary.org/obo/esmo.owl#Wholesale_value"/>
        <hasWholesaleValue rdf:datatype="http://www.w3.org/2001/XMLSchema#double">11.8</hasWholesaleValue>
        <hasYear rdf:datatype="http://www.w3.org/2001/XMLSchema#integer">2002</hasYear>
    </owl:NamedIndividual>
    


    <!-- http://purl.obolibrary.org/obo/esmo.owl#WholeSale03 -->

    <owl:NamedIndividual rdf:about="http://purl.obolibrary.org/obo/esmo.owl#WholeSale03">
        <rdf:type rdf:resource="http://purl.obolibrary.org/obo/esmo.owl#Wholesale_value"/>
        <hasWholesaleValue rdf:datatype="http://www.w3.org/2001/XMLSchema#double">17.3</hasWholesaleValue>
        <hasYear rdf:datatype="http://www.w3.org/2001/XMLSchema#integer">2003</hasYear>
    </owl:NamedIndividual>
    


    <!-- http://purl.obolibrary.org/obo/esmo.owl#WholeSale04 -->

    <owl:NamedIndividual rdf:about="http://purl.obolibrary.org/obo/esmo.owl#WholeSale04">
        <rdf:type rdf:resource="http://purl.obolibrary.org/obo/esmo.owl#Wholesale_value"/>
        <hasWholesaleValue rdf:datatype="http://www.w3.org/2001/XMLSchema#double">26.9</hasWholesaleValue>
        <hasYear rdf:datatype="http://www.w3.org/2001/XMLSchema#integer">2004</hasYear>
    </owl:NamedIndividual>
    


    <!-- http://purl.obolibrary.org/obo/esmo.owl#WholeSale05 -->

    <owl:NamedIndividual rdf:about="http://purl.obolibrary.org/obo/esmo.owl#WholeSale05">
        <rdf:type rdf:resource="http://purl.obolibrary.org/obo/esmo.owl#Wholesale_value"/>
        <hasWholesaleValue rdf:datatype="http://www.w3.org/2001/XMLSchema#double">24.9</hasWholesaleValue>
        <hasYear rdf:datatype="http://www.w3.org/2001/XMLSchema#integer">2005</hasYear>
    </owl:NamedIndividual>
    


    <!-- http://purl.obolibrary.org/obo/esmo.owl#WholeSale06 -->

    <owl:NamedIndividual rdf:about="http://purl.obolibrary.org/obo/esmo.owl#WholeSale06">
        <rdf:type rdf:resource="http://purl.obolibrary.org/obo/esmo.owl#Wholesale_value"/>
        <hasWholesaleValue rdf:datatype="http://www.w3.org/2001/XMLSchema#double">29.2</hasWholesaleValue>
        <hasYear rdf:datatype="http://www.w3.org/2001/XMLSchema#integer">2006</hasYear>
    </owl:NamedIndividual>
    


    <!-- http://purl.obolibrary.org/obo/esmo.owl#WholeSale07 -->

    <owl:NamedIndividual rdf:about="http://purl.obolibrary.org/obo/esmo.owl#WholeSale07">
        <rdf:type rdf:resource="http://purl.obolibrary.org/obo/esmo.owl#Wholesale_value"/>
        <hasWholesaleValue rdf:datatype="http://www.w3.org/2001/XMLSchema#double">23.8</hasWholesaleValue>
        <hasYear rdf:datatype="http://www.w3.org/2001/XMLSchema#integer">2007</hasYear>
    </owl:NamedIndividual>
    


    <!-- http://purl.obolibrary.org/obo/esmo.owl#WholeSale08 -->

    <owl:NamedIndividual rdf:about="http://purl.obolibrary.org/obo/esmo.owl#WholeSale08">
        <rdf:type rdf:resource="http://purl.obolibrary.org/obo/esmo.owl#Wholesale_value"/>
        <hasWholesaleValue rdf:datatype="http://www.w3.org/2001/XMLSchema#double">18.4</hasWholesaleValue>
        <hasYear rdf:datatype="http://www.w3.org/2001/XMLSchema#integer">2008</hasYear>
    </owl:NamedIndividual>
    


    <!-- http://purl.obolibrary.org/obo/esmo.owl#WholeSale09 -->

    <owl:NamedIndividual rdf:about="http://purl.obolibrary.org/obo/esmo.owl#WholeSale09">
        <rdf:type rdf:resource="http://purl.obolibrary.org/obo/esmo.owl#Wholesale_value"/>
        <hasWholesaleValue rdf:datatype="http://www.w3.org/2001/XMLSchema#double">16.1</hasWholesaleValue>
        <hasYear rdf:datatype="http://www.w3.org/2001/XMLSchema#integer">2009</hasYear>
    </owl:NamedIndividual>
    


    <!-- http://purl.obolibrary.org/obo/esmo.owl#WholeSale10 -->

    <owl:NamedIndividual rdf:about="http://purl.obolibrary.org/obo/esmo.owl#WholeSale10">
        <rdf:type rdf:resource="http://purl.obolibrary.org/obo/esmo.owl#Wholesale_value"/>
        <hasWholesaleValue rdf:datatype="http://www.w3.org/2001/XMLSchema#double">18.5</hasWholesaleValue>
        <hasYear rdf:datatype="http://www.w3.org/2001/XMLSchema#integer">2010</hasYear>
    </owl:NamedIndividual>
    


    <!-- http://purl.obolibrary.org/obo/esmo.owl#WholeSale11 -->

    <owl:NamedIndividual rdf:about="http://purl.obolibrary.org/obo/esmo.owl#WholeSale11">
        <rdf:type rdf:resource="http://purl.obolibrary.org/obo/esmo.owl#Wholesale_value"/>
        <hasWholesaleValue rdf:datatype="http://www.w3.org/2001/XMLSchema#double">21.4</hasWholesaleValue>
        <hasYear rdf:datatype="http://www.w3.org/2001/XMLSchema#integer">2011</hasYear>
    </owl:NamedIndividual>
    


    <!-- http://purl.obolibrary.org/obo/esmo.owl#WholeSale12 -->

    <owl:NamedIndividual rdf:about="http://purl.obolibrary.org/obo/esmo.owl#WholeSale12">
        <rdf:type rdf:resource="http://purl.obolibrary.org/obo/esmo.owl#Wholesale_value"/>
        <hasWholesaleValue rdf:datatype="http://www.w3.org/2001/XMLSchema#double">18.99999998</hasWholesaleValue>
        <hasYear rdf:datatype="http://www.w3.org/2001/XMLSchema#integer">2012</hasYear>
    </owl:NamedIndividual>
    


    <!-- http://purl.obolibrary.org/obo/esmo.owl#WholeSale13 -->

    <owl:NamedIndividual rdf:about="http://purl.obolibrary.org/obo/esmo.owl#WholeSale13">
        <rdf:type rdf:resource="http://purl.obolibrary.org/obo/esmo.owl#Wholesale_value"/>
        <hasWholesaleValue rdf:datatype="http://www.w3.org/2001/XMLSchema#double">12.3</hasWholesaleValue>
        <hasYear rdf:datatype="http://www.w3.org/2001/XMLSchema#integer">2013</hasYear>
    </owl:NamedIndividual>
    


    <!-- http://purl.obolibrary.org/obo/esmo.owl#WholeSale14 -->

    <owl:NamedIndividual rdf:about="http://purl.obolibrary.org/obo/esmo.owl#WholeSale14">
        <rdf:type rdf:resource="http://purl.obolibrary.org/obo/esmo.owl#Wholesale_value"/>
        <hasWholesaleValue rdf:datatype="http://www.w3.org/2001/XMLSchema#double">25.0</hasWholesaleValue>
        <hasYear rdf:datatype="http://www.w3.org/2001/XMLSchema#integer">2014</hasYear>
    </owl:NamedIndividual>
    


    <!-- http://purl.obolibrary.org/obo/esmo.owl#WholeSale15 -->

    <owl:NamedIndividual rdf:about="http://purl.obolibrary.org/obo/esmo.owl#WholeSale15">
        <rdf:type rdf:resource="http://purl.obolibrary.org/obo/esmo.owl#Wholesale_value"/>
        <hasWholesaleValue rdf:datatype="http://www.w3.org/2001/XMLSchema#double">25.0</hasWholesaleValue>
        <hasYear rdf:datatype="http://www.w3.org/2001/XMLSchema#integer">2015</hasYear>
    </owl:NamedIndividual>
    


    <!-- http://purl.obolibrary.org/obo/esmo.owl#WholeSale16 -->

    <owl:NamedIndividual rdf:about="http://purl.obolibrary.org/obo/esmo.owl#WholeSale16">
        <rdf:type rdf:resource="http://purl.obolibrary.org/obo/esmo.owl#Wholesale_value"/>
        <hasWholesaleValue rdf:datatype="http://www.w3.org/2001/XMLSchema#double">26.6</hasWholesaleValue>
        <hasYear rdf:datatype="http://www.w3.org/2001/XMLSchema#integer">2016</hasYear>
    </owl:NamedIndividual>
    


    <!-- http://purl.obolibrary.org/obo/esmo.owl#WholeSale17 -->

    <owl:NamedIndividual rdf:about="http://purl.obolibrary.org/obo/esmo.owl#WholeSale17">
        <rdf:type rdf:resource="http://purl.obolibrary.org/obo/esmo.owl#Wholesale_value"/>
        <hasWholesaleValue rdf:datatype="http://www.w3.org/2001/XMLSchema#double">26.58</hasWholesaleValue>
        <hasYear rdf:datatype="http://www.w3.org/2001/XMLSchema#integer">2017</hasYear>
    </owl:NamedIndividual>
    


    <!-- http://purl.obolibrary.org/obo/esmo.owl#WholeSale18 -->

    <owl:NamedIndividual rdf:about="http://purl.obolibrary.org/obo/esmo.owl#WholeSale18">
        <rdf:type rdf:resource="http://purl.obolibrary.org/obo/esmo.owl#Wholesale_value"/>
        <hasWholesaleValue rdf:datatype="http://www.w3.org/2001/XMLSchema#double">17.75</hasWholesaleValue>
        <hasYear rdf:datatype="http://www.w3.org/2001/XMLSchema#integer">2018</hasYear>
    </owl:NamedIndividual>
    


    <!-- http://purl.obolibrary.org/obo/esmo.owl#WholeSale19 -->

    <owl:NamedIndividual rdf:about="http://purl.obolibrary.org/obo/esmo.owl#WholeSale19">
        <rdf:type rdf:resource="http://purl.obolibrary.org/obo/esmo.owl#Wholesale_value"/>
        <hasWholesaleValue rdf:datatype="http://www.w3.org/2001/XMLSchema#double">16.2</hasWholesaleValue>
        <hasYear rdf:datatype="http://www.w3.org/2001/XMLSchema#integer">2019</hasYear>
    </owl:NamedIndividual>
    


    <!-- http://purl.obolibrary.org/obo/esmo.owl#WholeSale20 -->

    <owl:NamedIndividual rdf:about="http://purl.obolibrary.org/obo/esmo.owl#WholeSale20">
        <rdf:type rdf:resource="http://purl.obolibrary.org/obo/esmo.owl#Wholesale_value"/>
        <hasWholesaleValue rdf:datatype="http://www.w3.org/2001/XMLSchema#double">16.49</hasWholesaleValue>
        <hasYear rdf:datatype="http://www.w3.org/2001/XMLSchema#integer">2020</hasYear>
    </owl:NamedIndividual>
    


    <!-- http://purl.obolibrary.org/obo/esmo.owl#WholeSale21 -->

    <owl:NamedIndividual rdf:about="http://purl.obolibrary.org/obo/esmo.owl#WholeSale21">
        <rdf:type rdf:resource="http://purl.obolibrary.org/obo/esmo.owl#Wholesale_value"/>
        <hasWholesaleValue rdf:datatype="http://www.w3.org/2001/XMLSchema#double">25.89</hasWholesaleValue>
        <hasYear rdf:datatype="http://www.w3.org/2001/XMLSchema#integer">2021</hasYear>
    </owl:NamedIndividual>
    


    <!-- http://purl.obolibrary.org/obo/esmo.owl#Wholesale97 -->

    <owl:NamedIndividual rdf:about="http://purl.obolibrary.org/obo/esmo.owl#Wholesale97">
        <rdf:type rdf:resource="http://purl.obolibrary.org/obo/esmo.owl#Wholesale_value"/>
        <hasWholesaleValue rdf:datatype="http://www.w3.org/2001/XMLSchema#double">7.7</hasWholesaleValue>
        <hasYear rdf:datatype="http://www.w3.org/2001/XMLSchema#integer">1997</hasYear>
    </owl:NamedIndividual>
    


    <!-- http://purl.obolibrary.org/obo/esmo.owl#Wholesale98 -->

    <owl:NamedIndividual rdf:about="http://purl.obolibrary.org/obo/esmo.owl#Wholesale98">
        <rdf:type rdf:resource="http://purl.obolibrary.org/obo/esmo.owl#Wholesale_value"/>
        <hasWholesaleValue rdf:datatype="http://www.w3.org/2001/XMLSchema#double">9.200000001</hasWholesaleValue>
        <hasYear rdf:datatype="http://www.w3.org/2001/XMLSchema#integer">1998</hasYear>
    </owl:NamedIndividual>
    


    <!-- http://purl.obolibrary.org/obo/esmo.owl#Wholesale99 -->

    <owl:NamedIndividual rdf:about="http://purl.obolibrary.org/obo/esmo.owl#Wholesale99">
        <rdf:type rdf:resource="http://purl.obolibrary.org/obo/esmo.owl#Wholesale_value"/>
        <hasWholesaleValue rdf:datatype="http://www.w3.org/2001/XMLSchema#double">6.600000001</hasWholesaleValue>
        <hasYear rdf:datatype="http://www.w3.org/2001/XMLSchema#integer">1999</hasYear>
    </owl:NamedIndividual>
    


    <!-- 
    ///////////////////////////////////////////////////////////////////////////////////////
    //
    // General axioms
    //
    ///////////////////////////////////////////////////////////////////////////////////////
     -->

    <rdf:Description>
        <rdf:type rdf:resource="http://www.w3.org/2002/07/owl#AllDisjointClasses"/>
        <owl:members rdf:parseType="Collection">
            <rdf:Description rdf:about="http://purl.obolibrary.org/obo/BFO_0000008"/>
            <rdf:Description rdf:about="http://purl.obolibrary.org/obo/BFO_0000011"/>
            <rdf:Description rdf:about="http://purl.obolibrary.org/obo/BFO_0000015"/>
            <rdf:Description rdf:about="http://purl.obolibrary.org/obo/BFO_0000035"/>
        </owl:members>
    </rdf:Description>
    <rdf:Description>
        <rdf:type rdf:resource="http://www.w3.org/2002/07/owl#AllDisjointClasses"/>
        <owl:members rdf:parseType="Collection">
            <rdf:Description rdf:about="http://purl.obolibrary.org/obo/BFO_0000009"/>
            <rdf:Description rdf:about="http://purl.obolibrary.org/obo/BFO_0000018"/>
            <rdf:Description rdf:about="http://purl.obolibrary.org/obo/BFO_0000026"/>
            <rdf:Description rdf:about="http://purl.obolibrary.org/obo/BFO_0000028"/>
        </owl:members>
    </rdf:Description>
</rdf:RDF>



<!-- Generated by the OWL API (version 4.5.26.2023-07-17T20:34:13Z) https://github.com/owlcs/owlapi -->

